@prefix dct: <http://purl.org/dc/terms/> .
@prefix dc: <http://purl.org/dc/elements/1.1/> .
@prefix owl: <http://www.w3.org/2002/07/owl#> .
@prefix rdfs: <http://www.w3.org/2000/01/rdf-schema#> .
@prefix skos: <http://www.w3.org/2004/02/skos/core#> .
@prefix xsd: <http://www.w3.org/2001/XMLSchema#> .

@prefix bhstart: <http://linked.data.gov.au/def/borehole-surface-circumstance/> .

<http://linked.data.gov.au/def/borehole-surface-circumstance> a owl:Ontology .

bhstart:conceptScheme a skos:conceptScheme;
  dct:source <http://www.opengis.net/doc/geosciml/4.1> ;
  dc:source "The GeoSciML standard" ;
  dct:created "2019-02-19T14:43:40.371+10:00"^^xsd:dateTime;
  skos:prefLabel "Borehole Surface Circumstance"@en ;
  dct:description "The circumstances of a borehole's entrance which in GeoSciML is called Borehole Start"@en .

bhstart:natural_ground_surface a skos:Concept;
  dct:created "2019-02-19T14:44:09.271+10:00"^^xsd:dateTime;
  dct:modified "2019-02-19T14:47:43.387+10:00"^^xsd:dateTime;
  skos:definition "drilling started from a natural topographic surface";
  skos:inScheme bhstart:conceptScheme;
  skos:prefLabel "natural ground surface"@en;
  skos:topConceptOf bhstart:conceptScheme .

bhstart:open_pit_floor_or_wall a skos:Concept;
  dct:created "2019-02-19T14:44:34.754+10:00"^^xsd:dateTime;
  dct:modified "2019-02-19T14:47:09.302+10:00"^^xsd:dateTime;
  skos:definition "drilling started from the wall of an open pit or quarry";
  skos:inScheme bhstart:conceptScheme;
  skos:prefLabel "open pit floor or wall"@en;
  skos:topConceptOf bhstart:conceptScheme .

bhstart:underground a skos:Concept;
  dct:created "2019-02-19T14:44:41.489+10:00"^^xsd:dateTime;
  dct:modified "2019-02-19T14:46:24.471+10:00"^^xsd:dateTime;
  skos:definition "drilling started from an underground location, such as a driveway, chamber or open-stop";
  skos:inScheme bhstart:conceptScheme;
  skos:prefLabel "underground"@en;
  skos:topConceptOf bhstart:conceptScheme .

bhstart:from_pre-existing_hole a skos:Concept;
  dct:created "2019-02-19T14:44:53.161+10:00"^^xsd:dateTime;
  dct:modified "2019-02-19T14:45:35.599+10:00"^^xsd:dateTime;
  skos:definition "new drill hole (well bore) spudded off the wall of an existing hole";
  skos:inScheme bhstart:conceptScheme;
  skos:prefLabel "from pre-existing hole"@en;
  skos:topConceptOf bhstart:conceptScheme .
