@prefix adrss: <http://linked.data.gov.au/def/address-type/> .
@prefix dc: <http://purl.org/dc/elements/1.1/> .
@prefix dct: <http://purl.org/dc/terms/> .
@prefix owl: <http://www.w3.org/2002/07/owl#> .
@prefix rdf: <http://www.w3.org/1999/02/22-rdf-syntax-ns#> .
@prefix rdfs: <http://www.w3.org/2000/01/rdf-schema#> .
@prefix sdo: <https://schema.org/> .
@prefix skos: <http://www.w3.org/2004/02/skos/core#> .
@prefix xml: <http://www.w3.org/XML/1998/namespace> .
@prefix xsd: <http://www.w3.org/2001/XMLSchema#> .
        
<http://linked.data.gov.au/def/address-type> a owl:Ontology,
        skos:ConceptScheme ;
    dct:created "2020-03-25"^^xsd:date ;
    dct:creator <http://linked.data.gov.au/org/gsq> ;
    dct:modified "2020-03-25"^^xsd:date ;
    dct:publisher <http://linked.data.gov.au/org/gsq> ;
    dct:source "Derived from  Australian Standard AS 4590.1:2017" ;
    skos:definition "The role or use of the address in relation to a party. An address may have more than one purpose."@en ;
    skos:prefLabel "Address Type"@en .

<http://linked.data.gov.au/org/gsq> a sdo:Organization ;
    sdo:name "Geological Survey of Queensland" .

<http://linked.data.gov.au/def/address-type> a skos:ConceptScheme ;
    skos:hasTopConcept adrss:business-address,
        adrss:delivery-address,
        adrss:overseas-address,
        adrss:postal-address,
        adrss:primary-property-address,
        adrss:residential-address,
        adrss:secondary-property-address .

adrss:business-address a skos:Concept ;
    skos:altLabel "Company Address"@en,
        "Office Address"@en ;
    skos:definition "The address of the principal place of business for the client."@en ;
    skos:inScheme <http://linked.data.gov.au/def/address-type> ;
    skos:notation "BUS" ;
    skos:prefLabel "Business Address"@en ;
    skos:topConceptOf <http://linked.data.gov.au/def/address-type> .

adrss:delivery-address a skos:Concept ;
    skos:definition "The address used for goods delivery purposes."@en ;
    skos:inScheme <http://linked.data.gov.au/def/address-type> ;
    skos:notation "DEL" ;
    skos:prefLabel "Delivery Address"@en ;
    skos:topConceptOf <http://linked.data.gov.au/def/address-type> .

adrss:overseas-address a skos:Concept ;
    skos:definition "The address used by the client when overseas."@en ;
    skos:inScheme <http://linked.data.gov.au/def/address-type> ;
    skos:notation "OVS" ;
    skos:prefLabel "Overseas Address"@en ;
    skos:topConceptOf <http://linked.data.gov.au/def/address-type> .

adrss:postal-address a skos:Concept ;
    skos:altLabel "Correspondence Address"@en ;
    skos:definition "The address used by the client for receipt of correspondence."@en ;
    skos:inScheme <http://linked.data.gov.au/def/address-type> ;
    skos:notation "POS" ;
    skos:prefLabel "Postal Address"@en ;
    skos:topConceptOf <http://linked.data.gov.au/def/address-type> .

adrss:primary-property-address a skos:Concept ;
    skos:definition "The property address normally used by the client."@en ;
    skos:inScheme <http://linked.data.gov.au/def/address-type> ;
    skos:notation "PR" ;
    skos:prefLabel "Primary Property Address"@en ;
    skos:topConceptOf <http://linked.data.gov.au/def/address-type> .

adrss:residential-address a skos:Concept ;
    skos:definition "The address of the principal place of residence for the client."@en ;
    skos:inScheme <http://linked.data.gov.au/def/address-type> ;
    skos:notation "RES" ;
    skos:prefLabel "Residential Address"@en ;
    skos:topConceptOf <http://linked.data.gov.au/def/address-type> .

adrss:secondary-property-address a skos:Concept ;
    skos:definition "The address of an additional property attached to the client."@en ;
    skos:inScheme <http://linked.data.gov.au/def/address-type> ;
    skos:notation "SEC" ;
    skos:prefLabel "Secondary Property Address"@en ;
    skos:topConceptOf <http://linked.data.gov.au/def/address-type> .
