@prefix bhdd: <http://linked.data.gov.au/def/borehole-depth-datum/> .
@prefix dc: <http://purl.org/dc/elements/1.1/> .
@prefix dct: <http://purl.org/dc/terms/> .
@prefix owl: <http://www.w3.org/2002/07/owl#> .
@prefix rdf: <http://www.w3.org/1999/02/22-rdf-syntax-ns#> .
@prefix rdfs: <http://www.w3.org/2000/01/rdf-schema#> .
@prefix skos: <http://www.w3.org/2004/02/skos/core#> .
@prefix xml: <http://www.w3.org/XML/1998/namespace> .
@prefix xsd: <http://www.w3.org/2001/XMLSchema#> .

<http://linked.data.gov.au/def/borehole-depth-datum> a owl:Ontology , skos:ConceptScheme ;
    dct:creator "Geological Survey of Queensland" ;
    dct:modified "2020-01-21T11:03:47+10:00"^^xsd:dateTime,
        "2020-01-21T11:06:04+10:00"^^xsd:dateTime ;
    dct:source "Compiled by the Geological Survey of Queensland" ;
    skos:definition "The point from which all depths are measured in a well or bore (the depth reference datum). Typically referenced to a common global or regional reference datum such as the Australian Height Datum (AHD)."@en ;
    skos:hasTopConcept bhdd:drill-collar,
        bhdd:ground-level,
        bhdd:kelly-bushing,
        bhdd:rotary-table ;
    skos:prefLabel "Borehole Depth Datum"@en .

bhdd:drill-collar a skos:Concept ;
    skos:definition "A component of a drillstring that provides weight on bit for drilling. Drill collars are thick-walled tubular pieces machined from solid bars of steel or alloy. Source: Schlumberger Oilfield Glossary"@en ;
    skos:inScheme <http://linked.data.gov.au/def/borehole-depth-datum> ;
    skos:notation "DC" ;
    skos:prefLabel "Drill Collar"@en ;
    skos:topConceptOf <http://linked.data.gov.au/def/borehole-depth-datum> .

bhdd:ground-level a skos:Concept ;
    skos:definition "At surface ground level elevation absent of additional equipment."@en ;
    skos:inScheme <http://linked.data.gov.au/def/borehole-depth-datum> ;
    skos:notation "GL" ;
    skos:prefLabel "Ground Level"@en ;
    skos:topConceptOf <http://linked.data.gov.au/def/borehole-depth-datum> .

bhdd:kelly-bushing a skos:Concept ;
    skos:definition "An adapter that serves to connect the rotary table to the kelly (A long square or hexagonal steel bar with a hole drilled through the middle for a fluid path). Source: Schlumberger Oilfield Glossary"@en ;
    skos:inScheme <http://linked.data.gov.au/def/borehole-depth-datum> ;
    skos:notation "KB" ;
    skos:prefLabel "Kelly Bushing"@en ;
    skos:topConceptOf <http://linked.data.gov.au/def/borehole-depth-datum> .

bhdd:rotary-table a skos:Concept ;
    skos:definition "The revolving or spinning section of the drillfloor that provides power to turn the drillstring in a clockwise direction (as viewed from above). Source: Schlumberger Oilfield Glossary"@en ;
    skos:inScheme <http://linked.data.gov.au/def/borehole-depth-datum> ;
    skos:notation "RT" ;
    skos:prefLabel "Rotary Table"@en ;
    skos:topConceptOf <http://linked.data.gov.au/def/borehole-depth-datum> .

