@prefix bhpur: <http://linked.data.gov.au/def/borehole-purpose/> .
@prefix dcterms: <http://purl.org/dc/terms/> .
@prefix owl: <http://www.w3.org/2002/07/owl#> .
@prefix sdo: <https://schema.org/> .
@prefix skos: <http://www.w3.org/2004/02/skos/core#> .
@prefix xsd: <http://www.w3.org/2001/XMLSchema#> .

<http://linked.data.gov.au/def/borehole-purpose> a owl:Ontology , skos:ConceptScheme ;
    dcterms:creator <http://linked.data.gov.au/org/gsq> ;
    dcterms:publisher <http://linked.data.gov.au/org/gsq> ;
    dcterms:modified "2020-09-16"^^xsd:date ;
    dcterms:created "2020-07-17"^^xsd:date ;
    dcterms:source "Compiled by the Geological Survey of Queensland" ;
    skos:definition "The primary purpose of a borehole based on the legislative State Act and/or the resources industry sector."@en ;
    skos:hasTopConcept bhpur:coal,
        bhpur:geothermal,
        bhpur:greenhouse-gas-storage,
        bhpur:mineral,
        bhpur:non-industry,
        bhpur:oil-shale,
        bhpur:petroleum,
        bhpur:water ;
    skos:prefLabel "Borehole Purpose"@en .

<http://linked.data.gov.au/org/gsq> a sdo:Organization ;
    sdo:name "Geological Survey of Queensland" ;
    sdo:url <https://www.business.qld.gov.au/industries/mining-energy-water/resources/geoscience-information/gsq> .

bhpur:carbon-capture-and-storage a skos:Concept ;
    skos:broader bhpur:greenhouse-gas-storage ;
    skos:definition "Wells that deposit carbon dioxide into an underground geological formation after capture from large point sources, such as a cement factory or biomass power plant."@en ;
    skos:inScheme <http://linked.data.gov.au/def/borehole-purpose> ;
    skos:prefLabel "Carbon Capture and Storage"@en .

bhpur:coal-seam-gas a skos:Concept ;
    skos:broader bhpur:petroleum ;
    skos:definition "Wells targetting coal seams where hydrocarbons are kept in place via adsorption to the coal surface and hydrostatic pressure"@en ;
    skos:inScheme <http://linked.data.gov.au/def/borehole-purpose> ;
    skos:prefLabel "Coal Seam Gas"@en .

bhpur:conventional-petroleum a skos:Concept ;
    skos:broader bhpur:petroleum ;
    skos:definition "Wells targetting conventional petroleum reservoirs where buoyant forces keep hydrocarbons in place below a sealing caprock."@en ;
    skos:inScheme <http://linked.data.gov.au/def/borehole-purpose> ;
    skos:prefLabel "Conventional Petroleum"@en .

bhpur:open-cut-coal-mining a skos:Concept ;
    skos:broader bhpur:coal ;
    skos:definition "Wells drilled for the purpose of assessing coal resources for an open cut coal mine."@en ;
    skos:inScheme <http://linked.data.gov.au/def/borehole-purpose> ;
    skos:prefLabel "Open-Cut Coal Mining"@en .

bhpur:shale-gas a skos:Concept ;
    skos:broader bhpur:unconventional-petroleum ;
    skos:definition "Wells targetting shale that produces natural gas. A shale that is thermally mature enough and has sufficient gas content to produce economic quantities of natural gas."@en ; 
    skos:inScheme <http://linked.data.gov.au/def/borehole-purpose> ;
    skos:prefLabel "Shale Gas"@en .

bhpur:shale-oil a skos:Concept ;
    skos:broader bhpur:unconventional-petroleum ;
    skos:definition "Wells targetting shale that produces oil. Oil obtained by artificial maturation of oil shale. The process of artificial maturation uses controlled heating, or pyrolysis, of kerogen to release the shale oil."@en ;
    skos:inScheme <http://linked.data.gov.au/def/borehole-purpose> ;
    skos:prefLabel "Shale Oil"@en .

bhpur:tight-gas a skos:Concept ;
    skos:broader bhpur:unconventional-petroleum ;
    skos:definition "Wells targetting gas from relatively impermeable reservoir rock."@en ;
    skos:inScheme <http://linked.data.gov.au/def/borehole-purpose> ;
    skos:prefLabel "Tight Gas"@en .

bhpur:tight-oil a skos:Concept ;
    skos:broader bhpur:unconventional-petroleum ;
    skos:definition "Wells targetting oil from relatively impermeable reservoir rock."@en ;
    skos:inScheme <http://linked.data.gov.au/def/borehole-purpose> ;
    skos:prefLabel "Tight Oil"@en .

bhpur:underground-coal-mining a skos:Concept ;
    skos:broader bhpur:coal ;
    skos:definition "Wells drilled for the purpose of assessing coal resources for an underground coal mine."@en ;
    skos:inScheme <http://linked.data.gov.au/def/borehole-purpose> ;
    skos:prefLabel "Underground Coal Mining"@en .

bhpur:geothermal a skos:Concept ;
    skos:definition "Wells and bores drilled under permits governed by the Queensland Geothermal Energy Act 2010"@en ;
    skos:inScheme <http://linked.data.gov.au/def/borehole-purpose> ;
    skos:prefLabel "Geothermal"@en ;
    skos:topConceptOf <http://linked.data.gov.au/def/borehole-purpose> .

bhpur:mineral a skos:Concept ;
    skos:definition "Wells and bores drilled to facilitate the mining of minerals, excluding coal and oil shale, under permits governed by the Queensland Mineral Resources Act (1989)"@en ;
    skos:inScheme <http://linked.data.gov.au/def/borehole-purpose> ;
    skos:prefLabel "Mineral"@en ;
    skos:topConceptOf <http://linked.data.gov.au/def/borehole-purpose> .

bhpur:non-industry a skos:Concept ;
    skos:altLabel "Collaborative Drilling"@en,
        "Collaborative Exploration"@en,
        "Non-Industry"@en ;
    skos:definition "Wells and bores drilled by non-industry agents outside of the State Resources Acts"@en ;
    skos:inScheme <http://linked.data.gov.au/def/borehole-purpose> ;
    skos:prefLabel "Non-Industry and Collaborative Drilling"@en ;
    skos:topConceptOf <http://linked.data.gov.au/def/borehole-purpose> .

bhpur:oil-shale a skos:Concept ;
    skos:definition "Wells and bores drilled to facilitate the mining of oil shale under permits governed by the Queensland Mineral Resources Act 1989"@en ;
    skos:inScheme <http://linked.data.gov.au/def/borehole-purpose> ;
    skos:prefLabel "Oil Shale"@en ;
    skos:topConceptOf <http://linked.data.gov.au/def/borehole-purpose> .

bhpur:water a skos:Concept ;
    skos:definition "Wells and bores drilled under permits governed by the Queensland Water Act 2000"@en ;
    skos:inScheme <http://linked.data.gov.au/def/borehole-purpose> ;
    skos:prefLabel "Water"@en ;
    skos:topConceptOf <http://linked.data.gov.au/def/borehole-purpose> .

bhpur:greenhouse-gas-storage a skos:Concept ;
    skos:altLabel "GHG"@en ;
    skos:definition "Wells and bores drilled under permits governed by the Queensland Greenhouse Gas Storage Act 2009"@en ;
    skos:inScheme <http://linked.data.gov.au/def/borehole-purpose> ;
    skos:prefLabel "Greenhouse Gas Storage"@en ;
    skos:topConceptOf <http://linked.data.gov.au/def/borehole-purpose> .

bhpur:coal a skos:Concept ;
    skos:definition "Wells and bores drilled to facilitate the mining of coal under permits governed by the Queensland Mineral Resources Act 1989"@en ;
    skos:inScheme <http://linked.data.gov.au/def/borehole-purpose> ;
    skos:prefLabel "Coal"@en ;
    skos:topConceptOf <http://linked.data.gov.au/def/borehole-purpose> .

bhpur:petroleum a skos:Concept ;
    skos:definition "Wells and bores drilled under permits governed by the Queensland Petroleum Act 1923 and Petroleum and Gas (Production and Safety) Act 2004"@en ;
    skos:inScheme <http://linked.data.gov.au/def/borehole-purpose> ;
    skos:prefLabel "Petroleum"@en ;
    skos:topConceptOf <http://linked.data.gov.au/def/borehole-purpose> .

bhpur:unconventional-petroleum a skos:Concept ;
    skos:broader bhpur:petroleum ;
    skos:definition "Wells targetting unconventional reservoirs whose properties including porosity, permeability, or trapping mechanism differ from conventional reservoirs"@en ;
    skos:inScheme <http://linked.data.gov.au/def/borehole-purpose> ;
    skos:prefLabel "Unconventional Petroleum"@en .

bhpur:pggd a skos:Collection ;
    skos:definition "Borehole purposes applicable to regulatory notification forms."@en ;
    skos:member bhpur:conventional-petroleum,
            bhpur:coal-seam-gas,
            bhpur:unconventional-petroleum,
            bhpur:geothermal,
            bhpur:greenhouse-gas-storage;
    skos:prefLabel "PGGD selection"@en .
