@prefix bhse: <http://linked.data.gov.au/def/borehole-status-event/> .
@prefix dc: <http://purl.org/dc/elements/1.1/> .
@prefix dct: <http://purl.org/dc/terms/> .
@prefix owl: <http://www.w3.org/2002/07/owl#> .
@prefix rdf: <http://www.w3.org/1999/02/22-rdf-syntax-ns#> .
@prefix rdfs: <http://www.w3.org/2000/01/rdf-schema#> .
@prefix skos: <http://www.w3.org/2004/02/skos/core#> .
@prefix xml: <http://www.w3.org/XML/1998/namespace> .
@prefix xsd: <http://www.w3.org/2001/XMLSchema#> .

<http://linked.data.gov.au/def/borehole-status-event> a owl:Ontology , skos:ConceptScheme ;
    dct:creator "Geological Survey of Queensland" ;
    dct:modified "2020-01-21T15:03:09"^^xsd:dateTime,
        "2020-01-21T15:03:15"^^xsd:dateTime ;
    dct:source "Compiled by the Geological Survey of Queensland" ;
    skos:definition "The stage in the lifecycle of a project (e.g. mine site, petroleum field, quarry) that describes the maturity of resource defintion and production."@en ;
    skos:hasTopConcept bhse:notice-of-completion-alteration-or-abandonment-of-petroleum-well-or-bore,
        bhse:notice-of-completion-of-conversion-of-petroleum-well-to-water-supply-bore-or-water-observation-bore,
        bhse:notice-of-completion-of-hydraulic-fracturing-activities,
        bhse:notice-of-decommissioning-a-well-water-observation-bore-water-monitoring-bore-or-water-supply-bore,
        bhse:notice-of-intention-to-carry-out-hydraulic-fracturing-activities,
        bhse:notice-of-intention-to-convert-a-petroleum-well-to-a-water-observation-bore-or-water-supply-bore,
        bhse:notice-of-intention-to-drill-a-petroleum-well-or-bore,
        bhse:petroleum-production-report ;
    skos:prefLabel "Borehole Status Event"@en .

bhse:notice-of-completion-alteration-or-abandonment-of-petroleum-well-or-bore a skos:Concept ;
    skos:definition "A notice to inform the Department that a petroleum well or bore has been completed, altered, or abandoned. Changes status to drilled, suspended, or abandoned."@en ;
    skos:inScheme <http://linked.data.gov.au/def/borehole-status-event> ;
    skos:notation "PGGD-02" ;
    skos:prefLabel "Notice of completion, alteration or abandonment of petroleum well or bore"@en ;
    skos:topConceptOf <http://linked.data.gov.au/def/borehole-status-event> .

bhse:notice-of-completion-of-conversion-of-petroleum-well-to-water-supply-bore-or-water-observation-bore a skos:Concept ;
    skos:definition "A notice to inform the Department that a petroleum well has been converted to a water bore. Changes purpose from Petroleum, or narrower term, to Water. May trigger check for status change."@en ;
    skos:inScheme <http://linked.data.gov.au/def/borehole-status-event> ;
    skos:notation "WRA-05A" ;
    skos:prefLabel "Notice of completion of conversion of petroleum well to water supply bore or water observation bore"@en ;
    skos:topConceptOf <http://linked.data.gov.au/def/borehole-status-event> .

bhse:notice-of-completion-of-hydraulic-fracturing-activities a skos:Concept ;
    skos:definition "A notice to inform the Department that a petroleum well has had stimulation by hydraulically fracturing completed."@en ;
    skos:inScheme <http://linked.data.gov.au/def/borehole-status-event> ;
    skos:notation "PGGD-04" ;
    skos:prefLabel "Notice of completion of hydraulic fracturing activities"@en ;
    skos:topConceptOf <http://linked.data.gov.au/def/borehole-status-event> .

bhse:notice-of-intention-to-carry-out-hydraulic-fracturing-activities a skos:Concept ;
    skos:definition "A notice to inform the Department that a petroleum well is intended to be stimulated by hydraulically fracturing."@en ;
    skos:inScheme <http://linked.data.gov.au/def/borehole-status-event> ;
    skos:notation "PGGD-03" ;
    skos:prefLabel "Notice of intention to carry out hydraulic fracturing activities"@en ;
    skos:topConceptOf <http://linked.data.gov.au/def/borehole-status-event> .

bhse:notice-of-decommissioning-a-well-water-observation-bore-water-monitoring-bore-or-water-supply-bore a skos:Concept ;
    skos:definition "A notice to inform the Department that a well or water bore has been decommisioned."@en ;
    skos:inScheme <http://linked.data.gov.au/def/borehole-status-event> ;
    skos:historyNote "Form supersedes legacy form PA-40"@en ;
    skos:notation "PA-40",
        "MMOL-44";
    skos:altLabel "Notice of decommissioning a well, water observation bore, water monitoring bore or water supply bore"@en ;
    skos:prefLabel "Notice of decommissioning petroleum wells, water observation bores or water supply bores"@en ;
    skos:topConceptOf <http://linked.data.gov.au/def/borehole-status-event> .

bhse:notice-of-intention-to-convert-a-petroleum-well-to-a-water-observation-bore-or-water-supply-bore a skos:Concept ;
    skos:definition "A notice to inform the Department that a petroleum well is intended to be converted to a water bore."@en ;
    skos:inScheme <http://linked.data.gov.au/def/borehole-status-event> ;
    skos:notation "PA-42" ;
    skos:prefLabel "Notice of intention to convert a petroleum well to a water observation bore or water supply bore"@en ;
    skos:topConceptOf <http://linked.data.gov.au/def/borehole-status-event> .

bhse:notice-of-intention-to-drill-a-petroleum-well-or-bore a skos:Concept ;
    skos:definition "A notice to inform the Department that a petroleum well or bore is intended to be drilled. Triggers the creation of a well with the status: proposed."@en ;
    skos:inScheme <http://linked.data.gov.au/def/borehole-status-event> ;
    skos:notation "PGGD-01" ;
    skos:prefLabel "Notice of intention to drill a petroleum well or bore"@en ;
    skos:topConceptOf <http://linked.data.gov.au/def/borehole-status-event> .

bhse:petroleum-production-report a skos:Concept ;
    skos:definition "A petroleum production report. Triggers change to on production or on injection depending on contents of report."@en ;
    skos:inScheme <http://linked.data.gov.au/def/borehole-status-event> ;
    skos:prefLabel "Petroleum Production Report"@en ;
    skos:topConceptOf <http://linked.data.gov.au/def/borehole-status-event> .

bhse:manual-update a skos:Concept ;
    skos:definition "An update to a borehole status performed via direct creation or update in the database by an authorised user."@en ;
    skos:inScheme <http://linked.data.gov.au/def/borehole-status-event> ;
    skos:prefLabel "Manual Update or Creation"@en ;
    skos:topConceptOf <http://linked.data.gov.au/def/borehole-status-event> .
