@prefix dc: <http://purl.org/dc/elements/1.1/> .
@prefix dcterms: <http://purl.org/dc/terms/> .
@prefix owl: <http://www.w3.org/2002/07/owl#> .
@prefix rdf: <http://www.w3.org/1999/02/22-rdf-syntax-ns#> .
@prefix rdfs: <http://www.w3.org/2000/01/rdf-schema#> .
@prefix skos: <http://www.w3.org/2004/02/skos/core#> .
@prefix xsd: <http://www.w3.org/2001/XMLSchema#> .

@prefix gsqtheme: <http://linked.data.gov.au/def/gsq-dataset-theme/> .

<http://linked.data.gov.au/def/gsq-dataset-theme> a owl:Ontology .

gsqtheme:conceptScheme a skos:ConceptScheme ;
    skos:prefLabel "Geoscience Dataset Theme"@en ;
    skos:definition "A theme is used to categorise the different types of data resources that GSQ collects, stores, manages and publishes. Themes help users to discover data."@en ;
    dcterms:created "2019-03-06T10:57:30.681000+10:00"^^xsd:dateTime .

gsqtheme:industry-reports a skos:Concept ;
    skos:prefLabel "Industry reports"@en ;
    skos:definition "Resource authority holders need to submit a range of statutory reports on their activities. Reports include all mineral exploration, geothermal exploration, greenhouse gas exploration, petroleum exploration, petroleum well, seismic survey or airborne geophysical survey, mineral development licence, petroleum lease, and petroleum pipeline licence reports and some other exploration related reporting."@en ;
    skos:inScheme gsqtheme:conceptScheme ;
    skos:topConceptOf gsqtheme:conceptScheme .

gsqtheme:geochemistry-data a skos:Concept ;
    skos:prefLabel "Exploration geochemistry data"@en ;
    skos:definition "Geochemistry is the study of the chemicals, rocks and minerals that form and shape the Earth. Queensland exploration geochemistry data comprises surface and drillholes data generated from open file exploration reports submitted by mining companies doing mineral exploration work in Queensland."@en ;
    skos:inScheme gsqtheme:conceptScheme ;
    skos:topConceptOf gsqtheme:conceptScheme .

gsqtheme:seismic-data a skos:Concept ;
    skos:prefLabel "Seismic survey data"@en ;
    skos:definition "Seismic surveys produce detailed images of the various rock types and their location beneath the Earth's surface. Sound waves are bounced off underground rock formations and the waves that reflect back to the surface are captured by recording sensors. Analysing the time the waves take to return provides valuable information about rock types and possible gases or fluids in rock formations."@en ;
    skos:inScheme gsqtheme:conceptScheme ;
    skos:topConceptOf gsqtheme:conceptScheme .
