@prefix : <http://linked.data.gov.au/def/gsq-dataset-themes/> .
@prefix dc: <http://purl.org/dc/elements/1.1/> .
@prefix dct: <http://purl.org/dc/terms/> .
@prefix owl: <http://www.w3.org/2002/07/owl#> .
@prefix rdf: <http://www.w3.org/1999/02/22-rdf-syntax-ns#> .
@prefix rdfs: <http://www.w3.org/2000/01/rdf-schema#> .
@prefix skos: <http://www.w3.org/2004/02/skos/core#> .
@prefix xml: <http://www.w3.org/XML/1998/namespace> .
@prefix xsd: <http://www.w3.org/2001/XMLSchema#> .

<http://linked.data.gov.au/def/gsq-dataset-themes> a owl:Ontology .

:conceptScheme a skos:ConceptScheme ;
    dct:created "2019-10-02T15:00:47+10:00"^^xsd:dateTime ;
    dct:creator "Geological Survey of Queensland" ;
    dct:modified "2019-10-02T15:00:47+10:00"^^xsd:dateTime ;
    dct:source "Developed by the Geological Survey of Queensland." ;
    skos:definition "A list of broad thematic descriptions of datasets created, received, and held by the Geological Survey of Queensland."@en ;
    skos:prefLabel "GSQ Dataset Themes"@en .

:administrative-data a skos:Concept ;
    skos:definition "Ancillary information regarding the administration of Queensland Resources such as adminstrative boundaries, mining permits, legislation, and information about organisations such as DNRME and GSQ."@en ;
    skos:inScheme :conceptScheme ;
    skos:prefLabel "Administrative data"@en ;
    skos:topConceptOf :conceptScheme .

:geoscience-data a skos:Concept ;
    skos:definition "Primary descriptive data defining the geological attributes of a feature of interest."@en ;
    skos:inScheme :conceptScheme ;
    skos:prefLabel "Geoscience data"@en ;
    skos:topConceptOf :conceptScheme .

:geoscience-project-data a skos:Concept ;
    skos:definition "Data and media describing project information such as activities performed, planning and approvals for the collection and analysis of primary geoscience data."@en ;
    skos:inScheme :conceptScheme ;
    skos:prefLabel "Geoscience project data"@en ;
    skos:topConceptOf :conceptScheme .

:other a skos:Concept ;
    skos:definition "Any other metadata, data, or information that is not described by any of the other GSQ Dataset Themes."@en ;
    skos:inScheme :conceptScheme ;
    skos:prefLabel "Other"@en ;
    skos:topConceptOf :conceptScheme .

:operational-data a skos:Concept ;
    skos:definition "Data describing the operations of mining, drilling, processing, and sales operations e.g. borehole drilling, pipelines, processing facilities."@en ;
    skos:inScheme :conceptScheme ;
    skos:prefLabel "Operational data"@en ;
    skos:topConceptOf :conceptScheme .

:physical-samples a skos:Concept ;
    skos:definition "Data and metadata pertaining to physical samples taken during geoscience data acquisition e.g. drill core, rock chips, rock samples from outcrop, soil, sediment, water, drilling fluids, oil, gas etc."@en ;
    skos:inScheme :conceptScheme ;
    skos:prefLabel "Physical samples"@en ;
    skos:topConceptOf :conceptScheme .

:publications a skos:Concept ;
    skos:definition "Publications that describe the geology, resource potential, or other areas of departmental interest such as books, journals, periodicals, presentations, posters, academic publications, or multimedia products."@en ;
    skos:inScheme :conceptScheme ;
    skos:prefLabel "Publications"@en ;
    skos:topConceptOf :conceptScheme .

:reports a skos:Concept ;
    skos:definition "Reports lodged for compliance with permit grant and retention, or . These may be permit based such as a resource authority annual report, activity based such as a well completion report, or non-tenure reports such as departmental survey reports."@en ;
    skos:inScheme :conceptScheme ;
    skos:prefLabel "Reports"@en ;
    skos:topConceptOf :conceptScheme .

:resource-statistics a skos:Concept ;
    skos:definition "Statistical data and reports submitted to the department or collected/generated by the department, particularly production and sales quantities."@en ;
    skos:inScheme :conceptScheme ;
    skos:prefLabel "Resource statistics"@en ;
    skos:topConceptOf :conceptScheme .

:spatial-data a skos:Concept ;
    skos:definition "Data and metadata related to spatial objects and representations such as maps, aerial and satellite imagery, spatial data files and databases."@en ;
    skos:inScheme :conceptScheme ;
    skos:prefLabel "Spatial data"@en ;
    skos:topConceptOf :conceptScheme .

:activities-and-results a skos:Collection ;
    skos:definition "Primary dataset that describe the geological features of interest and the activities that generate those datasets."@en ;
    skos:member :geoscience-data,
        :geoscience-project-data,
        :operational-data,
        :physical-samples ;
    skos:prefLabel "Activities and results"@en .

:ancillary-information a skos:Collection ;
    skos:definition "Data descriptive of the organisations involved in data collection and the administrative constraints and associations under which data is collected or related."@en ;
    skos:member :administrative-data,
        :spatial-data ;
    skos:prefLabel "Ancillary information"@en .

:products-and-documents a skos:Collection ;
    skos:definition "The final products and official reports that synthesise the collected data into documentation that describe activities and/or provide interpretive and contextual information."@en ;
    skos:member :publications,
        :reports ;
    skos:prefLabel "Products and documents"@en .

