@prefix dc: <http://purl.org/dc/elements/1.1/> .
@prefix dcterms: <http://purl.org/dc/terms/> .
@prefix owl: <http://www.w3.org/2002/07/owl#> .
@prefix sdo: <https://schema.org/> .
@prefix skos: <http://www.w3.org/2004/02/skos/core#> .
@prefix fst: <http://linked.data.gov.au/def/gsq-feature-status/> .
@prefix xsd: <http://www.w3.org/2001/XMLSchema#> .

<http://linked.data.gov.au/def/gsq-feature-status> a owl:Ontology,
    skos:ConceptScheme ;
    dcterms:created "2021-02-10T10:00:00+10:00"^^xsd:dateTime ; 
    dcterms:creator <http://linked.data.gov.au/org/gsq> ;
    dcterms:publisher <http://linked.data.gov.au/org/gsq> ;
    dcterms:modified "2021-02-10T10:00:00+10:00"^^xsd:dateTime ;
    dcterms:source "Compiled by the Geological Survey of Queensland" ;
    skos:definition """The status of a geologic feature, which in name (and definition) may embrace formal, informal, obsolete or other terms, is generally regulated variously (depending on the feature type) by a national, international and/or other code or protocol that applies thereto, and, where applicable, may be administered and/or reviewed by a relevant authority, such as the Geological Survey of Queensland or (for Australian lithostratigraphic and lithodemic units) by Geoscience Australia in collaboration with the Australian Stratigraphy Commission of the Geological Society of Australia."""@en ;
    skos:hasTopConcept fst:Ambiguous,
        fst:Formal,
        fst:Informal,
        fst:Invalid,
        fst:NotDefined, 
        fst:Superseded, 
    skos:prefLabel "Geologic Feature Status"@en .

<http://linked.data.gov.au/org/gsq> a sdo:Organization ;
    sdo:name "Geological Survey of Queensland" ;
    sdo:url <https://www.business.qld.gov.au/industries/mining-energy-water/resources/geoscience-information/gsq> .

fst:Formal a skos:Concept ;
    skos:definition """The status of a geologic feature the name and parameters of which are in current use, and have been intentionally/formally defined and/or delineated by printed and/or digital publication in accordance, and where applicable, with a national, international and/or other code or protocol that applies thereto."""@en ;
    skos:inScheme <http://linked.data.gov.au/def/gsq-feature-status> ;
    skos:prefLabel "Formal"@en ;
    skos:topConceptOf <http://linked.data.gov.au/def/gsq-feature-status> .
        
fst:Informal a skos:Concept ;
    skos:definition """The status of a geologic feature the name and parameters of which are in current use, and have been informally defined and/or delineated by printed and/or digital publication (albeit including the Australian Stratigraphic Units Database) in accordance, and where applicable, with a national, international and/or other code or protocol that applies thereto."""@en ;
    skos:inScheme <http://linked.data.gov.au/def/gsq-feature-status> ;
    skos:prefLabel "Informal"@en ;
    skos:topConceptOf <http://linked.data.gov.au/def/gsq-feature-status> .
        
fst:Invalid a skos:Concept ;
    skos:altLabel "unacceptable"@en ;
    skos:altLabel "not valid"@en ;
    skos:definition """The status of a geologic feature the name and parameters of which have been published, but not in full accordance with a national, international and/or other code or protocol that applies thereto."""@en ;
    skos:scopeNote """For example: The 'Rodney Creek Sandstone' [Galilee Basin; Phillips et al., 2017:AJES 64(3), 283-300], as the name/unit was not published in accordance with The International Stratigraphic Guide. As of the current date (04.02.2021), this unit has not been entered into Geoscience Australia's Australian Stratigraphic Units Database, and has not been superceded/replaced by an informal term or otherwise dealt with, thus remaining 'invalid' pending supersedence."""@en ;
    skos:inScheme <http://linked.data.gov.au/def/gsq-feature-status> ;
    skos:prefLabel "Invalid"@en ;
    skos:topConceptOf <http://linked.data.gov.au/def/gsq-feature-status> .     
 
fst:Undefined a skos:Concept ;
    skos:altLabel "not defined"@en ;
    skos:definition "The status of a geologic feature that has been recorded in published or unpublished reports, records, maps, etc., but has not been defined, either informally or formally."@en ;
    skos:inScheme <http://linked.data.gov.au/def/gsq-feature-status> ;
    skos:prefLabel "Undefined"@en ;
    skos:topConceptOf <http://linked.data.gov.au/def/gsq-feature-status> .

fst:Superseded a skos:Concept ;
    skos:altLabel "superceded"@en ;
    skos:altLabel "superceeded"@en ;
    skos:altLabel "replaced"@en ; 
    skos:altLabel "redundant"@en ; 
    skos:definition "The broadly-delimited, non-current status of a geologic feature that has been replaced in name by another term."@en ;
    skos:scopeNote """Preferably, and when required, in a clear published record (outlining the reasons for replacement/change, and any specific accord with a national, international and/or other code or protocol). The non-current status of a geologic feature may result from: a change in, or a correction to, its rank, status, spelling/citation; a change in its name (in the case of a lithostratigraphic unit) where a lithologic term, used as a component of its name, has been either applied, withdrawn, or revised; amendment/modification where stratigraphic or other geologic terminology has been incorrectly applied or there has been a paradigm change; a change to its name when it is replaced by a senior synonymn/equivalent or homonym; or when the name, or the primary (name-giving) part thereof, is pre-occupied. Lithostratigraphic examples of supersedence include: 'Brisbane tuff' (ASUD Strat. No. 2583, superseded) and 'Brisbane Tuffs' (ASUD Strat. No. 32126, superseded) replaced by 'Brisbane Tuff' [ASUD Strat No. 2579, formal (='current formal')]; Stanwell Coal Measures (ASUD Strat No. 17284) replaced by Stanwell Formation (Murray, 2007, Jell, 2013; absence of coal); and 'Taroom beds' (ASUD Strat No. 39590, superseded) replaced by 'Chong beds' (ASUD Strat No. 78567, 'current informal'), as 'Taroom' is preoccupied ('Taroom Coal Measures', ASUD Strat No. 24514, 'current formal'; Jell, 2013). [ASUD, Geoscience Australia, accessed 04.02.2021]."""@en ;
    skos:inScheme <http://linked.data.gov.au/def/gsq-feature-status> ;
    skos:prefLabel "superseded"@en ;
    skos:topConceptOf <http://linked.data.gov.au/def/gsq-feature-status> .
