@prefix dc: <http://purl.org/dc/elements/1.1/> .
@prefix dct: <http://purl.org/dc/terms/> .
@prefix owl: <http://www.w3.org/2002/07/owl#> .
@prefix qldcrs: <http://linked.data.gov.au/def/queensland-crs/> .
@prefix rdf: <http://www.w3.org/1999/02/22-rdf-syntax-ns#> .
@prefix rdfs: <http://www.w3.org/2000/01/rdf-schema#> .
@prefix skos: <http://www.w3.org/2004/02/skos/core#> .
@prefix xml: <http://www.w3.org/XML/1998/namespace> .
@prefix xsd: <http://www.w3.org/2001/XMLSchema#> .

<http://linked.data.gov.au/def/queensland-crs> a owl:Ontology , skos:ConceptScheme ;
    dct:created "2020-01-30T15:57:41"^^xsd:dateTime ;
    dct:creator "Geological Survey of Queensland" ;
    dct:modified "2020-01-30T15:57:41"^^xsd:dateTime ;
    dct:source "Compiled by the Geological Survey of Queensland" ;
    skos:definition "The coordinate reference systems used and refered to within Queensland"@en ;
    skos:hasTopConcept qldcrs:australian-geodetic-datum-1966,
        qldcrs:australian-geodetic-datum-1984,
        qldcrs:australian-map-grid-1966,
        qldcrs:australian-map-grid-1984,
        qldcrs:geocentric-datum-of-australia-1994,
        qldcrs:geocentric-datum-of-australia-2020,
        qldcrs:map-grid-of-australia-1994,
        qldcrs:map-grid-of-australia-2020,
        qldcrs:world-geodetic-system-1984 ;
    skos:prefLabel "Queensland CRS"@en .

qldcrs:geographic a skos:Collection ;
    skos:definition "A geographic coordinate system (GCS) is a coordinate system which uses a three-dimensional spherical surface (ellipsoid) to define locations on the earth. A common choice of coordinates is latitude and longitude."@en ;
    skos:member qldcrs:australian-geodetic-datum-1966,
        qldcrs:australian-geodetic-datum-1984,
        qldcrs:geocentric-datum-of-australia-1994,
        qldcrs:geocentric-datum-of-australia-2020
        qldcrs:world-geodetic-system-1984 ;
    skos:prefLabel "Geographic"@en .

qldcrs:projected a skos:Collection ;
    skos:definition "A projected coordinate system (PCS) is a projection of the geographic coordinate to, on two-dimensional surface (the map). The used to convert between Australian Geodetic Data and their Projected equivalents is the Universal Transverse Mercator projection."@en ;
    skos:member qldcrs:australian-map-grid-1966,
        qldcrs:australian-map-grid-1984,
        qldcrs:map-grid-of-australia-1994,
        qldcrs:map-grid-of-australia-2020 ;
    skos:prefLabel "Projected"@en .

qldcrs:geocentric-datum-of-australia-2020 a skos:Concept ;
    skos:definition "The official geodetic datum adopted nationally in January 2000. GDA94 is a coordinate reference system whose origin coincides with a determination of the centre of mass of the earth, hence the term geocentric. GDA94 is a plate-fixed or static coordinate datum based on the International Terrestrial Reference Frame 1992 (ITRF92), held at the reference epoch of 1 January 1994."@en ;
    skos:inScheme <http://linked.data.gov.au/def/queensland-crs> ;
    skos:notation "GDA2020" ;
    skos:prefLabel "Geocentric Datum of Australia 2020"@en ;
    skos:topConceptOf <http://linked.data.gov.au/def/queensland-crs> .

qldcrs:australian-geodetic-datum-1966 a skos:Concept ;
    skos:definition "The first official national Australian geodetic datum proclaimed in the Australian Commonwealth Gazette No. 84 of 6 October 1966."@en ;
    skos:inScheme <http://linked.data.gov.au/def/queensland-crs> ;
    skos:notation "AGD66" ;
    skos:prefLabel "Australian Geodetic Datum 1966"@en ;
    skos:topConceptOf <http://linked.data.gov.au/def/queensland-crs> .

qldcrs:australian-geodetic-datum-1984 a skos:Concept ;
    skos:definition "The update to the official Australian geodetic datum, adopted and in effect from 1984"@en ;
    skos:inScheme <http://linked.data.gov.au/def/queensland-crs> ;
    skos:notation "AGD84" ;
    skos:prefLabel "Australian Geodetic Datum 1984"@en ;
    skos:topConceptOf <http://linked.data.gov.au/def/queensland-crs> .

qldcrs:australian-map-grid-1966 a skos:Concept ;
    skos:definition "The accompanying national map projection to AGD66, a transverse Mercator projection that conforms to the internationally accepted Universal Transverse Mercator Grid system."@en ;
    skos:inScheme <http://linked.data.gov.au/def/queensland-crs> ;
    skos:notation "AMG66" ;
    skos:prefLabel "Australian Map Grid 1966"@en ;
    skos:topConceptOf <http://linked.data.gov.au/def/queensland-crs> .

qldcrs:australian-map-grid-1984 a skos:Concept ;
    skos:definition "The accompanying national map projection to AGD84, a transverse Mercator projection that conforms to the internationally accepted Universal Transverse Mercator Grid system."@en ;
    skos:inScheme <http://linked.data.gov.au/def/queensland-crs> ;
    skos:notation "AMG84" ;
    skos:prefLabel "Australian Map Grid 1984"@en ;
    skos:topConceptOf <http://linked.data.gov.au/def/queensland-crs> .

qldcrs:geocentric-datum-of-australia-1994 a skos:Concept ;
    skos:definition "The official geodetic datum adopted nationally in June 2020. GDA2020 is a coordinate reference system whose origin coincides with a determination of the centre of mass of the earth, hence the term geocentric. GDA2020 is a plate-fixed or static coordinate datum based on the International Terrestrial Reference Frame 1992 (ITRF92), held at the reference epoch of 1 January 2020."@en ;
    skos:inScheme <http://linked.data.gov.au/def/queensland-crs> ;
    skos:notation "GDA94" ;
    skos:prefLabel "Geocentric Datum of Australia 1994"@en ;
    skos:topConceptOf <http://linked.data.gov.au/def/queensland-crs> .

qldcrs:map-grid-of-australia-1994 a skos:Concept ;
    skos:definition "The accompanying national map projection to GDA94, a transverse Mercator projection that conforms to the internationally accepted Universal Transverse Mercator Grid system."@en ;
    skos:inScheme <http://linked.data.gov.au/def/queensland-crs> ;
    skos:notation "MGA94" ;
    skos:prefLabel "Map Grid of Australia 1994"@en ;
    skos:topConceptOf <http://linked.data.gov.au/def/queensland-crs> .

qldcrs:map-grid-of-australia-2020 a skos:Concept ;
    skos:definition "The accompanying national map projection to GDA2020, a transverse Mercator projection that conforms to the internationally accepted Universal Transverse Mercator Grid system."@en ;
    skos:inScheme <http://linked.data.gov.au/def/queensland-crs> ;
    skos:notation "MGA2020" ;
    skos:prefLabel "Map Grid of Australia 2020"@en ;
    skos:topConceptOf <http://linked.data.gov.au/def/queensland-crs> .

qldcrs:world-geodetic-system-1984 a skos:Concept ;
    skos:definition "The official world geodetic datum adopted in 1984. WGS84 is a coordinate reference system whose origin coincides with a determination of the centre of mass of the earth. The datum defines meridan 0 as IERS Reference Meridian and the datum surface is an oblate spheroid."@en ;
    skos:inScheme <http://linked.data.gov.au/def/queensland-crs> ;
    skos:notation "WGS84" ;
    skos:prefLabel "World Geodetic System 1984"@en ;
    skos:topConceptOf <http://linked.data.gov.au/def/queensland-crs> .
