@prefix dc: <http://purl.org/dc/elements/1.1/> .
@prefix dct: <http://purl.org/dc/terms/> .
@prefix gmps: <http://linked.data.gov.au/def/qld-resource-permit-status/> .
@prefix owl: <http://www.w3.org/2002/07/owl#> .
@prefix rdf: <http://www.w3.org/1999/02/22-rdf-syntax-ns#> .
@prefix rdfs: <http://www.w3.org/2000/01/rdf-schema#> .
@prefix skos: <http://www.w3.org/2004/02/skos/core#> .
@prefix xml: <http://www.w3.org/XML/1998/namespace> .
@prefix xsd: <http://www.w3.org/2001/XMLSchema#> .

<http://linked.data.gov.au/def/qld-resource-permit-status> a owl:Ontology .

gmps:conceptScheme a skos:ConceptScheme ;
    dct:created "2019-09-13"^^xsd:date ;
    dct:creator "Geological Survey of Queensland" ;
    dct:source "https://myminesonline.business.qld.gov.au" ;
    skos:definition "The stage in the life cycle of a Queensland Resource Permit."@en ;
    skos:hasTopConcept gmps:Abandoned,
        gmps:abandoned,
        gmps:application,
        gmps:granted,
        gmps:non-current,
        gmps:unsuccessful ;
    skos:prefLabel "Queensland Resource Permit Status"@en .

gmps:abandoned a skos:Concept ;
    skos:AltLabel "Discarded"@en ;
    skos:definition "An application for the permit that has been abandoned or discarded by the applicant."@en ;
    skos:inScheme gmps:conceptScheme ;
    skos:prefLabel "Abandoned"@en ;
    skos:topConceptOf gmps:conceptScheme .

gmps:application a skos:Concept ;
    skos:AltLabel "Not Accepted"@en,
        "Pre-Lodgement"@en,
        "Submitted"@en ;
    skos:definition "An application has been made for a permit."@en ;
    skos:inScheme gmps:conceptScheme ;
    skos:prefLabel "Application"@en ;
    skos:topConceptOf gmps:conceptScheme .

gmps:granted a skos:Concept ;
    skos:AltLabel "Current"@en ;
    skos:definition "A permit that has been granted under legislation."@en ;
    skos:inScheme gmps:conceptScheme ;
    skos:prefLabel "Granted"@en ;
    skos:topConceptOf gmps:conceptScheme .

gmps:non-current a skos:Concept ;
    skos:definition "A permit that was once granted but is now no longer active."@en ;
    skos:inScheme gmps:conceptScheme ;
    skos:prefLabel "Non-Current"@en ;
    skos:topConceptOf gmps:conceptScheme .

gmps:unsuccessful a skos:Concept ;
    skos:definition "An application for the permit was deemed unsuccessful by the Department."@en ;
    skos:inScheme gmps:conceptScheme ;
    skos:prefLabel "Unsuccessful"@en ;
    skos:topConceptOf gmps:conceptScheme .
