#Version 0.3

@prefix dc: <http://purl.org/dc/elements/1.1/> .
@prefix dct: <http://purl.org/dc/terms/> .
@prefix owl: <http://www.w3.org/2002/07/owl#> .
@prefix rdf: <http://www.w3.org/1999/02/22-rdf-syntax-ns#> .
@prefix rdfs: <http://www.w3.org/2000/01/rdf-schema#> .
@prefix skos: <http://www.w3.org/2004/02/skos/core#> .
@prefix xml: <http://www.w3.org/XML/1998/namespace> .
@prefix xsd: <http://www.w3.org/2001/XMLSchema#> .
@prefix gmps: <http://linked.data.gov.au/def/qld-resource-permit-status/> .

<http://linked.data.gov.au/def/qld-resource-permit-status> a owl:Ontology .

gmps:conceptScheme a skos:ConceptScheme ;
    dct:created "2019-09-13"^^xsd:date ;
    dct:creator "Geological Survey of Queensland" ;
    dct:source "https://myminesonline.business.qld.gov.au" ;
    skos:definition "The stage in the life cycle of a Queensland Resource Permit."@en ;
    skos:hasTopConcept gmps:application,
        gmps:granted,
        gmps:non-current ;
    skos:prefLabel "Queensland Resource Permit Status"@en .

gmps:abandoned a skos:Concept ;
    skos:definition "The Resource Permit was not granted and the Application has been abandoned by the applicant."@en ;
    skos:broader gmps:application,
    skos:inScheme gmps:conceptScheme ;
    skos:prefLabel "Abandoned"@en .

gmps:accepted a skos:Concept ;
    skos:definition "The application has been accepted."@en ;
    skos:broader gmps:granted ;
    skos:inScheme gmps:conceptScheme ;
    skos:prefLabel "Accepted"@en .

gmps:competing-application a skos:Concept ;
    skos:definition "This application represents a competing application that was lodged on the same date for the same mineral."@en ;
    skos:broader gmps:application,
        gmps:granted ;
    skos:inScheme gmps:conceptScheme ;
    skos:prefLabel "Competing application"@en .

gmps:conditionally-surrendered a skos:Concept ;
    skos:definition "The Resource Permit has been surrendered in favour of a new Resource Permit."@en ;
    skos:broader gmps:application,
    skos:inScheme gmps:conceptScheme ;
    skos:prefLabel "Conditionally surrendered"@en .

gmps:conversion-of-ml-to-mc a skos:Concept ;
    skos:definition "The Mining Lease has been converted to a Mining Claim."@en ;
    skos:broader gmps:granted ;
    skos:inScheme gmps:conceptScheme ;
    skos:prefLabel "Conversion of ML to MC"@en .

gmps:expired a skos:Concept ;
    skos:definition "The Resource Permit has expired."@en ;
    skos:broader gmps:granted,
    skos:inScheme gmps:conceptScheme ;
    skos:prefLabel "Expired"@en .

gmps:finalised a skos:Concept ;
    skos:definition "The Resource Permit has no outstanding requirements."@en ;
    skos:broader gmps:non-current ;
    skos:inScheme gmps:conceptScheme ;
    skos:prefLabel "Finalised"@en .

gmps:on-hold-oil-shale-application a skos:Concept ;
    skos:definition "The oil-shale application has been placed on-hold."@en ;
    skos:broader gmps:application ;
    skos:inScheme gmps:conceptScheme ;
    skos:prefLabel "On-hold oil shale application"@en .

gmps:preferred-tenderer a skos:Concept ;
    skos:definition "The applicant is the preferred tenderer."@en ;
    skos:broader gmps:application,
    skos:inScheme gmps:conceptScheme ;
    skos:prefLabel "Preferred Tenderer"@en .

gmps:priority-applicant a skos:Concept ;
    skos:definition "The applicant is a Priority Applicant for competing application."@en ;
    skos:broader gmps:application ;
    skos:inScheme gmps:conceptScheme ;
    skos:prefLabel "Priority Applicant"@en .

gmps:ranked a skos:Concept ;
    skos:definition "The application for the Resource Permit is a Ranked Application, pending grant of a Priority Application."@en ;
    skos:broader gmps:application ;
    skos:inScheme gmps:conceptScheme ;
    skos:prefLabel "Ranked"@en .

gmps:renewal-lodged a skos:Concept ;
    skos:definition "The Application of Renewal for the Resource Permit has been lodged."@en ;
    skos:broader gmps:granted,
    skos:inScheme gmps:conceptScheme ;
    skos:prefLabel "Renewal lodged"@en .

gmps:renewal-withdrawn a skos:Concept ;
    skos:definition "The Application of Renewal for the Resource Permit has been withdrawn."@en ;
    skos:broader gmps:granted,
    skos:inScheme gmps:conceptScheme ;
    skos:prefLabel "Renewal withdrawn"@en .

gmps:replacement-permit-application a skos:Concept ;
    skos:definition "The application represents a Replacement Permit Application."@en ;
    skos:broader gmps:application,
        gmps:granted ;
    skos:inScheme gmps:conceptScheme ;
    skos:prefLabel "Replacement Permit Application"@en .

gmps:unfinalised a skos:Concept ;
    skos:definition "The Resource Permit has been terminated, but there are some outstanding requirements to be completed, to be compliant with the resources legislation."@en ;
    skos:broader gmps:non-current,
    skos:inScheme gmps:conceptScheme ;
    skos:prefLabel "Unfinalised"@en .

gmps:unsuccessful-application a skos:Concept ;
    skos:definition "The application represents an unsuccessful application."@en ;
    skos:broader gmps:application,
    skos:inScheme gmps:conceptScheme ;
    skos:prefLabel "Unsuccessful application"@en .

gmps:granted a skos:Concept ;
    skos:definition "The Resource Permit has been approved under the Resource Authority Legislation"@en ;
    skos:inScheme gmps:conceptScheme ;
    skos:prefLabel "Granted"@en ;
    skos:topConceptOf gmps:conceptScheme .

gmps:application a skos:Concept ;
    skos:definition "An application has been submitted and an outcome is pending."@en ;
    skos:inScheme gmps:conceptScheme ;
    skos:prefLabel "Application"@en ;
    skos:topConceptOf gmps:conceptScheme .

gmps:non-current a skos:Concept ;
    skos:definition "The Resource Permit has been terminated in the system and is longer current."@en ;
    skos:inScheme gmps:conceptScheme ;
    skos:prefLabel "Non-current"@en ;
    skos:topConceptOf gmps:conceptScheme .
