@prefix dcterms: <http://purl.org/dc/terms/> .
@prefix owl: <http://www.w3.org/2002/07/owl#> .
@prefix sdo: <https://schema.org/> .
@prefix skos: <http://www.w3.org/2004/02/skos/core#> .
@prefix smprl: <http://linked.data.gov.au/def/sample-relationship/> .
@prefix xsd: <http://www.w3.org/2001/XMLSchema#> .

<http://linked.data.gov.au/def/sample-relationship> a owl:Ontology,
        skos:ConceptScheme ;
    dcterms:created "2020-03-24"^^xsd:date ;
    dcterms:creator <http://linked.data.gov.au/org/gsq> ;
    dcterms:modified "2020-04-06"^^xsd:date ;
    dcterms:publisher <http://linked.data.gov.au/org/gsq> ;
    dcterms:source """Source information from https://www.w3.org/TR/vocab-ssn/#Sample_Relations modified by the Geological Survey of Queensland.""" ;
    skos:definition "Samples are often related to other samples, by sub-sampling, topological relationships (stations along a traverse, pixels within an image, probe spots on a polished section, specimens retrieved within a borehole) or as parts of sample processing chains (crushing, splitting, dissecting, disolving). There are an essentially unlimited set of relationships between samples, so the nature of the relationship has its own class."@en ;
    skos:prefLabel "Sample Relationship"@en ;
    skos:hasTopConcept smprl:has-originalsample,
        smprl:has-sample,
        smprl:is-sample-of .
    
<http://linked.data.gov.au/org/gsq> a sdo:Organization ;
    sdo:name "Geological Survey of Queensland" ;
    sdo:url <https://www.business.qld.gov.au/industries/mining-energy-water/resources/geoscience-information/gsq> .

smprl:has-originalsample a skos:Concept ;
    skos:definition "The link to the original sample that is related to the context sample through a chain of isSampleOf relations"@en ;
    skos:inScheme <http://linked.data.gov.au/def/sample-relationship> ;
    skos:notation "hasOriginalSample" ;
    skos:prefLabel "Has OriginalSample"@en ;
    skos:topConceptOf <http://linked.data.gov.au/def/sample-relationship> .

smprl:has-sample a skos:Concept ;
    skos:definition "Relation between a FeatureOfInterest, Site, or parent Sample and the Sample used to represent it."@en ;
    skos:inScheme <http://linked.data.gov.au/def/sample-relationship> ;
    skos:notation "hasSample" ;
    skos:prefLabel "Has Sample"@en ;
    skos:topConceptOf <http://linked.data.gov.au/def/sample-relationship> .

smprl:is-sample-of a skos:Concept ;
    skos:definition "Relation from a Sample to the FeatureOfInterest, Site, or parent Sample that it is intended to be representative of."@en ;
    skos:inScheme <http://linked.data.gov.au/def/sample-relationship> ;
    skos:notation "isSampleOf" ;
    skos:prefLabel "Is Sample Of"@en ;
    skos:topConceptOf <http://linked.data.gov.au/def/sample-relationship> .
