@prefix dc: <http://purl.org/dc/elements/1.1/> .
@prefix dct: <http://purl.org/dc/terms/> .
@prefix locdt: <http://linked.data.gov.au/def/sample-location-types/> .
@prefix owl: <http://www.w3.org/2002/07/owl#> .
@prefix rdf: <http://www.w3.org/1999/02/22-rdf-syntax-ns#> .
@prefix rdfs: <http://www.w3.org/2000/01/rdf-schema#> .
@prefix skos: <http://www.w3.org/2004/02/skos/core#> .
@prefix xml: <http://www.w3.org/XML/1998/namespace> .
@prefix xsd: <http://www.w3.org/2001/XMLSchema#> .


<http://linked.data.gov.au/def/sample-location-types> a owl:Ontology , skos:ConceptScheme ;
    dct:created "2020-02-07T11:48:51"^^xsd:dateTime ;
    dct:creator "Geological Survey of Queensland" ;
    dct:modified "2020-02-07T11:48:51"^^xsd:dateTime ;
    dct:source "Compiled by the Geological Survey of Queensland" ;
    skos:definition "Indexed storage items and locations used in storage facilities for inventory management and warehousing."@en ;
    skos:hasTopConcept locdt:bag,
        locdt:bin,
        locdt:cabinet,
        locdt:drawer,
        locdt:drum,
        locdt:dumpster,
        locdt:envelope,
        locdt:folder,
        locdt:pallet,
        locdt:rack,
        locdt:room,
        locdt:table,
        locdt:tray ;
    skos:prefLabel "Sample Location Types"@en .

locdt:bag a skos:Concept ;
    skos:altLabel "Pack"@en,
        "Pouch"@en,
        "Sac"@en,
        "Sack"@en ;
    skos:definition "A flexible container with an opening at the top, used for carrying or storing things."@en ;
    skos:inScheme <http://linked.data.gov.au/def/sample-location-types> ;
    skos:prefLabel "Bag"@en ;
    skos:topConceptOf <http://linked.data.gov.au/def/sample-location-types> .
    
locdt:bin a skos:Concept ;
    skos:definition "A capacious receptacle for storing a substances and/or artifacts."@en ;
    skos:inScheme <http://linked.data.gov.au/def/sample-location-types> ;
    skos:prefLabel "Bin"@en ;
    skos:topConceptOf <http://linked.data.gov.au/def/sample-location-types> .

locdt:cabinet a skos:Concept ;
    skos:altLabel "Cupboard"@en ;
    skos:definition "An enclosed piece of furniture, typically with internal shelves for the storage and organisation of items."@en ;
    skos:inScheme <http://linked.data.gov.au/def/sample-location-types> ;
    skos:prefLabel "Cabinet"@en ;
    skos:topConceptOf <http://linked.data.gov.au/def/sample-location-types> .

locdt:drawer a skos:Concept ;
    skos:altLabel "Draw"@en ;
    skos:definition "A a box-shaped container that fits into a piece of furniture in such a way that it can be drawn out horizontally to reach its contents."@en ;
    skos:inScheme <http://linked.data.gov.au/def/sample-location-types> ;
    skos:prefLabel "Drawer"@en ;
    skos:topConceptOf <http://linked.data.gov.au/def/sample-location-types> .

locdt:drum a skos:Concept ;
    skos:altLabel "Amphora"@en,
        "Barrel"@en,
        "Cask"@en,
        "Vat"@en ;
    skos:definition "A hollow cylindrical container with a bulging center, longer than it is wide."@en ;
    skos:inScheme <http://linked.data.gov.au/def/sample-location-types> ;
    skos:prefLabel "Drum"@en ;
    skos:topConceptOf <http://linked.data.gov.au/def/sample-location-types> .

locdt:dumpster a skos:Concept ;
    skos:definition "A movable waste container designed to be brought and taken away by a special collection vehicle, or to a bin that a specially designed garbage truck lifts, empties into its hopper, and lowers, on the spot."@en ;
    skos:inScheme <http://linked.data.gov.au/def/sample-location-types> ;
    skos:prefLabel "Dumpster"@en ;
    skos:topConceptOf <http://linked.data.gov.au/def/sample-location-types> .

locdt:envelope a skos:Concept ;
    skos:altLabel "File Folder"@en ;
    skos:definition "A packaging item, usually made of thin, flat material. It is designed to contain a flat object or objects, such as a letter, document, or card."@en ;
    skos:inScheme <http://linked.data.gov.au/def/sample-location-types> ;
    skos:prefLabel "Envelope"@en ;
    skos:topConceptOf <http://linked.data.gov.au/def/sample-location-types> .

locdt:folder a skos:Concept ;
    skos:definition "A sheet of heavy paper stock or other thin, but stiff, material which is folded in half, and used to keep paper documents or other flat items."@en ;
    skos:inScheme <http://linked.data.gov.au/def/sample-location-types> ;
    skos:prefLabel "Folder"@en ;
    skos:topConceptOf <http://linked.data.gov.au/def/sample-location-types> .

locdt:pallet a skos:Concept ;
    skos:definition "A flat transport structure, which supports goods in a stable fashion while being lifted by a forklift, a pallet jack, a front loader, a jacking device, or an erect crane."@en ;
    skos:inScheme <http://linked.data.gov.au/def/sample-location-types> ;
    skos:prefLabel "Pallet"@en ;
    skos:topConceptOf <http://linked.data.gov.au/def/sample-location-types> .

locdt:rack a skos:Concept ;
    skos:definition "A material handling storage aid system designed to store materials on pallets or other standard storage platforms."@en ;
    skos:inScheme <http://linked.data.gov.au/def/sample-location-types> ;
    skos:prefLabel "Rack"@en ;
    skos:topConceptOf <http://linked.data.gov.au/def/sample-location-types> .

locdt:room a skos:Concept ;
    skos:definition "Any enclosed space with walls, a ceiling and one-or-many entrances."@en ;
    skos:inScheme <http://linked.data.gov.au/def/sample-location-types> ;
    skos:prefLabel "Room"@en ;
    skos:topConceptOf <http://linked.data.gov.au/def/sample-location-types> .

locdt:table a skos:Concept ;
    skos:definition "An item of furniture with a flat top and one or more legs, used as a surface for working at or storing items."@en ;
    skos:inScheme <http://linked.data.gov.au/def/sample-location-types> ;
    skos:prefLabel "Table"@en ;
    skos:topConceptOf <http://linked.data.gov.au/def/sample-location-types> .

locdt:tray a skos:Concept ;
    skos:definition "A shallow platform designed for the carrying or storing of items."@en ;
    skos:inScheme <http://linked.data.gov.au/def/sample-location-types> ;
    skos:prefLabel "Tray"@en ;
    skos:topConceptOf <http://linked.data.gov.au/def/sample-location-types> .
