@prefix ststs: <http://linked.data.gov.au/def/site-status/> .
@prefix dc: <http://purl.org/dc/elements/1.1/> .
@prefix dct: <http://purl.org/dc/terms/> .
@prefix owl: <http://www.w3.org/2002/07/owl#> .
@prefix rdf: <http://www.w3.org/1999/02/22-rdf-syntax-ns#> .
@prefix rdfs: <http://www.w3.org/2000/01/rdf-schema#> .
@prefix skos: <http://www.w3.org/2004/02/skos/core#> .
@prefix xml: <http://www.w3.org/XML/1998/namespace> .
@prefix xsd: <http://www.w3.org/2001/XMLSchema#> .

<http://linked.data.gov.au/def/site-status> a owl:Ontology , skos:ConceptScheme ;
    dct:creator "Geological Survey of Queensland" ;
    dct:modified "2020-01-21T11:52:35"^^xsd:dateTime;
    dct:created "2020-02-07T14:52:42"^^xsd:dateTime ;
    dct:source "Compiled by the Geological Survey of Queensland" ;
    skos:definition "The status of a site describing the lifecycle of a site in the context of a project or survey. Lifecycle stages are commonly related to regulatory conditions administered by government agencies."@en ;
    skos:hasTopConcept ststs:abandoned,
        ststs:active,
        ststs:never-used,
        ststs:proposed,
        ststs:unknown ;
    skos:prefLabel "Site status"@en .

ststs:abandoned a skos:Concept ;
    skos:definition "A site that has been abandoned or usage has been completed."@en ;
    skos:inScheme <http://linked.data.gov.au/def/site-status> ;
    skos:prefLabel "Abandoned"@en ;
    skos:topConceptOf <http://linked.data.gov.au/def/site-status> .

ststs:active a skos:Concept ;
    skos:definition "A site in an active state of measuring, sampling or surveying."@en ;
    skos:inScheme <http://linked.data.gov.au/def/site-status> ;
    skos:prefLabel "Active"@en ;
    skos:topConceptOf <http://linked.data.gov.au/def/site-status> .

ststs:never-used a skos:Concept ;
    skos:definition "A site that was proposed but was never used as a survey location and is no longer intended to be used for its original purpose."@en ;
    skos:inScheme <http://linked.data.gov.au/def/site-status> ;
    skos:prefLabel "Never Used"@en ;
    skos:topConceptOf <http://linked.data.gov.au/def/site-status> .

ststs:proposed a skos:Concept ;
    skos:definition "A proposed survey site is not yet in-use."@en ;
    skos:inScheme <http://linked.data.gov.au/def/site-status> ;
    skos:prefLabel "Proposed"@en ;
    skos:topConceptOf <http://linked.data.gov.au/def/site-status> .

ststs:unknown a skos:Concept ;
    skos:definition "A site that has been surveyed or sampled, but whose further status is unknown."@en ;
    skos:inScheme <http://linked.data.gov.au/def/site-status> ;
    skos:prefLabel "Unknown"@en ;
    skos:topConceptOf <http://linked.data.gov.au/def/site-status> .
