@prefix skos: <http://www.w3.org/2004/02/skos/core#> .
@prefix dcterms: <http://purl.org/dc/terms/> .
@prefix rdf: <http://www.w3.org/1999/02/22-rdf-syntax-ns#> .
@prefix rdfs: <http://www.w3.org/2000/01/rdf-schema#> .
@prefix xml: <http://www.w3.org/XML/1998/namespace> .
@prefix xsd: <http://www.w3.org/2001/XMLSchema#> .

<http://linked.data.gov.au/def/tern-cv/5699eca7-9ef0-47a6-bcfb-9306e0e2b85e> a skos:ConceptScheme ;
    dcterms:created "2020-11-04T04:34:29"^^xsd:datetime ;
    dcterms:modified "2020-11-04T05:42:24"^^xsd:datetime ;
    dcterms:publisher <https://linkeddata.tern.org.au/> ;
    skos:prefLabel "Parameters Scheme"@en ;
    rdfs:isDefinedBy <http://linked.data.gov.au/def/tern-cv/5699eca7-9ef0-47a6-bcfb-9306e0e2b85e> ; 
    dcterms:provenance "Derived from TERN Core Vocabulary (https://linkeddata.tern.org.au/viewer/tern)"@en ; 
    skos:definition "A profile of the TERN Core Vocabulary of relevance to Queensland Environmental Science Data (QESD)."@en ;
    skos:editorialNote "The concepts and properties included here are from a copy from public TERN resources, with a slimmed down set of terms that are needed for the Queensland Environmental Science Data (QESD) Catalogue."@en ;
    skos:hasTopConcept <http://linked.data.gov.au/def/tern-cv/123f2efe-3891-4764-9047-609c8b30e925>,
        <http://linked.data.gov.au/def/tern-cv/29bd4356-5638-49c0-8d3e-57598ac2ea6c>,
        <http://linked.data.gov.au/def/tern-cv/2ffe4363-dea1-4188-9f8f-835983d47fe2>,
        <http://linked.data.gov.au/def/tern-cv/41a27c10-6dff-4ddc-9f8b-14e87fafc786>,
        <http://linked.data.gov.au/def/tern-cv/45ae73d8-92bd-4261-a05f-7bfac228e1f7>,
        <http://linked.data.gov.au/def/tern-cv/50b9def1-660b-4274-b10e-6dbe57243305>,
        <http://linked.data.gov.au/def/tern-cv/68add852-0a47-4412-8f8c-52bd8d0151b1>,
        <http://linked.data.gov.au/def/tern-cv/6e2ede4b-1e6f-4ea0-93d9-6597c5666d62>,
        <http://linked.data.gov.au/def/tern-cv/6f726a59-c330-44eb-898e-7d42d5fbdada>,
        <http://linked.data.gov.au/def/tern-cv/777773d0-cfb4-44ff-85e2-08b48e10ac52>,
        #<http://linked.data.gov.au/def/tern-cv/8e7a785a-8c57-4415-855f-cb6d35ad58bb>,
        <http://linked.data.gov.au/def/tern-cv/8fa1c4bd-73b3-432a-ab49-9ee89928e6d9>,
        <http://linked.data.gov.au/def/tern-cv/99bd0128-54d4-4a2b-8a2c-48010eb07d26>,
        <http://linked.data.gov.au/def/tern-cv/9e03a73d-8e89-4187-9f96-0306aad93458>,
        <http://linked.data.gov.au/def/tern-cv/bb5c1354-8d70-47b2-b333-87e3bf1157d6>,
        <http://linked.data.gov.au/def/tern-cv/c_012ebf32>,
        <http://linked.data.gov.au/def/tern-cv/d62a4664-89a1-49a1-9ef0-f30ee2c6d22b> ;
    skos:narrower <http://linked.data.gov.au/def/tern-cv/0986ce8c-4a8c-4132-91f9-b7380d45ce73>,
        <http://linked.data.gov.au/def/tern-cv/6c73ea38-c3d6-49bf-b6e9-4042d09bbee0>,
        <http://linked.data.gov.au/def/tern-cv/87ed6ce4-3354-4a3f-ba15-2b7cb0caf3da> ;
.

<http://linked.data.gov.au/def/tern-cv/29bd4356-5638-49c0-8d3e-57598ac2ea6c> a skos:Concept ;
    dcterms:created "2020-11-09T04:58:26"^^xsd:datetime ;
    dcterms:modified "2021-01-04T23:49:32"^^xsd:datetime ;
    skos:definition "The traits, patterns, and structure of a specific geographic area, including its biological composition, its physical environment, and its anthropogenic or social patterns. An area where interacting ecosystems are grouped and repeated in similar form."@en ;
    skos:inScheme <http://linked.data.gov.au/def/tern-cv/5699eca7-9ef0-47a6-bcfb-9306e0e2b85e> ;
    rdfs:isDefinedBy <http://linked.data.gov.au/def/tern-cv/5699eca7-9ef0-47a6-bcfb-9306e0e2b85e> ; 
    skos:narrower <http://linked.data.gov.au/def/tern-cv/0a92253d-a07b-4762-b653-4c363650cb44>,
        <http://linked.data.gov.au/def/tern-cv/18a1be66-3340-4db1-9731-a8ceb4118db9>,
        <http://linked.data.gov.au/def/tern-cv/2b5ac7b3-b4bf-4a06-97d6-8dee8b32d72d>,
        <http://linked.data.gov.au/def/tern-cv/647833d8-bba7-4115-b264-f9fc36c9195c>,
        <http://linked.data.gov.au/def/tern-cv/78b617e9-cd18-40b7-ad38-efc30579e680>,
        <http://linked.data.gov.au/def/tern-cv/7fa47d4b-1139-4d24-8ef2-8732ff64de4a>,
        <http://linked.data.gov.au/def/tern-cv/a40230bc-c1e9-4309-b883-c4ead1d143ce> ;
    skos:prefLabel "landscape parameter"@en ;
    skos:topConceptOf <http://linked.data.gov.au/def/tern-cv/5699eca7-9ef0-47a6-bcfb-9306e0e2b85e> .

<http://linked.data.gov.au/def/tern-cv/3a03227d-1b66-4c63-b7aa-f9ccbb70d1cf> a skos:Concept ;
    dcterms:created "2021-02-03T07:25:56"^^xsd:datetime ;
    dcterms:modified "2021-02-19T05:10:28"^^xsd:datetime ;
    skos:broader <http://linked.data.gov.au/def/tern-cv/41a27c10-6dff-4ddc-9f8b-14e87fafc786>,
        <http://linked.data.gov.au/def/tern-cv/99bd0128-54d4-4a2b-8a2c-48010eb07d26> ;
    skos:definition "Indicator of possible areas of hydroxyl minerals abundance across a landscape, for example hydroxyl-bearing clays, sulphates and carbonates. Calculated from a combination of spectral bands of satellite imagery, the indicator may vary in effectiveness across the landscape."@en ;
    skos:inScheme <http://linked.data.gov.au/def/tern-cv/5699eca7-9ef0-47a6-bcfb-9306e0e2b85e> ;
    rdfs:isDefinedBy <http://linked.data.gov.au/def/tern-cv/5699eca7-9ef0-47a6-bcfb-9306e0e2b85e> ; 
    skos:narrower <http://linked.data.gov.au/def/tern-cv/01a87ba3-0f0d-4854-8196-3e3d80010faf>,
        <http://linked.data.gov.au/def/tern-cv/1a7c69c6-8d8b-49c9-9f65-f3e288a6c33c>,
        <http://linked.data.gov.au/def/tern-cv/2e57142c-817d-420b-a097-e62f379afecc>,
        <http://linked.data.gov.au/def/tern-cv/5cba467e-a595-42fd-a177-2ac8e83ce17d>,
        <http://linked.data.gov.au/def/tern-cv/70c1e9c4-2949-4e49-a8ef-6c4c45dd5b65>,
        <http://linked.data.gov.au/def/tern-cv/f75ff7d2-d525-4a76-939b-5fa43f1e9d77> ;
    skos:prefLabel "hydroxyl minerals indices"@en .

<http://linked.data.gov.au/def/tern-cv/7dc7ae5c-f074-4536-9032-f59eba3f9270> a skos:Concept ;
    dcterms:created "2020-11-04T05:25:31"^^xsd:datetime ;
    dcterms:modified "2020-12-19T07:34:22"^^xsd:datetime ;
    skos:broader <http://linked.data.gov.au/def/tern-cv/d62a4664-89a1-49a1-9ef0-f30ee2c6d22b> ;
    skos:definition "Amount of ground covered by some material or bare; usually estimated as a percentage."@en ;
    skos:inScheme <http://linked.data.gov.au/def/tern-cv/5699eca7-9ef0-47a6-bcfb-9306e0e2b85e> ;
    rdfs:isDefinedBy <http://linked.data.gov.au/def/tern-cv/5699eca7-9ef0-47a6-bcfb-9306e0e2b85e> ; 
    skos:narrower <http://linked.data.gov.au/def/tern-cv/4392769d-ab14-4575-af5a-103e133eee3f>,
        <http://linked.data.gov.au/def/tern-cv/8b26b66b-9e39-47eb-807f-621f1119377d>,
        <http://linked.data.gov.au/def/tern-cv/998a886b-d40d-43cd-ac1a-0a682018b4e5>,
        <http://linked.data.gov.au/def/tern-cv/ab4ef0b1-bae1-476e-84c5-612e18282022>,
        <http://linked.data.gov.au/def/tern-cv/b053c016-d21f-4180-aaf5-f7f6f892325d>,
        <http://linked.data.gov.au/def/tern-cv/b31f9f9d-090f-46e7-b03c-36ca696621f5>,
        <http://linked.data.gov.au/def/tern-cv/cbff6d0c-c239-4858-8139-9fbd8c8646df>,
        <http://linked.data.gov.au/def/tern-cv/e06a20d2-ad09-4cf8-bb4b-9ebd66ed10b7>,
        <http://linked.data.gov.au/def/tern-cv/e3b19733-defc-417d-9513-f9260b9553af>,
        <http://linked.data.gov.au/def/tern-cv/e9d2e691-dd18-4a38-a987-2fa48c7d5562> ;
    skos:prefLabel "ground cover"@en .

<http://linked.data.gov.au/def/tern-cv/41a27c10-6dff-4ddc-9f8b-14e87fafc786> a skos:Concept ;
    dcterms:created "2020-11-09T04:57:22"^^xsd:datetime ;
    dcterms:modified "2020-12-19T07:17:47"^^xsd:datetime ;
    skos:definition "Related to the properties, composition, and structure of matter, the changes in structure and composition of matter, and energy changes."@en ;
    skos:inScheme <http://linked.data.gov.au/def/tern-cv/5699eca7-9ef0-47a6-bcfb-9306e0e2b85e> ;
    rdfs:isDefinedBy <http://linked.data.gov.au/def/tern-cv/5699eca7-9ef0-47a6-bcfb-9306e0e2b85e> ; 
    skos:narrower <http://linked.data.gov.au/def/tern-cv/12797115-2e0f-479f-8d06-1700da3ac394>,
        <http://linked.data.gov.au/def/tern-cv/1aa6aa3b-eb0a-47f0-9bc1-61c0b375fe73>,
        <http://linked.data.gov.au/def/tern-cv/26526741-5aa1-4cfa-9512-1d3182ea3b13>,
        <http://linked.data.gov.au/def/tern-cv/3a03227d-1b66-4c63-b7aa-f9ccbb70d1cf>,
        <http://linked.data.gov.au/def/tern-cv/57524a84-ddfa-4dfd-8bfe-878dcd826226>,
        <http://linked.data.gov.au/def/tern-cv/66d5552f-fa72-4032-8ac5-e087b214b770>,
        <http://linked.data.gov.au/def/tern-cv/700daf25-0a3f-461e-a799-be80ef2f8cd4>,
        <http://linked.data.gov.au/def/tern-cv/a54f0994-bac3-42e4-83d3-46c33affd8a9>,
        <http://linked.data.gov.au/def/tern-cv/a5cdedc4-6bdf-4f2d-922b-5d17ae957735>,
        <http://linked.data.gov.au/def/tern-cv/c06b51c6-8290-40bf-b192-b0dc2b44fde1>,
        <http://linked.data.gov.au/def/tern-cv/d4c0646c-2504-496b-bd01-95c1097b5021>,
        <http://linked.data.gov.au/def/tern-cv/fc383c4d-b8d2-4dbf-b897-5f511208ada1> ;
    skos:prefLabel "chemical parameter"@en ;
    skos:topConceptOf <http://linked.data.gov.au/def/tern-cv/5699eca7-9ef0-47a6-bcfb-9306e0e2b85e> .

<http://linked.data.gov.au/def/tern-cv/6f726a59-c330-44eb-898e-7d42d5fbdada> a skos:Concept ;
    dcterms:created "2021-03-11T04:17:12"^^xsd:datetime ;
    skos:inScheme <http://linked.data.gov.au/def/tern-cv/5699eca7-9ef0-47a6-bcfb-9306e0e2b85e> ;
    rdfs:isDefinedBy <http://linked.data.gov.au/def/tern-cv/5699eca7-9ef0-47a6-bcfb-9306e0e2b85e> ; 
    skos:narrower <http://linked.data.gov.au/def/tern-cv/1d1a868a-74f9-4d7b-8d70-f97d9530098e>,
        <http://linked.data.gov.au/def/tern-cv/28874068-9b9b-49b0-a754-0b7bd988d97c>,
        <http://linked.data.gov.au/def/tern-cv/29241828-9973-4854-a4b9-e972cd58c22a>,
        <http://linked.data.gov.au/def/tern-cv/3ab5a014-78d0-4424-9329-8dc370701f1a>,
        <http://linked.data.gov.au/def/tern-cv/486e60ea-affa-45ad-b331-027167d866bf>,
        <http://linked.data.gov.au/def/tern-cv/5a95ac61-94c5-4993-aad2-3e891156efe0>,
        <http://linked.data.gov.au/def/tern-cv/5d13d5e9-4465-4c75-8a41-60bf84882696>,
        <http://linked.data.gov.au/def/tern-cv/71934567-a90d-433c-a040-63df566c9faa>,
        <http://linked.data.gov.au/def/tern-cv/800cf33b-1c44-435d-89bd-5d80e3e8aba1>,
        <http://linked.data.gov.au/def/tern-cv/8c20f342-39fd-4abf-ab97-218c7c1ce499>,
        <http://linked.data.gov.au/def/tern-cv/be1916fa-a0cf-4e86-a0dc-dd49f7a78af7>,
        <http://linked.data.gov.au/def/tern-cv/c5f99536-8986-418e-932d-ae5d77312adc>,
        <http://linked.data.gov.au/def/tern-cv/d33f60ee-1934-4bd8-9919-06c0d54eee1a>,
        <http://linked.data.gov.au/def/tern-cv/ff4ce8d1-4c2b-4d6e-8aea-be4138fea452> ;
    skos:prefLabel "land surface parameter"@en ;
    skos:definition "land surface parameters"@en ;
    skos:topConceptOf <http://linked.data.gov.au/def/tern-cv/5699eca7-9ef0-47a6-bcfb-9306e0e2b85e> .

<http://linked.data.gov.au/def/tern-cv/777773d0-cfb4-44ff-85e2-08b48e10ac52> a skos:Concept ;
    dcterms:created "2021-02-26T03:30:24"^^xsd:datetime ;
    dcterms:modified "2021-03-11T03:53:45"^^xsd:datetime ;
    skos:inScheme <http://linked.data.gov.au/def/tern-cv/5699eca7-9ef0-47a6-bcfb-9306e0e2b85e> ;
    rdfs:isDefinedBy <http://linked.data.gov.au/def/tern-cv/5699eca7-9ef0-47a6-bcfb-9306e0e2b85e> ; 
    skos:narrower <http://linked.data.gov.au/def/tern-cv/18d64def-df3b-4fa2-ba2d-967c6e392406>,
        <http://linked.data.gov.au/def/tern-cv/1d1a868a-74f9-4d7b-8d70-f97d9530098e>,
        <http://linked.data.gov.au/def/tern-cv/20a2ab2e-cdbd-4c56-9e68-9c926fd589eb>,
        <http://linked.data.gov.au/def/tern-cv/28874068-9b9b-49b0-a754-0b7bd988d97c>,
        <http://linked.data.gov.au/def/tern-cv/29241828-9973-4854-a4b9-e972cd58c22a>,
        <http://linked.data.gov.au/def/tern-cv/3826b5a3-7128-4df3-90f3-8196c4c20d45>,
        <http://linked.data.gov.au/def/tern-cv/3ab5a014-78d0-4424-9329-8dc370701f1a>,
        <http://linked.data.gov.au/def/tern-cv/486e60ea-affa-45ad-b331-027167d866bf>,
        <http://linked.data.gov.au/def/tern-cv/4e272650-c4f7-412b-b7bf-031af0611acc>,
        <http://linked.data.gov.au/def/tern-cv/5a95ac61-94c5-4993-aad2-3e891156efe0>,
        <http://linked.data.gov.au/def/tern-cv/5d13d5e9-4465-4c75-8a41-60bf84882696>,
        <http://linked.data.gov.au/def/tern-cv/71934567-a90d-433c-a040-63df566c9faa>,
        <http://linked.data.gov.au/def/tern-cv/79b5755c-6de7-42e9-a652-c402faec2826>,
        <http://linked.data.gov.au/def/tern-cv/7e75402d-e3c6-41dd-9e17-7f44b26bbb10>,
        <http://linked.data.gov.au/def/tern-cv/800cf33b-1c44-435d-89bd-5d80e3e8aba1>,
        <http://linked.data.gov.au/def/tern-cv/8c20f342-39fd-4abf-ab97-218c7c1ce499>,
        <http://linked.data.gov.au/def/tern-cv/8f220426-6b5a-4b8f-a995-8eea263a4a19>,
        <http://linked.data.gov.au/def/tern-cv/a8e12e7f-6052-4e87-a69e-ceb34ad5c45d>,
        <http://linked.data.gov.au/def/tern-cv/b0dff759-ae91-4801-b520-b27e27215a40>,
        <http://linked.data.gov.au/def/tern-cv/be1916fa-a0cf-4e86-a0dc-dd49f7a78af7>,
        <http://linked.data.gov.au/def/tern-cv/c55de6b4-72f2-42ad-ad6e-f611db272e78>,
        <http://linked.data.gov.au/def/tern-cv/c5f99536-8986-418e-932d-ae5d77312adc>,
        <http://linked.data.gov.au/def/tern-cv/d33f60ee-1934-4bd8-9919-06c0d54eee1a>,
        <http://linked.data.gov.au/def/tern-cv/d5635c66-06d2-48e4-98ff-7e83e8a2b265>,
        <http://linked.data.gov.au/def/tern-cv/f3888501-98b1-4a53-a788-20b0f0b8a7e6>,
        <http://linked.data.gov.au/def/tern-cv/f57f6bf8-2a5e-47c5-bcc2-4ce7bb4b9dc7>,
        <http://linked.data.gov.au/def/tern-cv/fe9c70d4-415b-4152-b517-a8e7a15e36f7>,
        <http://linked.data.gov.au/def/tern-cv/ff4ce8d1-4c2b-4d6e-8aea-be4138fea452> ;
    skos:prefLabel "disturbance parameter"@en ;
    skos:definition "disturbance parameters"@en ;
    skos:topConceptOf <http://linked.data.gov.au/def/tern-cv/5699eca7-9ef0-47a6-bcfb-9306e0e2b85e> .

<http://linked.data.gov.au/def/tern-cv/8fa1c4bd-73b3-432a-ab49-9ee89928e6d9> a skos:Concept ;
    dcterms:created "2021-03-11T04:54:26"^^xsd:datetime ;
    dcterms:modified "2021-03-11T04:54:54"^^xsd:datetime ;
    rdfs:isDefinedBy <http://linked.data.gov.au/def/tern-cv/5699eca7-9ef0-47a6-bcfb-9306e0e2b85e> ; 
    skos:inScheme <http://linked.data.gov.au/def/tern-cv/5699eca7-9ef0-47a6-bcfb-9306e0e2b85e> ;
    skos:narrower <http://linked.data.gov.au/def/tern-cv/07abcf97-542d-4c2f-9fb1-c7c7508f484c>,
        <http://linked.data.gov.au/def/tern-cv/18d64def-df3b-4fa2-ba2d-967c6e392406>,
        <http://linked.data.gov.au/def/tern-cv/20a2ab2e-cdbd-4c56-9e68-9c926fd589eb>,
        <http://linked.data.gov.au/def/tern-cv/3826b5a3-7128-4df3-90f3-8196c4c20d45>,
        <http://linked.data.gov.au/def/tern-cv/46911a2e-826e-49bd-8150-830dd6a72cf3>,
        <http://linked.data.gov.au/def/tern-cv/4e272650-c4f7-412b-b7bf-031af0611acc>,
        <http://linked.data.gov.au/def/tern-cv/56195246-ec5d-4050-a1c6-af786fbec715>,
        <http://linked.data.gov.au/def/tern-cv/79b5755c-6de7-42e9-a652-c402faec2826>,
        <http://linked.data.gov.au/def/tern-cv/7e75402d-e3c6-41dd-9e17-7f44b26bbb10>,
        <http://linked.data.gov.au/def/tern-cv/82bca582-f0c2-480e-be0b-c33b19d80e73>,
        <http://linked.data.gov.au/def/tern-cv/8f220426-6b5a-4b8f-a995-8eea263a4a19>,
        <http://linked.data.gov.au/def/tern-cv/919d93eb-d7f1-40b3-86ed-91426d925013>,
        <http://linked.data.gov.au/def/tern-cv/9343e3b9-bca2-48e2-af02-eed8111e0147>,
        <http://linked.data.gov.au/def/tern-cv/9b2ab960-da97-473a-81af-d50ab6041739>,
        <http://linked.data.gov.au/def/tern-cv/9b704e6e-9475-4609-9b51-bf596d60c1ff>,
        <http://linked.data.gov.au/def/tern-cv/a8e12e7f-6052-4e87-a69e-ceb34ad5c45d>,
        <http://linked.data.gov.au/def/tern-cv/b0dff759-ae91-4801-b520-b27e27215a40>,
        <http://linked.data.gov.au/def/tern-cv/c3d26c6f-91b7-4627-91e6-2147fa44ad03>,
        <http://linked.data.gov.au/def/tern-cv/c55de6b4-72f2-42ad-ad6e-f611db272e78>,
        <http://linked.data.gov.au/def/tern-cv/cd11241d-9df9-48b9-88b1-3e6646f21562>,
        <http://linked.data.gov.au/def/tern-cv/d40b3e6d-db78-4031-b7f3-ed94d538a2af>,
        <http://linked.data.gov.au/def/tern-cv/d5635c66-06d2-48e4-98ff-7e83e8a2b265>,
        <http://linked.data.gov.au/def/tern-cv/d87a652c-0a30-415c-bef7-e20f75d94002>,
        <http://linked.data.gov.au/def/tern-cv/ea001a27-3217-45c2-a7b5-96a104986def>,
        <http://linked.data.gov.au/def/tern-cv/f3888501-98b1-4a53-a788-20b0f0b8a7e6>,
        <http://linked.data.gov.au/def/tern-cv/f57f6bf8-2a5e-47c5-bcc2-4ce7bb4b9dc7>,
        <http://linked.data.gov.au/def/tern-cv/f81aa91e-5f57-4e49-bc6e-4d821d1f9de2>,
        <http://linked.data.gov.au/def/tern-cv/fe9c70d4-415b-4152-b517-a8e7a15e36f7> ;
    skos:prefLabel "vegetation parameter"@en ;
    skos:definition "vegetation parameters"@en ;
    skos:topConceptOf <http://linked.data.gov.au/def/tern-cv/5699eca7-9ef0-47a6-bcfb-9306e0e2b85e> .

<http://linked.data.gov.au/def/tern-cv/99bd0128-54d4-4a2b-8a2c-48010eb07d26> a skos:Concept ;
    dcterms:created "2020-11-06T02:30:20"^^xsd:datetime ;
    dcterms:modified "2021-01-05T00:25:06"^^xsd:datetime ;
    skos:definition "The top layer of the land surface of the earth that is composed of disintegrated rock particles, humus, water and air."@en ;
    skos:exactMatch <http://vocabs.lter-europe.net/EnvThes/24> ;
    skos:inScheme <http://linked.data.gov.au/def/tern-cv/5699eca7-9ef0-47a6-bcfb-9306e0e2b85e> ;
    rdfs:isDefinedBy <http://linked.data.gov.au/def/tern-cv/5699eca7-9ef0-47a6-bcfb-9306e0e2b85e> ; 
    skos:narrower <http://linked.data.gov.au/def/tern-cv/05304603-1f89-4734-b929-57d7c64a56db>,
        <http://linked.data.gov.au/def/tern-cv/0531b8b6-7610-4fbd-9a66-8cd80d357a70>,
        <http://linked.data.gov.au/def/tern-cv/1046ab56-a29d-4a39-be33-db55bfafa32a>,
        <http://linked.data.gov.au/def/tern-cv/11c8f833-5cbd-4fc0-98f8-b1f0367c44e0>,
        <http://linked.data.gov.au/def/tern-cv/11decfe8-bbac-48f1-9773-f7694eff0498>,
        <http://linked.data.gov.au/def/tern-cv/12797115-2e0f-479f-8d06-1700da3ac394>,
        <http://linked.data.gov.au/def/tern-cv/13417a72-f4c3-4cf2-94bc-5120e0f4347f>,
        <http://linked.data.gov.au/def/tern-cv/1b1b8e39-095c-4572-a5b8-316744f7a4a2>,
        <http://linked.data.gov.au/def/tern-cv/1eeb07ce-9d72-4143-97e5-f12043a6b924>,
        <http://linked.data.gov.au/def/tern-cv/22bc900e-09ee-44a8-a7fd-6acb512ab31b>,
        <http://linked.data.gov.au/def/tern-cv/26c05fcc-9088-4c45-860b-9030b35c859f>,
        <http://linked.data.gov.au/def/tern-cv/2d99f42e-9773-43aa-945a-bb1fe0c47a1a>,
        <http://linked.data.gov.au/def/tern-cv/2e3b3cff-501b-43c2-9b36-18d4e5294c33>,
        <http://linked.data.gov.au/def/tern-cv/2f86eccf-9cab-4c45-905b-b8f769d65950>,
        <http://linked.data.gov.au/def/tern-cv/3a03227d-1b66-4c63-b7aa-f9ccbb70d1cf>,
        <http://linked.data.gov.au/def/tern-cv/40d04abb-0a50-43b8-8f19-2e1b5454fb11>,
        <http://linked.data.gov.au/def/tern-cv/40da61bc-aa52-4de7-b473-c660833c260e>,
        <http://linked.data.gov.au/def/tern-cv/46b1c8c4-5524-41df-bce2-e936e53e51f0>,
        <http://linked.data.gov.au/def/tern-cv/48f31b89-9367-4059-8c2b-cb3e0f1d9045>,
        <http://linked.data.gov.au/def/tern-cv/54b40732-25dc-4471-86ca-55e6d7c54b79>,
        <http://linked.data.gov.au/def/tern-cv/5a7ea957-5b52-4e3b-adb0-660091fa0e4f>,
        <http://linked.data.gov.au/def/tern-cv/5de10b81-3c57-46d2-9486-b5372566b1ae>,
        <http://linked.data.gov.au/def/tern-cv/5f2a89bd-06b5-48a0-83af-32f035a29f0c>,
        <http://linked.data.gov.au/def/tern-cv/65795a49-1f8f-4644-b088-2438301bbe0e>,
        <http://linked.data.gov.au/def/tern-cv/6c2bde95-4b97-4b63-a42b-7a2c253e6e3b>,
        <http://linked.data.gov.au/def/tern-cv/700daf25-0a3f-461e-a799-be80ef2f8cd4>,
        <http://linked.data.gov.au/def/tern-cv/7b3f70df-5c55-4b2b-9b45-ea978d9d3759>,
        <http://linked.data.gov.au/def/tern-cv/843f9a0b-8feb-437f-8a9c-441672698945>,
        <http://linked.data.gov.au/def/tern-cv/85417909-7db2-4216-b886-3aa2780be29e>,
        <http://linked.data.gov.au/def/tern-cv/8e2ee0f0-c6a7-4b8b-a05d-d7d3dae8c580>,
        <http://linked.data.gov.au/def/tern-cv/8e943bc6-f8af-4a77-9724-b4dd0058f815>,
        <http://linked.data.gov.au/def/tern-cv/92ac64e0-d019-4d66-9857-86d82fce7513>,
        <http://linked.data.gov.au/def/tern-cv/931507d7-0fb6-4fd9-932c-3015f83af9ab>,
        <http://linked.data.gov.au/def/tern-cv/939bdeec-f2ce-453c-8315-b36b639a4347>,
        <http://linked.data.gov.au/def/tern-cv/a54f0994-bac3-42e4-83d3-46c33affd8a9>,
        <http://linked.data.gov.au/def/tern-cv/a5596b19-095b-4f96-bf56-89ec679854c2>,
        <http://linked.data.gov.au/def/tern-cv/aa440954-9001-482c-8d0d-e4686ae3533d>,
        <http://linked.data.gov.au/def/tern-cv/b192dc62-970b-4815-a99b-59b3f659b404>,
        <http://linked.data.gov.au/def/tern-cv/b992af7a-414f-4278-a905-59ae1e04e35c>,
        <http://linked.data.gov.au/def/tern-cv/be409d33-8091-44da-899d-56e30e4a1cfa>,
        <http://linked.data.gov.au/def/tern-cv/beceaa5a-a296-4385-a55a-3b8c8d5b2369>,
        <http://linked.data.gov.au/def/tern-cv/c0a07e96-0838-44a9-a854-2196680cba01>,
        <http://linked.data.gov.au/def/tern-cv/c1588a6d-d5e4-44b4-8bf4-f04c5425ed89>,
        <http://linked.data.gov.au/def/tern-cv/c86c4e7f-5dc3-4a88-b5f6-88f5bc0973cd>,
        <http://linked.data.gov.au/def/tern-cv/c8d7ad1c-fb3d-48fc-ab15-dac8756f8a42>,
        <http://linked.data.gov.au/def/tern-cv/c973b6a5-c2eb-46bf-8f47-6eb8c0ba258f>,
        <http://linked.data.gov.au/def/tern-cv/ca1335d2-7257-415c-88b9-f7eb265fa64d>,
        <http://linked.data.gov.au/def/tern-cv/ccc27eac-2b83-4a8b-badf-df2c00464fad>,
        <http://linked.data.gov.au/def/tern-cv/ddb42a17-7409-4dc2-bc7e-4162af242c54>,
        <http://linked.data.gov.au/def/tern-cv/debeebce-d4cd-4dad-8655-32658af00827>,
        <http://linked.data.gov.au/def/tern-cv/e4789a46-8a2f-4987-8745-a9b048fa66e2>,
        <http://linked.data.gov.au/def/tern-cv/ec46ef8d-ad37-4b87-b344-f22599ec2207>,
        <http://linked.data.gov.au/def/tern-cv/fc1155cd-12cd-4355-9b07-051b10a8f4eb>,
        <http://linked.data.gov.au/def/tern-cv/fc383c4d-b8d2-4dbf-b897-5f511208ada1> ;
    skos:prefLabel "soil parameter"@en ;
    skos:topConceptOf <http://linked.data.gov.au/def/tern-cv/5699eca7-9ef0-47a6-bcfb-9306e0e2b85e> .

<http://linked.data.gov.au/def/tern-cv/45ae73d8-92bd-4261-a05f-7bfac228e1f7> a skos:Concept ;
    dcterms:created "2020-11-09T04:57:38"^^xsd:datetime ;
    dcterms:modified "2020-12-19T07:20:26"^^xsd:datetime ;
    skos:definition "The flow of energy and matter between organisms and their physical environment within an Earth-System context."@en ;
    skos:inScheme <http://linked.data.gov.au/def/tern-cv/5699eca7-9ef0-47a6-bcfb-9306e0e2b85e> ;
    rdfs:isDefinedBy <http://linked.data.gov.au/def/tern-cv/5699eca7-9ef0-47a6-bcfb-9306e0e2b85e> ; 
    skos:narrower <http://linked.data.gov.au/def/tern-cv/00c2b397-b61b-4dbe-8f07-7444c00a6af2>,
        <http://linked.data.gov.au/def/tern-cv/035d3a8f-1d73-4990-850a-18fd80120f43>,
        <http://linked.data.gov.au/def/tern-cv/0416e086-9568-48d5-9a12-bf90fd1889c4>,
        <http://linked.data.gov.au/def/tern-cv/05f1c7c3-e252-4f7b-853a-3ad199de2c2e>,
        <http://linked.data.gov.au/def/tern-cv/0b093c5b-2c67-4d22-8a49-85fb3b89553d>,
        <http://linked.data.gov.au/def/tern-cv/0bd7d3ce-9c2e-45ab-84b1-04003c0458d9>,
        <http://linked.data.gov.au/def/tern-cv/1cb8ec7b-9aa5-4ac7-927a-7032684b600c>,
        <http://linked.data.gov.au/def/tern-cv/1e56b253-6497-49b8-9805-0eae69da1d9b>,
        <http://linked.data.gov.au/def/tern-cv/20a2ab2e-cdbd-4c56-9e68-9c926fd589eb>,
        <http://linked.data.gov.au/def/tern-cv/2adc6b97-40f4-4331-8631-031008cb43d4>,
        <http://linked.data.gov.au/def/tern-cv/2e210a48-3c1c-4ef6-8449-9d836f8d8b31>,
        <http://linked.data.gov.au/def/tern-cv/2ed9a76c-195e-4c9c-aa7f-94339c0835b2>,
        <http://linked.data.gov.au/def/tern-cv/2f4c1e8a-7acd-4b79-b16b-04913233cc07>,
        <http://linked.data.gov.au/def/tern-cv/2fb464d4-feac-4e1b-b0ef-bb12e2d68480>,
        <http://linked.data.gov.au/def/tern-cv/313c3883-ae2a-4367-b4b4-1bb95f9d5b05>,
        <http://linked.data.gov.au/def/tern-cv/35506cfc-c7f0-4cb4-be3d-54e41e4ac691>,
        <http://linked.data.gov.au/def/tern-cv/39edcda9-ec99-47f7-9c73-5accc2e7aa72>,
        <http://linked.data.gov.au/def/tern-cv/3da7a464-609c-4294-9814-5f3aea0eb265>,
        <http://linked.data.gov.au/def/tern-cv/3f11b33a-bdee-4c19-b9a0-47a1f894a0d3>,
        <http://linked.data.gov.au/def/tern-cv/3f898b54-a260-4810-be35-f6b52c691345>,
        <http://linked.data.gov.au/def/tern-cv/49938851-6433-46bb-b070-56f1601a3033>,
        <http://linked.data.gov.au/def/tern-cv/4da6fe3c-5219-4ad6-97b1-df0225483de5>,
        <http://linked.data.gov.au/def/tern-cv/564e7135-e4f5-4114-b522-13686007291f>,
        <http://linked.data.gov.au/def/tern-cv/5653af0e-f853-4b98-b4c9-f8626456d314>,
        <http://linked.data.gov.au/def/tern-cv/5ddf2cec-0842-492f-b0fc-b507c421c4b3>,
        <http://linked.data.gov.au/def/tern-cv/6033d979-5b22-40f9-a081-19b9980fa396>,
        <http://linked.data.gov.au/def/tern-cv/6cd4c83a-6e69-4271-ae58-d9dd82ecd20b>,
        <http://linked.data.gov.au/def/tern-cv/6d57155a-1df0-4689-b3ed-551290a3517b>,
        <http://linked.data.gov.au/def/tern-cv/6e0b10ba-b6f2-4d2f-8a86-6873c565e95d>,
        <http://linked.data.gov.au/def/tern-cv/7402efec-a7ef-4f9c-a0ac-ccee0aeef26d>,
        <http://linked.data.gov.au/def/tern-cv/75208020-a087-4b31-89a3-c3028382b5eb>,
        <http://linked.data.gov.au/def/tern-cv/7fc3a450-a0e8-41c9-8597-2e017102bcc1>,
        <http://linked.data.gov.au/def/tern-cv/825b15c9-5f3f-4b24-9b71-baeb565d4201>,
        <http://linked.data.gov.au/def/tern-cv/869b3963-b276-48ac-a0b0-5d6e108eef50>,
        <http://linked.data.gov.au/def/tern-cv/88b78054-2c46-43e4-9222-db33a79c1a3b>,
        <http://linked.data.gov.au/def/tern-cv/894a2121-45ee-44d2-abfc-6ebae35d94c4>,
        <http://linked.data.gov.au/def/tern-cv/89ed531e-0ea0-49d6-8386-ef80c75f0f4f>,
        <http://linked.data.gov.au/def/tern-cv/8d763d15-1aa9-4369-a77b-a0ea4bd3d6ca>,
        <http://linked.data.gov.au/def/tern-cv/8e9797d9-d5f5-4c5b-8d0a-388cb3dd6253>,
        <http://linked.data.gov.au/def/tern-cv/91988f41-89de-4522-9f04-c8bf6bd68bfe>,
        <http://linked.data.gov.au/def/tern-cv/9343e3b9-bca2-48e2-af02-eed8111e0147>,
        <http://linked.data.gov.au/def/tern-cv/968ce393-cc9c-49d0-b910-d64f54e5cdf8>,
        <http://linked.data.gov.au/def/tern-cv/a609ef3e-0baf-4164-96b0-e5d100f56c2f>,
        <http://linked.data.gov.au/def/tern-cv/abce4dbb-e9e8-41ab-8f6d-fd4f63e2fb2a>,
        <http://linked.data.gov.au/def/tern-cv/b216e89a-94a2-4e59-ba6b-b92edd028c47>,
        <http://linked.data.gov.au/def/tern-cv/c3d26c6f-91b7-4627-91e6-2147fa44ad03>,
        <http://linked.data.gov.au/def/tern-cv/c424ab49-a9d8-41e5-b1aa-5607f87264ab>,
        <http://linked.data.gov.au/def/tern-cv/c_fb538aea>,
        <http://linked.data.gov.au/def/tern-cv/d0e0629e-7000-445a-a14f-40aca1cc6646>,
        <http://linked.data.gov.au/def/tern-cv/d2a16407-6155-4d3a-85e3-738006934b28>,
        <http://linked.data.gov.au/def/tern-cv/d42a1a60-c606-4967-a09a-26727b9b2bc8>,
        <http://linked.data.gov.au/def/tern-cv/da1ffee9-0121-4ef6-9323-1ad90efbb59e>,
        <http://linked.data.gov.au/def/tern-cv/dccdd389-7a32-4744-9f8e-990aaa151b49>,
        <http://linked.data.gov.au/def/tern-cv/df6d0f0e-81b0-4bf0-a567-382a4f4b8217>,
        <http://linked.data.gov.au/def/tern-cv/e0e2725a-2525-409a-b282-cc5b7c881646>,
        <http://linked.data.gov.au/def/tern-cv/e8e21a9e-908a-4b99-b2ac-5678d73ba3e3>,
        <http://linked.data.gov.au/def/tern-cv/e9947c8b-0d88-40d5-842a-4aa32fe6646a>,
        <http://linked.data.gov.au/def/tern-cv/eb29cf16-af57-4c8b-b5ec-8c35db9b9901>,
        <http://linked.data.gov.au/def/tern-cv/f9ae2722-732f-472a-8087-999240c6581a>,
        <http://linked.data.gov.au/def/tern-cv/fd9ffa6b-cffa-4e14-a536-06ab8e3505d7> ;
    skos:prefLabel "ecosystem parameter"@en ;
    skos:topConceptOf <http://linked.data.gov.au/def/tern-cv/5699eca7-9ef0-47a6-bcfb-9306e0e2b85e> .

<http://linked.data.gov.au/def/tern-cv/2ffe4363-dea1-4188-9f8f-835983d47fe2> a skos:Concept ;
    dcterms:created "2020-11-09T04:57:05"^^xsd:datetime ;
    dcterms:modified "2021-04-08T00:43:06"^^xsd:datetime ;
    skos:definition "Living organisms and life."@en ;
    skos:inScheme <http://linked.data.gov.au/def/tern-cv/5699eca7-9ef0-47a6-bcfb-9306e0e2b85e> ;
    rdfs:isDefinedBy <http://linked.data.gov.au/def/tern-cv/5699eca7-9ef0-47a6-bcfb-9306e0e2b85e> ; 
    skos:narrower <http://linked.data.gov.au/def/tern-cv/0079402f-aa8c-4c2c-ac0b-fd240405d369>,
        <http://linked.data.gov.au/def/tern-cv/01847226-c42a-4904-bbb8-dc69519bc5b4>,
        <http://linked.data.gov.au/def/tern-cv/0209017c-b3eb-41bc-bf21-38c10c5ee063>,
        <http://linked.data.gov.au/def/tern-cv/03c6e286-27b4-4671-bb9b-ae0819a28eaf>,
        <http://linked.data.gov.au/def/tern-cv/04674274-a548-4301-aba6-9813645226ed>,
        <http://linked.data.gov.au/def/tern-cv/04a4c009-2a51-4bdb-96dd-0bfd1bed8826>,
        <http://linked.data.gov.au/def/tern-cv/08dde64e-5f1b-48c3-8ed3-3469780cbf24>,
        <http://linked.data.gov.au/def/tern-cv/09296da0-c645-4165-950c-780c21b3c140>,
        <http://linked.data.gov.au/def/tern-cv/0a35c80d-f8b7-4a73-b2bf-d90c3872850f>,
        <http://linked.data.gov.au/def/tern-cv/0bbd7fcd-0782-4efc-96e6-1f0f7669c655>,
        <http://linked.data.gov.au/def/tern-cv/0fa08b3b-1204-4af4-ad4a-e976ba1cd945>,
        <http://linked.data.gov.au/def/tern-cv/119c166f-b952-47ca-8616-b16e45ce5286>,
        <http://linked.data.gov.au/def/tern-cv/195c45af-505c-4df4-98c3-d43867af01c2>,
        <http://linked.data.gov.au/def/tern-cv/1c2a4e34-eafc-4180-b7d3-e284e3d239ec>,
        <http://linked.data.gov.au/def/tern-cv/2023575a-f0f9-40cc-b211-febbb652da22>,
        <http://linked.data.gov.au/def/tern-cv/2a04912b-7940-4de1-9325-3902ec62d274>,
        <http://linked.data.gov.au/def/tern-cv/2b192e25-ee32-463b-941a-6a80b4cf5efd>,
        <http://linked.data.gov.au/def/tern-cv/2b32fef0-eee4-4734-b3ea-01f3f0dfb807>,
        <http://linked.data.gov.au/def/tern-cv/2c122d40-d404-4dcb-964a-ceda57ab5215>,
        <http://linked.data.gov.au/def/tern-cv/3c21b608-9164-4e65-913b-ed29801b6ed6>,
        <http://linked.data.gov.au/def/tern-cv/403a2c01-b81d-42a2-b5ad-a733351e6fb9>,
        <http://linked.data.gov.au/def/tern-cv/43ed01cc-0089-4a6b-8754-0990dd0f697b>,
        <http://linked.data.gov.au/def/tern-cv/4534b9ea-e779-455f-b8af-9fc6241e67fc>,
        <http://linked.data.gov.au/def/tern-cv/4c19f603-572e-471c-82eb-230f822c263d>,
        <http://linked.data.gov.au/def/tern-cv/4c5bf815-1d39-4a5e-a761-82eeed617608>,
        <http://linked.data.gov.au/def/tern-cv/4c6a55a6-3ea2-485f-82bc-c5b89a95a605>,
        <http://linked.data.gov.au/def/tern-cv/52d0752f-a8b9-40fc-9ba5-1d34cb602f62>,
        <http://linked.data.gov.au/def/tern-cv/5701d307-bbea-415a-8857-fbf27d5b93ed>,
        <http://linked.data.gov.au/def/tern-cv/5a7f318c-c91f-4477-b680-73b3de954fbe>,
        <http://linked.data.gov.au/def/tern-cv/61a29f86-c1ee-4730-bcb4-8394746baf67>,
        <http://linked.data.gov.au/def/tern-cv/63e33292-75e9-447d-8646-f84b2b11952b>,
        <http://linked.data.gov.au/def/tern-cv/6c73ea38-c3d6-49bf-b6e9-4042d09bbee0>,
        <http://linked.data.gov.au/def/tern-cv/743b223a-ef67-45e2-ab01-02c395434690>,
        <http://linked.data.gov.au/def/tern-cv/74c71500-0bae-43c9-8db0-bd6940899af1>,
        <http://linked.data.gov.au/def/tern-cv/83ac0278-51cd-4d1a-8e05-7c1fc68cf020>,
        <http://linked.data.gov.au/def/tern-cv/90380980-9914-4dd8-8d83-008fb6adeb24>,
        <http://linked.data.gov.au/def/tern-cv/959de812-0e1a-414d-b75f-4113d69fd49e>,
        <http://linked.data.gov.au/def/tern-cv/9b9f21a8-1f49-4cee-b537-3297bc706500>,
        <http://linked.data.gov.au/def/tern-cv/a3ad8f31-6896-416e-8ac6-bc61b93aaab5>,
        <http://linked.data.gov.au/def/tern-cv/abb0ee19-b2e8-42f3-8a25-d1f39ca3ebc3>,
        <http://linked.data.gov.au/def/tern-cv/add0c5d2-6db5-48e4-9ad3-d789ba9fe0a2>,
        <http://linked.data.gov.au/def/tern-cv/be0a9365-32ae-4c82-ac87-d65ff3a4dae7>,
        <http://linked.data.gov.au/def/tern-cv/c55de6b4-72f2-42ad-ad6e-f611db272e78>,
        <http://linked.data.gov.au/def/tern-cv/cd4b88cb-0d79-40e1-80de-bf323eb960e9>,
        <http://linked.data.gov.au/def/tern-cv/d6dcacd0-08dd-4c84-9331-e35d4047577e>,
        <http://linked.data.gov.au/def/tern-cv/dd6cdf8f-0fe0-4d6e-a59c-5a2b6a001f32>,
        <http://linked.data.gov.au/def/tern-cv/df732786-f97a-44ad-a923-7dcd79ef7238>,
        <http://linked.data.gov.au/def/tern-cv/e1a18f5f-b63e-4a67-b28e-52e6f838ac14>,
        <http://linked.data.gov.au/def/tern-cv/e349de93-86f4-490b-afdf-1b7fef5603a3>,
        <http://linked.data.gov.au/def/tern-cv/e3e69168-a959-4b8e-a1ea-2413fc3c2e4e>,
        <http://linked.data.gov.au/def/tern-cv/e88ad59e-0d19-4796-b0be-f7ec3edd7624>,
        <http://linked.data.gov.au/def/tern-cv/f0bcd32d-db46-45c4-b860-a099a5e06603>,
        <http://linked.data.gov.au/def/tern-cv/f1f46e83-769e-4d50-9212-d180ea72a0f0>,
        <http://linked.data.gov.au/def/tern-cv/f2c73e78-8f71-4b41-bfd9-f1cc447593c7>,
        <http://linked.data.gov.au/def/tern-cv/f3f88912-4aab-4d6c-b2ab-7b42ecfaae60>,
        <http://linked.data.gov.au/def/tern-cv/f724700d-d590-44dc-876f-9c09c256f196>,
        <http://linked.data.gov.au/def/tern-cv/fb6be3d6-5268-4b1c-8e59-d42cb08108f1> ;
    skos:prefLabel "biological parameter"@en ;
    skos:topConceptOf <http://linked.data.gov.au/def/tern-cv/5699eca7-9ef0-47a6-bcfb-9306e0e2b85e> .

<http://linked.data.gov.au/def/tern-cv/123f2efe-3891-4764-9047-609c8b30e925> a skos:Concept ;
    dcterms:created "2020-11-05T06:17:38"^^xsd:datetime ;
    dcterms:modified "2020-12-18T23:43:32"^^xsd:datetime ;
    skos:definition "Measures related to the layer of gases surrounding Earth"@en ;
    skos:inScheme <http://linked.data.gov.au/def/tern-cv/5699eca7-9ef0-47a6-bcfb-9306e0e2b85e> ;
    rdfs:isDefinedBy <http://linked.data.gov.au/def/tern-cv/5699eca7-9ef0-47a6-bcfb-9306e0e2b85e> ; 
    skos:narrower <http://linked.data.gov.au/def/tern-cv/c5ca86b0-c503-4590-87fb-0bc8ff9f1632> ,
        <http://linked.data.gov.au/def/tern-cv/c297eafd-9a76-4098-9860-b9f2c29737cc> ,
        <http://linked.data.gov.au/def/tern-cv/c7a0ab55-d1f5-4901-9dc7-a13c352dee6b> ,
        <http://linked.data.gov.au/def/tern-cv/cb2a4d5a-090c-431a-88fe-72afe197c35d> ,
        <http://linked.data.gov.au/def/tern-cv/ccbfa04b-a70b-4ee8-b3d2-0652d33b8c9e> ,
        <http://linked.data.gov.au/def/tern-cv/eaa90e7f-7e44-47b1-af26-e5606b9e3cea> ,
        <http://linked.data.gov.au/def/tern-cv/00062fdb-3f49-4d06-8ca0-804a154418ba> ,
        <http://linked.data.gov.au/def/tern-cv/4cb6258b-e46d-48e8-8f6c-8ec1d2c6cbf0> ,
        <http://linked.data.gov.au/def/tern-cv/8213a995-6c5b-4008-9b42-4376ce8fffee> ,
        <http://linked.data.gov.au/def/tern-cv/3504a016-8231-40f6-8447-96e5ba279aa1> ,
        <http://linked.data.gov.au/def/tern-cv/ceb884dc-f20b-49db-9b27-e2667b87edbb> ,
        <http://linked.data.gov.au/def/tern-cv/f63579ee-a834-4fc9-907a-82d6ae580efe> ,
        <http://linked.data.gov.au/def/tern-cv/fb66fbb3-3cca-43cf-bf3c-df047ac68a63> ,
        <http://linked.data.gov.au/def/tern-cv/993bad16-f465-4363-900e-b73637f7bdb8> ,
        <http://linked.data.gov.au/def/tern-cv/376865de-c13b-41ae-a8ff-d564da40abb7> ,
        <http://linked.data.gov.au/def/tern-cv/c_fb538aea> ,
        <http://linked.data.gov.au/def/tern-cv/c_fb538aea> ;
    skos:prefLabel "atmospheric parameter"@en ;
    skos:topConceptOf <http://linked.data.gov.au/def/tern-cv/5699eca7-9ef0-47a6-bcfb-9306e0e2b85e> .

<http://linked.data.gov.au/def/tern-cv/04a4c009-2a51-4bdb-96dd-0bfd1bed8826> 
    a skos:Concept ; 
    skos:inScheme <http://linked.data.gov.au/def/tern-cv/5699eca7-9ef0-47a6-bcfb-9306e0e2b85e> ; 
    rdfs:isDefinedBy <http://linked.data.gov.au/def/tern-cv/5699eca7-9ef0-47a6-bcfb-9306e0e2b85e> ; 
    skos:prefLabel "field species name"@en ; 
    skos:definition "Species name determined during the process of field observation."@en ; 
    skos:broader <http://linked.data.gov.au/def/tern-cv/2ffe4363-dea1-4188-9f8f-835983d47fe2> ; 
    dcterms:modified "2021-02-26T05:07:02"^^xsd:datetime ; 
. 

<http://linked.data.gov.au/def/tern-cv/09296da0-c645-4165-950c-780c21b3c140> 
    a skos:Concept ; 
    skos:inScheme <http://linked.data.gov.au/def/tern-cv/5699eca7-9ef0-47a6-bcfb-9306e0e2b85e> ; 
    rdfs:isDefinedBy <http://linked.data.gov.au/def/tern-cv/5699eca7-9ef0-47a6-bcfb-9306e0e2b85e> ; 
    skos:prefLabel "vegetative height"@en ; 
    skos:definition "The height of a whole plant from the ground to the highest vegetative component (i.e. non-reproductive)."@en ; 
    skos:broader <http://linked.data.gov.au/def/tern-cv/2ffe4363-dea1-4188-9f8f-835983d47fe2> ; 
    skos:narrower <http://linked.data.gov.au/def/tern-cv/07132d22-6c49-48b7-9dee-da17a424a583>,
        <http://linked.data.gov.au/def/tern-cv/2535509e-507a-4a49-aa11-712860c50520>,
        <http://linked.data.gov.au/def/tern-cv/675a343f-63bd-420c-b45a-5beddbc9d19e> ;
    dcterms:modified "2020-12-18T23:41:51"^^xsd:datetime ; 
. 

<http://linked.data.gov.au/def/tern-cv/0a35c80d-f8b7-4a73-b2bf-d90c3872850f> 
    a skos:Concept ; 
    skos:inScheme <http://linked.data.gov.au/def/tern-cv/5699eca7-9ef0-47a6-bcfb-9306e0e2b85e> ; 
    rdfs:isDefinedBy <http://linked.data.gov.au/def/tern-cv/5699eca7-9ef0-47a6-bcfb-9306e0e2b85e> ; 
    skos:prefLabel "plant mortality"@en ; 
    skos:definition "Indication of whether a plant is living (alive) or non-living (dead)."@en ; 
    skos:broader <http://linked.data.gov.au/def/tern-cv/2ffe4363-dea1-4188-9f8f-835983d47fe2> ; 
    dcterms:modified "2020-08-12T06:48:13.242000+00:00"^^xsd:datetime ; 
. 

<http://linked.data.gov.au/def/tern-cv/0bbd7fcd-0782-4efc-96e6-1f0f7669c655> 
    a skos:Concept ; 
    skos:inScheme <http://linked.data.gov.au/def/tern-cv/5699eca7-9ef0-47a6-bcfb-9306e0e2b85e> ; 
    rdfs:isDefinedBy <http://linked.data.gov.au/def/tern-cv/5699eca7-9ef0-47a6-bcfb-9306e0e2b85e> ; 
    skos:prefLabel "tree basal area"@en ; 
    skos:definition "The cross-sectional area of a tree trunk measured at breast height over bark. It can be thought of as the surface area of a cut stump at a height of 1.3 m."@en ; 
    skos:broader <http://linked.data.gov.au/def/tern-cv/2ffe4363-dea1-4188-9f8f-835983d47fe2> ; 
    dcterms:modified "2020-06-12T06:25:18.890000+00:00"^^xsd:datetime ; 
. 

<http://linked.data.gov.au/def/tern-cv/11c8f833-5cbd-4fc0-98f8-b1f0367c44e0> 
    a skos:Concept ; 
    skos:inScheme <http://linked.data.gov.au/def/tern-cv/5699eca7-9ef0-47a6-bcfb-9306e0e2b85e> ; 
    rdfs:isDefinedBy <http://linked.data.gov.au/def/tern-cv/5699eca7-9ef0-47a6-bcfb-9306e0e2b85e> ; 
    skos:prefLabel "soil type"@en ; 
    skos:definition "Broad soil types derived from HERBRECS code from the Corveg soil type and geological codes the categories in the tables aim to provide options for non-experts to recognise a broad category of soil and geology, while an expert soil scientist or geologist will be able to classify the soil or geology to a more precise level. CORVEG allows the entry of the soil or geological code provided on soil/ geological coverages and these should be added to the database. The nomenclature of the Australian Soil Classification (Isbell et al. 2016) has been applied to the soil codes used in Table 20. This classification should be used for all newly collected soils site data."@en ; 
    skos:broader <http://linked.data.gov.au/def/tern-cv/99bd0128-54d4-4a2b-8a2c-48010eb07d26> ; 
    dcterms:modified "2020-07-09T21:32:45.012000+00:00"^^xsd:datetime ; 
. 

<http://linked.data.gov.au/def/tern-cv/22bc900e-09ee-44a8-a7fd-6acb512ab31b> 
    a skos:Concept ; 
    skos:inScheme <http://linked.data.gov.au/def/tern-cv/5699eca7-9ef0-47a6-bcfb-9306e0e2b85e> ; 
    rdfs:isDefinedBy <http://linked.data.gov.au/def/tern-cv/5699eca7-9ef0-47a6-bcfb-9306e0e2b85e> ; 
    skos:prefLabel "soil pH"@en ; 
    skos:definition "Soil pH is a measure of the acidity or basicity (alkalinity) of a soil. The soil pH is determined in the field using a field pH kit based on the specifications of Raupach and Tucker (1959). Estimate to 0.5 of a unit."@en ; 
    skos:broader <http://linked.data.gov.au/def/tern-cv/99bd0128-54d4-4a2b-8a2c-48010eb07d26> ; 
    dcterms:modified "2020-06-12T03:31:08.413000+00:00"^^xsd:datetime ; 
. 

<http://linked.data.gov.au/def/tern-cv/46b1c8c4-5524-41df-bce2-e936e53e51f0> 
    a skos:Concept ; 
    skos:inScheme <http://linked.data.gov.au/def/tern-cv/5699eca7-9ef0-47a6-bcfb-9306e0e2b85e> ; 
    rdfs:isDefinedBy <http://linked.data.gov.au/def/tern-cv/5699eca7-9ef0-47a6-bcfb-9306e0e2b85e> ; 
    skos:prefLabel "soil texture"@en ; 
    skos:definition "soil texture"@en ; 
    skos:broader <http://linked.data.gov.au/def/tern-cv/99bd0128-54d4-4a2b-8a2c-48010eb07d26> ; 
    dcterms:modified "2021-02-16T03:09:49"^^xsd:datetime ; 
. 

<http://linked.data.gov.au/def/tern-cv/4c5bf815-1d39-4a5e-a761-82eeed617608> 
    a skos:Concept ; 
    skos:inScheme <http://linked.data.gov.au/def/tern-cv/5699eca7-9ef0-47a6-bcfb-9306e0e2b85e> ; 
    rdfs:isDefinedBy <http://linked.data.gov.au/def/tern-cv/5699eca7-9ef0-47a6-bcfb-9306e0e2b85e> ; 
    skos:prefLabel "dominant species leaf size"@en ; 
    skos:definition "Leaf size of the sun leaves of the tallest stratum (excluding emergent) trees in the rainforest."@en ; 
    skos:broader <http://linked.data.gov.au/def/tern-cv/2ffe4363-dea1-4188-9f8f-835983d47fe2> ; 
    dcterms:modified "2020-07-09T04:44:15.411000+00:00"^^xsd:datetime ; 
. 

<http://linked.data.gov.au/def/tern-cv/63e33292-75e9-447d-8646-f84b2b11952b> 
    a skos:Concept ; 
    skos:inScheme <http://linked.data.gov.au/def/tern-cv/5699eca7-9ef0-47a6-bcfb-9306e0e2b85e> ; 
    rdfs:isDefinedBy <http://linked.data.gov.au/def/tern-cv/5699eca7-9ef0-47a6-bcfb-9306e0e2b85e> ; 
    skos:prefLabel "crown cover class"@en ; 
    skos:definition "Crown cover classes are those used in Walker and Hopkins (1990) and these were selected to coincide as closely as possible with the cover classes of previous classifications (e.g. the projective foliage cover classes of Specht et al. 1974)."@en ; 
    skos:broader <http://linked.data.gov.au/def/tern-cv/2ffe4363-dea1-4188-9f8f-835983d47fe2> ; 
    dcterms:modified "2020-12-24T01:13:45"^^xsd:datetime ; 
. 

<http://linked.data.gov.au/def/tern-cv/76806e0f-61a2-447c-8177-7e666637e23a> 
    a skos:Concept ; 
    skos:inScheme <http://linked.data.gov.au/def/tern-cv/5699eca7-9ef0-47a6-bcfb-9306e0e2b85e> ; 
    rdfs:isDefinedBy <http://linked.data.gov.au/def/tern-cv/5699eca7-9ef0-47a6-bcfb-9306e0e2b85e> ; 
    skos:prefLabel "elevation of site"@en ; 
    skos:definition "The distance measurement, usually in the vertical or up direction, between a reference datum and a point or object. Elevation value is given in metres above sea level."@en ; 
    skos:broader <http://linked.data.gov.au/def/tern-cv/d62a4664-89a1-49a1-9ef0-f30ee2c6d22b> ; 
    dcterms:modified "2021-03-12T06:15:46"^^xsd:datetime ; 
. 

<http://linked.data.gov.au/def/tern-cv/8e9797d9-d5f5-4c5b-8d0a-388cb3dd6253> 
    a skos:Concept ; 
    skos:inScheme <http://linked.data.gov.au/def/tern-cv/5699eca7-9ef0-47a6-bcfb-9306e0e2b85e> ; 
    rdfs:isDefinedBy <http://linked.data.gov.au/def/tern-cv/5699eca7-9ef0-47a6-bcfb-9306e0e2b85e> ; 
    skos:prefLabel "disturbance (event)"@en ; 
    skos:definition "A disturbance is any relatively discrete event in time that disrupts ecosystem, community, or population structure and changes resources, substrate availability, or the physical environment."@en ; 
    skos:broader <http://linked.data.gov.au/def/tern-cv/45ae73d8-92bd-4261-a05f-7bfac228e1f7> ; 
    dcterms:modified "2021-01-05T00:22:14"^^xsd:datetime ; 
. 

<http://linked.data.gov.au/def/tern-cv/8f220426-6b5a-4b8f-a995-8eea263a4a19> 
    a skos:Concept ; 
    skos:inScheme <http://linked.data.gov.au/def/tern-cv/5699eca7-9ef0-47a6-bcfb-9306e0e2b85e> ; 
    rdfs:isDefinedBy <http://linked.data.gov.au/def/tern-cv/5699eca7-9ef0-47a6-bcfb-9306e0e2b85e> ; 
    skos:prefLabel "weed cover"@en ; 
    skos:definition "Plants (not necessarily alien) that grow in sites where they are not wanted, and which usually have detectable economic or environmental effects (synonyms: plant pests, harmful species; problem plants). ‘Environmental weeds’ are alien plant taxa that invade natural vegetation, usually adversely affecting native biodiversity and/or ecosystem functioning."@en ; 
    skos:broader <http://linked.data.gov.au/def/tern-cv/777773d0-cfb4-44ff-85e2-08b48e10ac52> ; 
    dcterms:modified "2021-03-12T00:59:55"^^xsd:datetime ; 
. 

<http://linked.data.gov.au/def/tern-cv/8f220426-6b5a-4b8f-a995-8eea263a4a19> 
    a skos:Concept ; 
    skos:inScheme <http://linked.data.gov.au/def/tern-cv/5699eca7-9ef0-47a6-bcfb-9306e0e2b85e> ; 
    rdfs:isDefinedBy <http://linked.data.gov.au/def/tern-cv/5699eca7-9ef0-47a6-bcfb-9306e0e2b85e> ; 
    skos:prefLabel "weed cover"@en ; 
    skos:definition "Plants (not necessarily alien) that grow in sites where they are not wanted, and which usually have detectable economic or environmental effects (synonyms: plant pests, harmful species; problem plants). ‘Environmental weeds’ are alien plant taxa that invade natural vegetation, usually adversely affecting native biodiversity and/or ecosystem functioning."@en ; 
    skos:broader <http://linked.data.gov.au/def/tern-cv/8fa1c4bd-73b3-432a-ab49-9ee89928e6d9> ; 
    dcterms:modified "2021-03-12T00:59:55"^^xsd:datetime ; 
. 

<http://linked.data.gov.au/def/tern-cv/939bdeec-f2ce-453c-8315-b36b639a4347> 
    a skos:Concept ; 
    skos:inScheme <http://linked.data.gov.au/def/tern-cv/5699eca7-9ef0-47a6-bcfb-9306e0e2b85e> ; 
    rdfs:isDefinedBy <http://linked.data.gov.au/def/tern-cv/5699eca7-9ef0-47a6-bcfb-9306e0e2b85e> ; 
    skos:prefLabel "state of erosion"@en ; 
    skos:definition "The state of erosion can be active, stabilised or partly stabilised."@en ; 
    skos:broader <http://linked.data.gov.au/def/tern-cv/99bd0128-54d4-4a2b-8a2c-48010eb07d26> ; 
    dcterms:modified "2020-06-17T02:03:31.749000+00:00"^^xsd:datetime ; 
. 

<http://linked.data.gov.au/def/tern-cv/d6dcacd0-08dd-4c84-9331-e35d4047577e> 
    a skos:Concept ; 
    skos:inScheme <http://linked.data.gov.au/def/tern-cv/5699eca7-9ef0-47a6-bcfb-9306e0e2b85e> ; 
    rdfs:isDefinedBy <http://linked.data.gov.au/def/tern-cv/5699eca7-9ef0-47a6-bcfb-9306e0e2b85e> ; 
    skos:prefLabel "rainforest floristics structure"@en ; 
    skos:definition "Floristic composition of tallest stratum trees. This can be mixed (M), have one or two tree descriptions (S) or mixed plus one species description (X)."@en ; 
    skos:broader <http://linked.data.gov.au/def/tern-cv/2ffe4363-dea1-4188-9f8f-835983d47fe2> ; 
    dcterms:modified "2020-07-09T07:01:36.207000+00:00"^^xsd:datetime ; 
. 

<http://linked.data.gov.au/def/tern-cv/f724700d-d590-44dc-876f-9c09c256f196> 
    a skos:Concept ; 
    skos:inScheme <http://linked.data.gov.au/def/tern-cv/5699eca7-9ef0-47a6-bcfb-9306e0e2b85e> ; 
    rdfs:isDefinedBy <http://linked.data.gov.au/def/tern-cv/5699eca7-9ef0-47a6-bcfb-9306e0e2b85e> ; 
    skos:prefLabel "stand stem density"@en ; 
    skos:definition "Number of stems per unit area."@en ; 
    skos:broader <http://linked.data.gov.au/def/tern-cv/2ffe4363-dea1-4188-9f8f-835983d47fe2> ; 
    dcterms:modified "2020-12-19T08:11:09"^^xsd:datetime ; 
. 

<http://linked.data.gov.au/def/tern-cv/f81aa91e-5f57-4e49-bc6e-4d821d1f9de2> 
    a skos:Concept ; 
    skos:inScheme <http://linked.data.gov.au/def/tern-cv/5699eca7-9ef0-47a6-bcfb-9306e0e2b85e> ; 
    rdfs:isDefinedBy <http://linked.data.gov.au/def/tern-cv/5699eca7-9ef0-47a6-bcfb-9306e0e2b85e> ; 
    skos:prefLabel "growth form"@en ; 
    skos:definition "Plant growth forms can be defined as the physical form a plant assumes under the conditions of its environment."@en ; 
    skos:broader <http://linked.data.gov.au/def/tern-cv/8fa1c4bd-73b3-432a-ab49-9ee89928e6d9> ; 
    dcterms:modified "2021-03-26T06:11:10"^^xsd:datetime ; 
. 

<http://linked.data.gov.au/def/tern-cv/0209017c-b3eb-41bc-bf21-38c10c5ee063> 
    a skos:Concept ; 
    skos:inScheme <http://linked.data.gov.au/def/tern-cv/5699eca7-9ef0-47a6-bcfb-9306e0e2b85e> ; 
    rdfs:isDefinedBy <http://linked.data.gov.au/def/tern-cv/5699eca7-9ef0-47a6-bcfb-9306e0e2b85e> ; 
    skos:prefLabel "substrate"@en ; 
    skos:definition "Uppermost ground surface layer material"@en ; 
    skos:broader <http://linked.data.gov.au/def/tern-cv/2ffe4363-dea1-4188-9f8f-835983d47fe2> ; 
    dcterms:created "2020-09-15T01:32:55.136000+00:00"^^xsd:datetime ; 
    dcterms:modified "2020-09-15T01:38:54.396000+00:00"^^xsd:datetime ; 
. 

<http://linked.data.gov.au/def/tern-cv/0fa08b3b-1204-4af4-ad4a-e976ba1cd945> 
    a skos:Concept ; 
    skos:inScheme <http://linked.data.gov.au/def/tern-cv/5699eca7-9ef0-47a6-bcfb-9306e0e2b85e> ; 
    rdfs:isDefinedBy <http://linked.data.gov.au/def/tern-cv/5699eca7-9ef0-47a6-bcfb-9306e0e2b85e> ; 
    skos:prefLabel "stand basal area"@en ; 
    skos:definition "The sum of the basal area of all live trees in a stand, is usually expressed in square metres per hectare (m2/ha)."@en ; 
    skos:broader <http://linked.data.gov.au/def/tern-cv/2ffe4363-dea1-4188-9f8f-835983d47fe2> ; 
    dcterms:modified "2020-06-17T05:05:47.634000+00:00"^^xsd:datetime ; 
. 

<http://linked.data.gov.au/def/tern-cv/08dde64e-5f1b-48c3-8ed3-3469780cbf24> 
    a skos:Concept ; 
    skos:inScheme <http://linked.data.gov.au/def/tern-cv/5699eca7-9ef0-47a6-bcfb-9306e0e2b85e> ; 
    rdfs:isDefinedBy <http://linked.data.gov.au/def/tern-cv/5699eca7-9ef0-47a6-bcfb-9306e0e2b85e> ; 
    skos:prefLabel "structural formation"@en ; 
    skos:definition "The structural class combined with the dominant life form of a vegetation community, e.g. open forest"@en ; 
    skos:broader <http://linked.data.gov.au/def/tern-cv/2ffe4363-dea1-4188-9f8f-835983d47fe2> ; 
    dcterms:created "2020-05-08T01:44:42.096000+00:00"^^xsd:datetime ; 
    dcterms:modified "2020-12-18T23:40:28"^^xsd:datetime ; 
. 

<http://linked.data.gov.au/def/tern-cv/0079402f-aa8c-4c2c-ac0b-fd240405d369> 
    a skos:Concept ; 
    skos:inScheme <http://linked.data.gov.au/def/tern-cv/5699eca7-9ef0-47a6-bcfb-9306e0e2b85e> ; 
    rdfs:isDefinedBy <http://linked.data.gov.au/def/tern-cv/5699eca7-9ef0-47a6-bcfb-9306e0e2b85e> ; 
    skos:prefLabel "vegetation condition"@en ; 
    skos:definition "The condition of the vegetation at a plot. Categories are 1. BurntN=no regeneration, 2.BurntR=regenerating, 3.Active vegetative growth, 4.Flowering/fruiting, 5.Dry"@en ; 
    skos:broader <http://linked.data.gov.au/def/tern-cv/2ffe4363-dea1-4188-9f8f-835983d47fe2> ; 
    dcterms:modified "2020-07-09T22:48:21.912000+00:00"^^xsd:datetime ; 
. 

<http://linked.data.gov.au/def/tern-cv/b053c016-d21f-4180-aaf5-f7f6f892325d> 
    a skos:Concept ; 
    skos:inScheme <http://linked.data.gov.au/def/tern-cv/5699eca7-9ef0-47a6-bcfb-9306e0e2b85e> ; 
    rdfs:isDefinedBy <http://linked.data.gov.au/def/tern-cv/5699eca7-9ef0-47a6-bcfb-9306e0e2b85e> ; 
    skos:prefLabel "ground cover - rock"@en ; 
    skos:definition "Amount of rock (i.e. individual rock fragments > 6 cm wide) that covers the ground; expressed as a percentage."@en ; 
    skos:broader <http://linked.data.gov.au/def/tern-cv/7dc7ae5c-f074-4536-9032-f59eba3f9270> ; 
    dcterms:modified "2020-12-24T01:17:57"^^xsd:datetime ; 
. 

<http://linked.data.gov.au/def/tern-cv/cbff6d0c-c239-4858-8139-9fbd8c8646df> 
    a skos:Concept ; 
    skos:inScheme <http://linked.data.gov.au/def/tern-cv/5699eca7-9ef0-47a6-bcfb-9306e0e2b85e> ; 
    rdfs:isDefinedBy <http://linked.data.gov.au/def/tern-cv/5699eca7-9ef0-47a6-bcfb-9306e0e2b85e> ; 
    skos:prefLabel "ground cover - litter"@en ; 
    skos:definition "Amount of litter and fine woody debris (i.e. dead wood pieces < 10 cm in diameter) that covers the ground; expressed as a percentage."@en ; 
    skos:broader <http://linked.data.gov.au/def/tern-cv/7dc7ae5c-f074-4536-9032-f59eba3f9270> ; 
    dcterms:modified "2020-12-24T01:21:17"^^xsd:datetime ; 
. 

<http://linked.data.gov.au/def/tern-cv/e06a20d2-ad09-4cf8-bb4b-9ebd66ed10b7> 
    a skos:Concept ; 
    skos:inScheme <http://linked.data.gov.au/def/tern-cv/5699eca7-9ef0-47a6-bcfb-9306e0e2b85e> ; 
    rdfs:isDefinedBy <http://linked.data.gov.au/def/tern-cv/5699eca7-9ef0-47a6-bcfb-9306e0e2b85e> ; 
    skos:prefLabel "ground cover - cryptogam"@en ; 
    skos:definition "Amount of cryptogams (i.e. lichens, bryophytes and an assortment of microscopic organisms) that covers the ground; expressed as a percentage."@en ; 
    skos:broader <http://linked.data.gov.au/def/tern-cv/7dc7ae5c-f074-4536-9032-f59eba3f9270> ; 
    dcterms:modified "2020-12-19T08:04:27"^^xsd:datetime ; 
. 

<http://linked.data.gov.au/def/tern-cv/05304603-1f89-4734-b929-57d7c64a56db> 
    a skos:Concept ; 
    skos:inScheme <http://linked.data.gov.au/def/tern-cv/5699eca7-9ef0-47a6-bcfb-9306e0e2b85e> ; 
    rdfs:isDefinedBy <http://linked.data.gov.au/def/tern-cv/5699eca7-9ef0-47a6-bcfb-9306e0e2b85e> ; 
    skos:prefLabel "fine earth volume"@en ; 
    skos:definition "Volume of fine earth (i.e. particles < 2 mm)."@en ; 
    skos:broader <http://linked.data.gov.au/def/tern-cv/99bd0128-54d4-4a2b-8a2c-48010eb07d26> ; 
    dcterms:modified "2020-07-09T03:28:44.827000+00:00"^^xsd:datetime ; 
. 

<http://linked.data.gov.au/def/tern-cv/0531b8b6-7610-4fbd-9a66-8cd80d357a70> 
    a skos:Concept ; 
    skos:inScheme <http://linked.data.gov.au/def/tern-cv/5699eca7-9ef0-47a6-bcfb-9306e0e2b85e> ; 
    rdfs:isDefinedBy <http://linked.data.gov.au/def/tern-cv/5699eca7-9ef0-47a6-bcfb-9306e0e2b85e> ; 
    skos:prefLabel "soil bulk density"@en ; 
    skos:definition "Soil bulk density (g/cm3) = mass of oven dried soil (g) / total volume of core (cm3)"@en ; 
    skos:broader <http://linked.data.gov.au/def/tern-cv/99bd0128-54d4-4a2b-8a2c-48010eb07d26> ; 
    skos:narrower <http://linked.data.gov.au/def/tern-cv/d7bbfb51-4697-4ca9-9846-2511056e3d9d>,
        <http://linked.data.gov.au/def/tern-cv/e27ee9af-4fde-46aa-a068-f847834269a6> ;
    dcterms:modified "2020-07-09T09:12:37.281000+00:00"^^xsd:datetime ; 
. 

<http://linked.data.gov.au/def/tern-cv/48f31b89-9367-4059-8c2b-cb3e0f1d9045> 
    a skos:Concept ; 
    skos:inScheme <http://linked.data.gov.au/def/tern-cv/5699eca7-9ef0-47a6-bcfb-9306e0e2b85e> ; 
    rdfs:isDefinedBy <http://linked.data.gov.au/def/tern-cv/5699eca7-9ef0-47a6-bcfb-9306e0e2b85e> ; 
    skos:prefLabel "gravel volume"@en ; 
    skos:definition "Volume of gravel (i.e. particles 2 mm to 2 cm)."@en ; 
    skos:broader <http://linked.data.gov.au/def/tern-cv/99bd0128-54d4-4a2b-8a2c-48010eb07d26> ; 
    dcterms:modified "2020-07-09T03:52:56.581000+00:00"^^xsd:datetime ; 
. 

<http://linked.data.gov.au/def/tern-cv/5f2a89bd-06b5-48a0-83af-32f035a29f0c> 
    a skos:Concept ; 
    skos:inScheme <http://linked.data.gov.au/def/tern-cv/5699eca7-9ef0-47a6-bcfb-9306e0e2b85e> ; 
    rdfs:isDefinedBy <http://linked.data.gov.au/def/tern-cv/5699eca7-9ef0-47a6-bcfb-9306e0e2b85e> ; 
    skos:prefLabel "gravel weight"@en ; 
    skos:definition "Weight of gravel (i.e. particles 2 mm to 2 cm)."@en ; 
    skos:broader <http://linked.data.gov.au/def/tern-cv/99bd0128-54d4-4a2b-8a2c-48010eb07d26> ; 
    dcterms:modified "2020-07-09T03:55:13.861000+00:00"^^xsd:datetime ; 
. 

<http://linked.data.gov.au/def/tern-cv/0a92253d-a07b-4762-b653-4c363650cb44> 
    a skos:Concept ; 
    skos:inScheme <http://linked.data.gov.au/def/tern-cv/5699eca7-9ef0-47a6-bcfb-9306e0e2b85e> ; 
    rdfs:isDefinedBy <http://linked.data.gov.au/def/tern-cv/5699eca7-9ef0-47a6-bcfb-9306e0e2b85e> ; 
    skos:prefLabel "aspect angle"@en ; 
    skos:definition "Give as compass bearing to nearest 10 degrees. On level lands (less than 1% slope), aspect need not be recorded."@en ; 
    skos:broader <http://linked.data.gov.au/def/tern-cv/29bd4356-5638-49c0-8d3e-57598ac2ea6c> ; 
    dcterms:modified "2021-03-16T01:04:11"^^xsd:datetime ; 
. 

<http://linked.data.gov.au/def/tern-cv/1046ab56-a29d-4a39-be33-db55bfafa32a> 
    a skos:Concept ; 
    skos:inScheme <http://linked.data.gov.au/def/tern-cv/5699eca7-9ef0-47a6-bcfb-9306e0e2b85e> ; 
    rdfs:isDefinedBy <http://linked.data.gov.au/def/tern-cv/5699eca7-9ef0-47a6-bcfb-9306e0e2b85e> ; 
    skos:prefLabel "soil fabric"@en ; 
    skos:definition "The definition of soil fabric in Australia is incomplete. The following description is adapted from Northcote (1979). Fabric describes the appearance of the soil material (under ×10 hand lens). Differences in fabric are associated with the presence or absence of peds, the lustre or lack of lustre of the ped surfaces, and the presence, size and arrangement of pores (voids) in the soil mass. The descriptions given below apply primarily to B horizons."@en ; 
    skos:broader <http://linked.data.gov.au/def/tern-cv/99bd0128-54d4-4a2b-8a2c-48010eb07d26> ; 
    dcterms:modified "2020-06-12T02:14:07.637000+00:00"^^xsd:datetime ; 
. 

<http://linked.data.gov.au/def/tern-cv/119c166f-b952-47ca-8616-b16e45ce5286> 
    a skos:Concept ; 
    skos:inScheme <http://linked.data.gov.au/def/tern-cv/5699eca7-9ef0-47a6-bcfb-9306e0e2b85e> ; 
    rdfs:isDefinedBy <http://linked.data.gov.au/def/tern-cv/5699eca7-9ef0-47a6-bcfb-9306e0e2b85e> ; 
    skos:prefLabel "stem density"@en ; 
    skos:definition "Number of woody plants per hectare."@en ; 
    skos:broader <http://linked.data.gov.au/def/tern-cv/2ffe4363-dea1-4188-9f8f-835983d47fe2> ; 
    dcterms:modified "2020-12-18T23:42:38"^^xsd:datetime ; 
. 

<http://linked.data.gov.au/def/tern-cv/13417a72-f4c3-4cf2-94bc-5120e0f4347f> 
    a skos:Concept ; 
    skos:inScheme <http://linked.data.gov.au/def/tern-cv/5699eca7-9ef0-47a6-bcfb-9306e0e2b85e> ; 
    rdfs:isDefinedBy <http://linked.data.gov.au/def/tern-cv/5699eca7-9ef0-47a6-bcfb-9306e0e2b85e> ; 
    skos:prefLabel "oven dried soil weight in bag"@en ; 
    skos:definition "Weight of oven dried soil and containing paper bag."@en ; 
    skos:broader <http://linked.data.gov.au/def/tern-cv/99bd0128-54d4-4a2b-8a2c-48010eb07d26> ; 
    dcterms:modified "2020-12-24T01:10:56"^^xsd:datetime ; 
. 

<http://linked.data.gov.au/def/tern-cv/18a1be66-3340-4db1-9731-a8ceb4118db9> 
    a skos:Concept ; 
    skos:inScheme <http://linked.data.gov.au/def/tern-cv/5699eca7-9ef0-47a6-bcfb-9306e0e2b85e> ; 
    rdfs:isDefinedBy <http://linked.data.gov.au/def/tern-cv/5699eca7-9ef0-47a6-bcfb-9306e0e2b85e> ; 
    skos:prefLabel "microrelief"@en ; 
    skos:definition "Microrelief refers to relief up to a few metres above the plane of the land surface (i.e. land surfaces irregularities that cause variation in elevation no taller than few meters). It includes gilgai, hummocky, biotic and other microrelief."@en ; 
    skos:broader <http://linked.data.gov.au/def/tern-cv/29bd4356-5638-49c0-8d3e-57598ac2ea6c> ; 
    dcterms:modified "2020-12-18T23:44:32"^^xsd:datetime ; 
. 

<http://linked.data.gov.au/def/tern-cv/1b1b8e39-095c-4572-a5b8-316744f7a4a2> 
    a skos:Concept ; 
    skos:inScheme <http://linked.data.gov.au/def/tern-cv/5699eca7-9ef0-47a6-bcfb-9306e0e2b85e> ; 
    rdfs:isDefinedBy <http://linked.data.gov.au/def/tern-cv/5699eca7-9ef0-47a6-bcfb-9306e0e2b85e> ; 
    skos:prefLabel "nature of segregations"@en ; 
    skos:definition "Chemical nature of discrete segregations (e.g. calcareous, manganiferous, saline) that has accumulated in the soil because of the concentration of some constituent, usually by chemical or biological action."@en ; 
    skos:broader <http://linked.data.gov.au/def/tern-cv/99bd0128-54d4-4a2b-8a2c-48010eb07d26> ; 
    dcterms:modified "2020-12-18T23:47:16"^^xsd:datetime ; 
. 

<http://linked.data.gov.au/def/tern-cv/1eeb07ce-9d72-4143-97e5-f12043a6b924> 
    a skos:Concept ; 
    skos:inScheme <http://linked.data.gov.au/def/tern-cv/5699eca7-9ef0-47a6-bcfb-9306e0e2b85e> ; 
    rdfs:isDefinedBy <http://linked.data.gov.au/def/tern-cv/5699eca7-9ef0-47a6-bcfb-9306e0e2b85e> ; 
    skos:prefLabel "fine earth weight"@en ; 
    skos:definition "Total weight of fine earth (i.e. particles < 2mm)."@en ; 
    skos:broader <http://linked.data.gov.au/def/tern-cv/99bd0128-54d4-4a2b-8a2c-48010eb07d26> ; 
    dcterms:modified "2021-02-09T00:49:45"^^xsd:datetime ; 
. 

<http://linked.data.gov.au/def/tern-cv/20a2ab2e-cdbd-4c56-9e68-9c926fd589eb> 
    a skos:Concept ; 
    skos:inScheme <http://linked.data.gov.au/def/tern-cv/5699eca7-9ef0-47a6-bcfb-9306e0e2b85e> ; 
    rdfs:isDefinedBy <http://linked.data.gov.au/def/tern-cv/5699eca7-9ef0-47a6-bcfb-9306e0e2b85e> ; 
    skos:prefLabel "fire height"@en ; 
    skos:definition "The highest mark or indication of the impact of fire on the vegetation."@en ; 
    skos:broader <http://linked.data.gov.au/def/tern-cv/45ae73d8-92bd-4261-a05f-7bfac228e1f7> ; 
    dcterms:modified "2021-03-11T06:28:14"^^xsd:datetime ; 
. 

<http://linked.data.gov.au/def/tern-cv/20a2ab2e-cdbd-4c56-9e68-9c926fd589eb> 
    a skos:Concept ; 
    skos:inScheme <http://linked.data.gov.au/def/tern-cv/5699eca7-9ef0-47a6-bcfb-9306e0e2b85e> ; 
    rdfs:isDefinedBy <http://linked.data.gov.au/def/tern-cv/5699eca7-9ef0-47a6-bcfb-9306e0e2b85e> ; 
    skos:prefLabel "fire height"@en ; 
    skos:definition "The highest mark or indication of the impact of fire on the vegetation."@en ; 
    skos:broader <http://linked.data.gov.au/def/tern-cv/777773d0-cfb4-44ff-85e2-08b48e10ac52> ; 
    dcterms:modified "2021-03-11T06:28:14"^^xsd:datetime ; 
. 

<http://linked.data.gov.au/def/tern-cv/20a2ab2e-cdbd-4c56-9e68-9c926fd589eb> 
    a skos:Concept ; 
    skos:inScheme <http://linked.data.gov.au/def/tern-cv/5699eca7-9ef0-47a6-bcfb-9306e0e2b85e> ; 
    rdfs:isDefinedBy <http://linked.data.gov.au/def/tern-cv/5699eca7-9ef0-47a6-bcfb-9306e0e2b85e> ; 
    skos:prefLabel "fire height"@en ; 
    skos:definition "The highest mark or indication of the impact of fire on the vegetation."@en ; 
    skos:broader <http://linked.data.gov.au/def/tern-cv/8fa1c4bd-73b3-432a-ab49-9ee89928e6d9> ; 
    dcterms:modified "2021-03-11T06:28:14"^^xsd:datetime ; 
. 

<http://linked.data.gov.au/def/tern-cv/c55de6b4-72f2-42ad-ad6e-f611db272e78> 
    a skos:Concept ; 
    skos:inScheme <http://linked.data.gov.au/def/tern-cv/5699eca7-9ef0-47a6-bcfb-9306e0e2b85e> ; 
    rdfs:isDefinedBy <http://linked.data.gov.au/def/tern-cv/5699eca7-9ef0-47a6-bcfb-9306e0e2b85e> ; 
    skos:prefLabel "animal grazing level"@en ; 
    skos:definition "Levels of grazing by domestic stock, feral animals and native animals evident in damage to the ground layer plants and/or presence of animal faeces or tracks. Levels are recorded as not apparent, present, severe (enough to make major impact on ground cover abundance or composition)."@en ; 
    skos:broader <http://linked.data.gov.au/def/tern-cv/2ffe4363-dea1-4188-9f8f-835983d47fe2> ; 
    dcterms:modified "2021-03-11T06:30:54"^^xsd:datetime ; 
. 

<http://linked.data.gov.au/def/tern-cv/c55de6b4-72f2-42ad-ad6e-f611db272e78> 
    a skos:Concept ; 
    skos:inScheme <http://linked.data.gov.au/def/tern-cv/5699eca7-9ef0-47a6-bcfb-9306e0e2b85e> ; 
    rdfs:isDefinedBy <http://linked.data.gov.au/def/tern-cv/5699eca7-9ef0-47a6-bcfb-9306e0e2b85e> ; 
    skos:prefLabel "animal grazing level"@en ; 
    skos:definition "Levels of grazing by domestic stock, feral animals and native animals evident in damage to the ground layer plants and/or presence of animal faeces or tracks. Levels are recorded as not apparent, present, severe (enough to make major impact on ground cover abundance or composition)."@en ; 
    skos:broader <http://linked.data.gov.au/def/tern-cv/777773d0-cfb4-44ff-85e2-08b48e10ac52> ; 
    dcterms:modified "2021-03-11T06:30:54"^^xsd:datetime ; 
. 

<http://linked.data.gov.au/def/tern-cv/c55de6b4-72f2-42ad-ad6e-f611db272e78> 
    a skos:Concept ; 
    skos:inScheme <http://linked.data.gov.au/def/tern-cv/5699eca7-9ef0-47a6-bcfb-9306e0e2b85e> ; 
    rdfs:isDefinedBy <http://linked.data.gov.au/def/tern-cv/5699eca7-9ef0-47a6-bcfb-9306e0e2b85e> ; 
    skos:prefLabel "animal grazing level"@en ; 
    skos:definition "Levels of grazing by domestic stock, feral animals and native animals evident in damage to the ground layer plants and/or presence of animal faeces or tracks. Levels are recorded as not apparent, present, severe (enough to make major impact on ground cover abundance or composition)."@en ; 
    skos:broader <http://linked.data.gov.au/def/tern-cv/8fa1c4bd-73b3-432a-ab49-9ee89928e6d9> ; 
    dcterms:modified "2021-03-11T06:30:54"^^xsd:datetime ; 
. 

<http://linked.data.gov.au/def/tern-cv/dccdd389-7a32-4744-9f8e-990aaa151b49> 
    a skos:Concept ; 
    skos:inScheme <http://linked.data.gov.au/def/tern-cv/5699eca7-9ef0-47a6-bcfb-9306e0e2b85e> ; 
    rdfs:isDefinedBy <http://linked.data.gov.au/def/tern-cv/5699eca7-9ef0-47a6-bcfb-9306e0e2b85e> ; 
    skos:prefLabel "disturbance age"@en ; 
    skos:definition "Estimated time since last disturbance event."@en ; 
    skos:broader <http://linked.data.gov.au/def/tern-cv/45ae73d8-92bd-4261-a05f-7bfac228e1f7> ; 
    dcterms:modified "2020-12-19T08:03:44"^^xsd:datetime ; 
. 

<http://linked.data.gov.au/def/tern-cv/e0e2725a-2525-409a-b282-cc5b7c881646> 
    a skos:Concept ; 
    skos:inScheme <http://linked.data.gov.au/def/tern-cv/5699eca7-9ef0-47a6-bcfb-9306e0e2b85e> ; 
    rdfs:isDefinedBy <http://linked.data.gov.au/def/tern-cv/5699eca7-9ef0-47a6-bcfb-9306e0e2b85e> ; 
    skos:prefLabel "disturbance proportion"@en ; 
    skos:definition "Proportion of site affected by anthropogenic disturbance. The categorisation refers to land use change, from 0 - no effective anthropogenic disturbance only natural disturbance to 8 - highly disturbed (e.g. quarrying, road works, mining, landfill, urban)."@en ; 
    skos:broader <http://linked.data.gov.au/def/tern-cv/45ae73d8-92bd-4261-a05f-7bfac228e1f7> ; 
    dcterms:modified "2021-03-10T00:10:39"^^xsd:datetime ; 
. 

<http://linked.data.gov.au/def/tern-cv/2023575a-f0f9-40cc-b211-febbb652da22> 
    a skos:Concept ; 
    skos:inScheme <http://linked.data.gov.au/def/tern-cv/5699eca7-9ef0-47a6-bcfb-9306e0e2b85e> ; 
    rdfs:isDefinedBy <http://linked.data.gov.au/def/tern-cv/5699eca7-9ef0-47a6-bcfb-9306e0e2b85e> ; 
    skos:prefLabel "basal area count"@en ; 
    skos:definition "The count of individual trunks within the sampling area that meet the size criteria of the basal area factor."@en ; 
    skos:broader <http://linked.data.gov.au/def/tern-cv/2ffe4363-dea1-4188-9f8f-835983d47fe2> ; 
    dcterms:modified "2020-06-08T06:50:23.518000+00:00"^^xsd:datetime ; 
. 

<http://linked.data.gov.au/def/tern-cv/26c05fcc-9088-4c45-860b-9030b35c859f> 
    a skos:Concept ; 
    skos:inScheme <http://linked.data.gov.au/def/tern-cv/5699eca7-9ef0-47a6-bcfb-9306e0e2b85e> ; 
    rdfs:isDefinedBy <http://linked.data.gov.au/def/tern-cv/5699eca7-9ef0-47a6-bcfb-9306e0e2b85e> ; 
    skos:prefLabel "form of segregations"@en ; 
    skos:definition "Form of discrete segregations that have accumulated in the soil because of the concentration of some constituent, usually by chemical or biological action."@en ; 
    skos:broader <http://linked.data.gov.au/def/tern-cv/99bd0128-54d4-4a2b-8a2c-48010eb07d26> ; 
    dcterms:modified "2020-07-09T03:40:10.366000+00:00"^^xsd:datetime ; 
. 

<http://linked.data.gov.au/def/tern-cv/2b32fef0-eee4-4734-b3ea-01f3f0dfb807> 
    a skos:Concept ; 
    skos:inScheme <http://linked.data.gov.au/def/tern-cv/5699eca7-9ef0-47a6-bcfb-9306e0e2b85e> ; 
    rdfs:isDefinedBy <http://linked.data.gov.au/def/tern-cv/5699eca7-9ef0-47a6-bcfb-9306e0e2b85e> ; 
    skos:prefLabel "crown density"@en ; 
    skos:definition "Number of crowns per unit area. Crown density as a percentage for each species enables the conversion of crown cover to foliage cover (see Walker and Hopkins 1990, Figure 6)."@en ; 
    skos:broader <http://linked.data.gov.au/def/tern-cv/2ffe4363-dea1-4188-9f8f-835983d47fe2> ; 
    dcterms:modified "2020-12-18T23:59:11"^^xsd:datetime ; 
. 

<http://linked.data.gov.au/def/tern-cv/2b5ac7b3-b4bf-4a06-97d6-8dee8b32d72d> 
    a skos:Concept ; 
    skos:inScheme <http://linked.data.gov.au/def/tern-cv/5699eca7-9ef0-47a6-bcfb-9306e0e2b85e> ; 
    rdfs:isDefinedBy <http://linked.data.gov.au/def/tern-cv/5699eca7-9ef0-47a6-bcfb-9306e0e2b85e> ; 
    skos:prefLabel "slope angle in degrees"@en ; 
    skos:definition "Slope tangent expressed in degrees."@en ; 
    skos:broader <http://linked.data.gov.au/def/tern-cv/29bd4356-5638-49c0-8d3e-57598ac2ea6c> ; 
    dcterms:modified "2020-06-11T06:11:04.103000+00:00"^^xsd:datetime ; 
. 

<http://linked.data.gov.au/def/tern-cv/2d99f42e-9773-43aa-945a-bb1fe0c47a1a> 
    a skos:Concept ; 
    skos:inScheme <http://linked.data.gov.au/def/tern-cv/5699eca7-9ef0-47a6-bcfb-9306e0e2b85e> ; 
    rdfs:isDefinedBy <http://linked.data.gov.au/def/tern-cv/5699eca7-9ef0-47a6-bcfb-9306e0e2b85e> ; 
    skos:prefLabel "abundance of coarse fragments"@en ; 
    skos:definition "Abundance of fragments coarser than 2mm in a soil sample, including rock fragments inferred to be not continuous with underlying bedrock, and other fragments such as charcoal, shells, but not segregation of pedogenic origin. The percentage is estimated by eye using the charts in Figure 11 for comparison."@en ; 
    skos:broader <http://linked.data.gov.au/def/tern-cv/99bd0128-54d4-4a2b-8a2c-48010eb07d26> ; 
    dcterms:modified "2020-07-01T07:13:29.055000+00:00"^^xsd:datetime ; 
. 

<http://linked.data.gov.au/def/tern-cv/2e3b3cff-501b-43c2-9b36-18d4e5294c33> 
    a skos:Concept ; 
    skos:inScheme <http://linked.data.gov.au/def/tern-cv/5699eca7-9ef0-47a6-bcfb-9306e0e2b85e> ; 
    rdfs:isDefinedBy <http://linked.data.gov.au/def/tern-cv/5699eca7-9ef0-47a6-bcfb-9306e0e2b85e> ; 
    skos:prefLabel "shape of coarse fragments"@en ; 
    skos:definition "Shape of fragments coarser than 2mm in a soil sample, including rock fragments inferred to be not continuous with underlying bedrock, and other fragments such as charcoal, shells, but not segregation of pedogenic origin."@en ; 
    skos:broader <http://linked.data.gov.au/def/tern-cv/99bd0128-54d4-4a2b-8a2c-48010eb07d26> ; 
    dcterms:modified "2020-06-11T04:51:08.015000+00:00"^^xsd:datetime ; 
. 

<http://linked.data.gov.au/def/tern-cv/40da61bc-aa52-4de7-b473-c660833c260e> 
    a skos:Concept ; 
    skos:inScheme <http://linked.data.gov.au/def/tern-cv/5699eca7-9ef0-47a6-bcfb-9306e0e2b85e> ; 
    rdfs:isDefinedBy <http://linked.data.gov.au/def/tern-cv/5699eca7-9ef0-47a6-bcfb-9306e0e2b85e> ; 
    skos:prefLabel "grade of pedality"@en ; 
    skos:definition "Refers to the degree of development and distinctness of peds (i.e. aggregates of soil particles formed as a result of pedogenic processes)."@en ; 
    skos:broader <http://linked.data.gov.au/def/tern-cv/99bd0128-54d4-4a2b-8a2c-48010eb07d26> ; 
    dcterms:modified "2020-12-19T07:16:48"^^xsd:datetime ; 
. 

<http://linked.data.gov.au/def/tern-cv/5a7ea957-5b52-4e3b-adb0-660091fa0e4f> 
    a skos:Concept ; 
    skos:inScheme <http://linked.data.gov.au/def/tern-cv/5699eca7-9ef0-47a6-bcfb-9306e0e2b85e> ; 
    rdfs:isDefinedBy <http://linked.data.gov.au/def/tern-cv/5699eca7-9ef0-47a6-bcfb-9306e0e2b85e> ; 
    skos:prefLabel "mottle colour"@en ; 
    skos:definition "Mottles are spots, blotches or streaks of subdominant colours different form the matrix colour and different from the colour of the ped surface. Mottle colour is described in terms of Munsell or Revised Standard Soil colours for both moist and dry soil"@en ; 
    skos:broader <http://linked.data.gov.au/def/tern-cv/99bd0128-54d4-4a2b-8a2c-48010eb07d26> ; 
    dcterms:modified "2020-06-11T02:19:40.899000+00:00"^^xsd:datetime ; 
. 

<http://linked.data.gov.au/def/tern-cv/8e2ee0f0-c6a7-4b8b-a05d-d7d3dae8c580> 
    a skos:Concept ; 
    skos:inScheme <http://linked.data.gov.au/def/tern-cv/5699eca7-9ef0-47a6-bcfb-9306e0e2b85e> ; 
    rdfs:isDefinedBy <http://linked.data.gov.au/def/tern-cv/5699eca7-9ef0-47a6-bcfb-9306e0e2b85e> ; 
    skos:prefLabel "mottle abundance"@en ; 
    skos:definition "Mottles are spots, blotches or streaks of subdominant colours different form the matrix colour and different from the colour of the ped surface. The percentage is estimated by eye using the chart in Figure 11 p 141 (R.C. McDonald, R.F. Isbell and J.G. Speight (2009) Land Surface) for comparison"@en ; 
    skos:broader <http://linked.data.gov.au/def/tern-cv/99bd0128-54d4-4a2b-8a2c-48010eb07d26> ; 
    dcterms:modified "2020-07-09T06:47:45.014000+00:00"^^xsd:datetime ; 
. 

<http://linked.data.gov.au/def/tern-cv/8e943bc6-f8af-4a77-9724-b4dd0058f815> 
    a skos:Concept ; 
    skos:inScheme <http://linked.data.gov.au/def/tern-cv/5699eca7-9ef0-47a6-bcfb-9306e0e2b85e> ; 
    rdfs:isDefinedBy <http://linked.data.gov.au/def/tern-cv/5699eca7-9ef0-47a6-bcfb-9306e0e2b85e> ; 
    skos:prefLabel "type of pedality"@en ; 
    skos:definition "The types of (peds) structure are consist of nine categories. Figure 17 (Page 174 - 180) illustrates the description in diagrammatic form."@en ; 
    skos:broader <http://linked.data.gov.au/def/tern-cv/99bd0128-54d4-4a2b-8a2c-48010eb07d26> ; 
    dcterms:modified "2020-07-09T22:40:40.059000+00:00"^^xsd:datetime ; 
. 

<http://linked.data.gov.au/def/tern-cv/92ac64e0-d019-4d66-9857-86d82fce7513> 
    a skos:Concept ; 
    skos:inScheme <http://linked.data.gov.au/def/tern-cv/5699eca7-9ef0-47a6-bcfb-9306e0e2b85e> ; 
    rdfs:isDefinedBy <http://linked.data.gov.au/def/tern-cv/5699eca7-9ef0-47a6-bcfb-9306e0e2b85e> ; 
    skos:prefLabel "size of peds"@en ; 
    skos:definition "The average least dimension of peds is used to determine the class interval. The least dimension is the vertical dimension for platy structure; the horizontal dimension for prismatic, columnar, blocky and polyhedral peds; the maximum separation of convex faces for lenticular peds; and the diameter for granular peds."@en ; 
    skos:broader <http://linked.data.gov.au/def/tern-cv/99bd0128-54d4-4a2b-8a2c-48010eb07d26> ; 
    dcterms:modified "2020-07-09T08:51:53.231000+00:00"^^xsd:datetime ; 
. 

<http://linked.data.gov.au/def/tern-cv/ec46ef8d-ad37-4b87-b344-f22599ec2207> 
    a skos:Concept ; 
    skos:inScheme <http://linked.data.gov.au/def/tern-cv/5699eca7-9ef0-47a6-bcfb-9306e0e2b85e> ; 
    rdfs:isDefinedBy <http://linked.data.gov.au/def/tern-cv/5699eca7-9ef0-47a6-bcfb-9306e0e2b85e> ; 
    skos:prefLabel "mottle size"@en ; 
    skos:definition "Mottles are spots, blotches or streaks of subdominant colours different form the matrix colour and different from the colour of the ped surface. Mottle size is measured along the greatest dimension except for streaks or linear forms, in which case measure width."@en ; 
    skos:broader <http://linked.data.gov.au/def/tern-cv/99bd0128-54d4-4a2b-8a2c-48010eb07d26> ; 
    dcterms:modified "2020-07-09T06:49:16.928000+00:00"^^xsd:datetime ; 
. 

<http://linked.data.gov.au/def/tern-cv/403a2c01-b81d-42a2-b5ad-a733351e6fb9> 
    a skos:Concept ; 
    skos:inScheme <http://linked.data.gov.au/def/tern-cv/5699eca7-9ef0-47a6-bcfb-9306e0e2b85e> ; 
    rdfs:isDefinedBy <http://linked.data.gov.au/def/tern-cv/5699eca7-9ef0-47a6-bcfb-9306e0e2b85e> ; 
    skos:prefLabel "leaf area index"@en ; 
    skos:definition "Functional (green) leaf area of the canopy per ground area."@en ; 
    skos:broader <http://linked.data.gov.au/def/tern-cv/2ffe4363-dea1-4188-9f8f-835983d47fe2> ; 
    dcterms:created "2020-09-29T10:56:13+00:00"^^xsd:datetime ; 
    dcterms:modified "2021-01-05T00:06:48"^^xsd:datetime ; 
. 

<http://linked.data.gov.au/def/tern-cv/4534b9ea-e779-455f-b8af-9fc6241e67fc> 
    a skos:Concept ; 
    skos:inScheme <http://linked.data.gov.au/def/tern-cv/5699eca7-9ef0-47a6-bcfb-9306e0e2b85e> ; 
    rdfs:isDefinedBy <http://linked.data.gov.au/def/tern-cv/5699eca7-9ef0-47a6-bcfb-9306e0e2b85e> ; 
    skos:prefLabel "vegetation community extent"@en ; 
    skos:definition "For linear communities the width of the community around the site is estimated in the categories from Table 11."@en ; 
    skos:broader <http://linked.data.gov.au/def/tern-cv/2ffe4363-dea1-4188-9f8f-835983d47fe2> ; 
    dcterms:modified "2020-07-09T22:45:35.495000+00:00"^^xsd:datetime ; 
. 

<http://linked.data.gov.au/def/tern-cv/54b40732-25dc-4471-86ca-55e6d7c54b79> 
    a skos:Concept ; 
    skos:inScheme <http://linked.data.gov.au/def/tern-cv/5699eca7-9ef0-47a6-bcfb-9306e0e2b85e> ; 
    rdfs:isDefinedBy <http://linked.data.gov.au/def/tern-cv/5699eca7-9ef0-47a6-bcfb-9306e0e2b85e> ; 
    skos:prefLabel "drainage type"@en ; 
    skos:definition "Drainage summarises local soil wetness conditions and provides a statement about soil and site drainage likely to occur in most years."@en ; 
    skos:broader <http://linked.data.gov.au/def/tern-cv/99bd0128-54d4-4a2b-8a2c-48010eb07d26> ; 
    dcterms:modified "2020-07-09T03:15:00.451000+00:00"^^xsd:datetime ; 
. 

<http://linked.data.gov.au/def/tern-cv/5a95ac61-94c5-4993-aad2-3e891156efe0> 
    a skos:Concept ; 
    skos:inScheme <http://linked.data.gov.au/def/tern-cv/5699eca7-9ef0-47a6-bcfb-9306e0e2b85e> ; 
    rdfs:isDefinedBy <http://linked.data.gov.au/def/tern-cv/5699eca7-9ef0-47a6-bcfb-9306e0e2b85e> ; 
    skos:prefLabel "erosion severity"@en ; 
    skos:definition "Severity of erosion (i.e. accelerated erosion), with categories 1= minor; 2 = moderate; 3 = severe.  Accelerated erosion follows the destruction or loss of protective cover often resulting from people’s influence on the soil, vegetation or landform."@en ; 
    skos:broader <http://linked.data.gov.au/def/tern-cv/777773d0-cfb4-44ff-85e2-08b48e10ac52> ; 
    dcterms:modified "2021-03-11T06:27:23"^^xsd:datetime ; 
. 

<http://linked.data.gov.au/def/tern-cv/5a95ac61-94c5-4993-aad2-3e891156efe0> 
    a skos:Concept ; 
    skos:inScheme <http://linked.data.gov.au/def/tern-cv/5699eca7-9ef0-47a6-bcfb-9306e0e2b85e> ; 
    rdfs:isDefinedBy <http://linked.data.gov.au/def/tern-cv/5699eca7-9ef0-47a6-bcfb-9306e0e2b85e> ; 
    skos:prefLabel "erosion severity"@en ; 
    skos:definition "Severity of erosion (i.e. accelerated erosion), with categories 1= minor; 2 = moderate; 3 = severe.  Accelerated erosion follows the destruction or loss of protective cover often resulting from people’s influence on the soil, vegetation or landform."@en ; 
    skos:broader <http://linked.data.gov.au/def/tern-cv/6f726a59-c330-44eb-898e-7d42d5fbdada> ; 
    dcterms:modified "2021-03-11T06:27:23"^^xsd:datetime ; 
. 

<http://linked.data.gov.au/def/tern-cv/5de10b81-3c57-46d2-9486-b5372566b1ae> 
    a skos:Concept ; 
    skos:inScheme <http://linked.data.gov.au/def/tern-cv/5699eca7-9ef0-47a6-bcfb-9306e0e2b85e> ; 
    rdfs:isDefinedBy <http://linked.data.gov.au/def/tern-cv/5699eca7-9ef0-47a6-bcfb-9306e0e2b85e> ; 
    skos:prefLabel "geology - stratigraphic map unit"@en ; 
    skos:definition "The geological map unit taken from the relevant geology map (such as Qa etc.). This code may differ from what is on the geology map if the latter is obviously wrong; for example, if the geology map shows sandstone when is obviously alluvium, then Qa is entered. In this case the source is listed as outcrop (surface observation)."@en ; 
    skos:broader <http://linked.data.gov.au/def/tern-cv/99bd0128-54d4-4a2b-8a2c-48010eb07d26> ; 
    dcterms:modified "2020-07-09T03:49:52.238000+00:00"^^xsd:datetime ; 
. 

<http://linked.data.gov.au/def/tern-cv/647833d8-bba7-4115-b264-f9fc36c9195c> 
    a skos:Concept ; 
    skos:inScheme <http://linked.data.gov.au/def/tern-cv/5699eca7-9ef0-47a6-bcfb-9306e0e2b85e> ; 
    rdfs:isDefinedBy <http://linked.data.gov.au/def/tern-cv/5699eca7-9ef0-47a6-bcfb-9306e0e2b85e> ; 
    skos:prefLabel "landform situation"@en ; 
    skos:definition "The HERBRECS code used to describe landform."@en ; 
    skos:broader <http://linked.data.gov.au/def/tern-cv/29bd4356-5638-49c0-8d3e-57598ac2ea6c> ; 
    dcterms:modified "2020-07-09T04:40:49.294000+00:00"^^xsd:datetime ; 
. 

<http://linked.data.gov.au/def/tern-cv/65795a49-1f8f-4644-b088-2438301bbe0e> 
    a skos:Concept ; 
    skos:inScheme <http://linked.data.gov.au/def/tern-cv/5699eca7-9ef0-47a6-bcfb-9306e0e2b85e> ; 
    rdfs:isDefinedBy <http://linked.data.gov.au/def/tern-cv/5699eca7-9ef0-47a6-bcfb-9306e0e2b85e> ; 
    skos:prefLabel "soil texture grade"@en ; 
    skos:definition "Soil texture is determined by the size distribution of mineral particles finer than 2 mm; that is, only material that will pass a 2 mm sieve should be used in determination of field texture."@en ; 
    skos:broader <http://linked.data.gov.au/def/tern-cv/99bd0128-54d4-4a2b-8a2c-48010eb07d26> ; 
    dcterms:modified "2021-02-09T01:40:39"^^xsd:datetime ; 
. 

<http://linked.data.gov.au/def/tern-cv/743b223a-ef67-45e2-ab01-02c395434690> 
    a skos:Concept ; 
    skos:inScheme <http://linked.data.gov.au/def/tern-cv/5699eca7-9ef0-47a6-bcfb-9306e0e2b85e> ; 
    rdfs:isDefinedBy <http://linked.data.gov.au/def/tern-cv/5699eca7-9ef0-47a6-bcfb-9306e0e2b85e> ; 
    skos:prefLabel "rainforest leaf-fall characteristic"@en ; 
    skos:definition "The degree of deciduousness associated with rainforest vegetation. It is determined as the proportion of deciduous, semi-deciduous, semi-evergreen and strictly evergreen species in the canopy that is highest is used to allocate leaf-fall classes."@en ; 
    skos:broader <http://linked.data.gov.au/def/tern-cv/2ffe4363-dea1-4188-9f8f-835983d47fe2> ; 
    dcterms:modified "2020-12-19T07:27:25"^^xsd:datetime ; 
. 

<http://linked.data.gov.au/def/tern-cv/78b617e9-cd18-40b7-ad38-efc30579e680> 
    a skos:Concept ; 
    skos:inScheme <http://linked.data.gov.au/def/tern-cv/5699eca7-9ef0-47a6-bcfb-9306e0e2b85e> ; 
    rdfs:isDefinedBy <http://linked.data.gov.au/def/tern-cv/5699eca7-9ef0-47a6-bcfb-9306e0e2b85e> ; 
    skos:prefLabel "landform pattern"@en ; 
    skos:definition "Land surfaces characteristics that are in the order of 600 metres wide."@en ; 
    skos:broader <http://linked.data.gov.au/def/tern-cv/29bd4356-5638-49c0-8d3e-57598ac2ea6c> ; 
    dcterms:modified "2021-01-05T00:08:19"^^xsd:datetime ; 
. 

<http://linked.data.gov.au/def/tern-cv/85417909-7db2-4216-b886-3aa2780be29e> 
    a skos:Concept ; 
    skos:inScheme <http://linked.data.gov.au/def/tern-cv/5699eca7-9ef0-47a6-bcfb-9306e0e2b85e> ; 
    rdfs:isDefinedBy <http://linked.data.gov.au/def/tern-cv/5699eca7-9ef0-47a6-bcfb-9306e0e2b85e> ; 
    skos:prefLabel "soil effervescence"@en ; 
    skos:definition "Amount of carbonate (e.g. Calcium carbonate (CaCO3), dolomite [CaMg(CO3)2], magnesian calcite [Ca1-yMgyCO3]) in the soil."@en ; 
    skos:broader <http://linked.data.gov.au/def/tern-cv/99bd0128-54d4-4a2b-8a2c-48010eb07d26> ; 
    dcterms:modified "2021-01-05T00:19:13"^^xsd:datetime ; 
. 

<http://linked.data.gov.au/def/tern-cv/931507d7-0fb6-4fd9-932c-3015f83af9ab> 
    a skos:Concept ; 
    skos:inScheme <http://linked.data.gov.au/def/tern-cv/5699eca7-9ef0-47a6-bcfb-9306e0e2b85e> ; 
    rdfs:isDefinedBy <http://linked.data.gov.au/def/tern-cv/5699eca7-9ef0-47a6-bcfb-9306e0e2b85e> ; 
    skos:prefLabel "soil horizon"@en ; 
    skos:definition "A soil horizon is a layer of soil, approximately parallel to the land surface, with morphological properties different from layers below and/or above it."@en ; 
    skos:broader <http://linked.data.gov.au/def/tern-cv/99bd0128-54d4-4a2b-8a2c-48010eb07d26> ; 
    dcterms:modified "2020-07-12T00:20:43.939000+00:00"^^xsd:datetime ; 
. 

<http://linked.data.gov.au/def/tern-cv/a5596b19-095b-4f96-bf56-89ec679854c2> 
    a skos:Concept ; 
    skos:inScheme <http://linked.data.gov.au/def/tern-cv/5699eca7-9ef0-47a6-bcfb-9306e0e2b85e> ; 
    rdfs:isDefinedBy <http://linked.data.gov.au/def/tern-cv/5699eca7-9ef0-47a6-bcfb-9306e0e2b85e> ; 
    skos:prefLabel "soil texture qualification"@en ; 
    skos:definition "The non-clay field texture grades (clay loams and coarser) may be qualified according to whether they are at, or near, the light (lower clay content) or heavy (higher clay content) end of the range for that particular field texture grade."@en ; 
    skos:broader <http://linked.data.gov.au/def/tern-cv/99bd0128-54d4-4a2b-8a2c-48010eb07d26> ; 
    dcterms:modified "2020-06-12T04:06:53.659000+00:00"^^xsd:datetime ; 
. 

<http://linked.data.gov.au/def/tern-cv/beceaa5a-a296-4385-a55a-3b8c8d5b2369> 
    a skos:Concept ; 
    skos:inScheme <http://linked.data.gov.au/def/tern-cv/5699eca7-9ef0-47a6-bcfb-9306e0e2b85e> ; 
    rdfs:isDefinedBy <http://linked.data.gov.au/def/tern-cv/5699eca7-9ef0-47a6-bcfb-9306e0e2b85e> ; 
    skos:prefLabel "dry soil colour"@en ; 
    skos:definition "Soil colour in terms of the Munsell Soil Colour Charts or the Revised Standard Soil Colour Charts (Oyama and Takehara 1970)."@en ; 
    skos:broader <http://linked.data.gov.au/def/tern-cv/99bd0128-54d4-4a2b-8a2c-48010eb07d26> ; 
    dcterms:modified "2020-06-12T02:15:02.882000+00:00"^^xsd:datetime ; 
. 

<http://linked.data.gov.au/def/tern-cv/c1588a6d-d5e4-44b4-8bf4-f04c5425ed89> 
    a skos:Concept ; 
    skos:inScheme <http://linked.data.gov.au/def/tern-cv/5699eca7-9ef0-47a6-bcfb-9306e0e2b85e> ; 
    rdfs:isDefinedBy <http://linked.data.gov.au/def/tern-cv/5699eca7-9ef0-47a6-bcfb-9306e0e2b85e> ; 
    skos:prefLabel "soil texture modifier"@en ; 
    skos:definition "Each of the clay field texture grades may also be modified according to the sand or silt fractions, where K is coarse sandy, S is medium sandy, F is fine sandy and Z is silty. These modifiers immediately precede the clay texture codes (e.g. KSLC for coarse sandy light clay; SLC for sandy light clay; ZLC for silty light clay)."@en ; 
    skos:broader <http://linked.data.gov.au/def/tern-cv/99bd0128-54d4-4a2b-8a2c-48010eb07d26> ; 
    dcterms:modified "2020-06-12T04:04:39.229000+00:00"^^xsd:datetime ; 
. 

<http://linked.data.gov.au/def/tern-cv/ccc27eac-2b83-4a8b-badf-df2c00464fad> 
    a skos:Concept ; 
    skos:inScheme <http://linked.data.gov.au/def/tern-cv/5699eca7-9ef0-47a6-bcfb-9306e0e2b85e> ; 
    rdfs:isDefinedBy <http://linked.data.gov.au/def/tern-cv/5699eca7-9ef0-47a6-bcfb-9306e0e2b85e> ; 
    skos:prefLabel "wet soil colour"@en ; 
    skos:definition "Soil colour in terms of the Munsell Soil Colour Charts or the Revised Standard Soil Colour Charts (Oyama and Takehara 1970)."@en ; 
    skos:broader <http://linked.data.gov.au/def/tern-cv/99bd0128-54d4-4a2b-8a2c-48010eb07d26> ; 
    dcterms:modified "2020-06-12T02:14:37.328000+00:00"^^xsd:datetime ; 
. 

<http://linked.data.gov.au/def/tern-cv/e4789a46-8a2f-4987-8745-a9b048fa66e2> 
    a skos:Concept ; 
    skos:inScheme <http://linked.data.gov.au/def/tern-cv/5699eca7-9ef0-47a6-bcfb-9306e0e2b85e> ; 
    rdfs:isDefinedBy <http://linked.data.gov.au/def/tern-cv/5699eca7-9ef0-47a6-bcfb-9306e0e2b85e> ; 
    skos:prefLabel "condition of soil surface when dry"@en ; 
    skos:definition "Physical condition of the surface soil when dry (e.g. cracking, loose, soft, self-mulching, etc.)."@en ; 
    skos:broader <http://linked.data.gov.au/def/tern-cv/99bd0128-54d4-4a2b-8a2c-48010eb07d26> ; 
    dcterms:modified "2020-12-19T08:08:31"^^xsd:datetime ; 
. 

<http://linked.data.gov.au/def/tern-cv/7fa47d4b-1139-4d24-8ef2-8732ff64de4a> 
    a skos:Concept ; 
    skos:inScheme <http://linked.data.gov.au/def/tern-cv/5699eca7-9ef0-47a6-bcfb-9306e0e2b85e> ; 
    rdfs:isDefinedBy <http://linked.data.gov.au/def/tern-cv/5699eca7-9ef0-47a6-bcfb-9306e0e2b85e> ; 
    skos:prefLabel "landform morphological type"@en ; 
    skos:definition "Morphological type is broadly classified into types from Speight (2009) from the codes in Table 13, and consist of: Crest, Ridge, Hillock, Simple slope, Upper slope, Mid slope, Lower slope, Flat, Open Depression and Closed depression."@en ; 
    skos:broader <http://linked.data.gov.au/def/tern-cv/29bd4356-5638-49c0-8d3e-57598ac2ea6c> ; 
    dcterms:modified "2020-07-09T09:01:40.521000+00:00"^^xsd:datetime ; 
. 

<http://linked.data.gov.au/def/tern-cv/83ac0278-51cd-4d1a-8e05-7c1fc68cf020> 
    a skos:Concept ; 
    skos:inScheme <http://linked.data.gov.au/def/tern-cv/5699eca7-9ef0-47a6-bcfb-9306e0e2b85e> ; 
    rdfs:isDefinedBy <http://linked.data.gov.au/def/tern-cv/5699eca7-9ef0-47a6-bcfb-9306e0e2b85e> ; 
    skos:prefLabel "crown cover"@en ; 
    skos:definition "Crown cover (C) (Walker and Hopkins 1990) is the percentage of the sample site within the vertical projection of the periphery of the crowns with the crowns considered to be opaque. This is also the generic definition of canopy cover or plant cover."@en ; 
    skos:broader <http://linked.data.gov.au/def/tern-cv/2ffe4363-dea1-4188-9f8f-835983d47fe2> ; 
    skos:narrower <http://linked.data.gov.au/def/tern-cv/0b96bc02-0a9b-43b9-81fa-de13bf46a5ff>,
        <http://linked.data.gov.au/def/tern-cv/13dabcca-eaf5-46ee-96bf-7364031c3b73>,
        <http://linked.data.gov.au/def/tern-cv/97bc6039-73be-4a1b-bf29-54e4cb097ef3> ;
    dcterms:modified "2020-07-12T00:05:53.800000+00:00"^^xsd:datetime ; 
. 

<http://linked.data.gov.au/def/tern-cv/843f9a0b-8feb-437f-8a9c-441672698945> 
    a skos:Concept ; 
    skos:inScheme <http://linked.data.gov.au/def/tern-cv/5699eca7-9ef0-47a6-bcfb-9306e0e2b85e> ; 
    rdfs:isDefinedBy <http://linked.data.gov.au/def/tern-cv/5699eca7-9ef0-47a6-bcfb-9306e0e2b85e> ; 
    skos:prefLabel "size of segregations"@en ; 
    skos:definition "Size of discrete segregations that have accumulated in the soil because of the concentration of some constituent, usually by chemical or biological action. Approximately equidimensional segregations (concretions, nodules) are measured in the greatest dimension. Segregations where one dimension is much greater than the other two (tubules, root linings, veins, laminae) are measured in the least dimension."@en ; 
    skos:broader <http://linked.data.gov.au/def/tern-cv/99bd0128-54d4-4a2b-8a2c-48010eb07d26> ; 
    dcterms:modified "2020-07-09T09:14:42.007000+00:00"^^xsd:datetime ; 
. 

<http://linked.data.gov.au/def/tern-cv/b192dc62-970b-4815-a99b-59b3f659b404> 
    a skos:Concept ; 
    skos:inScheme <http://linked.data.gov.au/def/tern-cv/5699eca7-9ef0-47a6-bcfb-9306e0e2b85e> ; 
    rdfs:isDefinedBy <http://linked.data.gov.au/def/tern-cv/5699eca7-9ef0-47a6-bcfb-9306e0e2b85e> ; 
    skos:prefLabel "erosional landform pattern"@en ; 
    skos:definition "Land surface characteristics that range between 9m to > 500m, and are the result of erosion (e.g. undulating hills, level plain, precipitous mountains, badlands)."@en ; 
    skos:broader <http://linked.data.gov.au/def/tern-cv/99bd0128-54d4-4a2b-8a2c-48010eb07d26> ; 
    dcterms:modified "2020-12-19T07:50:18"^^xsd:datetime ; 
. 

<http://linked.data.gov.au/def/tern-cv/debeebce-d4cd-4dad-8655-32658af00827> 
    a skos:Concept ; 
    skos:inScheme <http://linked.data.gov.au/def/tern-cv/5699eca7-9ef0-47a6-bcfb-9306e0e2b85e> ; 
    rdfs:isDefinedBy <http://linked.data.gov.au/def/tern-cv/5699eca7-9ef0-47a6-bcfb-9306e0e2b85e> ; 
    skos:prefLabel "accelerated erosion type"@en ; 
    skos:definition "Accelerated erosion is a more rapid erosion than natural erosion that follows the destruction or loss of protective cover often resulting from people's influence on the soil, vegetation or landform."@en ; 
    skos:broader <http://linked.data.gov.au/def/tern-cv/99bd0128-54d4-4a2b-8a2c-48010eb07d26> ; 
    dcterms:modified "2020-06-08T05:49:25.465000+00:00"^^xsd:datetime ; 
. 

<http://linked.data.gov.au/def/tern-cv/959de812-0e1a-414d-b75f-4113d69fd49e> 
    a skos:Concept ; 
    skos:inScheme <http://linked.data.gov.au/def/tern-cv/5699eca7-9ef0-47a6-bcfb-9306e0e2b85e> ; 
    rdfs:isDefinedBy <http://linked.data.gov.au/def/tern-cv/5699eca7-9ef0-47a6-bcfb-9306e0e2b85e> ; 
    skos:prefLabel "vegetation community area"@en ; 
    skos:definition "The vegetation community area is an estimate of the pre-clear extent of the vegetation community in the immediate area that the site represents."@en ; 
    skos:broader <http://linked.data.gov.au/def/tern-cv/2ffe4363-dea1-4188-9f8f-835983d47fe2> ; 
    dcterms:modified "2020-07-09T22:42:33.562000+00:00"^^xsd:datetime ; 
. 

<http://linked.data.gov.au/def/tern-cv/9b2ab960-da97-473a-81af-d50ab6041739> 
    a skos:Concept ; 
    skos:inScheme <http://linked.data.gov.au/def/tern-cv/5699eca7-9ef0-47a6-bcfb-9306e0e2b85e> ; 
    rdfs:isDefinedBy <http://linked.data.gov.au/def/tern-cv/5699eca7-9ef0-47a6-bcfb-9306e0e2b85e> ; 
    skos:prefLabel "in-canopy sky"@en ; 
    skos:definition "If foliage or branches are not intercepted, it is recorded as in-canopy sky. If foliage or branches are intercepted, the species is recorded as a canopy hit and an estimate of the height is recorded."@en ; 
    skos:broader <http://linked.data.gov.au/def/tern-cv/8fa1c4bd-73b3-432a-ab49-9ee89928e6d9> ; 
    dcterms:modified "2021-03-18T04:53:16"^^xsd:datetime ; 
. 

<http://linked.data.gov.au/def/tern-cv/9b704e6e-9475-4609-9b51-bf596d60c1ff> 
    a skos:Concept ; 
    skos:inScheme <http://linked.data.gov.au/def/tern-cv/5699eca7-9ef0-47a6-bcfb-9306e0e2b85e> ; 
    rdfs:isDefinedBy <http://linked.data.gov.au/def/tern-cv/5699eca7-9ef0-47a6-bcfb-9306e0e2b85e> ; 
    skos:prefLabel "mass flowering event exists"@en ; 
    skos:definition "Recorded if mass flowering event occurred. Production of great masses of flowers at certain unique times of year. This is normally due to synchronization of flowering periods of different individual plants so that the flowering season of a species may only be a few days each year."@en ; 
    skos:broader <http://linked.data.gov.au/def/tern-cv/8fa1c4bd-73b3-432a-ab49-9ee89928e6d9> ; 
    dcterms:modified "2021-03-19T02:29:32"^^xsd:datetime ; 
. 

<http://linked.data.gov.au/def/tern-cv/add0c5d2-6db5-48e4-9ad3-d789ba9fe0a2> 
    a skos:Concept ; 
    skos:inScheme <http://linked.data.gov.au/def/tern-cv/5699eca7-9ef0-47a6-bcfb-9306e0e2b85e> ; 
    rdfs:isDefinedBy <http://linked.data.gov.au/def/tern-cv/5699eca7-9ef0-47a6-bcfb-9306e0e2b85e> ; 
    skos:prefLabel "vegetation community site context"@en ; 
    skos:definition "1: A description of the community represented by the site in terms of the predominant species and structure and if appropriate, associated environment (such as landform geology). 2: A set of images captured at the site annually or less frequently using the same protocol, to provide information about the vegetation community represented at the site and any changes that occur over time."@en ; 
    skos:broader <http://linked.data.gov.au/def/tern-cv/2ffe4363-dea1-4188-9f8f-835983d47fe2> ; 
    dcterms:modified "2021-04-28T00:02:50"^^xsd:datetime ; 
. 

<http://linked.data.gov.au/def/tern-cv/b992af7a-414f-4278-a905-59ae1e04e35c> 
    a skos:Concept ; 
    skos:inScheme <http://linked.data.gov.au/def/tern-cv/5699eca7-9ef0-47a6-bcfb-9306e0e2b85e> ; 
    rdfs:isDefinedBy <http://linked.data.gov.au/def/tern-cv/5699eca7-9ef0-47a6-bcfb-9306e0e2b85e> ; 
    skos:prefLabel "lithology of coarse fragments"@en ; 
    skos:definition "Lithology of fragments coarser than 2mm in a soil sample, including rock fragments inferred to be not continuous with underlying bedrock, and other fragments such as charcoal, shells, but not segregation of pedogenic origin. The lithology of the coarse fragments is usually identified as coming from the substrate or from rock outcrop. Where the lithology of the coarse fragments is different from that of the substrate material and/or rock outcrop, describe it as for lithology of substrate material only where the rock type is definitely known or is confidently presumed. Some coarse fragments are commonly encountered that are not directly related to the substrate material."@en ; 
    skos:broader <http://linked.data.gov.au/def/tern-cv/99bd0128-54d4-4a2b-8a2c-48010eb07d26> ; 
    dcterms:modified "2020-06-10T06:38:22.421000+00:00"^^xsd:datetime ; 
. 

<http://linked.data.gov.au/def/tern-cv/be409d33-8091-44da-899d-56e30e4a1cfa> 
    a skos:Concept ; 
    skos:inScheme <http://linked.data.gov.au/def/tern-cv/5699eca7-9ef0-47a6-bcfb-9306e0e2b85e> ; 
    rdfs:isDefinedBy <http://linked.data.gov.au/def/tern-cv/5699eca7-9ef0-47a6-bcfb-9306e0e2b85e> ; 
    skos:prefLabel "abundance of segregations"@en ; 
    skos:definition "Abundance of discrete segregations that have accumulated in the soil because of the concentration of some constituent, usually by chemical or biological action."@en ; 
    skos:broader <http://linked.data.gov.au/def/tern-cv/99bd0128-54d4-4a2b-8a2c-48010eb07d26> ; 
    dcterms:modified "2020-07-01T07:15:09.279000+00:00"^^xsd:datetime ; 
. 

<http://linked.data.gov.au/def/tern-cv/c0a07e96-0838-44a9-a854-2196680cba01> 
    a skos:Concept ; 
    skos:inScheme <http://linked.data.gov.au/def/tern-cv/5699eca7-9ef0-47a6-bcfb-9306e0e2b85e> ; 
    rdfs:isDefinedBy <http://linked.data.gov.au/def/tern-cv/5699eca7-9ef0-47a6-bcfb-9306e0e2b85e> ; 
    skos:prefLabel "size of coarse fragments"@en ; 
    skos:definition "The size of coarse soil fragments (i.e. particles > 2 mm). They include unattached rock fragments and other fragments such as charcoal and shell. The scale adopted employs class boundaries at (2 × 10n/2) mm, where n is an integer. This system is an extension of that used for particles smaller than 2 mm both in the scheme of the British Standards Institution and the Massachusetts Institute of Technology and the original Atterberg (1905) scheme on which the International Scheme was based. It is thus compatible with both the International Scheme referred to in the field texture section and the grain size criteria for substrate materials."@en ; 
    skos:broader <http://linked.data.gov.au/def/tern-cv/99bd0128-54d4-4a2b-8a2c-48010eb07d26> ; 
    dcterms:modified "2020-12-19T07:54:05"^^xsd:datetime ; 
. 

<http://linked.data.gov.au/def/tern-cv/ddb42a17-7409-4dc2-bc7e-4162af242c54> 
    a skos:Concept ; 
    skos:inScheme <http://linked.data.gov.au/def/tern-cv/5699eca7-9ef0-47a6-bcfb-9306e0e2b85e> ; 
    rdfs:isDefinedBy <http://linked.data.gov.au/def/tern-cv/5699eca7-9ef0-47a6-bcfb-9306e0e2b85e> ; 
    skos:prefLabel "dominant substrate lithology"@en ; 
    skos:definition "The main most dominant outcrop lithology. The lithology of the coarse fragments is usually identified as coming from the substrate or from rock outcrop. Where the lithology of the coarse fragments is different from that of the substrate material and/or rock outcrop, describe it as for lithology of substrate material only where the rock type is definitely known or is confidently presumed. Some coarse fragments are commonly encountered that are not directly related to the substrate material."@en ; 
    skos:broader <http://linked.data.gov.au/def/tern-cv/99bd0128-54d4-4a2b-8a2c-48010eb07d26> ; 
    dcterms:modified "2021-01-12T05:38:17"^^xsd:datetime ; 
. 

<http://linked.data.gov.au/def/tern-cv/c5ca86b0-c503-4590-87fb-0bc8ff9f1632> 
    a skos:Concept ; 
    skos:inScheme <http://linked.data.gov.au/def/tern-cv/5699eca7-9ef0-47a6-bcfb-9306e0e2b85e> ; 
    rdfs:isDefinedBy <http://linked.data.gov.au/def/tern-cv/5699eca7-9ef0-47a6-bcfb-9306e0e2b85e> ; 
    skos:prefLabel "climatic condition"@en ; 
    skos:definition "Climatic condition describes whether a recent rainfall event (wet) has occurred at the site or no evidence of recent rain (dry) is visible."@en ; 
    skos:broader <http://linked.data.gov.au/def/tern-cv/123f2efe-3891-4764-9047-609c8b30e925> ; 
    dcterms:modified "2021-02-09T01:42:31"^^xsd:datetime ; 
. 

<http://linked.data.gov.au/def/tern-cv/c8d7ad1c-fb3d-48fc-ab15-dac8756f8a42> 
    a skos:Concept ; 
    skos:inScheme <http://linked.data.gov.au/def/tern-cv/5699eca7-9ef0-47a6-bcfb-9306e0e2b85e> ; 
    rdfs:isDefinedBy <http://linked.data.gov.au/def/tern-cv/5699eca7-9ef0-47a6-bcfb-9306e0e2b85e> ; 
    skos:prefLabel "soil electrical conductivity"@en ; 
    skos:definition "Electrical conductivity (EC) can be determined in the field using a portable EC meter. EC is the ability of a material to transmit (conduct) an electrical current and is commonly expressed in units of milliSiemens per meter (mS/m). Soil EC measurements may also be reported in units of deciSiemens per meter (dS/m), which is equal to the reading in mS/m divided by 100."@en ; 
    skos:broader <http://linked.data.gov.au/def/tern-cv/99bd0128-54d4-4a2b-8a2c-48010eb07d26> ; 
    dcterms:modified "2020-07-09T03:16:56.803000+00:00"^^xsd:datetime ; 
. 

<http://linked.data.gov.au/def/tern-cv/cd4b88cb-0d79-40e1-80de-bf323eb960e9> 
    a skos:Concept ; 
    skos:inScheme <http://linked.data.gov.au/def/tern-cv/5699eca7-9ef0-47a6-bcfb-9306e0e2b85e> ; 
    rdfs:isDefinedBy <http://linked.data.gov.au/def/tern-cv/5699eca7-9ef0-47a6-bcfb-9306e0e2b85e> ; 
    skos:prefLabel "vegetation community is representative of regional ecosystem"@en ; 
    skos:definition "Indication of whether the vegetation community of the site represents the regional ecosystem."@en ; 
    skos:broader <http://linked.data.gov.au/def/tern-cv/2ffe4363-dea1-4188-9f8f-835983d47fe2> ; 
    dcterms:modified "2020-07-09T22:44:30.530000+00:00"^^xsd:datetime ; 
. 

<http://linked.data.gov.au/def/tern-cv/dd6cdf8f-0fe0-4d6e-a59c-5a2b6a001f32> 
    a skos:Concept ; 
    skos:inScheme <http://linked.data.gov.au/def/tern-cv/5699eca7-9ef0-47a6-bcfb-9306e0e2b85e> ; 
    rdfs:isDefinedBy <http://linked.data.gov.au/def/tern-cv/5699eca7-9ef0-47a6-bcfb-9306e0e2b85e> ; 
    skos:prefLabel "rainforest structural complexity"@en ; 
    skos:definition "Structural complexity of the rainforest site is assessed by using the following characteristics : most dominant species, structural features, indicator growth forms, stem size, number of distinct strata."@en ; 
    skos:broader <http://linked.data.gov.au/def/tern-cv/2ffe4363-dea1-4188-9f8f-835983d47fe2> ; 
    dcterms:modified "2020-07-12T00:16:41.795000+00:00"^^xsd:datetime ; 
. 

<http://linked.data.gov.au/def/tern-cv/e5b70249-76a8-4087-8ac9-588c7e29b944> 
    a skos:Concept ; 
    skos:inScheme <http://linked.data.gov.au/def/tern-cv/5699eca7-9ef0-47a6-bcfb-9306e0e2b85e> ; 
    rdfs:isDefinedBy <http://linked.data.gov.au/def/tern-cv/5699eca7-9ef0-47a6-bcfb-9306e0e2b85e> ; 
    skos:prefLabel "lithology type"@en ; 
    skos:definition "Description of a rock unit composition and texture."@en ; 
    skos:broader <http://linked.data.gov.au/def/tern-cv/6e2ede4b-1e6f-4ea0-93d9-6597c5666d62> ; 
    dcterms:modified "2021-03-12T06:14:52"^^xsd:datetime ; 
. 

<http://linked.data.gov.au/def/tern-cv/f2c73e78-8f71-4b41-bfd9-f1cc447593c7> 
    a skos:Concept ; 
    skos:inScheme <http://linked.data.gov.au/def/tern-cv/5699eca7-9ef0-47a6-bcfb-9306e0e2b85e> ; 
    rdfs:isDefinedBy <http://linked.data.gov.au/def/tern-cv/5699eca7-9ef0-47a6-bcfb-9306e0e2b85e> ; 
    skos:prefLabel "vegetation community is mapped to regional ecosystem"@en ; 
    skos:definition "Indication of whether the vegetation community of the site corresponds to the regional ecosystem mapping."@en ; 
    skos:broader <http://linked.data.gov.au/def/tern-cv/2ffe4363-dea1-4188-9f8f-835983d47fe2> ; 
    dcterms:modified "2020-07-09T22:43:47.211000+00:00"^^xsd:datetime ; 
. 

<http://linked.data.gov.au/def/tern-cv/fb6be3d6-5268-4b1c-8e59-d42cb08108f1> 
    a skos:Concept ; 
    skos:inScheme <http://linked.data.gov.au/def/tern-cv/5699eca7-9ef0-47a6-bcfb-9306e0e2b85e> ; 
    rdfs:isDefinedBy <http://linked.data.gov.au/def/tern-cv/5699eca7-9ef0-47a6-bcfb-9306e0e2b85e> ; 
    skos:prefLabel "rainforest indicator growth form"@en ; 
    skos:definition "Many of the simple forests and some of the complex and simple-complex forests develop strata that are visually dominated by particular growth forms. Four growth forms have particular environmental significance (Webb 1968) and the fifth can indicate prior catastrophic disturbance (see below). Refer to Illustrations in Webb et al. (1976): 1 moss; 2 fern; 3 fan palm; 4 feather palm; 5 vine; 6 no dominant indicator."@en ; 
    skos:broader <http://linked.data.gov.au/def/tern-cv/2ffe4363-dea1-4188-9f8f-835983d47fe2> ; 
    dcterms:modified "2020-12-19T08:12:23"^^xsd:datetime ; 
. 

<http://linked.data.gov.au/def/tern-cv/ab4ef0b1-bae1-476e-84c5-612e18282022> 
    a skos:Concept ; 
    skos:inScheme <http://linked.data.gov.au/def/tern-cv/5699eca7-9ef0-47a6-bcfb-9306e0e2b85e> ; 
    rdfs:isDefinedBy <http://linked.data.gov.au/def/tern-cv/5699eca7-9ef0-47a6-bcfb-9306e0e2b85e> ; 
    skos:prefLabel "ground cover - bare"@en ; 
    skos:definition "Amount of ground without cover; expressed as a percentage."@en ; 
    skos:broader <http://linked.data.gov.au/def/tern-cv/7dc7ae5c-f074-4536-9032-f59eba3f9270> ; 
    dcterms:created "2020-05-27T04:53:57.237000+00:00"^^xsd:datetime ; 
    dcterms:modified "2020-12-19T07:46:21"^^xsd:datetime ; 
. 

<http://linked.data.gov.au/def/tern-cv/a40230bc-c1e9-4309-b883-c4ead1d143ce> 
    a skos:Concept ; 
    skos:inScheme <http://linked.data.gov.au/def/tern-cv/5699eca7-9ef0-47a6-bcfb-9306e0e2b85e> ; 
    rdfs:isDefinedBy <http://linked.data.gov.au/def/tern-cv/5699eca7-9ef0-47a6-bcfb-9306e0e2b85e> ; 
    skos:prefLabel "landform element"@en ; 
    skos:definition "A landform element may be described by the following attributes, assessed within a circle of about 20 m radius: slope; morphological type; dimensions; mode of geomorphological activity; geomorphological agent. The three-letter code is taken from Speight (2009), such as cliff, crest, bank etc. and listed in reference Table 26. Landform elements are in the order of 40 metres wide (Speight 2009)."@en ; 
    skos:broader <http://linked.data.gov.au/def/tern-cv/29bd4356-5638-49c0-8d3e-57598ac2ea6c> ; 
    dcterms:created "2020-05-27T05:59:12.356000+00:00"^^xsd:datetime ; 
    dcterms:modified "2020-07-09T04:17:58.694000+00:00"^^xsd:datetime ; 
. 

<http://linked.data.gov.au/def/tern-cv/6c2bde95-4b97-4b63-a42b-7a2c253e6e3b> 
    a skos:Concept ; 
    skos:inScheme <http://linked.data.gov.au/def/tern-cv/5699eca7-9ef0-47a6-bcfb-9306e0e2b85e> ; 
    rdfs:isDefinedBy <http://linked.data.gov.au/def/tern-cv/5699eca7-9ef0-47a6-bcfb-9306e0e2b85e> ; 
    skos:prefLabel "surface strew lithology"@en ; 
    skos:definition "surface strew lithology"@en ; 
    skos:broader <http://linked.data.gov.au/def/tern-cv/99bd0128-54d4-4a2b-8a2c-48010eb07d26> ; 
    dcterms:created "2020-06-01T06:15:12.569000+00:00"^^xsd:datetime ; 
    dcterms:modified "2020-09-18T05:17:49.121000+00:00"^^xsd:datetime ; 
. 

<http://linked.data.gov.au/def/tern-cv/40d04abb-0a50-43b8-8f19-2e1b5454fb11> 
    a skos:Concept ; 
    skos:inScheme <http://linked.data.gov.au/def/tern-cv/5699eca7-9ef0-47a6-bcfb-9306e0e2b85e> ; 
    rdfs:isDefinedBy <http://linked.data.gov.au/def/tern-cv/5699eca7-9ef0-47a6-bcfb-9306e0e2b85e> ; 
    skos:prefLabel "surface strew size"@en ; 
    skos:definition "surface strew size"@en ; 
    skos:broader <http://linked.data.gov.au/def/tern-cv/99bd0128-54d4-4a2b-8a2c-48010eb07d26> ; 
    dcterms:created "2020-06-01T06:24:11.532000+00:00"^^xsd:datetime ; 
    dcterms:modified "2020-09-18T05:18:01.783000+00:00"^^xsd:datetime ; 
. 

<http://linked.data.gov.au/def/tern-cv/07132d22-6c49-48b7-9dee-da17a424a583> 
    a skos:Concept ; 
    skos:inScheme <http://linked.data.gov.au/def/tern-cv/5699eca7-9ef0-47a6-bcfb-9306e0e2b85e> ; 
    rdfs:isDefinedBy <http://linked.data.gov.au/def/tern-cv/5699eca7-9ef0-47a6-bcfb-9306e0e2b85e> ; 
    skos:prefLabel "average vegetative height"@en ; 
    skos:definition "The average height of a vegetation strata."@en ; 
    skos:broader <http://linked.data.gov.au/def/tern-cv/09296da0-c645-4165-950c-780c21b3c140> ; 
    dcterms:created "2020-06-02T00:02:10.010000+00:00"^^xsd:datetime ; 
    dcterms:modified "2021-02-16T23:25:49"^^xsd:datetime ; 
. 

<http://linked.data.gov.au/def/tern-cv/2535509e-507a-4a49-aa11-712860c50520> 
    a skos:Concept ; 
    skos:inScheme <http://linked.data.gov.au/def/tern-cv/5699eca7-9ef0-47a6-bcfb-9306e0e2b85e> ; 
    rdfs:isDefinedBy <http://linked.data.gov.au/def/tern-cv/5699eca7-9ef0-47a6-bcfb-9306e0e2b85e> ; 
    skos:prefLabel "minimum vegetative height"@en ; 
    skos:definition "The minimum height of a vegetation strata."@en ; 
    skos:broader <http://linked.data.gov.au/def/tern-cv/09296da0-c645-4165-950c-780c21b3c140> ; 
    dcterms:created "2020-06-02T00:08:53.773000+00:00"^^xsd:datetime ; 
    dcterms:modified "2021-02-16T23:25:27"^^xsd:datetime ; 
. 

<http://linked.data.gov.au/def/tern-cv/675a343f-63bd-420c-b45a-5beddbc9d19e> 
    a skos:Concept ; 
    skos:inScheme <http://linked.data.gov.au/def/tern-cv/5699eca7-9ef0-47a6-bcfb-9306e0e2b85e> ; 
    rdfs:isDefinedBy <http://linked.data.gov.au/def/tern-cv/5699eca7-9ef0-47a6-bcfb-9306e0e2b85e> ; 
    skos:prefLabel "maximum vegetative height"@en ; 
    skos:definition "The maximum height of a vegetation strata."@en ; 
    skos:broader <http://linked.data.gov.au/def/tern-cv/09296da0-c645-4165-950c-780c21b3c140> ; 
    dcterms:created "2020-06-02T00:10:08.052000+00:00"^^xsd:datetime ; 
    dcterms:modified "2021-02-16T23:25:36"^^xsd:datetime ; 
. 

<http://linked.data.gov.au/def/tern-cv/97bc6039-73be-4a1b-bf29-54e4cb097ef3> 
    a skos:Concept ; 
    skos:inScheme <http://linked.data.gov.au/def/tern-cv/5699eca7-9ef0-47a6-bcfb-9306e0e2b85e> ; 
    rdfs:isDefinedBy <http://linked.data.gov.au/def/tern-cv/5699eca7-9ef0-47a6-bcfb-9306e0e2b85e> ; 
    skos:prefLabel "average crown cover"@en ; 
    skos:definition "Crown cover (C) (Walker and Hopkins 1990) is the percentage of the sample site within the vertical projection of the periphery of the crowns with the crowns considered to be opaque. This is also the generic definition of canopy cover or plant cover."@en ; 
    skos:broader <http://linked.data.gov.au/def/tern-cv/83ac0278-51cd-4d1a-8e05-7c1fc68cf020> ; 
    dcterms:created "2020-06-02T00:11:44.372000+00:00"^^xsd:datetime ; 
    dcterms:modified "2020-11-19T04:46:31"^^xsd:datetime ; 
. 

<http://linked.data.gov.au/def/tern-cv/0b96bc02-0a9b-43b9-81fa-de13bf46a5ff> 
    a skos:Concept ; 
    skos:inScheme <http://linked.data.gov.au/def/tern-cv/5699eca7-9ef0-47a6-bcfb-9306e0e2b85e> ; 
    rdfs:isDefinedBy <http://linked.data.gov.au/def/tern-cv/5699eca7-9ef0-47a6-bcfb-9306e0e2b85e> ; 
    skos:prefLabel "maximum crown cover"@en ; 
    skos:definition "Crown cover (C) (Walker and Hopkins 1990) is the percentage of the sample site within the vertical projection of the periphery of the crowns with the crowns considered to be opaque. This is also the generic definition of canopy cover or plant cover."@en ; 
    skos:broader <http://linked.data.gov.au/def/tern-cv/83ac0278-51cd-4d1a-8e05-7c1fc68cf020> ; 
    dcterms:created "2020-06-02T00:12:46.606000+00:00"^^xsd:datetime ; 
    dcterms:modified "2020-11-19T04:57:49"^^xsd:datetime ; 
. 

<http://linked.data.gov.au/def/tern-cv/13dabcca-eaf5-46ee-96bf-7364031c3b73> 
    a skos:Concept ; 
    skos:inScheme <http://linked.data.gov.au/def/tern-cv/5699eca7-9ef0-47a6-bcfb-9306e0e2b85e> ; 
    rdfs:isDefinedBy <http://linked.data.gov.au/def/tern-cv/5699eca7-9ef0-47a6-bcfb-9306e0e2b85e> ; 
    skos:prefLabel "minimum crown cover"@en ; 
    skos:definition "Crown cover (C) (Walker and Hopkins 1990) is the percentage of the sample site within the vertical projection of the periphery of the crowns with the crowns considered to be opaque. This is also the generic definition of canopy cover or plant cover."@en ; 
    skos:broader <http://linked.data.gov.au/def/tern-cv/83ac0278-51cd-4d1a-8e05-7c1fc68cf020> ; 
    dcterms:created "2020-06-02T00:14:08.982000+00:00"^^xsd:datetime ; 
    dcterms:modified "2020-11-19T05:07:05"^^xsd:datetime ; 
. 

<http://linked.data.gov.au/def/tern-cv/2b192e25-ee32-463b-941a-6a80b4cf5efd> 
    a skos:Concept ; 
    skos:inScheme <http://linked.data.gov.au/def/tern-cv/5699eca7-9ef0-47a6-bcfb-9306e0e2b85e> ; 
    rdfs:isDefinedBy <http://linked.data.gov.au/def/tern-cv/5699eca7-9ef0-47a6-bcfb-9306e0e2b85e> ; 
    skos:prefLabel "average projective foliage cover"@en ; 
    skos:definition "Average projective foliage cover recorded at the site. Projective foliage cover (PFC) (Specht et al. 1974) is the percentage of the sample site occupied by the vertical projection of foliage only. PFC and foliage cover for plants are sensitive to season and drought because foliage may change greatly depending on the water available. This variation is not usually considered in vegetation classification."@en ; 
    skos:broader <http://linked.data.gov.au/def/tern-cv/2ffe4363-dea1-4188-9f8f-835983d47fe2> ; 
    dcterms:created "2020-06-02T04:38:54.283000+00:00"^^xsd:datetime ; 
    dcterms:modified "2020-06-15T04:36:57.540000+00:00"^^xsd:datetime ; 
. 

<http://linked.data.gov.au/def/tern-cv/1c2a4e34-eafc-4180-b7d3-e284e3d239ec> 
    a skos:Concept ; 
    skos:inScheme <http://linked.data.gov.au/def/tern-cv/5699eca7-9ef0-47a6-bcfb-9306e0e2b85e> ; 
    rdfs:isDefinedBy <http://linked.data.gov.au/def/tern-cv/5699eca7-9ef0-47a6-bcfb-9306e0e2b85e> ; 
    skos:prefLabel "minimum projective foliage cover"@en ; 
    skos:definition "Minimum projective foliage cover recorded at the site. Projective foliage cover (PFC) (Specht et al. 1974) is the percentage of the sample site occupied by the vertical projection of foliage only. PFC and foliage cover for plants are sensitive to season and drought because foliage may change greatly depending on the water available. This variation is not usually considered in vegetation classification."@en ; 
    skos:broader <http://linked.data.gov.au/def/tern-cv/2ffe4363-dea1-4188-9f8f-835983d47fe2> ; 
    dcterms:created "2020-06-02T04:42:02.869000+00:00"^^xsd:datetime ; 
    dcterms:modified "2020-10-07T01:36:19"^^xsd:datetime ; 
. 

<http://linked.data.gov.au/def/tern-cv/04674274-a548-4301-aba6-9813645226ed> 
    a skos:Concept ; 
    skos:inScheme <http://linked.data.gov.au/def/tern-cv/5699eca7-9ef0-47a6-bcfb-9306e0e2b85e> ; 
    rdfs:isDefinedBy <http://linked.data.gov.au/def/tern-cv/5699eca7-9ef0-47a6-bcfb-9306e0e2b85e> ; 
    skos:prefLabel "maximum projective foliage cover"@en ; 
    skos:definition "Maximum projective foliage cover recorded at the site. Projective foliage cover (PFC) (Specht et al. 1974) is the percentage of the sample site occupied by the vertical projection of foliage only. PFC and foliage cover for plants are sensitive to season and drought because foliage may change greatly depending on the water available. This variation is not usually considered in vegetation classification."@en ; 
    skos:broader <http://linked.data.gov.au/def/tern-cv/2ffe4363-dea1-4188-9f8f-835983d47fe2> ; 
    dcterms:created "2020-06-02T04:42:32.047000+00:00"^^xsd:datetime ; 
    dcterms:modified "2020-10-07T01:36:02"^^xsd:datetime ; 
. 

<http://linked.data.gov.au/def/tern-cv/2f86eccf-9cab-4c45-905b-b8f769d65950> 
    a skos:Concept ; 
    skos:inScheme <http://linked.data.gov.au/def/tern-cv/5699eca7-9ef0-47a6-bcfb-9306e0e2b85e> ; 
    rdfs:isDefinedBy <http://linked.data.gov.au/def/tern-cv/5699eca7-9ef0-47a6-bcfb-9306e0e2b85e> ; 
    skos:prefLabel "erosion extent"@en ; 
    skos:definition "Presence/absence or extent of accelerated erosion."@en ; 
    skos:broader <http://linked.data.gov.au/def/tern-cv/99bd0128-54d4-4a2b-8a2c-48010eb07d26> ; 
    dcterms:created "2020-06-17T01:19:52.305000+00:00"^^xsd:datetime ; 
    dcterms:modified "2020-07-09T03:21:21.484000+00:00"^^xsd:datetime ; 
. 

<http://linked.data.gov.au/def/tern-cv/c297eafd-9a76-4098-9860-b9f2c29737cc> 
    a skos:Concept ; 
    skos:inScheme <http://linked.data.gov.au/def/tern-cv/5699eca7-9ef0-47a6-bcfb-9306e0e2b85e> ; 
    rdfs:isDefinedBy <http://linked.data.gov.au/def/tern-cv/5699eca7-9ef0-47a6-bcfb-9306e0e2b85e> ; 
    skos:prefLabel "solar radiation mean"@en ; 
    skos:definition "Mean daily incident solar radiation of each month for all years on record."@en ; 
    skos:broader <http://linked.data.gov.au/def/tern-cv/123f2efe-3891-4764-9047-609c8b30e925> ; 
    dcterms:created "2020-06-25T01:11:28.671000+00:00"^^xsd:datetime ; 
    dcterms:modified "2020-12-19T07:58:02"^^xsd:datetime ; 
. 

<http://linked.data.gov.au/def/tern-cv/c7a0ab55-d1f5-4901-9dc7-a13c352dee6b> 
    a skos:Concept ; 
    skos:inScheme <http://linked.data.gov.au/def/tern-cv/5699eca7-9ef0-47a6-bcfb-9306e0e2b85e> ; 
    rdfs:isDefinedBy <http://linked.data.gov.au/def/tern-cv/5699eca7-9ef0-47a6-bcfb-9306e0e2b85e> ; 
    skos:prefLabel "maximum temperature"@en ; 
    skos:definition "The average daily maximum air temperature, for each month, and as an annual statistic, calculated over all years of record."@en ; 
    skos:broader <http://linked.data.gov.au/def/tern-cv/123f2efe-3891-4764-9047-609c8b30e925> ; 
    dcterms:created "2020-06-23T05:32:00.747000+00:00"^^xsd:datetime ; 
    dcterms:modified "2020-12-19T07:58:52"^^xsd:datetime ; 
. 

<http://linked.data.gov.au/def/tern-cv/cb2a4d5a-090c-431a-88fe-72afe197c35d> 
    a skos:Concept ; 
    skos:inScheme <http://linked.data.gov.au/def/tern-cv/5699eca7-9ef0-47a6-bcfb-9306e0e2b85e> ; 
    rdfs:isDefinedBy <http://linked.data.gov.au/def/tern-cv/5699eca7-9ef0-47a6-bcfb-9306e0e2b85e> ; 
    skos:prefLabel "precipitation annual mean"@en ; 
    skos:definition "The arithmetically averaged total amount of precipitation recorded during a year, calculated over all years on record."@en ; 
    skos:broader <http://linked.data.gov.au/def/tern-cv/123f2efe-3891-4764-9047-609c8b30e925> ; 
    dcterms:created "2020-06-23T05:30:41.305000+00:00"^^xsd:datetime ; 
    dcterms:modified "2020-12-19T07:59:37"^^xsd:datetime ; 
. 

<http://linked.data.gov.au/def/tern-cv/ccbfa04b-a70b-4ee8-b3d2-0652d33b8c9e> 
    a skos:Concept ; 
    skos:inScheme <http://linked.data.gov.au/def/tern-cv/5699eca7-9ef0-47a6-bcfb-9306e0e2b85e> ; 
    rdfs:isDefinedBy <http://linked.data.gov.au/def/tern-cv/5699eca7-9ef0-47a6-bcfb-9306e0e2b85e> ; 
    skos:prefLabel "minimum temperature"@en ; 
    skos:definition "The average daily minimum air temperature, for each month, and as an annual statistic, calculated over all years of record."@en ; 
    skos:broader <http://linked.data.gov.au/def/tern-cv/123f2efe-3891-4764-9047-609c8b30e925> ; 
    dcterms:created "2020-06-23T05:32:27.016000+00:00"^^xsd:datetime ; 
    dcterms:modified "2020-12-19T08:01:24"^^xsd:datetime ; 
. 

<http://linked.data.gov.au/def/tern-cv/eaa90e7f-7e44-47b1-af26-e5606b9e3cea> 
    a skos:Concept ; 
    skos:inScheme <http://linked.data.gov.au/def/tern-cv/5699eca7-9ef0-47a6-bcfb-9306e0e2b85e> ; 
    rdfs:isDefinedBy <http://linked.data.gov.au/def/tern-cv/5699eca7-9ef0-47a6-bcfb-9306e0e2b85e> ; 
    skos:prefLabel "temperature annual mean"@en ; 
    skos:definition "The average daily mean air temperature, for each month and as an annual statistic, calculated over all years of record."@en ; 
    skos:broader <http://linked.data.gov.au/def/tern-cv/123f2efe-3891-4764-9047-609c8b30e925> ; 
    dcterms:created "2020-06-25T01:09:23.556000+00:00"^^xsd:datetime ; 
    dcterms:modified "2020-12-19T08:10:30"^^xsd:datetime ; 
. 

<http://linked.data.gov.au/def/tern-cv/05f1c7c3-e252-4f7b-853a-3ad199de2c2e> 
    a skos:Concept ; 
    skos:inScheme <http://linked.data.gov.au/def/tern-cv/5699eca7-9ef0-47a6-bcfb-9306e0e2b85e> ; 
    rdfs:isDefinedBy <http://linked.data.gov.au/def/tern-cv/5699eca7-9ef0-47a6-bcfb-9306e0e2b85e> ; 
    skos:prefLabel "carbon mass - aboveground"@en ; 
    skos:definition "Carbon mass is the above-ground mass of carbon from the ecosystem. Biomass is typically approximated as double the carbon mass."@en ; 
    skos:broader <http://linked.data.gov.au/def/tern-cv/45ae73d8-92bd-4261-a05f-7bfac228e1f7> ; 
    dcterms:created "2020-06-19T15:03:14+00:00"^^xsd:datetime ; 
    dcterms:modified "2020-12-18T23:31:39"^^xsd:datetime ; 
. 

<http://linked.data.gov.au/def/tern-cv/313c3883-ae2a-4367-b4b4-1bb95f9d5b05> 
    a skos:Concept ; 
    skos:inScheme <http://linked.data.gov.au/def/tern-cv/5699eca7-9ef0-47a6-bcfb-9306e0e2b85e> ; 
    rdfs:isDefinedBy <http://linked.data.gov.au/def/tern-cv/5699eca7-9ef0-47a6-bcfb-9306e0e2b85e> ; 
    skos:prefLabel "gross primary productivity"@en ; 
    skos:definition "Total amount of carbon fixed through photosynthesis at the ecosystem level."@en ; 
    skos:broader <http://linked.data.gov.au/def/tern-cv/45ae73d8-92bd-4261-a05f-7bfac228e1f7> ; 
    dcterms:created "2020-06-19T15:03:14+00:00"^^xsd:datetime ; 
    dcterms:modified "2021-05-21T06:30:36"^^xsd:datetime ; 
. 

<http://linked.data.gov.au/def/tern-cv/7fc3a450-a0e8-41c9-8597-2e017102bcc1> 
    a skos:Concept ; 
    skos:inScheme <http://linked.data.gov.au/def/tern-cv/5699eca7-9ef0-47a6-bcfb-9306e0e2b85e> ; 
    rdfs:isDefinedBy <http://linked.data.gov.au/def/tern-cv/5699eca7-9ef0-47a6-bcfb-9306e0e2b85e> ; 
    skos:prefLabel "photosynthetic vegetation fraction"@en ; 
    skos:definition "The fraction of an area (or of a pixel) that contains Photosynthetic Vegetation."@en ; 
    skos:broader <http://linked.data.gov.au/def/tern-cv/45ae73d8-92bd-4261-a05f-7bfac228e1f7> ; 
    dcterms:created "2020-06-19T15:46:43+00:00"^^xsd:datetime ; 
    dcterms:modified "2020-10-26T06:37:17"^^xsd:datetime ; 
. 

<http://linked.data.gov.au/def/tern-cv/c973b6a5-c2eb-46bf-8f47-6eb8c0ba258f> 
    a skos:Concept ; 
    skos:inScheme <http://linked.data.gov.au/def/tern-cv/5699eca7-9ef0-47a6-bcfb-9306e0e2b85e> ; 
    rdfs:isDefinedBy <http://linked.data.gov.au/def/tern-cv/5699eca7-9ef0-47a6-bcfb-9306e0e2b85e> ; 
    skos:prefLabel "bare soil fraction"@en ; 
    skos:definition "The fraction of an area (or of a pixel) that contains Bare Soil."@en ; 
    skos:broader <http://linked.data.gov.au/def/tern-cv/99bd0128-54d4-4a2b-8a2c-48010eb07d26> ; 
    dcterms:created "2020-06-19T15:46:43+00:00"^^xsd:datetime ; 
    dcterms:modified "2020-10-26T06:35:18"^^xsd:datetime ; 
. 

<http://linked.data.gov.au/def/tern-cv/da1ffee9-0121-4ef6-9323-1ad90efbb59e> 
    a skos:Concept ; 
    skos:inScheme <http://linked.data.gov.au/def/tern-cv/5699eca7-9ef0-47a6-bcfb-9306e0e2b85e> ; 
    rdfs:isDefinedBy <http://linked.data.gov.au/def/tern-cv/5699eca7-9ef0-47a6-bcfb-9306e0e2b85e> ; 
    skos:prefLabel "net primary productivity"@en ; 
    skos:definition "The net rate of carbon fixed through photosynthesis (GPP minus plant respiration)."@en ; 
    skos:broader <http://linked.data.gov.au/def/tern-cv/45ae73d8-92bd-4261-a05f-7bfac228e1f7> ; 
    dcterms:created "2020-06-19T15:03:14+00:00"^^xsd:datetime ; 
    dcterms:modified "2021-01-05T00:37:11"^^xsd:datetime ; 
. 

<http://linked.data.gov.au/def/tern-cv/e8e21a9e-908a-4b99-b2ac-5678d73ba3e3> 
    a skos:Concept ; 
    skos:inScheme <http://linked.data.gov.au/def/tern-cv/5699eca7-9ef0-47a6-bcfb-9306e0e2b85e> ; 
    rdfs:isDefinedBy <http://linked.data.gov.au/def/tern-cv/5699eca7-9ef0-47a6-bcfb-9306e0e2b85e> ; 
    skos:prefLabel "non-photosynthetic vegetation fraction"@en ; 
    skos:definition "The fraction of an area (or of a pixel) that contains Non-Photosynthetic Vegetation."@en ; 
    skos:broader <http://linked.data.gov.au/def/tern-cv/45ae73d8-92bd-4261-a05f-7bfac228e1f7> ; 
    dcterms:created "2020-06-19T15:46:43+00:00"^^xsd:datetime ; 
    dcterms:modified "2021-03-26T06:03:24"^^xsd:datetime ; 
. 

<http://linked.data.gov.au/def/tern-cv/00062fdb-3f49-4d06-8ca0-804a154418ba> 
    a skos:Concept ; 
    skos:inScheme <http://linked.data.gov.au/def/tern-cv/5699eca7-9ef0-47a6-bcfb-9306e0e2b85e> ; 
    rdfs:isDefinedBy <http://linked.data.gov.au/def/tern-cv/5699eca7-9ef0-47a6-bcfb-9306e0e2b85e> ; 
    skos:prefLabel "heatwave peak temperature"@en ; 
    skos:definition "Maximum temperature of all heatwave events in a given year"@en ; 
    skos:broader <http://linked.data.gov.au/def/tern-cv/123f2efe-3891-4764-9047-609c8b30e925> ; 
    dcterms:created "2020-08-28T12:23:18+00:00"^^xsd:datetime ; 
    dcterms:modified "2020-08-28T04:28:26.703000+00:00"^^xsd:datetime ; 
. 

<http://linked.data.gov.au/def/tern-cv/4cb6258b-e46d-48e8-8f6c-8ec1d2c6cbf0> 
    a skos:Concept ; 
    skos:inScheme <http://linked.data.gov.au/def/tern-cv/5699eca7-9ef0-47a6-bcfb-9306e0e2b85e> ; 
    rdfs:isDefinedBy <http://linked.data.gov.au/def/tern-cv/5699eca7-9ef0-47a6-bcfb-9306e0e2b85e> ; 
    skos:prefLabel "heatwaves per year"@en ; 
    skos:definition "Number of heatwave events per year"@en ; 
    skos:broader <http://linked.data.gov.au/def/tern-cv/123f2efe-3891-4764-9047-609c8b30e925> ; 
    dcterms:created "2020-08-28T12:31:47+00:00"^^xsd:datetime ; 
    dcterms:modified "2020-08-28T04:28:35.756000+00:00"^^xsd:datetime ; 
. 

<http://linked.data.gov.au/def/tern-cv/8213a995-6c5b-4008-9b42-4376ce8fffee> 
    a skos:Concept ; 
    skos:inScheme <http://linked.data.gov.au/def/tern-cv/5699eca7-9ef0-47a6-bcfb-9306e0e2b85e> ; 
    rdfs:isDefinedBy <http://linked.data.gov.au/def/tern-cv/5699eca7-9ef0-47a6-bcfb-9306e0e2b85e> ; 
    skos:prefLabel "heatwave duration"@en ; 
    skos:definition "Length of the longest heatwave of the year (days)"@en ; 
    skos:broader <http://linked.data.gov.au/def/tern-cv/123f2efe-3891-4764-9047-609c8b30e925> ; 
    dcterms:created "2020-08-28T12:42:00+00:00"^^xsd:datetime ; 
    dcterms:modified "2020-08-28T04:28:10.277000+00:00"^^xsd:datetime ; 
. 

<http://linked.data.gov.au/def/tern-cv/3504a016-8231-40f6-8447-96e5ba279aa1> 
    a skos:Concept ; 
    skos:inScheme <http://linked.data.gov.au/def/tern-cv/5699eca7-9ef0-47a6-bcfb-9306e0e2b85e> ; 
    rdfs:isDefinedBy <http://linked.data.gov.au/def/tern-cv/5699eca7-9ef0-47a6-bcfb-9306e0e2b85e> ; 
    skos:prefLabel "heatwave frequency"@en ; 
    skos:definition "Number of heatwave days relative to number of days in an year calculated as (number of heatwave days/365) ∗ 100 (%)"@en ; 
    skos:broader <http://linked.data.gov.au/def/tern-cv/123f2efe-3891-4764-9047-609c8b30e925> ; 
    dcterms:created "2020-08-28T12:49:58+00:00"^^xsd:datetime ; 
    dcterms:modified "2020-08-28T04:28:18.583000+00:00"^^xsd:datetime ; 
. 

<http://linked.data.gov.au/def/tern-cv/3826b5a3-7128-4df3-90f3-8196c4c20d45> 
    a skos:Concept ; 
    skos:inScheme <http://linked.data.gov.au/def/tern-cv/5699eca7-9ef0-47a6-bcfb-9306e0e2b85e> ; 
    rdfs:isDefinedBy <http://linked.data.gov.au/def/tern-cv/5699eca7-9ef0-47a6-bcfb-9306e0e2b85e> ; 
    skos:prefLabel "stumps count"@en ; 
    skos:definition "Number of stumps per unit area"@en ; 
    skos:broader <http://linked.data.gov.au/def/tern-cv/777773d0-cfb4-44ff-85e2-08b48e10ac52> ; 
    dcterms:created "2020-09-15T01:39:32.273000+00:00"^^xsd:datetime ; 
    dcterms:modified "2021-03-12T00:53:41"^^xsd:datetime ; 
. 

<http://linked.data.gov.au/def/tern-cv/3826b5a3-7128-4df3-90f3-8196c4c20d45> 
    a skos:Concept ; 
    skos:inScheme <http://linked.data.gov.au/def/tern-cv/5699eca7-9ef0-47a6-bcfb-9306e0e2b85e> ; 
    rdfs:isDefinedBy <http://linked.data.gov.au/def/tern-cv/5699eca7-9ef0-47a6-bcfb-9306e0e2b85e> ; 
    skos:prefLabel "stumps count"@en ; 
    skos:definition "Number of stumps per unit area"@en ; 
    skos:broader <http://linked.data.gov.au/def/tern-cv/8fa1c4bd-73b3-432a-ab49-9ee89928e6d9> ; 
    dcterms:created "2020-09-15T01:39:32.273000+00:00"^^xsd:datetime ; 
    dcterms:modified "2021-03-12T00:53:41"^^xsd:datetime ; 
. 

<http://linked.data.gov.au/def/tern-cv/18d64def-df3b-4fa2-ba2d-967c6e392406> 
    a skos:Concept ; 
    skos:inScheme <http://linked.data.gov.au/def/tern-cv/5699eca7-9ef0-47a6-bcfb-9306e0e2b85e> ; 
    rdfs:isDefinedBy <http://linked.data.gov.au/def/tern-cv/5699eca7-9ef0-47a6-bcfb-9306e0e2b85e> ; 
    skos:prefLabel "ringbarked stem count"@en ; 
    skos:definition "Number of stems in the site ringbarked (i.e. complete removal of the bark, including cork cambium to cambium, and even xylem, from around the entire circumference of a trunk of a woody plant), poisoned or thinned."@en ; 
    skos:broader <http://linked.data.gov.au/def/tern-cv/777773d0-cfb4-44ff-85e2-08b48e10ac52> ; 
    dcterms:created "2020-09-15T01:39:57.818000+00:00"^^xsd:datetime ; 
    dcterms:modified "2021-03-12T00:57:24"^^xsd:datetime ; 
. 

<http://linked.data.gov.au/def/tern-cv/18d64def-df3b-4fa2-ba2d-967c6e392406> 
    a skos:Concept ; 
    skos:inScheme <http://linked.data.gov.au/def/tern-cv/5699eca7-9ef0-47a6-bcfb-9306e0e2b85e> ; 
    rdfs:isDefinedBy <http://linked.data.gov.au/def/tern-cv/5699eca7-9ef0-47a6-bcfb-9306e0e2b85e> ; 
    skos:prefLabel "ringbarked stem count"@en ; 
    skos:definition "Number of stems in the site ringbarked (i.e. complete removal of the bark, including cork cambium to cambium, and even xylem, from around the entire circumference of a trunk of a woody plant), poisoned or thinned."@en ; 
    skos:broader <http://linked.data.gov.au/def/tern-cv/8fa1c4bd-73b3-432a-ab49-9ee89928e6d9> ; 
    dcterms:created "2020-09-15T01:39:57.818000+00:00"^^xsd:datetime ; 
    dcterms:modified "2021-03-12T00:57:24"^^xsd:datetime ; 
. 

<http://linked.data.gov.au/def/tern-cv/e349de93-86f4-490b-afdf-1b7fef5603a3> 
    a skos:Concept ; 
    skos:inScheme <http://linked.data.gov.au/def/tern-cv/5699eca7-9ef0-47a6-bcfb-9306e0e2b85e> ; 
    rdfs:isDefinedBy <http://linked.data.gov.au/def/tern-cv/5699eca7-9ef0-47a6-bcfb-9306e0e2b85e> ; 
    skos:prefLabel "presence of vegetation stratum"@en ; 
    skos:definition "presence of vegetation stratum"@en ; 
    skos:broader <http://linked.data.gov.au/def/tern-cv/2ffe4363-dea1-4188-9f8f-835983d47fe2> ; 
    dcterms:created "2020-09-18T05:23:21.978000+00:00"^^xsd:datetime ; 
    dcterms:modified "2021-02-08T01:59:44"^^xsd:datetime ; 
. 

<http://linked.data.gov.au/def/tern-cv/2c122d40-d404-4dcb-964a-ceda57ab5215> 
    a skos:Concept ; 
    skos:inScheme <http://linked.data.gov.au/def/tern-cv/5699eca7-9ef0-47a6-bcfb-9306e0e2b85e> ; 
    rdfs:isDefinedBy <http://linked.data.gov.au/def/tern-cv/5699eca7-9ef0-47a6-bcfb-9306e0e2b85e> ; 
    skos:prefLabel "foliage projective cover"@en ; 
    skos:definition "Foliage Projective Cover (FPC) is a measure of the proportion of the ground area covered by foliage (or photosynthetic tissue) held in a vertical plane. FPC is usually expressed as the percentage of ground covered by foliage and can be separated according to vegetation strata, in particular overstorey or understorey."@en ; 
    skos:broader <http://linked.data.gov.au/def/tern-cv/2ffe4363-dea1-4188-9f8f-835983d47fe2> ; 
    dcterms:created "2020-09-29T10:56:13+00:00"^^xsd:datetime ; 
    dcterms:modified "2020-10-07T06:46:47"^^xsd:datetime ; 
. 

<http://linked.data.gov.au/def/tern-cv/9b9f21a8-1f49-4cee-b537-3297bc706500> 
    a skos:Concept ; 
    skos:inScheme <http://linked.data.gov.au/def/tern-cv/5699eca7-9ef0-47a6-bcfb-9306e0e2b85e> ; 
    rdfs:isDefinedBy <http://linked.data.gov.au/def/tern-cv/5699eca7-9ef0-47a6-bcfb-9306e0e2b85e> ; 
    skos:prefLabel "plant area index"@en ; 
    skos:definition "Plant area index is the projected area of the functional canopy, stems and branches per ground area."@en ; 
    skos:broader <http://linked.data.gov.au/def/tern-cv/2ffe4363-dea1-4188-9f8f-835983d47fe2> ; 
    dcterms:created "2020-09-29T16:52:07+00:00"^^xsd:datetime ; 
    dcterms:modified "2020-12-19T07:44:38"^^xsd:datetime ; 
. 

<http://linked.data.gov.au/def/tern-cv/e9d2e691-dd18-4a38-a987-2fa48c7d5562> 
    a skos:Concept ; 
    skos:inScheme <http://linked.data.gov.au/def/tern-cv/5699eca7-9ef0-47a6-bcfb-9306e0e2b85e> ; 
    rdfs:isDefinedBy <http://linked.data.gov.au/def/tern-cv/5699eca7-9ef0-47a6-bcfb-9306e0e2b85e> ; 
    skos:prefLabel "ground cover - cwd"@en ; 
    skos:definition "Amount of coarse woody debris (i.e. dead wood pieces > 10 cm in diameter for at least a length of 1.5 m) that covers the ground; expressed as a percentage."@en ; 
    skos:broader <http://linked.data.gov.au/def/tern-cv/7dc7ae5c-f074-4536-9032-f59eba3f9270> ; 
    dcterms:created "2020-10-28T05:31:18"^^xsd:datetime ; 
    dcterms:modified "2020-12-19T08:10:06"^^xsd:datetime ; 
. 

<http://linked.data.gov.au/def/tern-cv/e3b19733-defc-417d-9513-f9260b9553af> 
    a skos:Concept ; 
    skos:inScheme <http://linked.data.gov.au/def/tern-cv/5699eca7-9ef0-47a6-bcfb-9306e0e2b85e> ; 
    rdfs:isDefinedBy <http://linked.data.gov.au/def/tern-cv/5699eca7-9ef0-47a6-bcfb-9306e0e2b85e> ; 
    skos:prefLabel "ground cover - outcrop"@en ; 
    skos:definition "Estimate of the percentage of the site that is outcrop (exposed consolidated rock (bedrock))."@en ; 
    skos:broader <http://linked.data.gov.au/def/tern-cv/7dc7ae5c-f074-4536-9032-f59eba3f9270> ; 
    dcterms:created "2020-10-28T05:32:34"^^xsd:datetime ; 
    dcterms:modified "2020-11-09T02:14:48"^^xsd:datetime ; 
. 

<http://linked.data.gov.au/def/tern-cv/4392769d-ab14-4575-af5a-103e133eee3f> 
    a skos:Concept ; 
    skos:inScheme <http://linked.data.gov.au/def/tern-cv/5699eca7-9ef0-47a6-bcfb-9306e0e2b85e> ; 
    rdfs:isDefinedBy <http://linked.data.gov.au/def/tern-cv/5699eca7-9ef0-47a6-bcfb-9306e0e2b85e> ; 
    skos:prefLabel "ground cover - gravel"@en ; 
    skos:definition "Amount of gravel (i.e. particles > 2mm) that covers the ground expressed as a percentage."@en ; 
    skos:broader <http://linked.data.gov.au/def/tern-cv/7dc7ae5c-f074-4536-9032-f59eba3f9270> ; 
    dcterms:created "2020-10-28T05:33:01"^^xsd:datetime ; 
    dcterms:modified "2020-12-19T07:19:06"^^xsd:datetime ; 
. 

<http://linked.data.gov.au/def/tern-cv/998a886b-d40d-43cd-ac1a-0a682018b4e5> 
    a skos:Concept ; 
    skos:inScheme <http://linked.data.gov.au/def/tern-cv/5699eca7-9ef0-47a6-bcfb-9306e0e2b85e> ; 
    rdfs:isDefinedBy <http://linked.data.gov.au/def/tern-cv/5699eca7-9ef0-47a6-bcfb-9306e0e2b85e> ; 
    skos:prefLabel "ground cover - not collected"@en ; 
    skos:definition "Amount of cover type that was not collected; expressed as a percentage."@en ; 
    skos:broader <http://linked.data.gov.au/def/tern-cv/7dc7ae5c-f074-4536-9032-f59eba3f9270> ; 
    dcterms:created "2020-10-28T05:33:30"^^xsd:datetime ; 
    dcterms:modified "2020-12-19T07:39:55"^^xsd:datetime ; 
. 

<http://linked.data.gov.au/def/tern-cv/03c6e286-27b4-4671-bb9b-ae0819a28eaf> 
    a skos:Concept ; 
    skos:inScheme <http://linked.data.gov.au/def/tern-cv/5699eca7-9ef0-47a6-bcfb-9306e0e2b85e> ; 
    rdfs:isDefinedBy <http://linked.data.gov.au/def/tern-cv/5699eca7-9ef0-47a6-bcfb-9306e0e2b85e> ; 
    skos:prefLabel "species richness"@en ; 
    skos:definition "The total number of species in the sample (i.e. site, plot)."@en ; 
    skos:broader <http://linked.data.gov.au/def/tern-cv/2ffe4363-dea1-4188-9f8f-835983d47fe2> ; 
    dcterms:created "2020-10-28T06:37:47"^^xsd:datetime ; 
    dcterms:modified "2021-01-04T23:42:33"^^xsd:datetime ; 
. 

<http://linked.data.gov.au/def/tern-cv/3c21b608-9164-4e65-913b-ed29801b6ed6> 
    a skos:Concept ; 
    skos:inScheme <http://linked.data.gov.au/def/tern-cv/5699eca7-9ef0-47a6-bcfb-9306e0e2b85e> ; 
    rdfs:isDefinedBy <http://linked.data.gov.au/def/tern-cv/5699eca7-9ef0-47a6-bcfb-9306e0e2b85e> ; 
    skos:prefLabel "relative species abundance"@en ; 
    skos:definition "Relative frequency of species in a sample calculated from raw species abundance (i.e. percent Frequency[i] = a[i]/Sigma(a[i])) x 100)"@en ; 
    skos:broader <http://linked.data.gov.au/def/tern-cv/2ffe4363-dea1-4188-9f8f-835983d47fe2> ; 
    dcterms:created "2020-10-28T06:38:29"^^xsd:datetime ; 
    dcterms:modified "2020-12-19T07:12:54"^^xsd:datetime ; 
. 

<http://linked.data.gov.au/def/tern-cv/b31f9f9d-090f-46e7-b03c-36ca696621f5> 
    a skos:Concept ; 
    skos:inScheme <http://linked.data.gov.au/def/tern-cv/5699eca7-9ef0-47a6-bcfb-9306e0e2b85e> ; 
    rdfs:isDefinedBy <http://linked.data.gov.au/def/tern-cv/5699eca7-9ef0-47a6-bcfb-9306e0e2b85e> ; 
    skos:prefLabel "ground cover - unknown"@en ; 
    skos:definition "Amount of unknown cover that covers the ground; expressed as a percentage."@en ; 
    skos:broader <http://linked.data.gov.au/def/tern-cv/7dc7ae5c-f074-4536-9032-f59eba3f9270> ; 
    dcterms:created "2020-10-28T05:34:02"^^xsd:datetime ; 
    dcterms:modified "2020-12-19T07:50:54"^^xsd:datetime ; 
. 

<http://linked.data.gov.au/def/tern-cv/7dc7ae5c-f074-4536-9032-f59eba3f9270> 
    a skos:Concept ; 
    skos:inScheme <http://linked.data.gov.au/def/tern-cv/5699eca7-9ef0-47a6-bcfb-9306e0e2b85e> ; 
    rdfs:isDefinedBy <http://linked.data.gov.au/def/tern-cv/5699eca7-9ef0-47a6-bcfb-9306e0e2b85e> ; 
    skos:prefLabel "ground cover"@en ; 
    skos:definition "Amount of ground covered by some material or bare; usually estimated as a percentage."@en ; 
    skos:broader <http://linked.data.gov.au/def/tern-cv/d62a4664-89a1-49a1-9ef0-f30ee2c6d22b> ; 
    dcterms:created "2020-11-04T05:25:31"^^xsd:datetime ; 
    dcterms:modified "2020-12-19T07:34:22"^^xsd:datetime ; 
. 

<http://linked.data.gov.au/def/tern-cv/123f2efe-3891-4764-9047-609c8b30e925> 
    a skos:Concept ; 
    skos:inScheme <http://linked.data.gov.au/def/tern-cv/5699eca7-9ef0-47a6-bcfb-9306e0e2b85e> ; 
    rdfs:isDefinedBy <http://linked.data.gov.au/def/tern-cv/5699eca7-9ef0-47a6-bcfb-9306e0e2b85e> ; 
    skos:prefLabel "atmospheric parameter"@en ; 
    skos:definition "Measures related to the layer of gases surrounding Earth"@en ; 
    skos:topConceptOf <http://linked.data.gov.au/def/tern-cv/5699eca7-9ef0-47a6-bcfb-9306e0e2b85e>  ; 
    dcterms:created "2020-11-05T06:17:38"^^xsd:datetime ; 
    dcterms:modified "2020-12-18T23:43:32"^^xsd:datetime ; 
. 

<http://linked.data.gov.au/def/tern-cv/e27ee9af-4fde-46aa-a068-f847834269a6> 
    a skos:Concept ; 
    skos:inScheme <http://linked.data.gov.au/def/tern-cv/5699eca7-9ef0-47a6-bcfb-9306e0e2b85e> ; 
    rdfs:isDefinedBy <http://linked.data.gov.au/def/tern-cv/5699eca7-9ef0-47a6-bcfb-9306e0e2b85e> ; 
    skos:prefLabel "fine earth bulk density"@en ; 
    skos:definition "Field soil bulk density for particles < 2mm. Bulk density was determined as the ratio of the mass of solids to the total volume of a moist soil core of known volume. The total volume includes the volume of both solids and pore space. For fine earth bulk density (<2-mm particles) the mass and volume of rock fragments are subtracted from the total mass and volume."@en ; 
    skos:broader <http://linked.data.gov.au/def/tern-cv/0531b8b6-7610-4fbd-9a66-8cd80d357a70> ; 
    dcterms:created "2020-11-06T00:27:04"^^xsd:datetime ; 
    dcterms:modified "2021-01-05T00:38:35"^^xsd:datetime ; 
. 

<http://linked.data.gov.au/def/tern-cv/d7bbfb51-4697-4ca9-9846-2511056e3d9d> 
    a skos:Concept ; 
    skos:inScheme <http://linked.data.gov.au/def/tern-cv/5699eca7-9ef0-47a6-bcfb-9306e0e2b85e> ; 
    rdfs:isDefinedBy <http://linked.data.gov.au/def/tern-cv/5699eca7-9ef0-47a6-bcfb-9306e0e2b85e> ; 
    skos:prefLabel "gravel bulk density"@en ; 
    skos:definition "Bulk density of particles > 2mm to < 2cm (see Vincent et al 1994). Gravel Bulk density is determined as the ratio of the mass of gravel to the total volume of gravel from a soil sample (Vincent et al 1994). Gravel is oven dried without washing off the fine earth for 24 h at 105°C, and weighed. Then gravel volume is determined using the volumetric displacement method."@en ; 
    skos:broader <http://linked.data.gov.au/def/tern-cv/0531b8b6-7610-4fbd-9a66-8cd80d357a70> ; 
    dcterms:created "2020-11-06T00:28:07"^^xsd:datetime ; 
    dcterms:modified "2021-01-05T00:32:25"^^xsd:datetime ; 
. 

<http://linked.data.gov.au/def/tern-cv/99bd0128-54d4-4a2b-8a2c-48010eb07d26> 
    a skos:Concept ; 
    skos:inScheme <http://linked.data.gov.au/def/tern-cv/5699eca7-9ef0-47a6-bcfb-9306e0e2b85e> ; 
    rdfs:isDefinedBy <http://linked.data.gov.au/def/tern-cv/5699eca7-9ef0-47a6-bcfb-9306e0e2b85e> ; 
    skos:prefLabel "soil parameter"@en ; 
    skos:definition "The top layer of the land surface of the earth that is composed of disintegrated rock particles, humus, water and air."@en ; 
    skos:topConceptOf <http://linked.data.gov.au/def/tern-cv/5699eca7-9ef0-47a6-bcfb-9306e0e2b85e>  ; 
    dcterms:created "2020-11-06T02:30:20"^^xsd:datetime ; 
    dcterms:modified "2021-01-05T00:25:06"^^xsd:datetime ; 
. 

<http://linked.data.gov.au/def/tern-cv/68add852-0a47-4412-8f8c-52bd8d0151b1> 
    a skos:Concept ; 
    skos:inScheme <http://linked.data.gov.au/def/tern-cv/5699eca7-9ef0-47a6-bcfb-9306e0e2b85e> ; 
    rdfs:isDefinedBy <http://linked.data.gov.au/def/tern-cv/5699eca7-9ef0-47a6-bcfb-9306e0e2b85e> ; 
    skos:prefLabel "agricultural parameter"@en ; 
    skos:definition "Measures related to the cultivation of plants and livestock."@en ; 
    skos:topConceptOf <http://linked.data.gov.au/def/tern-cv/5699eca7-9ef0-47a6-bcfb-9306e0e2b85e>  ; 
    dcterms:created "2020-11-09T04:56:37"^^xsd:datetime ; 
    dcterms:modified "2020-12-19T07:25:07"^^xsd:datetime ; 
. 

<http://linked.data.gov.au/def/tern-cv/2ffe4363-dea1-4188-9f8f-835983d47fe2> 
    a skos:Concept ; 
    skos:inScheme <http://linked.data.gov.au/def/tern-cv/5699eca7-9ef0-47a6-bcfb-9306e0e2b85e> ; 
    rdfs:isDefinedBy <http://linked.data.gov.au/def/tern-cv/5699eca7-9ef0-47a6-bcfb-9306e0e2b85e> ; 
    skos:prefLabel "biological parameter"@en ; 
    skos:definition "Living organisms and life."@en ; 
    skos:topConceptOf <http://linked.data.gov.au/def/tern-cv/5699eca7-9ef0-47a6-bcfb-9306e0e2b85e>  ; 
    dcterms:created "2020-11-09T04:57:05"^^xsd:datetime ; 
    dcterms:modified "2021-04-08T00:43:06"^^xsd:datetime ; 
. 


<http://linked.data.gov.au/def/tern-cv/45ae73d8-92bd-4261-a05f-7bfac228e1f7> 
    a skos:Concept ; 
    skos:inScheme <http://linked.data.gov.au/def/tern-cv/5699eca7-9ef0-47a6-bcfb-9306e0e2b85e> ; 
    rdfs:isDefinedBy <http://linked.data.gov.au/def/tern-cv/5699eca7-9ef0-47a6-bcfb-9306e0e2b85e> ; 
    skos:prefLabel "ecosystem parameter"@en ; 
    skos:definition "The flow of energy and matter between organisms and their physical environment within an Earth-System context."@en ; 
    skos:topConceptOf <http://linked.data.gov.au/def/tern-cv/5699eca7-9ef0-47a6-bcfb-9306e0e2b85e>  ; 
    dcterms:created "2020-11-09T04:57:38"^^xsd:datetime ; 
    dcterms:modified "2020-12-19T07:20:26"^^xsd:datetime ; 
. 

<http://linked.data.gov.au/def/tern-cv/d62a4664-89a1-49a1-9ef0-f30ee2c6d22b> 
    a skos:Concept ; 
    skos:inScheme <http://linked.data.gov.au/def/tern-cv/5699eca7-9ef0-47a6-bcfb-9306e0e2b85e> ; 
    rdfs:isDefinedBy <http://linked.data.gov.au/def/tern-cv/5699eca7-9ef0-47a6-bcfb-9306e0e2b85e> ; 
    skos:prefLabel "environmental parameter"@en ; 
    skos:definition "The external elements and conditions which surround, influence, and affect the life and development of an organism or population."@en ; 
    skos:topConceptOf <http://linked.data.gov.au/def/tern-cv/5699eca7-9ef0-47a6-bcfb-9306e0e2b85e>  ; 
    skos:narrower <http://linked.data.gov.au/def/tern-cv/76806e0f-61a2-447c-8177-7e666637e23a>,
        <http://linked.data.gov.au/def/tern-cv/7dc7ae5c-f074-4536-9032-f59eba3f9270> ;
    dcterms:created "2020-11-09T04:57:55"^^xsd:datetime ; 
    dcterms:modified "2021-01-05T00:28:35"^^xsd:datetime ; 
. 

<http://linked.data.gov.au/def/tern-cv/50b9def1-660b-4274-b10e-6dbe57243305> 
    a skos:Concept ; 
    skos:inScheme <http://linked.data.gov.au/def/tern-cv/5699eca7-9ef0-47a6-bcfb-9306e0e2b85e> ; 
    rdfs:isDefinedBy <http://linked.data.gov.au/def/tern-cv/5699eca7-9ef0-47a6-bcfb-9306e0e2b85e> ; 
    skos:prefLabel "genetic parameter"@en ; 
    skos:definition "Measures concern with the study of genes, genetic variation, and heredity in organisms."@en ; 
    skos:topConceptOf <http://linked.data.gov.au/def/tern-cv/5699eca7-9ef0-47a6-bcfb-9306e0e2b85e>  ; 
    dcterms:created "2020-11-09T04:58:07"^^xsd:datetime ; 
    dcterms:modified "2020-12-19T07:22:09"^^xsd:datetime ; 
. 

<http://linked.data.gov.au/def/tern-cv/29bd4356-5638-49c0-8d3e-57598ac2ea6c> 
    a skos:Concept ; 
    skos:inScheme <http://linked.data.gov.au/def/tern-cv/5699eca7-9ef0-47a6-bcfb-9306e0e2b85e> ; 
    rdfs:isDefinedBy <http://linked.data.gov.au/def/tern-cv/5699eca7-9ef0-47a6-bcfb-9306e0e2b85e> ; 
    skos:prefLabel "landscape parameter"@en ; 
    skos:definition "The traits, patterns, and structure of a specific geographic area, including its biological composition, its physical environment, and its anthropogenic or social patterns. An area where interacting ecosystems are grouped and repeated in similar form."@en ; 
    skos:topConceptOf <http://linked.data.gov.au/def/tern-cv/5699eca7-9ef0-47a6-bcfb-9306e0e2b85e>  ; 
    dcterms:created "2020-11-09T04:58:26"^^xsd:datetime ; 
    dcterms:modified "2021-01-04T23:49:32"^^xsd:datetime ; 
. 

<http://linked.data.gov.au/def/tern-cv/9e03a73d-8e89-4187-9f96-0306aad93458> 
    a skos:Concept ; 
    skos:inScheme <http://linked.data.gov.au/def/tern-cv/5699eca7-9ef0-47a6-bcfb-9306e0e2b85e> ; 
    rdfs:isDefinedBy <http://linked.data.gov.au/def/tern-cv/5699eca7-9ef0-47a6-bcfb-9306e0e2b85e> ; 
    skos:prefLabel "physical parameter"@en ; 
    skos:definition "Measurable physical characteristic. Its value describes a state of a physical system."@en ; 
    skos:topConceptOf <http://linked.data.gov.au/def/tern-cv/5699eca7-9ef0-47a6-bcfb-9306e0e2b85e>  ; 
    skos:narrower <http://linked.data.gov.au/def/tern-cv/54fd271e-d0a9-4e82-967a-c013c47760d9>,
        <http://linked.data.gov.au/def/tern-cv/aa7d5f61-99e6-4e34-8a46-40ac5fbd7b14> ;
    dcterms:created "2020-11-09T04:58:47"^^xsd:datetime ; 
    dcterms:modified "2020-12-19T07:45:31"^^xsd:datetime ; 
. 

<http://linked.data.gov.au/def/tern-cv/bb5c1354-8d70-47b2-b333-87e3bf1157d6> 
    a skos:Concept ; 
    skos:inScheme <http://linked.data.gov.au/def/tern-cv/5699eca7-9ef0-47a6-bcfb-9306e0e2b85e> ; 
    rdfs:isDefinedBy <http://linked.data.gov.au/def/tern-cv/5699eca7-9ef0-47a6-bcfb-9306e0e2b85e> ; 
    skos:prefLabel "water parameter"@en ; 
    skos:definition "A clear, odorless, tasteless liquid that is essential for most animal and plant life, and is an excellent solvent for many substances."@en ; 
    skos:topConceptOf <http://linked.data.gov.au/def/tern-cv/5699eca7-9ef0-47a6-bcfb-9306e0e2b85e>  ; 
    skos:narrower <http://linked.data.gov.au/def/tern-cv/2cf66d7b-6625-44d5-85d9-91f350afe7f0>,
        <http://linked.data.gov.au/def/tern-cv/809b2517-819e-4c8f-92e8-7dd11a95cc72> ;
    dcterms:created "2020-11-09T04:59:03"^^xsd:datetime ; 
    dcterms:modified "2021-01-05T00:27:43"^^xsd:datetime ; 
. 

<http://linked.data.gov.au/def/tern-cv/8b26b66b-9e39-47eb-807f-621f1119377d> 
    a skos:Concept ; 
    skos:inScheme <http://linked.data.gov.au/def/tern-cv/5699eca7-9ef0-47a6-bcfb-9306e0e2b85e> ; 
    rdfs:isDefinedBy <http://linked.data.gov.au/def/tern-cv/5699eca7-9ef0-47a6-bcfb-9306e0e2b85e> ; 
    skos:prefLabel "ground cover - green"@en ; 
    skos:definition "Amount of ground covered by vegetation; expressed as a percentage."@en ; 
    skos:broader <http://linked.data.gov.au/def/tern-cv/7dc7ae5c-f074-4536-9032-f59eba3f9270> ; 
    dcterms:created "2020-12-09T06:52:28"^^xsd:datetime ; 
    dcterms:modified "2020-12-19T07:34:08"^^xsd:datetime ; 
. 

<http://linked.data.gov.au/def/tern-cv/74c71500-0bae-43c9-8db0-bd6940899af1> 
    a skos:Concept ; 
    skos:inScheme <http://linked.data.gov.au/def/tern-cv/5699eca7-9ef0-47a6-bcfb-9306e0e2b85e> ; 
    rdfs:isDefinedBy <http://linked.data.gov.au/def/tern-cv/5699eca7-9ef0-47a6-bcfb-9306e0e2b85e> ; 
    skos:prefLabel "individual count"@en ; 
    skos:definition "The number of individuals present at the time of sampling."@en ; 
    skos:broader <http://linked.data.gov.au/def/tern-cv/2ffe4363-dea1-4188-9f8f-835983d47fe2> ; 
    dcterms:created "2020-12-09T23:49:34"^^xsd:datetime ; 
    dcterms:modified "2021-03-11T06:24:10"^^xsd:datetime ; 
. 

<http://linked.data.gov.au/def/tern-cv/57524a84-ddfa-4dfd-8bfe-878dcd826226> 
    a skos:Concept ; 
    skos:inScheme <http://linked.data.gov.au/def/tern-cv/5699eca7-9ef0-47a6-bcfb-9306e0e2b85e> ; 
    rdfs:isDefinedBy <http://linked.data.gov.au/def/tern-cv/5699eca7-9ef0-47a6-bcfb-9306e0e2b85e> ; 
    skos:prefLabel "visible wavelengths"@en ; 
    skos:definition "The region of the electromagnetic spectrum (0.4 to 0.7 μm) that is visible to the human eye, and can be interpreted as different colours related to different proportions of red, green and blue wavelengths. This spectral region is of special interest in sensing of leaf pigments, surface water quality, and soil minerals and can be captured as reflected light using a camera or imaging spectrometer."@en ; 
    skos:broader <http://linked.data.gov.au/def/tern-cv/41a27c10-6dff-4ddc-9f8b-14e87fafc786> ; 
    dcterms:modified "2021-04-23T08:20:21"^^xsd:datetime ; 
. 

<http://linked.data.gov.au/def/tern-cv/66d5552f-fa72-4032-8ac5-e087b214b770> 
    a skos:Concept ; 
    skos:inScheme <http://linked.data.gov.au/def/tern-cv/5699eca7-9ef0-47a6-bcfb-9306e0e2b85e> ; 
    rdfs:isDefinedBy <http://linked.data.gov.au/def/tern-cv/5699eca7-9ef0-47a6-bcfb-9306e0e2b85e> ; 
    skos:prefLabel "near-infrared wavelengths"@en ; 
    skos:definition "The near-infrared region of the electromagnetic spectrum (NIR, 0.7 to 1.3 μm). This portion of the spectrum lies outside the human eye’s sensing capability. NIR has high sensitivity to leaf structure and morphology and can be captured as reflected light using a camera or imaging spectrometer."@en ; 
    skos:broader <http://linked.data.gov.au/def/tern-cv/41a27c10-6dff-4ddc-9f8b-14e87fafc786> ; 
. 

<http://linked.data.gov.au/def/tern-cv/d4c0646c-2504-496b-bd01-95c1097b5021> 
    a skos:Concept ; 
    skos:inScheme <http://linked.data.gov.au/def/tern-cv/5699eca7-9ef0-47a6-bcfb-9306e0e2b85e> ; 
    rdfs:isDefinedBy <http://linked.data.gov.au/def/tern-cv/5699eca7-9ef0-47a6-bcfb-9306e0e2b85e> ; 
    skos:prefLabel "normalised difference vegetation index"@en ; 
    skos:definition "A vegetation index to depict canopy greenness as an integrative measure of variations in leaf physiology, structure and area-averaged canopy photosynthetic activity.  NDVI is calculated as the ratio of electromagnetic wavelengths (NIR-Red)/(NIR+Red), as captured by a camera or imaging spectrometer."@en ; 
    skos:broader <http://linked.data.gov.au/def/tern-cv/41a27c10-6dff-4ddc-9f8b-14e87fafc786> ; 
.

<http://linked.data.gov.au/def/tern-cv/26526741-5aa1-4cfa-9512-1d3182ea3b13> 
    a skos:Concept ; 
    skos:inScheme <http://linked.data.gov.au/def/tern-cv/5699eca7-9ef0-47a6-bcfb-9306e0e2b85e> ; 
    rdfs:isDefinedBy <http://linked.data.gov.au/def/tern-cv/5699eca7-9ef0-47a6-bcfb-9306e0e2b85e> ; 
    skos:prefLabel "visible and near-infrared wavelengths"@en ; 
    skos:definition "The visible and the near-infrared regions of the electromagnetic spectrum (VNIR, 0.4 to 1.3 μm).  The visible range of the spectrum can be interpreted as different colours related to different proportions of red, green and blue wavelengths,  while the infrared range lies outside the human eye’s sensing capability. These wavelengths can be captured as reflected light using a camera or imaging spectrometer to provide information about the structure, composition and properties of the reflecting objects."@en ; 
    skos:broader <http://linked.data.gov.au/def/tern-cv/41a27c10-6dff-4ddc-9f8b-14e87fafc786> ; 
.

<http://linked.data.gov.au/def/tern-cv/fc1155cd-12cd-4355-9b07-051b10a8f4eb> 
    a skos:Concept ; 
    skos:inScheme <http://linked.data.gov.au/def/tern-cv/5699eca7-9ef0-47a6-bcfb-9306e0e2b85e> ; 
    rdfs:isDefinedBy <http://linked.data.gov.au/def/tern-cv/5699eca7-9ef0-47a6-bcfb-9306e0e2b85e> ; 
    skos:prefLabel "subdominant substrate lithology"@en ; 
    skos:definition "The second most (sub)dominant outcrop lithology. The lithology of the coarse fragments is usually identified as coming from the substrate or from rock outcrop. Where the lithology of the coarse fragments is different from that of the substrate material and/or rock outcrop, describe it as for lithology of substrate material only where the rock type is definitely known or is confidently presumed. Some coarse fragments are commonly encountered that are not directly related to the substrate material."@en ; 
    skos:broader <http://linked.data.gov.au/def/tern-cv/99bd0128-54d4-4a2b-8a2c-48010eb07d26> ; 
    dcterms:modified "2020-07-09T06:54:56.425000+00:00"^^xsd:datetime ; 
. 

<http://linked.data.gov.au/def/tern-cv/82bca582-f0c2-480e-be0b-c33b19d80e73> 
    a skos:Concept ; 
    skos:inScheme <http://linked.data.gov.au/def/tern-cv/5699eca7-9ef0-47a6-bcfb-9306e0e2b85e> ; 
    rdfs:isDefinedBy <http://linked.data.gov.au/def/tern-cv/5699eca7-9ef0-47a6-bcfb-9306e0e2b85e> ; 
    skos:prefLabel "angle count sampling hits"@en ; 
    skos:definition "The count of individual trunks within the sampling area that meet the size criteria of the basal area factor when using a basal wedge."@en ; 
    skos:broader <http://linked.data.gov.au/def/tern-cv/8fa1c4bd-73b3-432a-ab49-9ee89928e6d9> ; 
    dcterms:created "2021-02-01T04:46:09"^^xsd:datetime ; 
    dcterms:modified "2021-05-10T01:37:18"^^xsd:datetime ; 
. 

<http://linked.data.gov.au/def/tern-cv/cd11241d-9df9-48b9-88b1-3e6646f21562> 
    a skos:Concept ; 
    skos:inScheme <http://linked.data.gov.au/def/tern-cv/5699eca7-9ef0-47a6-bcfb-9306e0e2b85e> ; 
    rdfs:isDefinedBy <http://linked.data.gov.au/def/tern-cv/5699eca7-9ef0-47a6-bcfb-9306e0e2b85e> ; 
    skos:prefLabel "dead plant"@en ; 
    skos:definition "dead plant"@en ; 
    skos:broader <http://linked.data.gov.au/def/tern-cv/8fa1c4bd-73b3-432a-ab49-9ee89928e6d9> ; 
    dcterms:created "2021-02-01T05:02:46"^^xsd:datetime ; 
    dcterms:modified "2021-03-26T06:01:00"^^xsd:datetime ; 
. 

<http://linked.data.gov.au/def/tern-cv/700daf25-0a3f-461e-a799-be80ef2f8cd4> 
    a skos:Concept ; 
    skos:inScheme <http://linked.data.gov.au/def/tern-cv/5699eca7-9ef0-47a6-bcfb-9306e0e2b85e> ; 
    rdfs:isDefinedBy <http://linked.data.gov.au/def/tern-cv/5699eca7-9ef0-47a6-bcfb-9306e0e2b85e> ; 
    skos:prefLabel "iron oxide or ferrous minerals indices"@en ; 
    skos:definition "Indicator of possible areas of iron oxide or ferrous minerals abundance across a landscape. Calculated from a ratio of two or more spectral bands from satellite imagery, for example Landsat Bands 3/1, the indicator may vary in effectiveness across the landscape."@en ; 
    skos:broader <http://linked.data.gov.au/def/tern-cv/99bd0128-54d4-4a2b-8a2c-48010eb07d26> ; 
    skos:narrower <http://linked.data.gov.au/def/tern-cv/1beaac85-44c0-4097-aa11-8d44f6381bc9>,
        <http://linked.data.gov.au/def/tern-cv/1e762c90-28e3-41e9-957f-f4cf672aee44>,
        <http://linked.data.gov.au/def/tern-cv/803a7efd-71b6-4e4b-b018-4fe884f86491>,
        <http://linked.data.gov.au/def/tern-cv/8f398304-d6c1-475e-bb12-72fc90d3a69c>,
        <http://linked.data.gov.au/def/tern-cv/cd934e78-f84d-4a36-a373-d3e817c306be> ;
    dcterms:created "2021-02-03T06:15:57"^^xsd:datetime ; 
    dcterms:modified "2021-02-04T03:21:09"^^xsd:datetime ; 
. 

<http://linked.data.gov.au/def/tern-cv/700daf25-0a3f-461e-a799-be80ef2f8cd4> 
    a skos:Concept ; 
    skos:inScheme <http://linked.data.gov.au/def/tern-cv/5699eca7-9ef0-47a6-bcfb-9306e0e2b85e> ; 
    rdfs:isDefinedBy <http://linked.data.gov.au/def/tern-cv/5699eca7-9ef0-47a6-bcfb-9306e0e2b85e> ; 
    skos:prefLabel "iron oxide or ferrous minerals indices"@en ; 
    skos:definition "Indicator of possible areas of iron oxide or ferrous minerals abundance across a landscape. Calculated from a ratio of two or more spectral bands from satellite imagery, for example Landsat Bands 3/1, the indicator may vary in effectiveness across the landscape."@en ; 
    skos:broader <http://linked.data.gov.au/def/tern-cv/41a27c10-6dff-4ddc-9f8b-14e87fafc786> ; 
    dcterms:created "2021-02-03T06:15:57"^^xsd:datetime ; 
    dcterms:modified "2021-02-04T03:21:09"^^xsd:datetime ; 
. 

<http://linked.data.gov.au/def/tern-cv/cd934e78-f84d-4a36-a373-d3e817c306be> 
    a skos:Concept ; 
    skos:inScheme <http://linked.data.gov.au/def/tern-cv/5699eca7-9ef0-47a6-bcfb-9306e0e2b85e> ; 
    rdfs:isDefinedBy <http://linked.data.gov.au/def/tern-cv/5699eca7-9ef0-47a6-bcfb-9306e0e2b85e> ; 
    skos:prefLabel "iron oxide index (RED/BLUE)"@en ; 
    skos:definition "Indicator of possible areas of iron oxide abundance across a landscape. Calculated from a ratio of RED/BLUE spectral bands from satellite imagery, the indicator may vary in effectiveness across the landscape."@en ; 
    skos:broader <http://linked.data.gov.au/def/tern-cv/700daf25-0a3f-461e-a799-be80ef2f8cd4> ; 
    dcterms:created "2021-02-03T07:25:56"^^xsd:datetime ; 
    dcterms:modified "2021-02-04T02:11:31"^^xsd:datetime ; 
. 

<http://linked.data.gov.au/def/tern-cv/8f398304-d6c1-475e-bb12-72fc90d3a69c> 
    a skos:Concept ; 
    skos:inScheme <http://linked.data.gov.au/def/tern-cv/5699eca7-9ef0-47a6-bcfb-9306e0e2b85e> ; 
    rdfs:isDefinedBy <http://linked.data.gov.au/def/tern-cv/5699eca7-9ef0-47a6-bcfb-9306e0e2b85e> ; 
    skos:prefLabel "iron oxide index (SWIR2/NIR)"@en ; 
    skos:definition "Indicator of possible areas of iron oxide abundance across a landscape. Calculated from a ratio of SWIR2/NIR spectral bands from satellite imagery, the indicator may vary in effectiveness across the landscape."@en ; 
    skos:broader <http://linked.data.gov.au/def/tern-cv/700daf25-0a3f-461e-a799-be80ef2f8cd4> ; 
    dcterms:created "2021-02-03T07:25:56"^^xsd:datetime ; 
    dcterms:modified "2021-02-04T01:10:53"^^xsd:datetime ; 
. 

<http://linked.data.gov.au/def/tern-cv/12797115-2e0f-479f-8d06-1700da3ac394> 
    a skos:Concept ; 
    skos:inScheme <http://linked.data.gov.au/def/tern-cv/5699eca7-9ef0-47a6-bcfb-9306e0e2b85e> ; 
    rdfs:isDefinedBy <http://linked.data.gov.au/def/tern-cv/5699eca7-9ef0-47a6-bcfb-9306e0e2b85e> ; 
    skos:prefLabel "carbonate/quartz index"@en ; 
    skos:definition "Indicator of possible areas of highly reflective carbonate/quartz abundance across a landscape. Calculated from a combination of spectral bands of satellite imagery, the indicator may vary in effectiveness across the landscape."@en ; 
    skos:broader <http://linked.data.gov.au/def/tern-cv/99bd0128-54d4-4a2b-8a2c-48010eb07d26> ; 
    skos:narrower <http://linked.data.gov.au/def/tern-cv/bb942400-8bc5-4831-bcf5-7a891ef00ef4> ;
    dcterms:created "2021-02-03T06:15:57"^^xsd:datetime ; 
    dcterms:modified "2021-02-04T01:53:23"^^xsd:datetime ; 
. 

<http://linked.data.gov.au/def/tern-cv/12797115-2e0f-479f-8d06-1700da3ac394> 
    a skos:Concept ; 
    skos:inScheme <http://linked.data.gov.au/def/tern-cv/5699eca7-9ef0-47a6-bcfb-9306e0e2b85e> ; 
    rdfs:isDefinedBy <http://linked.data.gov.au/def/tern-cv/5699eca7-9ef0-47a6-bcfb-9306e0e2b85e> ; 
    skos:prefLabel "carbonate/quartz index"@en ; 
    skos:definition "Indicator of possible areas of highly reflective carbonate/quartz abundance across a landscape. Calculated from a combination of spectral bands of satellite imagery, the indicator may vary in effectiveness across the landscape."@en ; 
    skos:broader <http://linked.data.gov.au/def/tern-cv/99bd0128-54d4-4a2b-8a2c-48010eb07d26> ; 
    dcterms:created "2021-02-03T07:25:56"^^xsd:datetime ; 
    dcterms:modified "2021-02-04T01:53:23"^^xsd:datetime ; 
. 

<http://linked.data.gov.au/def/tern-cv/12797115-2e0f-479f-8d06-1700da3ac394> 
    a skos:Concept ; 
    skos:inScheme <http://linked.data.gov.au/def/tern-cv/5699eca7-9ef0-47a6-bcfb-9306e0e2b85e> ; 
    rdfs:isDefinedBy <http://linked.data.gov.au/def/tern-cv/5699eca7-9ef0-47a6-bcfb-9306e0e2b85e> ; 
    skos:prefLabel "carbonate/quartz index"@en ; 
    skos:definition "Indicator of possible areas of highly reflective carbonate/quartz abundance across a landscape. Calculated from a combination of spectral bands of satellite imagery, the indicator may vary in effectiveness across the landscape."@en ; 
    skos:broader <http://linked.data.gov.au/def/tern-cv/41a27c10-6dff-4ddc-9f8b-14e87fafc786> ; 
    dcterms:created "2021-02-03T06:15:57"^^xsd:datetime ; 
    dcterms:modified "2021-02-04T01:53:23"^^xsd:datetime ; 
. 

<http://linked.data.gov.au/def/tern-cv/12797115-2e0f-479f-8d06-1700da3ac394> 
    a skos:Concept ; 
    skos:inScheme <http://linked.data.gov.au/def/tern-cv/5699eca7-9ef0-47a6-bcfb-9306e0e2b85e> ; 
    rdfs:isDefinedBy <http://linked.data.gov.au/def/tern-cv/5699eca7-9ef0-47a6-bcfb-9306e0e2b85e> ; 
    skos:prefLabel "carbonate/quartz index"@en ; 
    skos:definition "Indicator of possible areas of highly reflective carbonate/quartz abundance across a landscape. Calculated from a combination of spectral bands of satellite imagery, the indicator may vary in effectiveness across the landscape."@en ; 
    skos:broader <http://linked.data.gov.au/def/tern-cv/41a27c10-6dff-4ddc-9f8b-14e87fafc786> ; 
    dcterms:created "2021-02-03T07:25:56"^^xsd:datetime ; 
    dcterms:modified "2021-02-04T01:53:23"^^xsd:datetime ; 
. 

<http://linked.data.gov.au/def/tern-cv/c06b51c6-8290-40bf-b192-b0dc2b44fde1> 
    a skos:Concept ; 
    skos:inScheme <http://linked.data.gov.au/def/tern-cv/5699eca7-9ef0-47a6-bcfb-9306e0e2b85e> ; 
    rdfs:isDefinedBy <http://linked.data.gov.au/def/tern-cv/5699eca7-9ef0-47a6-bcfb-9306e0e2b85e> ; 
    skos:prefLabel "bedrock indices"@en ; 
    skos:definition "Indicator to assist with classification of bedrock units across a landscape. Calculated from a combination of spectral bands of satellite imagery, the indicator may vary in effectiveness across the landscape."@en ; 
    skos:broader <http://linked.data.gov.au/def/tern-cv/41a27c10-6dff-4ddc-9f8b-14e87fafc786> ; 
    skos:narrower <http://linked.data.gov.au/def/tern-cv/0b0869d5-c2f5-48cd-b8c0-e42e90ae808a>,
        <http://linked.data.gov.au/def/tern-cv/1e762c90-28e3-41e9-957f-f4cf672aee44>,
        <http://linked.data.gov.au/def/tern-cv/e523389f-7fee-4ec1-8843-c847245ba2fd> ;
    dcterms:created "2021-02-03T06:15:57"^^xsd:datetime ; 
    dcterms:modified "2021-02-19T05:11:56"^^xsd:datetime ; 
. 

<http://linked.data.gov.au/def/tern-cv/0b0869d5-c2f5-48cd-b8c0-e42e90ae808a> 
    a skos:Concept ; 
    skos:inScheme <http://linked.data.gov.au/def/tern-cv/5699eca7-9ef0-47a6-bcfb-9306e0e2b85e> ; 
    rdfs:isDefinedBy <http://linked.data.gov.au/def/tern-cv/5699eca7-9ef0-47a6-bcfb-9306e0e2b85e> ; 
    skos:prefLabel "bedrock index (RED/GREEN)"@en ; 
    skos:definition "Indicator to assist with classification of bedrock units across a landscape. Calculated from a ratio of RED/GREEN spectral bands from satellite imagery, the indicator may vary in effectiveness across the landscape."@en ; 
    skos:broader <http://linked.data.gov.au/def/tern-cv/c06b51c6-8290-40bf-b192-b0dc2b44fde1> ; 
    dcterms:created "2021-02-03T07:25:56"^^xsd:datetime ; 
    dcterms:modified "2021-02-04T01:08:57"^^xsd:datetime ; 
. 

<http://linked.data.gov.au/def/tern-cv/e523389f-7fee-4ec1-8843-c847245ba2fd> 
    a skos:Concept ; 
    skos:inScheme <http://linked.data.gov.au/def/tern-cv/5699eca7-9ef0-47a6-bcfb-9306e0e2b85e> ; 
    rdfs:isDefinedBy <http://linked.data.gov.au/def/tern-cv/5699eca7-9ef0-47a6-bcfb-9306e0e2b85e> ; 
    skos:prefLabel "bedrock index (SWIR2/RED)"@en ; 
    skos:definition "Indicator to assist with classification of bedrock units across a landscape. Calculated from a ratio of SWIR2/RED spectral bands from satellite imagery, the indicator may vary in effectiveness across the landscape."@en ; 
    skos:broader <http://linked.data.gov.au/def/tern-cv/c06b51c6-8290-40bf-b192-b0dc2b44fde1> ; 
    dcterms:created "2021-02-03T07:25:56"^^xsd:datetime ; 
    dcterms:modified "2021-02-04T01:09:53"^^xsd:datetime ; 
. 

<http://linked.data.gov.au/def/tern-cv/1e762c90-28e3-41e9-957f-f4cf672aee44> 
    a skos:Concept ; 
    skos:inScheme <http://linked.data.gov.au/def/tern-cv/5699eca7-9ef0-47a6-bcfb-9306e0e2b85e> ; 
    rdfs:isDefinedBy <http://linked.data.gov.au/def/tern-cv/5699eca7-9ef0-47a6-bcfb-9306e0e2b85e> ; 
    skos:prefLabel "iron oxide and bedrock index (SWIR1/BLUE)"@en ; 
    skos:definition "Indicator to assist with classification of bedrock units and possible areas of iron oxide abundance across a landscape. Calculated from a ratio of SWIR1/BLUE spectral bands from satellite imagery, the indicator may vary in effectiveness across the landscape."@en ; 
    skos:broader <http://linked.data.gov.au/def/tern-cv/700daf25-0a3f-461e-a799-be80ef2f8cd4> ; 
    dcterms:created "2021-02-03T07:25:56"^^xsd:datetime ; 
    dcterms:modified "2021-02-04T02:14:02"^^xsd:datetime ; 
. 

<http://linked.data.gov.au/def/tern-cv/1e762c90-28e3-41e9-957f-f4cf672aee44> 
    a skos:Concept ; 
    skos:inScheme <http://linked.data.gov.au/def/tern-cv/5699eca7-9ef0-47a6-bcfb-9306e0e2b85e> ; 
    rdfs:isDefinedBy <http://linked.data.gov.au/def/tern-cv/5699eca7-9ef0-47a6-bcfb-9306e0e2b85e> ; 
    skos:prefLabel "iron oxide and bedrock index (SWIR1/BLUE)"@en ; 
    skos:definition "Indicator to assist with classification of bedrock units and possible areas of iron oxide abundance across a landscape. Calculated from a ratio of SWIR1/BLUE spectral bands from satellite imagery, the indicator may vary in effectiveness across the landscape."@en ; 
    skos:broader <http://linked.data.gov.au/def/tern-cv/c06b51c6-8290-40bf-b192-b0dc2b44fde1> ; 
    dcterms:created "2021-02-03T07:25:56"^^xsd:datetime ; 
    dcterms:modified "2021-02-04T02:14:02"^^xsd:datetime ; 
. 

<http://linked.data.gov.au/def/tern-cv/803a7efd-71b6-4e4b-b018-4fe884f86491> 
    a skos:Concept ; 
    skos:inScheme <http://linked.data.gov.au/def/tern-cv/5699eca7-9ef0-47a6-bcfb-9306e0e2b85e> ; 
    rdfs:isDefinedBy <http://linked.data.gov.au/def/tern-cv/5699eca7-9ef0-47a6-bcfb-9306e0e2b85e> ; 
    skos:prefLabel "iron oxide index (SWIR2/GREEN)"@en ; 
    skos:definition "Indicator of possible areas of iron oxide abundance across a landscape. Calculated from a ratio of SWIR2/GREEN spectral bands from satellite imagery, the indicator may vary in effectiveness across the landscape."@en ; 
    skos:broader <http://linked.data.gov.au/def/tern-cv/700daf25-0a3f-461e-a799-be80ef2f8cd4> ; 
    dcterms:created "2021-02-03T06:15:57"^^xsd:datetime ; 
    dcterms:modified "2021-02-04T00:29:49"^^xsd:datetime ; 
. 

<http://linked.data.gov.au/def/tern-cv/803a7efd-71b6-4e4b-b018-4fe884f86491> 
    a skos:Concept ; 
    skos:inScheme <http://linked.data.gov.au/def/tern-cv/5699eca7-9ef0-47a6-bcfb-9306e0e2b85e> ; 
    rdfs:isDefinedBy <http://linked.data.gov.au/def/tern-cv/5699eca7-9ef0-47a6-bcfb-9306e0e2b85e> ; 
    skos:prefLabel "iron oxide index (SWIR2/GREEN)"@en ; 
    skos:definition "Indicator of possible areas of iron oxide abundance across a landscape. Calculated from a ratio of SWIR2/GREEN spectral bands from satellite imagery, the indicator may vary in effectiveness across the landscape."@en ; 
    skos:broader <http://linked.data.gov.au/def/tern-cv/700daf25-0a3f-461e-a799-be80ef2f8cd4> ; 
    dcterms:created "2021-02-03T06:15:57"^^xsd:datetime ; 
    dcterms:modified "2021-02-04T00:54:28"^^xsd:datetime ; 
. 

<http://linked.data.gov.au/def/tern-cv/803a7efd-71b6-4e4b-b018-4fe884f86491> 
    a skos:Concept ; 
    skos:inScheme <http://linked.data.gov.au/def/tern-cv/5699eca7-9ef0-47a6-bcfb-9306e0e2b85e> ; 
    rdfs:isDefinedBy <http://linked.data.gov.au/def/tern-cv/5699eca7-9ef0-47a6-bcfb-9306e0e2b85e> ; 
    skos:prefLabel "iron oxide index (SWIR2/GREEN)"@en ; 
    skos:definition "Indicator of possible areas of iron oxide abundance across a landscape. Calculated from a ratio of SWIR2/GREEN spectral bands from satellite imagery, the indicator may vary in effectiveness across the landscape."@en ; 
    skos:broader <http://linked.data.gov.au/def/tern-cv/700daf25-0a3f-461e-a799-be80ef2f8cd4> ; 
    dcterms:created "2021-02-03T07:25:56"^^xsd:datetime ; 
    dcterms:modified "2021-02-04T00:29:49"^^xsd:datetime ; 
. 

<http://linked.data.gov.au/def/tern-cv/803a7efd-71b6-4e4b-b018-4fe884f86491> 
    a skos:Concept ; 
    skos:inScheme <http://linked.data.gov.au/def/tern-cv/5699eca7-9ef0-47a6-bcfb-9306e0e2b85e> ; 
    rdfs:isDefinedBy <http://linked.data.gov.au/def/tern-cv/5699eca7-9ef0-47a6-bcfb-9306e0e2b85e> ; 
    skos:prefLabel "iron oxide index (SWIR2/GREEN)"@en ; 
    skos:definition "Indicator of possible areas of iron oxide abundance across a landscape. Calculated from a ratio of SWIR2/GREEN spectral bands from satellite imagery, the indicator may vary in effectiveness across the landscape."@en ; 
    skos:broader <http://linked.data.gov.au/def/tern-cv/700daf25-0a3f-461e-a799-be80ef2f8cd4> ; 
    dcterms:created "2021-02-03T07:25:56"^^xsd:datetime ; 
    dcterms:modified "2021-02-04T00:54:28"^^xsd:datetime ; 
. 

<http://linked.data.gov.au/def/tern-cv/bb942400-8bc5-4831-bcf5-7a891ef00ef4> 
    a skos:Concept ; 
    skos:inScheme <http://linked.data.gov.au/def/tern-cv/5699eca7-9ef0-47a6-bcfb-9306e0e2b85e> ; 
    rdfs:isDefinedBy <http://linked.data.gov.au/def/tern-cv/5699eca7-9ef0-47a6-bcfb-9306e0e2b85e> ; 
    skos:prefLabel "carbonate/quartz index (BLUE/SWIR2)"@en ; 
    skos:definition "Indicator of possible areas of highly reflective carbonate/quartz abundance across a landscape. Calculated from a ratio of BLUE/SWIR2 spectral bands from satellite imagery, the indicator may vary in effectiveness across the landscape."@en ; 
    skos:broader <http://linked.data.gov.au/def/tern-cv/12797115-2e0f-479f-8d06-1700da3ac394> ; 
    dcterms:created "2021-02-03T07:25:56"^^xsd:datetime ; 
    dcterms:modified "2021-02-04T01:09:07"^^xsd:datetime ; 
. 

<http://linked.data.gov.au/def/tern-cv/a54f0994-bac3-42e4-83d3-46c33affd8a9> 
    a skos:Concept ; 
    skos:inScheme <http://linked.data.gov.au/def/tern-cv/5699eca7-9ef0-47a6-bcfb-9306e0e2b85e> ; 
    rdfs:isDefinedBy <http://linked.data.gov.au/def/tern-cv/5699eca7-9ef0-47a6-bcfb-9306e0e2b85e> ; 
    skos:prefLabel "ferric iron (Fe3+) indices"@en ; 
    skos:definition "Indicator of possible areas of ferric iron (Fe3+) abundance across a landscape. Calculated from a combination of spectral bands of satellite imagery, the indicator may vary in effectiveness across the landscape."@en ; 
    skos:broader <http://linked.data.gov.au/def/tern-cv/99bd0128-54d4-4a2b-8a2c-48010eb07d26> ; 
    skos:narrower <http://linked.data.gov.au/def/tern-cv/22a1a113-5453-4725-84df-cfd7e6a51890>,
        <http://linked.data.gov.au/def/tern-cv/d82bdbb7-3f9c-4aaa-8a09-759cedec4161> ;
    dcterms:created "2021-02-03T06:15:57"^^xsd:datetime ; 
    dcterms:modified "2021-02-19T05:13:32"^^xsd:datetime ; 
. 

<http://linked.data.gov.au/def/tern-cv/a54f0994-bac3-42e4-83d3-46c33affd8a9> 
    a skos:Concept ; 
    skos:inScheme <http://linked.data.gov.au/def/tern-cv/5699eca7-9ef0-47a6-bcfb-9306e0e2b85e> ; 
    rdfs:isDefinedBy <http://linked.data.gov.au/def/tern-cv/5699eca7-9ef0-47a6-bcfb-9306e0e2b85e> ; 
    skos:prefLabel "ferric iron (Fe3+) indices"@en ; 
    skos:definition "Indicator of possible areas of ferric iron (Fe3+) abundance across a landscape. Calculated from a combination of spectral bands of satellite imagery, the indicator may vary in effectiveness across the landscape."@en ; 
    skos:broader <http://linked.data.gov.au/def/tern-cv/99bd0128-54d4-4a2b-8a2c-48010eb07d26> ; 
    dcterms:created "2021-02-03T07:25:56"^^xsd:datetime ; 
    dcterms:modified "2021-02-19T05:13:32"^^xsd:datetime ; 
. 

<http://linked.data.gov.au/def/tern-cv/a54f0994-bac3-42e4-83d3-46c33affd8a9> 
    a skos:Concept ; 
    skos:inScheme <http://linked.data.gov.au/def/tern-cv/5699eca7-9ef0-47a6-bcfb-9306e0e2b85e> ; 
    rdfs:isDefinedBy <http://linked.data.gov.au/def/tern-cv/5699eca7-9ef0-47a6-bcfb-9306e0e2b85e> ; 
    skos:prefLabel "ferric iron (Fe3+) indices"@en ; 
    skos:definition "Indicator of possible areas of ferric iron (Fe3+) abundance across a landscape. Calculated from a combination of spectral bands of satellite imagery, the indicator may vary in effectiveness across the landscape."@en ; 
    skos:broader <http://linked.data.gov.au/def/tern-cv/41a27c10-6dff-4ddc-9f8b-14e87fafc786> ; 
    dcterms:created "2021-02-03T06:15:57"^^xsd:datetime ; 
    dcterms:modified "2021-02-19T05:13:32"^^xsd:datetime ; 
. 

<http://linked.data.gov.au/def/tern-cv/a54f0994-bac3-42e4-83d3-46c33affd8a9> 
    a skos:Concept ; 
    skos:inScheme <http://linked.data.gov.au/def/tern-cv/5699eca7-9ef0-47a6-bcfb-9306e0e2b85e> ; 
    rdfs:isDefinedBy <http://linked.data.gov.au/def/tern-cv/5699eca7-9ef0-47a6-bcfb-9306e0e2b85e> ; 
    skos:prefLabel "ferric iron (Fe3+) indices"@en ; 
    skos:definition "Indicator of possible areas of ferric iron (Fe3+) abundance across a landscape. Calculated from a combination of spectral bands of satellite imagery, the indicator may vary in effectiveness across the landscape."@en ; 
    skos:broader <http://linked.data.gov.au/def/tern-cv/41a27c10-6dff-4ddc-9f8b-14e87fafc786> ; 
    dcterms:created "2021-02-03T07:25:56"^^xsd:datetime ; 
    dcterms:modified "2021-02-19T05:13:32"^^xsd:datetime ; 
. 

<http://linked.data.gov.au/def/tern-cv/22a1a113-5453-4725-84df-cfd7e6a51890> 
    a skos:Concept ; 
    skos:inScheme <http://linked.data.gov.au/def/tern-cv/5699eca7-9ef0-47a6-bcfb-9306e0e2b85e> ; 
    rdfs:isDefinedBy <http://linked.data.gov.au/def/tern-cv/5699eca7-9ef0-47a6-bcfb-9306e0e2b85e> ; 
    skos:prefLabel "ferric iron (Fe3+) index (PC2 of RED and BLUE)"@en ; 
    skos:definition "Indicator of possible areas of ferric iron (Fe3+) abundance across a landscape. Calculated from Principal Components Analysis (PCA) of blue and red spectral bands of satellite imagery, the indicator may vary in effectiveness across the landscape."@en ; 
    skos:broader <http://linked.data.gov.au/def/tern-cv/a54f0994-bac3-42e4-83d3-46c33affd8a9> ; 
    dcterms:created "2021-02-03T07:25:56"^^xsd:datetime ; 
    dcterms:modified "2021-02-04T01:31:48"^^xsd:datetime ; 
. 

<http://linked.data.gov.au/def/tern-cv/d82bdbb7-3f9c-4aaa-8a09-759cedec4161> 
    a skos:Concept ; 
    skos:inScheme <http://linked.data.gov.au/def/tern-cv/5699eca7-9ef0-47a6-bcfb-9306e0e2b85e> ; 
    rdfs:isDefinedBy <http://linked.data.gov.au/def/tern-cv/5699eca7-9ef0-47a6-bcfb-9306e0e2b85e> ; 
    skos:prefLabel "ferric iron (Fe3+) index (PC4 of BLUE, RED, NIR and SWIR1)"@en ; 
    skos:definition "Indicator of possible areas of ferric iron (Fe3+) abundance across a landscape. Calculated from Principal Components Analysis (PCA) of  BLUE, RED, NIR and SWIR1 spectral bands of satellite imagery, the indicator may vary in effectiveness across the landscape."@en ; 
    skos:broader <http://linked.data.gov.au/def/tern-cv/a54f0994-bac3-42e4-83d3-46c33affd8a9> ; 
    dcterms:created "2021-02-03T07:25:56"^^xsd:datetime ; 
    dcterms:modified "2021-02-04T01:09:07"^^xsd:datetime ; 
. 

<http://linked.data.gov.au/def/tern-cv/1beaac85-44c0-4097-aa11-8d44f6381bc9> 
    a skos:Concept ; 
    skos:inScheme <http://linked.data.gov.au/def/tern-cv/5699eca7-9ef0-47a6-bcfb-9306e0e2b85e> ; 
    rdfs:isDefinedBy <http://linked.data.gov.au/def/tern-cv/5699eca7-9ef0-47a6-bcfb-9306e0e2b85e> ; 
    skos:prefLabel "ferrous minerals index (SWIR1/NIR)"@en ; 
    skos:definition "Indicator of possible areas of ferrous minerals abundance across a landscape. Calculated from a ratio of SWIR1/NIR spectral bands from satellite imagery, the indicator may vary in effectiveness across the landscape."@en ; 
    skos:broader <http://linked.data.gov.au/def/tern-cv/700daf25-0a3f-461e-a799-be80ef2f8cd4> ; 
    dcterms:created "2021-02-03T07:25:56"^^xsd:datetime ; 
    dcterms:modified "2021-02-04T01:29:32"^^xsd:datetime ; 
. 

<http://linked.data.gov.au/def/tern-cv/3a03227d-1b66-4c63-b7aa-f9ccbb70d1cf> 
    a skos:Concept ; 
    skos:inScheme <http://linked.data.gov.au/def/tern-cv/5699eca7-9ef0-47a6-bcfb-9306e0e2b85e> ; 
    rdfs:isDefinedBy <http://linked.data.gov.au/def/tern-cv/5699eca7-9ef0-47a6-bcfb-9306e0e2b85e> ; 
    skos:prefLabel "hydroxyl minerals indices"@en ; 
    skos:definition "Indicator of possible areas of hydroxyl minerals abundance across a landscape, for example hydroxyl-bearing clays, sulphates and carbonates. Calculated from a combination of spectral bands of satellite imagery, the indicator may vary in effectiveness across the landscape."@en ; 
    skos:broader <http://linked.data.gov.au/def/tern-cv/99bd0128-54d4-4a2b-8a2c-48010eb07d26> ; 
    dcterms:created "2021-02-03T06:15:57"^^xsd:datetime ; 
    dcterms:modified "2021-02-19T05:10:28"^^xsd:datetime ; 
. 

<http://linked.data.gov.au/def/tern-cv/3a03227d-1b66-4c63-b7aa-f9ccbb70d1cf> 
    a skos:Concept ; 
    skos:inScheme <http://linked.data.gov.au/def/tern-cv/5699eca7-9ef0-47a6-bcfb-9306e0e2b85e> ; 
    rdfs:isDefinedBy <http://linked.data.gov.au/def/tern-cv/5699eca7-9ef0-47a6-bcfb-9306e0e2b85e> ; 
    skos:prefLabel "hydroxyl minerals indices"@en ; 
    skos:definition "Indicator of possible areas of hydroxyl minerals abundance across a landscape, for example hydroxyl-bearing clays, sulphates and carbonates. Calculated from a combination of spectral bands of satellite imagery, the indicator may vary in effectiveness across the landscape."@en ; 
    skos:broader <http://linked.data.gov.au/def/tern-cv/99bd0128-54d4-4a2b-8a2c-48010eb07d26> ; 
    dcterms:created "2021-02-03T07:25:56"^^xsd:datetime ; 
    dcterms:modified "2021-02-19T05:10:28"^^xsd:datetime ; 
. 

<http://linked.data.gov.au/def/tern-cv/3a03227d-1b66-4c63-b7aa-f9ccbb70d1cf> 
    a skos:Concept ; 
    skos:inScheme <http://linked.data.gov.au/def/tern-cv/5699eca7-9ef0-47a6-bcfb-9306e0e2b85e> ; 
    rdfs:isDefinedBy <http://linked.data.gov.au/def/tern-cv/5699eca7-9ef0-47a6-bcfb-9306e0e2b85e> ; 
    skos:prefLabel "hydroxyl minerals indices"@en ; 
    skos:definition "Indicator of possible areas of hydroxyl minerals abundance across a landscape, for example hydroxyl-bearing clays, sulphates and carbonates. Calculated from a combination of spectral bands of satellite imagery, the indicator may vary in effectiveness across the landscape."@en ; 
    skos:broader <http://linked.data.gov.au/def/tern-cv/41a27c10-6dff-4ddc-9f8b-14e87fafc786> ; 
    dcterms:created "2021-02-03T06:15:57"^^xsd:datetime ; 
    dcterms:modified "2021-02-19T05:10:28"^^xsd:datetime ; 
. 

<http://linked.data.gov.au/def/tern-cv/3a03227d-1b66-4c63-b7aa-f9ccbb70d1cf> 
    a skos:Concept ; 
    skos:inScheme <http://linked.data.gov.au/def/tern-cv/5699eca7-9ef0-47a6-bcfb-9306e0e2b85e> ; 
    rdfs:isDefinedBy <http://linked.data.gov.au/def/tern-cv/5699eca7-9ef0-47a6-bcfb-9306e0e2b85e> ; 
    skos:prefLabel "hydroxyl minerals indices"@en ; 
    skos:definition "Indicator of possible areas of hydroxyl minerals abundance across a landscape, for example hydroxyl-bearing clays, sulphates and carbonates. Calculated from a combination of spectral bands of satellite imagery, the indicator may vary in effectiveness across the landscape."@en ; 
    skos:broader <http://linked.data.gov.au/def/tern-cv/41a27c10-6dff-4ddc-9f8b-14e87fafc786> ; 
    dcterms:created "2021-02-03T07:25:56"^^xsd:datetime ; 
    dcterms:modified "2021-02-19T05:10:28"^^xsd:datetime ; 
. 

<http://linked.data.gov.au/def/tern-cv/f75ff7d2-d525-4a76-939b-5fa43f1e9d77> 
    a skos:Concept ; 
    skos:inScheme <http://linked.data.gov.au/def/tern-cv/5699eca7-9ef0-47a6-bcfb-9306e0e2b85e> ; 
    rdfs:isDefinedBy <http://linked.data.gov.au/def/tern-cv/5699eca7-9ef0-47a6-bcfb-9306e0e2b85e> ; 
    skos:prefLabel "hydroxyl minerals index (PC1 of SWIR1/SWIR2 and NIR/RED)"@en ; 
    skos:definition "Indicator of possible areas of hydroxyl minerals abundance across a landscape. Calculated from Principal Components Analysis on SWIR1/SWIR2 and NIR/RED spectral bands of satellite imagery, the indicator may vary in effectiveness across the landscape."@en ; 
    skos:broader <http://linked.data.gov.au/def/tern-cv/3a03227d-1b66-4c63-b7aa-f9ccbb70d1cf> ; 
    dcterms:created "2021-02-03T07:25:56"^^xsd:datetime ; 
    dcterms:modified "2021-02-04T03:09:25"^^xsd:datetime ; 
. 

<http://linked.data.gov.au/def/tern-cv/2e57142c-817d-420b-a097-e62f379afecc> 
    a skos:Concept ; 
    skos:inScheme <http://linked.data.gov.au/def/tern-cv/5699eca7-9ef0-47a6-bcfb-9306e0e2b85e> ; 
    rdfs:isDefinedBy <http://linked.data.gov.au/def/tern-cv/5699eca7-9ef0-47a6-bcfb-9306e0e2b85e> ; 
    skos:prefLabel "hydroxyl minerals index (SWIR1/SWIR2)"@en ; 
    skos:definition "Indicator of possible areas of hydroxyl minerals abundance across a landscape and can also include a vegetation response. Calculated from a ratio of SWIR1/SWIR2 spectral bands of satellite imagery from satellite imagery, the indicator may vary in effectiveness across the landscape."@en ; 
    skos:broader <http://linked.data.gov.au/def/tern-cv/3a03227d-1b66-4c63-b7aa-f9ccbb70d1cf> ; 
    dcterms:created "2021-02-03T07:25:56"^^xsd:datetime ; 
    dcterms:modified "2021-02-19T04:52:53"^^xsd:datetime ; 
. 

<http://linked.data.gov.au/def/tern-cv/fc383c4d-b8d2-4dbf-b897-5f511208ada1> 
    a skos:Concept ; 
    skos:inScheme <http://linked.data.gov.au/def/tern-cv/5699eca7-9ef0-47a6-bcfb-9306e0e2b85e> ; 
    rdfs:isDefinedBy <http://linked.data.gov.au/def/tern-cv/5699eca7-9ef0-47a6-bcfb-9306e0e2b85e> ; 
    skos:prefLabel "ferruginous/non-ferruginous regolith index"@en ; 
    skos:definition "Indicator to differentiate ferruginous versus non-ferruginous regolith abundance across a landscape. Calculated from a combination of spectral bands of satellite imagery, the indicator may vary in effectiveness across the landscape."@en ; 
    skos:broader <http://linked.data.gov.au/def/tern-cv/99bd0128-54d4-4a2b-8a2c-48010eb07d26> ; 
    skos:narrower <http://linked.data.gov.au/def/tern-cv/903b2a07-47df-451e-b533-f4c34732e631> ;
    dcterms:created "2021-02-03T06:15:57"^^xsd:datetime ; 
    dcterms:modified "2021-02-04T01:23:24"^^xsd:datetime ; 
. 

<http://linked.data.gov.au/def/tern-cv/fc383c4d-b8d2-4dbf-b897-5f511208ada1> 
    a skos:Concept ; 
    skos:inScheme <http://linked.data.gov.au/def/tern-cv/5699eca7-9ef0-47a6-bcfb-9306e0e2b85e> ; 
    rdfs:isDefinedBy <http://linked.data.gov.au/def/tern-cv/5699eca7-9ef0-47a6-bcfb-9306e0e2b85e> ; 
    skos:prefLabel "ferruginous/non-ferruginous regolith index"@en ; 
    skos:definition "Indicator to differentiate ferruginous versus non-ferruginous regolith abundance across a landscape. Calculated from a combination of spectral bands of satellite imagery, the indicator may vary in effectiveness across the landscape."@en ; 
    skos:broader <http://linked.data.gov.au/def/tern-cv/99bd0128-54d4-4a2b-8a2c-48010eb07d26> ; 
    dcterms:created "2021-02-03T07:25:56"^^xsd:datetime ; 
    dcterms:modified "2021-02-04T01:23:24"^^xsd:datetime ; 
. 

<http://linked.data.gov.au/def/tern-cv/fc383c4d-b8d2-4dbf-b897-5f511208ada1> 
    a skos:Concept ; 
    skos:inScheme <http://linked.data.gov.au/def/tern-cv/5699eca7-9ef0-47a6-bcfb-9306e0e2b85e> ; 
    rdfs:isDefinedBy <http://linked.data.gov.au/def/tern-cv/5699eca7-9ef0-47a6-bcfb-9306e0e2b85e> ; 
    skos:prefLabel "ferruginous/non-ferruginous regolith index"@en ; 
    skos:definition "Indicator to differentiate ferruginous versus non-ferruginous regolith abundance across a landscape. Calculated from a combination of spectral bands of satellite imagery, the indicator may vary in effectiveness across the landscape."@en ; 
    skos:broader <http://linked.data.gov.au/def/tern-cv/41a27c10-6dff-4ddc-9f8b-14e87fafc786> ; 
    dcterms:created "2021-02-03T06:15:57"^^xsd:datetime ; 
    dcterms:modified "2021-02-04T01:23:24"^^xsd:datetime ; 
. 

<http://linked.data.gov.au/def/tern-cv/fc383c4d-b8d2-4dbf-b897-5f511208ada1> 
    a skos:Concept ; 
    skos:inScheme <http://linked.data.gov.au/def/tern-cv/5699eca7-9ef0-47a6-bcfb-9306e0e2b85e> ; 
    rdfs:isDefinedBy <http://linked.data.gov.au/def/tern-cv/5699eca7-9ef0-47a6-bcfb-9306e0e2b85e> ; 
    skos:prefLabel "ferruginous/non-ferruginous regolith index"@en ; 
    skos:definition "Indicator to differentiate ferruginous versus non-ferruginous regolith abundance across a landscape. Calculated from a combination of spectral bands of satellite imagery, the indicator may vary in effectiveness across the landscape."@en ; 
    skos:broader <http://linked.data.gov.au/def/tern-cv/41a27c10-6dff-4ddc-9f8b-14e87fafc786> ; 
    dcterms:created "2021-02-03T07:25:56"^^xsd:datetime ; 
    dcterms:modified "2021-02-04T01:23:24"^^xsd:datetime ; 
. 

<http://linked.data.gov.au/def/tern-cv/903b2a07-47df-451e-b533-f4c34732e631> 
    a skos:Concept ; 
    skos:inScheme <http://linked.data.gov.au/def/tern-cv/5699eca7-9ef0-47a6-bcfb-9306e0e2b85e> ; 
    rdfs:isDefinedBy <http://linked.data.gov.au/def/tern-cv/5699eca7-9ef0-47a6-bcfb-9306e0e2b85e> ; 
    skos:prefLabel "ferruginous/non-ferruginous regolith index (NIR/GREEN)"@en ; 
    skos:definition "Indicator to differentiate ferruginous versus non-ferruginous regolith abundance across a landscape. Calculated from a ratio of NIR/GREEN spectral bands from satellite imagery, the indicator may vary in effectiveness across the landscape."@en ; 
    skos:broader <http://linked.data.gov.au/def/tern-cv/fc383c4d-b8d2-4dbf-b897-5f511208ada1> ; 
    dcterms:created "2021-02-03T07:25:56"^^xsd:datetime ; 
    dcterms:modified "2021-02-04T02:00:16"^^xsd:datetime ; 
. 

<http://linked.data.gov.au/def/tern-cv/1a7c69c6-8d8b-49c9-9f65-f3e288a6c33c> 
    a skos:Concept ; 
    skos:inScheme <http://linked.data.gov.au/def/tern-cv/5699eca7-9ef0-47a6-bcfb-9306e0e2b85e> ; 
    rdfs:isDefinedBy <http://linked.data.gov.au/def/tern-cv/5699eca7-9ef0-47a6-bcfb-9306e0e2b85e> ; 
    skos:prefLabel "hydroxyl minerals index (PC2 of SWIR1/SWIR2 and NIR/RED)"@en ; 
    skos:definition "Indicator of possible areas of hydroxyl minerals abundance across a landscape. Calculated from Principal Components Analysis on SWIR1/SWIR2 and NIR/RED spectral bands of satellite imagery, the indicator may vary in effectiveness across the landscape."@en ; 
    skos:broader <http://linked.data.gov.au/def/tern-cv/3a03227d-1b66-4c63-b7aa-f9ccbb70d1cf> ; 
    dcterms:created "2021-02-03T07:25:56"^^xsd:datetime ; 
    dcterms:modified "2021-02-04T03:03:30"^^xsd:datetime ; 
. 

<http://linked.data.gov.au/def/tern-cv/01a87ba3-0f0d-4854-8196-3e3d80010faf> 
    a skos:Concept ; 
    skos:inScheme <http://linked.data.gov.au/def/tern-cv/5699eca7-9ef0-47a6-bcfb-9306e0e2b85e> ; 
    rdfs:isDefinedBy <http://linked.data.gov.au/def/tern-cv/5699eca7-9ef0-47a6-bcfb-9306e0e2b85e> ; 
    skos:prefLabel "hydroxyl minerals index (PC2 of SWIR1, SWIR2)"@en ; 
    skos:definition "Indicator of possible areas of hydroxyl minerals abundance across a landscape. Calculated from Principal Components Analysis on SWIR1/SWIR2 spectral bands of satellite imagery, the indicator may vary in effectiveness across the landscape."@en ; 
    skos:broader <http://linked.data.gov.au/def/tern-cv/3a03227d-1b66-4c63-b7aa-f9ccbb70d1cf> ; 
    dcterms:created "2021-02-03T07:25:56"^^xsd:datetime ; 
    dcterms:modified "2021-02-04T03:04:49"^^xsd:datetime ; 
. 

<http://linked.data.gov.au/def/tern-cv/70c1e9c4-2949-4e49-a8ef-6c4c45dd5b65> 
    a skos:Concept ; 
    skos:inScheme <http://linked.data.gov.au/def/tern-cv/5699eca7-9ef0-47a6-bcfb-9306e0e2b85e> ; 
    rdfs:isDefinedBy <http://linked.data.gov.au/def/tern-cv/5699eca7-9ef0-47a6-bcfb-9306e0e2b85e> ; 
    skos:prefLabel "hydroxyl minerals index (PC3 of BLUE, NIR, SWIR1, SWIR2)"@en ; 
    skos:definition "Indicator of possible areas of hydroxyl minerals abundance across a landscape. Calculated from Principal Components Analysis on BLUE, NIR, SWIR1 and SWIR2 spectral bands of satellite imagery, the indicator may vary in effectiveness across the landscape."@en ; 
    skos:broader <http://linked.data.gov.au/def/tern-cv/3a03227d-1b66-4c63-b7aa-f9ccbb70d1cf> ; 
    dcterms:created "2021-02-03T07:25:56"^^xsd:datetime ; 
    dcterms:modified "2021-02-04T03:06:15"^^xsd:datetime ; 
. 

<http://linked.data.gov.au/def/tern-cv/5cba467e-a595-42fd-a177-2ac8e83ce17d> 
    a skos:Concept ; 
    skos:inScheme <http://linked.data.gov.au/def/tern-cv/5699eca7-9ef0-47a6-bcfb-9306e0e2b85e> ; 
    rdfs:isDefinedBy <http://linked.data.gov.au/def/tern-cv/5699eca7-9ef0-47a6-bcfb-9306e0e2b85e> ; 
    skos:prefLabel "hydroxyl minerals index (PC4 of BLUE, NIR, SWIR1, SWIR2)"@en ; 
    skos:definition "Indicator of possible areas of hydroxyl minerals abundance across a landscape. Calculated from Principal Components Analysis on BLUE, NIR, SWIR1 and SWIR2 spectral bands of satellite imagery, the indicator may vary in effectiveness across the landscape."@en ; 
    skos:broader <http://linked.data.gov.au/def/tern-cv/3a03227d-1b66-4c63-b7aa-f9ccbb70d1cf> ; 
    dcterms:created "2021-02-03T07:25:56"^^xsd:datetime ; 
    dcterms:modified "2021-02-04T03:07:46"^^xsd:datetime ; 
. 

<http://linked.data.gov.au/def/tern-cv/d42a1a60-c606-4967-a09a-26727b9b2bc8> 
    a skos:Concept ; 
    skos:inScheme <http://linked.data.gov.au/def/tern-cv/5699eca7-9ef0-47a6-bcfb-9306e0e2b85e> ; 
    rdfs:isDefinedBy <http://linked.data.gov.au/def/tern-cv/5699eca7-9ef0-47a6-bcfb-9306e0e2b85e> ; 
    skos:prefLabel "actual evapotranspiration"@en ; 
    skos:definition "The amount of water that evaporates from the surface and is transpired by plants if the total amount of water is limited."@en ; 
    skos:broader <http://linked.data.gov.au/def/tern-cv/45ae73d8-92bd-4261-a05f-7bfac228e1f7> ; 
    dcterms:created "2021-02-03T06:15:57"^^xsd:datetime ; 
    dcterms:modified "2021-02-04T03:34:41"^^xsd:datetime ; 
. 

<http://linked.data.gov.au/def/tern-cv/6033d979-5b22-40f9-a081-19b9980fa396> 
    a skos:Concept ; 
    skos:inScheme <http://linked.data.gov.au/def/tern-cv/5699eca7-9ef0-47a6-bcfb-9306e0e2b85e> ; 
    rdfs:isDefinedBy <http://linked.data.gov.au/def/tern-cv/5699eca7-9ef0-47a6-bcfb-9306e0e2b85e> ; 
    skos:prefLabel "evapotranspiration"@en ; 
    skos:definition "Combined term for water lost as vapour from a soil or open water surface (evaporation) and water lost from the surface of a plant, mainly via the stomata (transpiration). The combined term is often used since in practice it is very difficult to distinguish water vapour from these two sources in water-balance and atmospheric studies."@en ; 
    skos:broader <http://linked.data.gov.au/def/tern-cv/45ae73d8-92bd-4261-a05f-7bfac228e1f7> ; 
    dcterms:created "2021-02-03T06:15:57"^^xsd:datetime ; 
    dcterms:modified "2021-02-04T01:41:12"^^xsd:datetime ; 
. 

<http://linked.data.gov.au/def/tern-cv/1aa6aa3b-eb0a-47f0-9bc1-61c0b375fe73> 
    a skos:Concept ; 
    skos:inScheme <http://linked.data.gov.au/def/tern-cv/5699eca7-9ef0-47a6-bcfb-9306e0e2b85e> ; 
    rdfs:isDefinedBy <http://linked.data.gov.au/def/tern-cv/5699eca7-9ef0-47a6-bcfb-9306e0e2b85e> ; 
    skos:prefLabel "at-surface reflectance"@en ; 
    skos:definition "satellite (or aerial) imagery corrected for noise introduced by image acquisition, including atmospheric scattering and absorption, surface BRDF, terrain illumination and scanner operation to provide the ratio of electromagnetic radiation reflected by a surface to that which is incident upon it. The ideal is that the resulting image represents the value that would be measured by an ideal sensor held at the same sun-view geometry and located just above the Earth’s surface if there was no atmosphere."@en ; 
    skos:broader <http://linked.data.gov.au/def/tern-cv/41a27c10-6dff-4ddc-9f8b-14e87fafc786> ; 
    dcterms:modified "2021-03-18T04:57:37"^^xsd:datetime ; 
. 

<http://linked.data.gov.au/def/tern-cv/46911a2e-826e-49bd-8150-830dd6a72cf3> 
    a skos:Concept ; 
    skos:inScheme <http://linked.data.gov.au/def/tern-cv/5699eca7-9ef0-47a6-bcfb-9306e0e2b85e> ; 
    rdfs:isDefinedBy <http://linked.data.gov.au/def/tern-cv/5699eca7-9ef0-47a6-bcfb-9306e0e2b85e> ; 
    skos:prefLabel "species rank abundance"@en ; 
    skos:definition "species rank abundance"@en ; 
    skos:broader <http://linked.data.gov.au/def/tern-cv/8fa1c4bd-73b3-432a-ab49-9ee89928e6d9> ; 
    dcterms:modified "2021-05-10T00:39:11"^^xsd:datetime ; 
. 

<http://linked.data.gov.au/def/tern-cv/c_012ebf32> 
    a skos:Concept ; 
    skos:inScheme <http://linked.data.gov.au/def/tern-cv/5699eca7-9ef0-47a6-bcfb-9306e0e2b85e> ; 
    rdfs:isDefinedBy <http://linked.data.gov.au/def/tern-cv/5699eca7-9ef0-47a6-bcfb-9306e0e2b85e> ; 
    skos:prefLabel "land use"@en ; 
    skos:definition "land use"@en ; 
    skos:narrower <http://linked.data.gov.au/def/tern-cv/e926b2ca-2688-486c-aa28-435f91c3c110> ;
    skos:topConceptOf <http://linked.data.gov.au/def/tern-cv/5699eca7-9ef0-47a6-bcfb-9306e0e2b85e> ;
    dcterms:created "2021-02-08T01:49:47"^^xsd:datetime ; 
.

<http://linked.data.gov.au/def/tern-cv/43ed01cc-0089-4a6b-8754-0990dd0f697b> 
    a skos:Concept ; 
    skos:inScheme <http://linked.data.gov.au/def/tern-cv/5699eca7-9ef0-47a6-bcfb-9306e0e2b85e> ; 
    rdfs:isDefinedBy <http://linked.data.gov.au/def/tern-cv/5699eca7-9ef0-47a6-bcfb-9306e0e2b85e> ; 
    skos:prefLabel "stratum type"@en ; 
    skos:definition "stratum type"@en ; 
    skos:broader <http://linked.data.gov.au/def/tern-cv/2ffe4363-dea1-4188-9f8f-835983d47fe2> ; 
    dcterms:modified "2021-05-12T01:22:03"^^xsd:datetime ; 
. 

<http://linked.data.gov.au/def/tern-cv/7b3f70df-5c55-4b2b-9b45-ea978d9d3759> 
    a skos:Concept ; 
    skos:inScheme <http://linked.data.gov.au/def/tern-cv/5699eca7-9ef0-47a6-bcfb-9306e0e2b85e> ; 
    rdfs:isDefinedBy <http://linked.data.gov.au/def/tern-cv/5699eca7-9ef0-47a6-bcfb-9306e0e2b85e> ; 
    skos:prefLabel "soil wet weight"@en ; 
    skos:definition "soil wet weight"@en ; 
    skos:broader <http://linked.data.gov.au/def/tern-cv/99bd0128-54d4-4a2b-8a2c-48010eb07d26> ; 
.

<http://linked.data.gov.au/def/tern-cv/c86c4e7f-5dc3-4a88-b5f6-88f5bc0973cd> 
    a skos:Concept ; 
    skos:inScheme <http://linked.data.gov.au/def/tern-cv/5699eca7-9ef0-47a6-bcfb-9306e0e2b85e> ; 
    rdfs:isDefinedBy <http://linked.data.gov.au/def/tern-cv/5699eca7-9ef0-47a6-bcfb-9306e0e2b85e> ; 
    skos:prefLabel "soil oven dried weight"@en ; 
    skos:definition "soil oven dried weight"@en ; 
    skos:broader <http://linked.data.gov.au/def/tern-cv/99bd0128-54d4-4a2b-8a2c-48010eb07d26> ; 
.

<http://linked.data.gov.au/def/tern-cv/e926b2ca-2688-486c-aa28-435f91c3c110> 
    a skos:Concept ; 
    skos:inScheme <http://linked.data.gov.au/def/tern-cv/5699eca7-9ef0-47a6-bcfb-9306e0e2b85e> ; 
    rdfs:isDefinedBy <http://linked.data.gov.au/def/tern-cv/5699eca7-9ef0-47a6-bcfb-9306e0e2b85e> ; 
    skos:prefLabel "distance to nearest human infrastructure"@en ; 
    skos:definition "distance to nearest human infrastructure"@en ; 
    skos:broader <http://linked.data.gov.au/def/tern-cv/c_012ebf32> ; 
    dcterms:modified "2021-03-12T06:15:43"^^xsd:datetime ; 
. 

<http://linked.data.gov.au/def/tern-cv/09aae763-babb-4926-b1ed-52630195564d> 
    a skos:Concept ; 
    skos:inScheme <http://linked.data.gov.au/def/tern-cv/5699eca7-9ef0-47a6-bcfb-9306e0e2b85e> ; 
    rdfs:isDefinedBy <http://linked.data.gov.au/def/tern-cv/5699eca7-9ef0-47a6-bcfb-9306e0e2b85e> ; 
    skos:prefLabel "dominant outcrop lithology"@en ; 
    skos:definition "dominant outcrop lithology"@en ; 
    skos:broader <http://linked.data.gov.au/def/tern-cv/6e2ede4b-1e6f-4ea0-93d9-6597c5666d62> ; 
    dcterms:created "2021-02-09T02:00:10"^^xsd:datetime ; 
    dcterms:modified "2021-03-12T06:09:39"^^xsd:datetime ; 
. 

<http://linked.data.gov.au/def/tern-cv/54fd271e-d0a9-4e82-967a-c013c47760d9> 
    a skos:Concept ; 
    skos:inScheme <http://linked.data.gov.au/def/tern-cv/5699eca7-9ef0-47a6-bcfb-9306e0e2b85e> ; 
    rdfs:isDefinedBy <http://linked.data.gov.au/def/tern-cv/5699eca7-9ef0-47a6-bcfb-9306e0e2b85e> ; 
    skos:prefLabel "plot perimeter point"@en ; 
    skos:definition "plot perimeter point"@en ; 
    skos:broader <http://linked.data.gov.au/def/tern-cv/9e03a73d-8e89-4187-9f96-0306aad93458> ; 
    dcterms:created "2021-02-11T02:05:22"^^xsd:datetime ; 
    dcterms:modified "2021-02-11T02:06:36"^^xsd:datetime ; 
. 

<http://linked.data.gov.au/def/tern-cv/56195246-ec5d-4050-a1c6-af786fbec715> 
    a skos:Concept ; 
    skos:inScheme <http://linked.data.gov.au/def/tern-cv/5699eca7-9ef0-47a6-bcfb-9306e0e2b85e> ; 
    rdfs:isDefinedBy <http://linked.data.gov.au/def/tern-cv/5699eca7-9ef0-47a6-bcfb-9306e0e2b85e> ; 
    skos:prefLabel "scientific name"@en ; 
    skos:definition "scientific name"@en ; 
    skos:broader <http://linked.data.gov.au/def/tern-cv/8fa1c4bd-73b3-432a-ab49-9ee89928e6d9> ; 
    dcterms:created "2021-02-01T04:37:24"^^xsd:datetime ; 
    dcterms:modified "2021-05-17T01:17:13"^^xsd:datetime ; 
. 

<http://linked.data.gov.au/def/tern-cv/a3ad8f31-6896-416e-8ac6-bc61b93aaab5> 
    a skos:Concept ; 
    skos:inScheme <http://linked.data.gov.au/def/tern-cv/5699eca7-9ef0-47a6-bcfb-9306e0e2b85e> ; 
    rdfs:isDefinedBy <http://linked.data.gov.au/def/tern-cv/5699eca7-9ef0-47a6-bcfb-9306e0e2b85e> ; 
    skos:prefLabel "diameter at breast height"@en ; 
    skos:definition "diameter at breast height"@en ; 
    skos:broader <http://linked.data.gov.au/def/tern-cv/2ffe4363-dea1-4188-9f8f-835983d47fe2> ; 
    dcterms:created "2021-02-18T01:50:11"^^xsd:datetime ; 
    dcterms:modified "2021-02-18T01:54:47"^^xsd:datetime ; 
. 

<http://linked.data.gov.au/def/tern-cv/777773d0-cfb4-44ff-85e2-08b48e10ac52> 
    a skos:Concept ; 
    skos:inScheme <http://linked.data.gov.au/def/tern-cv/5699eca7-9ef0-47a6-bcfb-9306e0e2b85e> ; 
    rdfs:isDefinedBy <http://linked.data.gov.au/def/tern-cv/5699eca7-9ef0-47a6-bcfb-9306e0e2b85e> ; 
    skos:prefLabel "disturbance parameter"@en ; 
    skos:definition "disturbance parameter"@en ; 
    skos:topConceptOf <http://linked.data.gov.au/def/tern-cv/5699eca7-9ef0-47a6-bcfb-9306e0e2b85e> ;
    skos:narrower <http://linked.data.gov.au/def/tern-cv/18d64def-df3b-4fa2-ba2d-967c6e392406>,
        <http://linked.data.gov.au/def/tern-cv/1d1a868a-74f9-4d7b-8d70-f97d9530098e>,
        <http://linked.data.gov.au/def/tern-cv/20a2ab2e-cdbd-4c56-9e68-9c926fd589eb>,
        <http://linked.data.gov.au/def/tern-cv/28874068-9b9b-49b0-a754-0b7bd988d97c>,
        <http://linked.data.gov.au/def/tern-cv/29241828-9973-4854-a4b9-e972cd58c22a>,
        <http://linked.data.gov.au/def/tern-cv/3826b5a3-7128-4df3-90f3-8196c4c20d45>,
        <http://linked.data.gov.au/def/tern-cv/3ab5a014-78d0-4424-9329-8dc370701f1a>,
        <http://linked.data.gov.au/def/tern-cv/486e60ea-affa-45ad-b331-027167d866bf>,
        <http://linked.data.gov.au/def/tern-cv/4e272650-c4f7-412b-b7bf-031af0611acc>,
        <http://linked.data.gov.au/def/tern-cv/5a95ac61-94c5-4993-aad2-3e891156efe0>,
        <http://linked.data.gov.au/def/tern-cv/5d13d5e9-4465-4c75-8a41-60bf84882696>,
        <http://linked.data.gov.au/def/tern-cv/71934567-a90d-433c-a040-63df566c9faa>,
        <http://linked.data.gov.au/def/tern-cv/79b5755c-6de7-42e9-a652-c402faec2826>,
        <http://linked.data.gov.au/def/tern-cv/7e75402d-e3c6-41dd-9e17-7f44b26bbb10>,
        <http://linked.data.gov.au/def/tern-cv/800cf33b-1c44-435d-89bd-5d80e3e8aba1>,
        <http://linked.data.gov.au/def/tern-cv/8c20f342-39fd-4abf-ab97-218c7c1ce499>,
        <http://linked.data.gov.au/def/tern-cv/8f220426-6b5a-4b8f-a995-8eea263a4a19>,
        <http://linked.data.gov.au/def/tern-cv/a8e12e7f-6052-4e87-a69e-ceb34ad5c45d>,
        <http://linked.data.gov.au/def/tern-cv/b0dff759-ae91-4801-b520-b27e27215a40>,
        <http://linked.data.gov.au/def/tern-cv/be1916fa-a0cf-4e86-a0dc-dd49f7a78af7>,
        <http://linked.data.gov.au/def/tern-cv/c55de6b4-72f2-42ad-ad6e-f611db272e78>,
        <http://linked.data.gov.au/def/tern-cv/c5f99536-8986-418e-932d-ae5d77312adc>,
        <http://linked.data.gov.au/def/tern-cv/d33f60ee-1934-4bd8-9919-06c0d54eee1a>,
        <http://linked.data.gov.au/def/tern-cv/d5635c66-06d2-48e4-98ff-7e83e8a2b265>,
        <http://linked.data.gov.au/def/tern-cv/f3888501-98b1-4a53-a788-20b0f0b8a7e6>,
        <http://linked.data.gov.au/def/tern-cv/f57f6bf8-2a5e-47c5-bcc2-4ce7bb4b9dc7>,
        <http://linked.data.gov.au/def/tern-cv/fe9c70d4-415b-4152-b517-a8e7a15e36f7>,
        <http://linked.data.gov.au/def/tern-cv/ff4ce8d1-4c2b-4d6e-8aea-be4138fea452> ;
    dcterms:created "2021-02-26T03:30:24"^^xsd:datetime ; 
    dcterms:modified "2021-03-11T03:53:45"^^xsd:datetime ; 
. 

<http://linked.data.gov.au/def/tern-cv/1d1a868a-74f9-4d7b-8d70-f97d9530098e> 
    a skos:Concept ; 
    skos:inScheme <http://linked.data.gov.au/def/tern-cv/5699eca7-9ef0-47a6-bcfb-9306e0e2b85e> ; 
    rdfs:isDefinedBy <http://linked.data.gov.au/def/tern-cv/5699eca7-9ef0-47a6-bcfb-9306e0e2b85e> ; 
    skos:prefLabel "erosion type"@en ; 
    skos:definition "erosion type"@en ; 
    skos:broader <http://linked.data.gov.au/def/tern-cv/6f726a59-c330-44eb-898e-7d42d5fbdada>,
        <http://linked.data.gov.au/def/tern-cv/777773d0-cfb4-44ff-85e2-08b48e10ac52> ;
    dcterms:created "2021-02-26T03:31:27"^^xsd:datetime ; 
    dcterms:modified "2021-03-11T06:18:42"^^xsd:datetime ; 
. 

<http://linked.data.gov.au/def/tern-cv/28874068-9b9b-49b0-a754-0b7bd988d97c> 
    a skos:Concept ; 
    skos:inScheme <http://linked.data.gov.au/def/tern-cv/5699eca7-9ef0-47a6-bcfb-9306e0e2b85e> ; 
    rdfs:isDefinedBy <http://linked.data.gov.au/def/tern-cv/5699eca7-9ef0-47a6-bcfb-9306e0e2b85e> ; 
    skos:prefLabel "time since roadwork"@en ; 
    skos:definition "time since roadwork"@en ; 
    skos:broader <http://linked.data.gov.au/def/tern-cv/777773d0-cfb4-44ff-85e2-08b48e10ac52> ,
        <http://linked.data.gov.au/def/tern-cv/6f726a59-c330-44eb-898e-7d42d5fbdada> ; 
    dcterms:created "2021-02-26T03:37:51"^^xsd:datetime ; 
    dcterms:modified "2021-03-11T06:34:41"^^xsd:datetime ; 
. 

<http://linked.data.gov.au/def/tern-cv/be1916fa-a0cf-4e86-a0dc-dd49f7a78af7> 
    a skos:Concept ; 
    skos:inScheme <http://linked.data.gov.au/def/tern-cv/5699eca7-9ef0-47a6-bcfb-9306e0e2b85e> ; 
    rdfs:isDefinedBy <http://linked.data.gov.au/def/tern-cv/5699eca7-9ef0-47a6-bcfb-9306e0e2b85e> ; 
    skos:prefLabel "time since storm"@en ; 
    skos:definition "time since storm"@en ; 
    skos:broader <http://linked.data.gov.au/def/tern-cv/777773d0-cfb4-44ff-85e2-08b48e10ac52> ,
        <http://linked.data.gov.au/def/tern-cv/6f726a59-c330-44eb-898e-7d42d5fbdada> ; 
    dcterms:created "2021-02-26T03:39:49"^^xsd:datetime ; 
    dcterms:modified "2021-03-11T06:37:50"^^xsd:datetime ; 
. 

<http://linked.data.gov.au/def/tern-cv/7e75402d-e3c6-41dd-9e17-7f44b26bbb10> 
    a skos:Concept ; 
    skos:inScheme <http://linked.data.gov.au/def/tern-cv/5699eca7-9ef0-47a6-bcfb-9306e0e2b85e> ; 
    rdfs:isDefinedBy <http://linked.data.gov.au/def/tern-cv/5699eca7-9ef0-47a6-bcfb-9306e0e2b85e> ; 
    skos:prefLabel "time since fire"@en ; 
    skos:definition "time since fire"@en ; 
    skos:broader <http://linked.data.gov.au/def/tern-cv/777773d0-cfb4-44ff-85e2-08b48e10ac52> ,
        <http://linked.data.gov.au/def/tern-cv/8fa1c4bd-73b3-432a-ab49-9ee89928e6d9>  ; 
    dcterms:created "2021-02-26T03:40:41"^^xsd:datetime ; 
    dcterms:modified "2021-03-11T06:32:35"^^xsd:datetime ; 
. 

<http://linked.data.gov.au/def/tern-cv/79b5755c-6de7-42e9-a652-c402faec2826> 
    a skos:Concept ; 
    skos:inScheme <http://linked.data.gov.au/def/tern-cv/5699eca7-9ef0-47a6-bcfb-9306e0e2b85e> ; 
    rdfs:isDefinedBy <http://linked.data.gov.au/def/tern-cv/5699eca7-9ef0-47a6-bcfb-9306e0e2b85e> ; 
    skos:prefLabel "fire proportion"@en ; 
    skos:definition "fire proportion"@en ; 
    skos:broader <http://linked.data.gov.au/def/tern-cv/777773d0-cfb4-44ff-85e2-08b48e10ac52> ,
        <http://linked.data.gov.au/def/tern-cv/8fa1c4bd-73b3-432a-ab49-9ee89928e6d9>  ; 
    dcterms:created "2021-03-09T03:40:41"^^xsd:datetime ; 
    dcterms:modified "2021-03-11T23:48:29"^^xsd:datetime ; 
. 

<http://linked.data.gov.au/def/tern-cv/4e272650-c4f7-412b-b7bf-031af0611acc> 
    a skos:Concept ; 
    skos:inScheme <http://linked.data.gov.au/def/tern-cv/5699eca7-9ef0-47a6-bcfb-9306e0e2b85e> ; 
    rdfs:isDefinedBy <http://linked.data.gov.au/def/tern-cv/5699eca7-9ef0-47a6-bcfb-9306e0e2b85e> ; 
    skos:prefLabel "storm proportion"@en ; 
    skos:definition "storm proportion"@en ; 
    skos:broader <http://linked.data.gov.au/def/tern-cv/777773d0-cfb4-44ff-85e2-08b48e10ac52> ,
        <http://linked.data.gov.au/def/tern-cv/8fa1c4bd-73b3-432a-ab49-9ee89928e6d9>  ; 
    dcterms:created "2021-03-09T03:40:41"^^xsd:datetime ; 
    dcterms:modified "2021-03-11T23:50:55"^^xsd:datetime ; 
. 

<http://linked.data.gov.au/def/tern-cv/c5f99536-8986-418e-932d-ae5d77312adc> 
    a skos:Concept ; 
    skos:inScheme <http://linked.data.gov.au/def/tern-cv/5699eca7-9ef0-47a6-bcfb-9306e0e2b85e> ; 
    rdfs:isDefinedBy <http://linked.data.gov.au/def/tern-cv/5699eca7-9ef0-47a6-bcfb-9306e0e2b85e> ; 
    skos:prefLabel "roadwork proportion"@en ; 
    skos:definition "roadwork proportion"@en ; 
    skos:broader <http://linked.data.gov.au/def/tern-cv/777773d0-cfb4-44ff-85e2-08b48e10ac52> ,
       <http://linked.data.gov.au/def/tern-cv/6f726a59-c330-44eb-898e-7d42d5fbdada> ; 
    dcterms:created "2021-03-09T03:40:41"^^xsd:datetime ; 
    dcterms:modified "2021-03-12T00:42:32"^^xsd:datetime ; 
. 

<http://linked.data.gov.au/def/tern-cv/71934567-a90d-433c-a040-63df566c9faa> 
    a skos:Concept ; 
    skos:inScheme <http://linked.data.gov.au/def/tern-cv/5699eca7-9ef0-47a6-bcfb-9306e0e2b85e> ; 
    rdfs:isDefinedBy <http://linked.data.gov.au/def/tern-cv/5699eca7-9ef0-47a6-bcfb-9306e0e2b85e> ; 
    skos:prefLabel "extensive clearing present"@en ; 
    skos:definition "extensive clearing present"@en ; 
    skos:broader <http://linked.data.gov.au/def/tern-cv/777773d0-cfb4-44ff-85e2-08b48e10ac52> ,
       <http://linked.data.gov.au/def/tern-cv/6f726a59-c330-44eb-898e-7d42d5fbdada> ; 
    dcterms:created "2021-03-09T03:40:41"^^xsd:datetime ; 
    dcterms:modified "2021-03-11T04:43:56"^^xsd:datetime ; 
. 

<http://linked.data.gov.au/def/tern-cv/486e60ea-affa-45ad-b331-027167d866bf> 
    a skos:Concept ; 
    skos:inScheme <http://linked.data.gov.au/def/tern-cv/5699eca7-9ef0-47a6-bcfb-9306e0e2b85e> ; 
    rdfs:isDefinedBy <http://linked.data.gov.au/def/tern-cv/5699eca7-9ef0-47a6-bcfb-9306e0e2b85e> ; 
    skos:prefLabel "feral digging present"@en ; 
    skos:definition "feral digging present"@en ; 
    skos:broader <http://linked.data.gov.au/def/tern-cv/777773d0-cfb4-44ff-85e2-08b48e10ac52> ,
       <http://linked.data.gov.au/def/tern-cv/6f726a59-c330-44eb-898e-7d42d5fbdada> ; 
    dcterms:created "2021-03-09T03:40:41"^^xsd:datetime ; 
    dcterms:modified "2021-03-11T04:45:33"^^xsd:datetime ; 
. 

<http://linked.data.gov.au/def/tern-cv/800cf33b-1c44-435d-89bd-5d80e3e8aba1> 
    a skos:Concept ; 
    skos:inScheme <http://linked.data.gov.au/def/tern-cv/5699eca7-9ef0-47a6-bcfb-9306e0e2b85e> ; 
    rdfs:isDefinedBy <http://linked.data.gov.au/def/tern-cv/5699eca7-9ef0-47a6-bcfb-9306e0e2b85e> ; 
    skos:prefLabel "fire present"@en ; 
    skos:definition "fire present"@en ; 
    skos:broader <http://linked.data.gov.au/def/tern-cv/777773d0-cfb4-44ff-85e2-08b48e10ac52> ,
       <http://linked.data.gov.au/def/tern-cv/6f726a59-c330-44eb-898e-7d42d5fbdada> ; 
    dcterms:created "2021-03-09T03:40:41"^^xsd:datetime ; 
    dcterms:modified "2021-03-11T04:46:25"^^xsd:datetime ; 
. 

<http://linked.data.gov.au/def/tern-cv/8c20f342-39fd-4abf-ab97-218c7c1ce499> 
    a skos:Concept ; 
    skos:inScheme <http://linked.data.gov.au/def/tern-cv/5699eca7-9ef0-47a6-bcfb-9306e0e2b85e> ; 
    rdfs:isDefinedBy <http://linked.data.gov.au/def/tern-cv/5699eca7-9ef0-47a6-bcfb-9306e0e2b85e> ; 
    skos:prefLabel "flood present"@en ; 
    skos:definition "flood present"@en ; 
    skos:broader <http://linked.data.gov.au/def/tern-cv/777773d0-cfb4-44ff-85e2-08b48e10ac52> ,
      <http://linked.data.gov.au/def/tern-cv/6f726a59-c330-44eb-898e-7d42d5fbdada>; 
    dcterms:created "2021-03-09T03:40:41"^^xsd:datetime ; 
    dcterms:modified "2021-03-11T04:49:33"^^xsd:datetime ; 
. 

<http://linked.data.gov.au/def/tern-cv/f57f6bf8-2a5e-47c5-bcc2-4ce7bb4b9dc7> 
    a skos:Concept ; 
    skos:inScheme <http://linked.data.gov.au/def/tern-cv/5699eca7-9ef0-47a6-bcfb-9306e0e2b85e> ; 
    rdfs:isDefinedBy <http://linked.data.gov.au/def/tern-cv/5699eca7-9ef0-47a6-bcfb-9306e0e2b85e> ; 
    skos:prefLabel "grazing present"@en ; 
    skos:definition "grazing present"@en ; 
    skos:broader <http://linked.data.gov.au/def/tern-cv/777773d0-cfb4-44ff-85e2-08b48e10ac52> ,
       <http://linked.data.gov.au/def/tern-cv/8fa1c4bd-73b3-432a-ab49-9ee89928e6d9> ; 
    dcterms:created "2021-03-09T03:40:41"^^xsd:datetime ; 
    dcterms:modified "2021-03-11T04:55:35"^^xsd:datetime ; 
. 

<http://linked.data.gov.au/def/tern-cv/f3888501-98b1-4a53-a788-20b0f0b8a7e6> 
    a skos:Concept ; 
    skos:inScheme <http://linked.data.gov.au/def/tern-cv/5699eca7-9ef0-47a6-bcfb-9306e0e2b85e> ; 
    rdfs:isDefinedBy <http://linked.data.gov.au/def/tern-cv/5699eca7-9ef0-47a6-bcfb-9306e0e2b85e> ; 
    skos:prefLabel "non-remnant present"@en ; 
    skos:definition "non-remnant present"@en ; 
    skos:broader <http://linked.data.gov.au/def/tern-cv/777773d0-cfb4-44ff-85e2-08b48e10ac52> ,
       <http://linked.data.gov.au/def/tern-cv/8fa1c4bd-73b3-432a-ab49-9ee89928e6d9> ; 
    dcterms:created "2021-03-09T03:40:41"^^xsd:datetime ; 
    dcterms:modified "2021-03-11T05:13:18"^^xsd:datetime ; 
. 

<http://linked.data.gov.au/def/tern-cv/29241828-9973-4854-a4b9-e972cd58c22a> 
    a skos:Concept ; 
    skos:inScheme <http://linked.data.gov.au/def/tern-cv/5699eca7-9ef0-47a6-bcfb-9306e0e2b85e> ; 
    rdfs:isDefinedBy <http://linked.data.gov.au/def/tern-cv/5699eca7-9ef0-47a6-bcfb-9306e0e2b85e> ; 
    skos:prefLabel "roadwork present"@en ; 
    skos:definition "roadwork present"@en ; 
    skos:broader <http://linked.data.gov.au/def/tern-cv/777773d0-cfb4-44ff-85e2-08b48e10ac52> ,
      <http://linked.data.gov.au/def/tern-cv/6f726a59-c330-44eb-898e-7d42d5fbdada>; 
    dcterms:created "2021-03-09T03:40:41"^^xsd:datetime ; 
    dcterms:modified "2021-03-11T05:19:56"^^xsd:datetime ; 
. 

<http://linked.data.gov.au/def/tern-cv/d33f60ee-1934-4bd8-9919-06c0d54eee1a> 
    a skos:Concept ; 
    skos:inScheme <http://linked.data.gov.au/def/tern-cv/5699eca7-9ef0-47a6-bcfb-9306e0e2b85e> ; 
    rdfs:isDefinedBy <http://linked.data.gov.au/def/tern-cv/5699eca7-9ef0-47a6-bcfb-9306e0e2b85e> ; 
    skos:prefLabel "salinity present"@en ; 
    skos:definition "salinity present"@en ; 
    skos:broader <http://linked.data.gov.au/def/tern-cv/777773d0-cfb4-44ff-85e2-08b48e10ac52> ,
       <http://linked.data.gov.au/def/tern-cv/6f726a59-c330-44eb-898e-7d42d5fbdada> ; 
    dcterms:created "2021-03-09T03:40:41"^^xsd:datetime ; 
    dcterms:modified "2021-03-11T05:20:32"^^xsd:datetime ; 
. 

<http://linked.data.gov.au/def/tern-cv/d5635c66-06d2-48e4-98ff-7e83e8a2b265> 
    a skos:Concept ; 
    skos:inScheme <http://linked.data.gov.au/def/tern-cv/5699eca7-9ef0-47a6-bcfb-9306e0e2b85e> ; 
    rdfs:isDefinedBy <http://linked.data.gov.au/def/tern-cv/5699eca7-9ef0-47a6-bcfb-9306e0e2b85e> ; 
    skos:prefLabel "storm damage present"@en ; 
    skos:definition "storm damage present"@en ; 
    skos:broader <http://linked.data.gov.au/def/tern-cv/777773d0-cfb4-44ff-85e2-08b48e10ac52> ,
       <http://linked.data.gov.au/def/tern-cv/8fa1c4bd-73b3-432a-ab49-9ee89928e6d9> ; 
    dcterms:created "2021-03-09T03:40:41"^^xsd:datetime ; 
    dcterms:modified "2021-03-11T05:24:58"^^xsd:datetime ; 
. 

<http://linked.data.gov.au/def/tern-cv/fe9c70d4-415b-4152-b517-a8e7a15e36f7> 
    a skos:Concept ; 
    skos:inScheme <http://linked.data.gov.au/def/tern-cv/5699eca7-9ef0-47a6-bcfb-9306e0e2b85e> ; 
    rdfs:isDefinedBy <http://linked.data.gov.au/def/tern-cv/5699eca7-9ef0-47a6-bcfb-9306e0e2b85e> ; 
    skos:prefLabel "logging present"@en ; 
    skos:definition "logging present"@en ; 
    skos:broader <http://linked.data.gov.au/def/tern-cv/777773d0-cfb4-44ff-85e2-08b48e10ac52> ,
      <http://linked.data.gov.au/def/tern-cv/8fa1c4bd-73b3-432a-ab49-9ee89928e6d9>; 
    dcterms:created "2021-03-09T03:40:41"^^xsd:datetime ; 
    dcterms:modified "2021-03-11T04:56:40"^^xsd:datetime ; 
. 

<http://linked.data.gov.au/def/tern-cv/b0dff759-ae91-4801-b520-b27e27215a40> 
    a skos:Concept ; 
    skos:inScheme <http://linked.data.gov.au/def/tern-cv/5699eca7-9ef0-47a6-bcfb-9306e0e2b85e> ; 
    rdfs:isDefinedBy <http://linked.data.gov.au/def/tern-cv/5699eca7-9ef0-47a6-bcfb-9306e0e2b85e> ; 
    skos:prefLabel "ringbarking present"@en ; 
    skos:definition "ringbarking present"@en ; 
    skos:broader <http://linked.data.gov.au/def/tern-cv/777773d0-cfb4-44ff-85e2-08b48e10ac52> ,
      <http://linked.data.gov.au/def/tern-cv/8fa1c4bd-73b3-432a-ab49-9ee89928e6d9> ; 
    dcterms:created "2021-03-09T03:40:41"^^xsd:datetime ; 
    dcterms:modified "2021-03-11T05:14:22"^^xsd:datetime ; 
. 

<http://linked.data.gov.au/def/tern-cv/a8e12e7f-6052-4e87-a69e-ceb34ad5c45d> 
    a skos:Concept ; 
    skos:inScheme <http://linked.data.gov.au/def/tern-cv/5699eca7-9ef0-47a6-bcfb-9306e0e2b85e> ; 
    rdfs:isDefinedBy <http://linked.data.gov.au/def/tern-cv/5699eca7-9ef0-47a6-bcfb-9306e0e2b85e> ; 
    skos:prefLabel "weeds present"@en ; 
    skos:definition "weeds present"@en ; 
    skos:broader <http://linked.data.gov.au/def/tern-cv/777773d0-cfb4-44ff-85e2-08b48e10ac52> ,
      <http://linked.data.gov.au/def/tern-cv/8fa1c4bd-73b3-432a-ab49-9ee89928e6d9> ; 
    dcterms:created "2021-03-09T03:40:41"^^xsd:datetime ; 
    dcterms:modified "2021-03-11T05:35:10"^^xsd:datetime ; 
. 

<http://linked.data.gov.au/def/tern-cv/ff4ce8d1-4c2b-4d6e-8aea-be4138fea452> 
    a skos:Concept ; 
    skos:inScheme <http://linked.data.gov.au/def/tern-cv/5699eca7-9ef0-47a6-bcfb-9306e0e2b85e> ; 
    rdfs:isDefinedBy <http://linked.data.gov.au/def/tern-cv/5699eca7-9ef0-47a6-bcfb-9306e0e2b85e> ; 
    skos:prefLabel "erosion present"@en ; 
    skos:definition "erosion present"@en ; 
    skos:broader <http://linked.data.gov.au/def/tern-cv/777773d0-cfb4-44ff-85e2-08b48e10ac52> ,
      <http://linked.data.gov.au/def/tern-cv/6f726a59-c330-44eb-898e-7d42d5fbdada>  ; 
    dcterms:created "2021-03-09T03:40:41"^^xsd:datetime ; 
    dcterms:modified "2021-03-11T04:18:34"^^xsd:datetime ; 
. 

<http://linked.data.gov.au/def/tern-cv/6f726a59-c330-44eb-898e-7d42d5fbdada> 
    a skos:Concept ; 
    skos:inScheme <http://linked.data.gov.au/def/tern-cv/5699eca7-9ef0-47a6-bcfb-9306e0e2b85e> ; 
    rdfs:isDefinedBy <http://linked.data.gov.au/def/tern-cv/5699eca7-9ef0-47a6-bcfb-9306e0e2b85e> ; 
    skos:prefLabel "land surface parameter"@en ; 
    skos:definition "land surface parameter"@en ; 
    skos:topConceptOf <http://linked.data.gov.au/def/tern-cv/5699eca7-9ef0-47a6-bcfb-9306e0e2b85e> ;
    dcterms:created "2021-03-11T04:17:12"^^xsd:datetime ; 
. 

#<http://linked.data.gov.au/def/tern-cv/8e7a785a-8c57-4415-855f-cb6d35ad58bb> 
#    a skos:Concept ; 
#    skos:inScheme <http://linked.data.gov.au/def/tern-cv/5699eca7-9ef0-47a6-bcfb-9306e0e2b85e> ; 
#    skos:prefLabel "CF standard name"@en ; 
#    dcterms:created "2021-03-11T04:24:29"^^xsd:datetime ; 
#. 

<http://linked.data.gov.au/def/tern-cv/8fa1c4bd-73b3-432a-ab49-9ee89928e6d9> 
    a skos:Concept ; 
    skos:inScheme <http://linked.data.gov.au/def/tern-cv/5699eca7-9ef0-47a6-bcfb-9306e0e2b85e> ; 
    rdfs:isDefinedBy <http://linked.data.gov.au/def/tern-cv/5699eca7-9ef0-47a6-bcfb-9306e0e2b85e> ; 
    skos:prefLabel "vegetation parameter"@en ; 
    skos:definition "vegetation parameter"@en ; 
    skos:topConceptOf <http://linked.data.gov.au/def/tern-cv/5699eca7-9ef0-47a6-bcfb-9306e0e2b85e> ;
    dcterms:created "2021-03-11T04:54:26"^^xsd:datetime ; 
    dcterms:modified "2021-03-11T04:54:54"^^xsd:datetime ; 
. 

<http://linked.data.gov.au/def/tern-cv/3ab5a014-78d0-4424-9329-8dc370701f1a> 
    a skos:Concept ; 
    skos:inScheme <http://linked.data.gov.au/def/tern-cv/5699eca7-9ef0-47a6-bcfb-9306e0e2b85e> ; 
    rdfs:isDefinedBy <http://linked.data.gov.au/def/tern-cv/5699eca7-9ef0-47a6-bcfb-9306e0e2b85e> ; 
    skos:prefLabel "salinity proportion"@en ; 
    skos:definition "salinity proportion"@en ; 
    skos:broader <http://linked.data.gov.au/def/tern-cv/777773d0-cfb4-44ff-85e2-08b48e10ac52> ,
      <http://linked.data.gov.au/def/tern-cv/6f726a59-c330-44eb-898e-7d42d5fbdada> ; 
    dcterms:created "2021-03-12T01:58:24"^^xsd:datetime ; 
    dcterms:modified "2021-03-12T01:58:59"^^xsd:datetime ; 
. 

<http://linked.data.gov.au/def/tern-cv/5d13d5e9-4465-4c75-8a41-60bf84882696> 
    a skos:Concept ; 
    skos:inScheme <http://linked.data.gov.au/def/tern-cv/5699eca7-9ef0-47a6-bcfb-9306e0e2b85e> ; 
    rdfs:isDefinedBy <http://linked.data.gov.au/def/tern-cv/5699eca7-9ef0-47a6-bcfb-9306e0e2b85e> ; 
    skos:prefLabel "time since salinity"@en ; 
    skos:definition "time since salinity"@en ; 
    skos:broader <http://linked.data.gov.au/def/tern-cv/777773d0-cfb4-44ff-85e2-08b48e10ac52> ,
      <http://linked.data.gov.au/def/tern-cv/6f726a59-c330-44eb-898e-7d42d5fbdada> ; 
    dcterms:created "2021-03-12T02:01:55"^^xsd:datetime ; 
    dcterms:modified "2021-03-12T02:02:41"^^xsd:datetime ; 
. 

<http://linked.data.gov.au/def/tern-cv/6e2ede4b-1e6f-4ea0-93d9-6597c5666d62> 
    a skos:Concept ; 
    skos:inScheme <http://linked.data.gov.au/def/tern-cv/5699eca7-9ef0-47a6-bcfb-9306e0e2b85e> ; 
    rdfs:isDefinedBy <http://linked.data.gov.au/def/tern-cv/5699eca7-9ef0-47a6-bcfb-9306e0e2b85e> ; 
    skos:prefLabel "lithological parameter"@en ; 
    skos:definition "lithological parameter"@en ; 
    skos:narrower <http://linked.data.gov.au/def/tern-cv/09aae763-babb-4926-b1ed-52630195564d>,
        <http://linked.data.gov.au/def/tern-cv/e5b70249-76a8-4087-8ac9-588c7e29b944> ;
    skos:topConceptOf <http://linked.data.gov.au/def/tern-cv/5699eca7-9ef0-47a6-bcfb-9306e0e2b85e> ; 
    dcterms:created "2021-03-12T06:07:18"^^xsd:datetime ; 
. 

<http://linked.data.gov.au/def/tern-cv/2cf66d7b-6625-44d5-85d9-91f350afe7f0> 
    a skos:Concept ; 
    skos:inScheme <http://linked.data.gov.au/def/tern-cv/5699eca7-9ef0-47a6-bcfb-9306e0e2b85e> ; 
    rdfs:isDefinedBy <http://linked.data.gov.au/def/tern-cv/5699eca7-9ef0-47a6-bcfb-9306e0e2b85e> ; 
    skos:prefLabel "water count"@en ; 
    skos:definition "count of the number of observations with water present in the time series"@en ; 
    skos:broader <http://linked.data.gov.au/def/tern-cv/bb5c1354-8d70-47b2-b333-87e3bf1157d6> ; 
    dcterms:modified "2021-03-18T05:16:50"^^xsd:datetime ; 
. 

<http://linked.data.gov.au/def/tern-cv/809b2517-819e-4c8f-92e8-7dd11a95cc72> 
    a skos:Concept ; 
    skos:inScheme <http://linked.data.gov.au/def/tern-cv/5699eca7-9ef0-47a6-bcfb-9306e0e2b85e> ; 
    rdfs:isDefinedBy <http://linked.data.gov.au/def/tern-cv/5699eca7-9ef0-47a6-bcfb-9306e0e2b85e> ; 
    skos:prefLabel "water prevalence"@en ; 
    skos:definition "based on the water count, prevalence is a classification indicating the percentage of time a pixel has had water present out of the total number of observations for that pixel over the time series"@en ; 
    skos:broader <http://linked.data.gov.au/def/tern-cv/bb5c1354-8d70-47b2-b333-87e3bf1157d6> ; 
    dcterms:modified "2021-03-18T06:52:37"^^xsd:datetime ; 
. 

<http://linked.data.gov.au/def/tern-cv/a5cdedc4-6bdf-4f2d-922b-5d17ae957735> 
    a skos:Concept ; 
    skos:inScheme <http://linked.data.gov.au/def/tern-cv/5699eca7-9ef0-47a6-bcfb-9306e0e2b85e> ; 
    rdfs:isDefinedBy <http://linked.data.gov.au/def/tern-cv/5699eca7-9ef0-47a6-bcfb-9306e0e2b85e> ; 
    skos:prefLabel "green accumulation index"@en ; 
    skos:definition "assessed over a time series to indicate how long an area stays green following a greening event, such as grass growth in response to rainfall"@en ; 
    skos:broader <http://linked.data.gov.au/def/tern-cv/41a27c10-6dff-4ddc-9f8b-14e87fafc786> ; 
    dcterms:modified "2021-03-18T01:41:19"^^xsd:datetime ; 
. 

<http://linked.data.gov.au/def/tern-cv/ceb884dc-f20b-49db-9b27-e2667b87edbb> 
    a skos:Concept ; 
    skos:inScheme <http://linked.data.gov.au/def/tern-cv/5699eca7-9ef0-47a6-bcfb-9306e0e2b85e> ; 
    rdfs:isDefinedBy <http://linked.data.gov.au/def/tern-cv/5699eca7-9ef0-47a6-bcfb-9306e0e2b85e> ; 
    skos:prefLabel "absolute humidity"@en ; 
    skos:definition "In a system of moist air, the ratio of the mass of water vapor present to the volume occupied by the mixture; that is, the density of the water vapor component."@en ; 
    skos:broader <http://linked.data.gov.au/def/tern-cv/123f2efe-3891-4764-9047-609c8b30e925> ; 
    dcterms:created "2021-03-22T03:28:39"^^xsd:datetime ; 
    dcterms:modified "2021-03-22T04:08:24"^^xsd:datetime ; 
. 

<http://linked.data.gov.au/def/tern-cv/6d57155a-1df0-4689-b3ed-551290a3517b> 
    a skos:Concept ; 
    skos:inScheme <http://linked.data.gov.au/def/tern-cv/5699eca7-9ef0-47a6-bcfb-9306e0e2b85e> ; 
    rdfs:isDefinedBy <http://linked.data.gov.au/def/tern-cv/5699eca7-9ef0-47a6-bcfb-9306e0e2b85e> ; 
    skos:prefLabel "persistent green vegetation fraction"@en ; 
    skos:definition "Estimate of the vertically-projected green-vegetation fraction, where vegetation is deemed to persist over time."@en ; 
    skos:broader <http://linked.data.gov.au/def/tern-cv/45ae73d8-92bd-4261-a05f-7bfac228e1f7> ; 
    dcterms:created "2021-03-26T15:46:43+00:00"^^xsd:datetime ; 
    dcterms:modified "2021-03-26T15:46:43"^^xsd:datetime ; 
. 

<http://linked.data.gov.au/def/tern-cv/ea001a27-3217-45c2-a7b5-96a104986def> 
    a skos:Concept ; 
    skos:inScheme <http://linked.data.gov.au/def/tern-cv/5699eca7-9ef0-47a6-bcfb-9306e0e2b85e> ; 
    rdfs:isDefinedBy <http://linked.data.gov.au/def/tern-cv/5699eca7-9ef0-47a6-bcfb-9306e0e2b85e> ; 
    skos:prefLabel "most dominant species"@en ; 
    skos:definition "most dominant species"@en ; 
    skos:broader <http://linked.data.gov.au/def/tern-cv/8fa1c4bd-73b3-432a-ab49-9ee89928e6d9> ; 
    dcterms:created "2021-03-29T07:12:53"^^xsd:datetime ; 
    dcterms:modified "2021-03-29T07:14:07"^^xsd:datetime ; 
. 

<http://linked.data.gov.au/def/tern-cv/d40b3e6d-db78-4031-b7f3-ed94d538a2af> 
    a skos:Concept ; 
    skos:inScheme <http://linked.data.gov.au/def/tern-cv/5699eca7-9ef0-47a6-bcfb-9306e0e2b85e> ; 
    rdfs:isDefinedBy <http://linked.data.gov.au/def/tern-cv/5699eca7-9ef0-47a6-bcfb-9306e0e2b85e> ; 
    skos:prefLabel "second most dominant species"@en ; 
    skos:definition "second most dominant species"@en ; 
    skos:broader <http://linked.data.gov.au/def/tern-cv/8fa1c4bd-73b3-432a-ab49-9ee89928e6d9> ; 
    dcterms:created "2021-03-29T07:21:46"^^xsd:datetime ; 
. 

<http://linked.data.gov.au/def/tern-cv/07abcf97-542d-4c2f-9fb1-c7c7508f484c> 
    a skos:Concept ; 
    skos:inScheme <http://linked.data.gov.au/def/tern-cv/5699eca7-9ef0-47a6-bcfb-9306e0e2b85e> ; 
    rdfs:isDefinedBy <http://linked.data.gov.au/def/tern-cv/5699eca7-9ef0-47a6-bcfb-9306e0e2b85e> ; 
    skos:prefLabel "third most dominant species"@en ; 
    skos:definition "third most dominant species"@en ; 
    skos:broader <http://linked.data.gov.au/def/tern-cv/8fa1c4bd-73b3-432a-ab49-9ee89928e6d9> ; 
    dcterms:created "2021-03-29T07:22:47"^^xsd:datetime ; 
. 

<http://linked.data.gov.au/def/tern-cv/abb0ee19-b2e8-42f3-8a25-d1f39ca3ebc3> 
    a skos:Concept ; 
    skos:inScheme <http://linked.data.gov.au/def/tern-cv/5699eca7-9ef0-47a6-bcfb-9306e0e2b85e> ; 
    rdfs:isDefinedBy <http://linked.data.gov.au/def/tern-cv/5699eca7-9ef0-47a6-bcfb-9306e0e2b85e> ; 
    skos:prefLabel "life stage"@en ; 
    skos:definition "The age class or life stage of the biological individual(s) at the time the Occurrence was recorded."@en ; 
    skos:broader <http://linked.data.gov.au/def/tern-cv/2ffe4363-dea1-4188-9f8f-835983d47fe2> ; 
    dcterms:created "2021-04-07T01:33:53"^^xsd:datetime ; 
    dcterms:modified "2021-04-07T01:41:38"^^xsd:datetime ; 
. 

<http://linked.data.gov.au/def/tern-cv/be0a9365-32ae-4c82-ac87-d65ff3a4dae7> 
    a skos:Concept ; 
    skos:inScheme <http://linked.data.gov.au/def/tern-cv/5699eca7-9ef0-47a6-bcfb-9306e0e2b85e> ; 
    rdfs:isDefinedBy <http://linked.data.gov.au/def/tern-cv/5699eca7-9ef0-47a6-bcfb-9306e0e2b85e> ; 
    skos:prefLabel "bole height"@en ; 
    skos:definition "bole height"@en ; 
    skos:broader <http://linked.data.gov.au/def/tern-cv/2ffe4363-dea1-4188-9f8f-835983d47fe2> ; 
    dcterms:created "2021-04-07T01:48:30"^^xsd:datetime ; 
    dcterms:modified "2021-04-07T01:52:32"^^xsd:datetime ; 
. 

<http://linked.data.gov.au/def/tern-cv/5701d307-bbea-415a-8857-fbf27d5b93ed> 
    a skos:Concept ; 
    skos:inScheme <http://linked.data.gov.au/def/tern-cv/5699eca7-9ef0-47a6-bcfb-9306e0e2b85e> ; 
    rdfs:isDefinedBy <http://linked.data.gov.au/def/tern-cv/5699eca7-9ef0-47a6-bcfb-9306e0e2b85e> ; 
    skos:prefLabel "stem diameter"@en ; 
    skos:definition "Length from the outside of the bole, through the centre, to the opposite side."@en ; 
    skos:broader <http://linked.data.gov.au/def/tern-cv/2ffe4363-dea1-4188-9f8f-835983d47fe2> ; 
    dcterms:created "2021-04-07T01:57:09"^^xsd:datetime ; 
    dcterms:modified "2021-04-07T02:10:10"^^xsd:datetime ; 
. 

<http://linked.data.gov.au/def/tern-cv/f1f46e83-769e-4d50-9212-d180ea72a0f0> 
    a skos:Concept ; 
    skos:inScheme <http://linked.data.gov.au/def/tern-cv/5699eca7-9ef0-47a6-bcfb-9306e0e2b85e> ; 
    rdfs:isDefinedBy <http://linked.data.gov.au/def/tern-cv/5699eca7-9ef0-47a6-bcfb-9306e0e2b85e> ; 
    skos:prefLabel "tree break height"@en ; 
    skos:definition "For broken trees height at which breakage occurred."@en ; 
    skos:broader <http://linked.data.gov.au/def/tern-cv/2ffe4363-dea1-4188-9f8f-835983d47fe2> ; 
    dcterms:created "2021-04-07T03:07:31"^^xsd:datetime ; 
    dcterms:modified "2021-04-07T03:08:35"^^xsd:datetime ; 
. 

<http://linked.data.gov.au/def/tern-cv/90380980-9914-4dd8-8d83-008fb6adeb24> 
    a skos:Concept ; 
    skos:inScheme <http://linked.data.gov.au/def/tern-cv/5699eca7-9ef0-47a6-bcfb-9306e0e2b85e> ; 
    rdfs:isDefinedBy <http://linked.data.gov.au/def/tern-cv/5699eca7-9ef0-47a6-bcfb-9306e0e2b85e> ; 
    skos:prefLabel "tree mode of death"@en ; 
    skos:definition "Mode of dead of individual trees (e.g. uprooted, standind, snapped-off)."@en ; 
    skos:broader <http://linked.data.gov.au/def/tern-cv/2ffe4363-dea1-4188-9f8f-835983d47fe2> ; 
    dcterms:created "2021-04-08T00:18:33"^^xsd:datetime ; 
    dcterms:modified "2021-04-08T00:43:31"^^xsd:datetime ; 
. 

<http://linked.data.gov.au/def/tern-cv/e3e69168-a959-4b8e-a1ea-2413fc3c2e4e> 
    a skos:Concept ; 
    skos:inScheme <http://linked.data.gov.au/def/tern-cv/5699eca7-9ef0-47a6-bcfb-9306e0e2b85e> ; 
    rdfs:isDefinedBy <http://linked.data.gov.au/def/tern-cv/5699eca7-9ef0-47a6-bcfb-9306e0e2b85e> ; 
    skos:prefLabel "tree alive status"@en ; 
    skos:definition "Live trees condition when measured (e.g. normal, new recruit, burnt, snapped), dead trees are recorded but their condition is not described."@en ; 
    skos:broader <http://linked.data.gov.au/def/tern-cv/2ffe4363-dea1-4188-9f8f-835983d47fe2> ; 
    dcterms:created "2021-04-08T00:42:40"^^xsd:datetime ; 
    dcterms:modified "2021-04-08T01:39:23"^^xsd:datetime ; 
. 

<http://linked.data.gov.au/def/tern-cv/0986ce8c-4a8c-4132-91f9-b7380d45ce73> 
    a skos:Concept ; 
    skos:inScheme <http://linked.data.gov.au/def/tern-cv/5699eca7-9ef0-47a6-bcfb-9306e0e2b85e> ; 
    rdfs:isDefinedBy <http://linked.data.gov.au/def/tern-cv/5699eca7-9ef0-47a6-bcfb-9306e0e2b85e> ; 
    skos:prefLabel "position x coordinate"@en ; 
    skos:definition "Position of an organisms or object inside plot, x coordinate."@en ; 
    skos:broader <http://linked.data.gov.au/def/tern-cv/5699eca7-9ef0-47a6-bcfb-9306e0e2b85e> ; 
    dcterms:created "2021-04-08T00:58:05"^^xsd:datetime ; 
    dcterms:modified "2021-04-22T03:21:29"^^xsd:datetime ; 
. 

<http://linked.data.gov.au/def/tern-cv/87ed6ce4-3354-4a3f-ba15-2b7cb0caf3da> 
    a skos:Concept ; 
    skos:inScheme <http://linked.data.gov.au/def/tern-cv/5699eca7-9ef0-47a6-bcfb-9306e0e2b85e> ; 
    rdfs:isDefinedBy <http://linked.data.gov.au/def/tern-cv/5699eca7-9ef0-47a6-bcfb-9306e0e2b85e> ; 
    skos:prefLabel "position y coordinate"@en ; 
    skos:definition "Position of an organism or object inside of plot, y coordinate."@en ; 
    skos:broader <http://linked.data.gov.au/def/tern-cv/5699eca7-9ef0-47a6-bcfb-9306e0e2b85e> ; 
    dcterms:created "2021-04-08T01:34:59"^^xsd:datetime ; 
    dcterms:modified "2021-04-22T03:20:15"^^xsd:datetime ; 
. 

<http://linked.data.gov.au/def/tern-cv/e1a18f5f-b63e-4a67-b28e-52e6f838ac14> 
    a skos:Concept ; 
    skos:inScheme <http://linked.data.gov.au/def/tern-cv/5699eca7-9ef0-47a6-bcfb-9306e0e2b85e> ; 
    rdfs:isDefinedBy <http://linked.data.gov.au/def/tern-cv/5699eca7-9ef0-47a6-bcfb-9306e0e2b85e> ; 
    skos:prefLabel "tree status"@en ; 
    skos:definition "Whether a tree is alive, dead or regenerating when censused."@en ; 
    skos:broader <http://linked.data.gov.au/def/tern-cv/2ffe4363-dea1-4188-9f8f-835983d47fe2> ; 
    dcterms:created "2021-04-08T01:54:07"^^xsd:datetime ; 
    dcterms:modified "2021-04-08T01:56:21"^^xsd:datetime ; 
. 

<http://linked.data.gov.au/def/tern-cv/894a2121-45ee-44d2-abfc-6ebae35d94c4> 
    a skos:Concept ; 
    skos:inScheme <http://linked.data.gov.au/def/tern-cv/5699eca7-9ef0-47a6-bcfb-9306e0e2b85e> ; 
    rdfs:isDefinedBy <http://linked.data.gov.au/def/tern-cv/5699eca7-9ef0-47a6-bcfb-9306e0e2b85e> ; 
    skos:prefLabel "fire event notes"@en ; 
    skos:definition "Comments or notes about the severity, frequency and last observed fire event."@en ; 
    skos:broader <http://linked.data.gov.au/def/tern-cv/45ae73d8-92bd-4261-a05f-7bfac228e1f7> ; 
    dcterms:created "2021-04-08T06:25:33"^^xsd:datetime ; 
    dcterms:modified "2021-04-08T06:27:01"^^xsd:datetime ; 
. 

<http://linked.data.gov.au/def/tern-cv/11decfe8-bbac-48f1-9773-f7694eff0498> 
    a skos:Concept ; 
    skos:inScheme <http://linked.data.gov.au/def/tern-cv/5699eca7-9ef0-47a6-bcfb-9306e0e2b85e> ; 
    rdfs:isDefinedBy <http://linked.data.gov.au/def/tern-cv/5699eca7-9ef0-47a6-bcfb-9306e0e2b85e> ; 
    skos:prefLabel "nitrogen content"@en ; 
    skos:definition "nitrogen content"@en ; 
    skos:broader <http://linked.data.gov.au/def/tern-cv/99bd0128-54d4-4a2b-8a2c-48010eb07d26> ; 
    dcterms:created "2021-04-12T01:51:22"^^xsd:datetime ; 
    dcterms:modified "2021-04-12T04:07:25"^^xsd:datetime ; 
. 

<http://linked.data.gov.au/def/tern-cv/ca1335d2-7257-415c-88b9-f7eb265fa64d> 
    a skos:Concept ; 
    skos:inScheme <http://linked.data.gov.au/def/tern-cv/5699eca7-9ef0-47a6-bcfb-9306e0e2b85e> ; 
    rdfs:isDefinedBy <http://linked.data.gov.au/def/tern-cv/5699eca7-9ef0-47a6-bcfb-9306e0e2b85e> ; 
    skos:prefLabel "carbon content"@en ; 
    skos:definition "All organic and inorganic forms of carbon present in a sample, usually measured as percentage weight."@en ; 
    skos:broader <http://linked.data.gov.au/def/tern-cv/99bd0128-54d4-4a2b-8a2c-48010eb07d26> ; 
    dcterms:created "2021-04-12T02:07:10"^^xsd:datetime ; 
    dcterms:modified "2021-04-12T02:54:20"^^xsd:datetime ; 
. 

<http://linked.data.gov.au/def/tern-cv/aa440954-9001-482c-8d0d-e4686ae3533d> 
    a skos:Concept ; 
    skos:inScheme <http://linked.data.gov.au/def/tern-cv/5699eca7-9ef0-47a6-bcfb-9306e0e2b85e> ; 
    rdfs:isDefinedBy <http://linked.data.gov.au/def/tern-cv/5699eca7-9ef0-47a6-bcfb-9306e0e2b85e> ; 
    skos:prefLabel "hydrogen content"@en ; 
    skos:definition "hydrogen content"@en ; 
    skos:broader <http://linked.data.gov.au/def/tern-cv/99bd0128-54d4-4a2b-8a2c-48010eb07d26> ; 
    dcterms:created "2021-04-12T23:30:17"^^xsd:datetime ; 
. 

<http://linked.data.gov.au/def/tern-cv/c424ab49-a9d8-41e5-b1aa-5607f87264ab> 
    a skos:Concept ; 
    skos:inScheme <http://linked.data.gov.au/def/tern-cv/5699eca7-9ef0-47a6-bcfb-9306e0e2b85e> ; 
    rdfs:isDefinedBy <http://linked.data.gov.au/def/tern-cv/5699eca7-9ef0-47a6-bcfb-9306e0e2b85e> ; 
    skos:prefLabel "negative exponential decay constant"@en ; 
    skos:definition "Decay model, assuming a constant negative exponential mass loss."@en ; 
    skos:broader <http://linked.data.gov.au/def/tern-cv/45ae73d8-92bd-4261-a05f-7bfac228e1f7> ; 
    dcterms:created "2021-04-13T04:54:33"^^xsd:datetime ; 
    dcterms:modified "2021-04-13T05:11:31"^^xsd:datetime ; 
. 

<http://linked.data.gov.au/def/tern-cv/df732786-f97a-44ad-a923-7dcd79ef7238> 
    a skos:Concept ; 
    skos:inScheme <http://linked.data.gov.au/def/tern-cv/5699eca7-9ef0-47a6-bcfb-9306e0e2b85e> ; 
    rdfs:isDefinedBy <http://linked.data.gov.au/def/tern-cv/5699eca7-9ef0-47a6-bcfb-9306e0e2b85e> ; 
    skos:prefLabel "fresh mass"@en ; 
    skos:definition "The weight of a sample fresh living material."@en ; 
    skos:broader <http://linked.data.gov.au/def/tern-cv/2ffe4363-dea1-4188-9f8f-835983d47fe2> ; 
    dcterms:created "2021-04-19T05:19:21"^^xsd:datetime ; 
    dcterms:modified "2021-04-19T05:26:00"^^xsd:datetime ; 
. 

<http://linked.data.gov.au/def/tern-cv/2a04912b-7940-4de1-9325-3902ec62d274> 
    a skos:Concept ; 
    skos:inScheme <http://linked.data.gov.au/def/tern-cv/5699eca7-9ef0-47a6-bcfb-9306e0e2b85e> ; 
    rdfs:isDefinedBy <http://linked.data.gov.au/def/tern-cv/5699eca7-9ef0-47a6-bcfb-9306e0e2b85e> ; 
    skos:prefLabel "dry mass"@en ; 
    skos:definition "The weight of dried biomass sample."@en ; 
    skos:broader <http://linked.data.gov.au/def/tern-cv/2ffe4363-dea1-4188-9f8f-835983d47fe2> ; 
    dcterms:created "2021-04-19T05:26:23"^^xsd:datetime ; 
    dcterms:modified "2021-04-19T05:28:12"^^xsd:datetime ; 
. 

<http://linked.data.gov.au/def/tern-cv/61a29f86-c1ee-4730-bcb4-8394746baf67> 
    a skos:Concept ; 
    skos:inScheme <http://linked.data.gov.au/def/tern-cv/5699eca7-9ef0-47a6-bcfb-9306e0e2b85e> ; 
    rdfs:isDefinedBy <http://linked.data.gov.au/def/tern-cv/5699eca7-9ef0-47a6-bcfb-9306e0e2b85e> ; 
    skos:prefLabel "water content"@en ; 
    skos:definition "Quantity of water contained in a material"@en ; 
    skos:broader <http://linked.data.gov.au/def/tern-cv/2ffe4363-dea1-4188-9f8f-835983d47fe2> ; 
    dcterms:created "2021-04-19T05:30:09"^^xsd:datetime ; 
    dcterms:modified "2021-04-19T05:31:21"^^xsd:datetime ; 
. 

<http://linked.data.gov.au/def/tern-cv/f0bcd32d-db46-45c4-b860-a099a5e06603> 
    a skos:Concept ; 
    skos:inScheme <http://linked.data.gov.au/def/tern-cv/5699eca7-9ef0-47a6-bcfb-9306e0e2b85e> ; 
    rdfs:isDefinedBy <http://linked.data.gov.au/def/tern-cv/5699eca7-9ef0-47a6-bcfb-9306e0e2b85e> ; 
    skos:prefLabel "stem count"@en ; 
    skos:definition "Number of woody plants."@en ; 
    skos:broader <http://linked.data.gov.au/def/tern-cv/2ffe4363-dea1-4188-9f8f-835983d47fe2> ; 
    dcterms:created "2021-04-20T03:07:32"^^xsd:datetime ; 
    dcterms:modified "2021-04-20T03:09:24"^^xsd:datetime ; 
. 

<http://linked.data.gov.au/def/tern-cv/52d0752f-a8b9-40fc-9ba5-1d34cb602f62> 
    a skos:Concept ; 
    skos:inScheme <http://linked.data.gov.au/def/tern-cv/5699eca7-9ef0-47a6-bcfb-9306e0e2b85e> ; 
    rdfs:isDefinedBy <http://linked.data.gov.au/def/tern-cv/5699eca7-9ef0-47a6-bcfb-9306e0e2b85e> ; 
    skos:prefLabel "diameter class"@en ; 
    skos:definition "Ordinal classification of trees based on diameter outside bark."@en ; 
    skos:broader <http://linked.data.gov.au/def/tern-cv/2ffe4363-dea1-4188-9f8f-835983d47fe2> ; 
    dcterms:created "2021-04-20T04:43:01"^^xsd:datetime ; 
    dcterms:modified "2021-04-21T05:23:22"^^xsd:datetime ; 
. 

<http://linked.data.gov.au/def/tern-cv/e88ad59e-0d19-4796-b0be-f7ec3edd7624> 
    a skos:Concept ; 
    skos:inScheme <http://linked.data.gov.au/def/tern-cv/5699eca7-9ef0-47a6-bcfb-9306e0e2b85e> ; 
    rdfs:isDefinedBy <http://linked.data.gov.au/def/tern-cv/5699eca7-9ef0-47a6-bcfb-9306e0e2b85e> ; 
    skos:prefLabel "litterfall"@en ; 
    skos:definition "Dead plant material, such as leaves, bark, needles, and twigs, that has fallen to the ground."@en ; 
    skos:broader <http://linked.data.gov.au/def/tern-cv/2ffe4363-dea1-4188-9f8f-835983d47fe2> ; 
    skos:narrower <http://linked.data.gov.au/def/tern-cv/bc921a02-a757-4071-b39a-383af90d31cd>,
        <http://linked.data.gov.au/def/tern-cv/de1e9c3a-8ed7-4d91-8b67-37c7488b7478> ;
    dcterms:created "2021-04-20T04:55:38"^^xsd:datetime ; 
    dcterms:modified "2021-04-20T04:56:39"^^xsd:datetime ; 
. 

<http://linked.data.gov.au/def/tern-cv/bc921a02-a757-4071-b39a-383af90d31cd> 
    a skos:Concept ; 
    skos:inScheme <http://linked.data.gov.au/def/tern-cv/5699eca7-9ef0-47a6-bcfb-9306e0e2b85e> ; 
    rdfs:isDefinedBy <http://linked.data.gov.au/def/tern-cv/5699eca7-9ef0-47a6-bcfb-9306e0e2b85e> ; 
    skos:prefLabel "coarse litterfall mass"@en ; 
    skos:definition "Weight of dead plant material that has fallen to the ground with diameter >6 mm."@en ; 
    skos:broader <http://linked.data.gov.au/def/tern-cv/e88ad59e-0d19-4796-b0be-f7ec3edd7624> ; 
    dcterms:created "2021-04-20T04:57:18"^^xsd:datetime ; 
    dcterms:modified "2021-04-20T05:01:42"^^xsd:datetime ; 
. 

<http://linked.data.gov.au/def/tern-cv/de1e9c3a-8ed7-4d91-8b67-37c7488b7478> 
    a skos:Concept ; 
    skos:inScheme <http://linked.data.gov.au/def/tern-cv/5699eca7-9ef0-47a6-bcfb-9306e0e2b85e> ; 
    rdfs:isDefinedBy <http://linked.data.gov.au/def/tern-cv/5699eca7-9ef0-47a6-bcfb-9306e0e2b85e> ; 
    skos:prefLabel "fine litterfall mass"@en ; 
    skos:definition "Weight of dead plant material that has fallen to the ground with diameter <6 mm."@en ; 
    skos:broader <http://linked.data.gov.au/def/tern-cv/e88ad59e-0d19-4796-b0be-f7ec3edd7624> ; 
    dcterms:created "2021-04-20T04:58:02"^^xsd:datetime ; 
    dcterms:modified "2021-04-20T05:02:12"^^xsd:datetime ; 
. 

<http://linked.data.gov.au/def/tern-cv/5a7f318c-c91f-4477-b680-73b3de954fbe> 
    a skos:Concept ; 
    skos:inScheme <http://linked.data.gov.au/def/tern-cv/5699eca7-9ef0-47a6-bcfb-9306e0e2b85e> ; 
    rdfs:isDefinedBy <http://linked.data.gov.au/def/tern-cv/5699eca7-9ef0-47a6-bcfb-9306e0e2b85e> ; 
    skos:prefLabel "diameter of hollow"@en ; 
    skos:definition "Diameter of tree hollow."@en ; 
    skos:broader <http://linked.data.gov.au/def/tern-cv/2ffe4363-dea1-4188-9f8f-835983d47fe2> ; 
    dcterms:created "2021-04-20T05:15:42"^^xsd:datetime ; 
    dcterms:modified "2021-04-20T05:18:14"^^xsd:datetime ; 
. 

<http://linked.data.gov.au/def/tern-cv/4c6a55a6-3ea2-485f-82bc-c5b89a95a605> 
    a skos:Concept ; 
    skos:inScheme <http://linked.data.gov.au/def/tern-cv/5699eca7-9ef0-47a6-bcfb-9306e0e2b85e> ; 
    rdfs:isDefinedBy <http://linked.data.gov.au/def/tern-cv/5699eca7-9ef0-47a6-bcfb-9306e0e2b85e> ; 
    skos:prefLabel "species cover"@en ; 
    skos:definition "The cover for each plant species evaluated independently from the cover of other species, expressed as a percentage of the area occupied by each species, The sum of the combined species covers can exceeed 100%."@en ; 
    skos:broader <http://linked.data.gov.au/def/tern-cv/2ffe4363-dea1-4188-9f8f-835983d47fe2> ; 
    dcterms:created "2021-04-20T05:23:43"^^xsd:datetime ; 
    dcterms:modified "2021-04-20T05:27:07"^^xsd:datetime ; 
. 

<http://linked.data.gov.au/def/tern-cv/f3f88912-4aab-4d6c-b2ab-7b42ecfaae60> 
    a skos:Concept ; 
    skos:inScheme <http://linked.data.gov.au/def/tern-cv/5699eca7-9ef0-47a6-bcfb-9306e0e2b85e> ; 
    rdfs:isDefinedBy <http://linked.data.gov.au/def/tern-cv/5699eca7-9ef0-47a6-bcfb-9306e0e2b85e> ; 
    skos:prefLabel "cover"@en ; 
    skos:definition "The cover for each plant species, groweth form, matter type evaluated independently from the cover of other elements, expressed as a percentage of the area occupied by each element, The sum of the combined covers can exceeed 100%."@en ; 
    skos:broader <http://linked.data.gov.au/def/tern-cv/2ffe4363-dea1-4188-9f8f-835983d47fe2> ; 
    dcterms:created "2021-04-20T05:32:07"^^xsd:datetime ; 
    dcterms:modified "2021-04-20T05:33:08"^^xsd:datetime ; 
. 

<http://linked.data.gov.au/def/tern-cv/9343e3b9-bca2-48e2-af02-eed8111e0147> 
    a skos:Concept ; 
    skos:inScheme <http://linked.data.gov.au/def/tern-cv/5699eca7-9ef0-47a6-bcfb-9306e0e2b85e> ; 
    rdfs:isDefinedBy <http://linked.data.gov.au/def/tern-cv/5699eca7-9ef0-47a6-bcfb-9306e0e2b85e> ; 
    skos:prefLabel "canopy greenness"@en ; 
    skos:definition "An estimate of vegetation condition based on the combined ‘colour’ resulting from the chlorophyll content of foliage, the area covered by leaves, and the density and structure of the vegetation. Plant or canopy greeness may be assessed at a site level using photopoints or phenocamera images, or at a landscape level using satellite remote sensing indices such as the Normalised Difference Vegetation Index (NDVI)."@en ; 
    skos:broader <http://linked.data.gov.au/def/tern-cv/45ae73d8-92bd-4261-a05f-7bfac228e1f7> ; 
    dcterms:created "2021-04-21T04:28:02"^^xsd:datetime ; 
    dcterms:modified "2021-04-22T03:29:12"^^xsd:datetime ; 
. 

<http://linked.data.gov.au/def/tern-cv/9343e3b9-bca2-48e2-af02-eed8111e0147> 
    a skos:Concept ; 
    skos:inScheme <http://linked.data.gov.au/def/tern-cv/5699eca7-9ef0-47a6-bcfb-9306e0e2b85e> ; 
    rdfs:isDefinedBy <http://linked.data.gov.au/def/tern-cv/5699eca7-9ef0-47a6-bcfb-9306e0e2b85e> ; 
    skos:prefLabel "canopy greenness"@en ; 
    skos:definition "An estimate of vegetation condition based on the combined ‘colour’ resulting from the chlorophyll content of foliage, the area covered by leaves, and the density and structure of the vegetation. Plant or canopy greeness may be assessed at a site level using photopoints or phenocamera images, or at a landscape level using satellite remote sensing indices such as the Normalised Difference Vegetation Index (NDVI)."@en ; 
    skos:broader <http://linked.data.gov.au/def/tern-cv/8fa1c4bd-73b3-432a-ab49-9ee89928e6d9> ; 
    dcterms:created "2021-04-21T04:28:02"^^xsd:datetime ; 
    dcterms:modified "2021-04-22T03:29:12"^^xsd:datetime ; 
. 

<http://linked.data.gov.au/def/tern-cv/d87a652c-0a30-415c-bef7-e20f75d94002> 
    a skos:Concept ; 
    skos:inScheme <http://linked.data.gov.au/def/tern-cv/5699eca7-9ef0-47a6-bcfb-9306e0e2b85e> ; 
    rdfs:isDefinedBy <http://linked.data.gov.au/def/tern-cv/5699eca7-9ef0-47a6-bcfb-9306e0e2b85e> ; 
    skos:prefLabel "plant phenology"@en ; 
    skos:definition "The study of the timing of recurring climate or weather-driven plant biological changes, the causes of periodicity, the relationship with biotic (e.g. fruit availability) and abiotic (e.g. rain) drivers and the interrelations between the seasonal cycle of the same or different species."@en ; 
    skos:broader <http://linked.data.gov.au/def/tern-cv/8fa1c4bd-73b3-432a-ab49-9ee89928e6d9> ; 
    dcterms:created "2021-04-21T06:37:36"^^xsd:datetime ; 
    dcterms:modified "2021-04-21T07:04:08"^^xsd:datetime ; 
. 

<http://linked.data.gov.au/def/tern-cv/c3d26c6f-91b7-4627-91e6-2147fa44ad03> 
    a skos:Concept ; 
    skos:inScheme <http://linked.data.gov.au/def/tern-cv/5699eca7-9ef0-47a6-bcfb-9306e0e2b85e> ; 
    rdfs:isDefinedBy <http://linked.data.gov.au/def/tern-cv/5699eca7-9ef0-47a6-bcfb-9306e0e2b85e> ; 
    skos:prefLabel "above-ground biomass"@en ; 
    skos:definition "All living organic matter above the soil, including stem, stump, branches, bark, seeds and foliage."@en ; 
    skos:broader <http://linked.data.gov.au/def/tern-cv/45ae73d8-92bd-4261-a05f-7bfac228e1f7> ; 
    dcterms:created "2021-04-21T07:21:15"^^xsd:datetime ; 
    dcterms:modified "2021-04-22T03:48:01"^^xsd:datetime ; 
. 

<http://linked.data.gov.au/def/tern-cv/c3d26c6f-91b7-4627-91e6-2147fa44ad03> 
    a skos:Concept ; 
    skos:inScheme <http://linked.data.gov.au/def/tern-cv/5699eca7-9ef0-47a6-bcfb-9306e0e2b85e> ; 
    rdfs:isDefinedBy <http://linked.data.gov.au/def/tern-cv/5699eca7-9ef0-47a6-bcfb-9306e0e2b85e> ; 
    skos:prefLabel "above-ground biomass"@en ; 
    skos:definition "All living organic matter above the soil, including stem, stump, branches, bark, seeds and foliage."@en ; 
    skos:broader <http://linked.data.gov.au/def/tern-cv/8fa1c4bd-73b3-432a-ab49-9ee89928e6d9> ; 
    dcterms:created "2021-04-21T07:21:15"^^xsd:datetime ; 
    dcterms:modified "2021-04-22T03:48:01"^^xsd:datetime ; 
. 

<http://linked.data.gov.au/def/tern-cv/6c73ea38-c3d6-49bf-b6e9-4042d09bbee0> 
    a skos:Concept ; 
    skos:inScheme <http://linked.data.gov.au/def/tern-cv/5699eca7-9ef0-47a6-bcfb-9306e0e2b85e> ; 
    rdfs:isDefinedBy <http://linked.data.gov.au/def/tern-cv/5699eca7-9ef0-47a6-bcfb-9306e0e2b85e> ; 
    skos:prefLabel "height"@en ; 
    skos:definition "The height of an organism or object."@en ; 
    skos:broader <http://linked.data.gov.au/def/tern-cv/2ffe4363-dea1-4188-9f8f-835983d47fe2> ; 
    dcterms:created "2021-04-22T03:15:39"^^xsd:datetime ; 
    dcterms:modified "2021-04-22T03:23:33"^^xsd:datetime ; 
. 

<http://linked.data.gov.au/def/tern-cv/4c19f603-572e-471c-82eb-230f822c263d> 
    a skos:Concept ; 
    skos:inScheme <http://linked.data.gov.au/def/tern-cv/5699eca7-9ef0-47a6-bcfb-9306e0e2b85e> ; 
    rdfs:isDefinedBy <http://linked.data.gov.au/def/tern-cv/5699eca7-9ef0-47a6-bcfb-9306e0e2b85e> ; 
    skos:prefLabel "animal occurrence"@en ; 
    skos:definition "An existence of an animal or group of animals at a particular place at a particular time."@en ; 
    skos:broader <http://linked.data.gov.au/def/tern-cv/2ffe4363-dea1-4188-9f8f-835983d47fe2> ; 
    dcterms:created "2021-04-21T06:30:18"^^xsd:datetime ; 
    dcterms:modified "2021-04-28T03:03:32"^^xsd:datetime ; 
. 

<http://linked.data.gov.au/def/tern-cv/01847226-c42a-4904-bbb8-dc69519bc5b4> 
    a skos:Concept ; 
    skos:inScheme <http://linked.data.gov.au/def/tern-cv/5699eca7-9ef0-47a6-bcfb-9306e0e2b85e> ; 
    rdfs:isDefinedBy <http://linked.data.gov.au/def/tern-cv/5699eca7-9ef0-47a6-bcfb-9306e0e2b85e> ; 
    skos:prefLabel "flora occurrence"@en ; 
    skos:definition "An existence of a plant(s) at a particular place at a particular time."@en ; 
    skos:broader <http://linked.data.gov.au/def/tern-cv/2ffe4363-dea1-4188-9f8f-835983d47fe2> ; 
    dcterms:created "2021-04-21T06:30:18"^^xsd:datetime ; 
    dcterms:modified "2021-04-28T03:02:32"^^xsd:datetime ; 
. 

<http://linked.data.gov.au/def/tern-cv/195c45af-505c-4df4-98c3-d43867af01c2> 
    a skos:Concept ; 
    skos:inScheme <http://linked.data.gov.au/def/tern-cv/5699eca7-9ef0-47a6-bcfb-9306e0e2b85e> ; 
    rdfs:isDefinedBy <http://linked.data.gov.au/def/tern-cv/5699eca7-9ef0-47a6-bcfb-9306e0e2b85e> ; 
    skos:prefLabel "fungus occurrence"@en ; 
    skos:definition "An existence of a fungi at a particular place at a particular time."@en ; 
    skos:broader <http://linked.data.gov.au/def/tern-cv/2ffe4363-dea1-4188-9f8f-835983d47fe2> ; 
    dcterms:created "2021-04-21T06:30:18"^^xsd:datetime ; 
    dcterms:modified "2021-04-28T03:04:31"^^xsd:datetime ; 
. 

<http://linked.data.gov.au/def/tern-cv/aa7d5f61-99e6-4e34-8a46-40ac5fbd7b14> 
    a skos:Concept ; 
    skos:inScheme <http://linked.data.gov.au/def/tern-cv/5699eca7-9ef0-47a6-bcfb-9306e0e2b85e> ; 
    rdfs:isDefinedBy <http://linked.data.gov.au/def/tern-cv/5699eca7-9ef0-47a6-bcfb-9306e0e2b85e> ; 
    skos:prefLabel "RGB values"@en ; 
    skos:definition "Data represented as integer values assigned to the red, blue and green wavelengths of the electromagnetic spectrum, which interact to represent different colours to the human eye. The data can be captured/presented in a grid format as a two dimensional digital image with three colour bands or layers."@en ; 
    skos:broader <http://linked.data.gov.au/def/tern-cv/9e03a73d-8e89-4187-9f96-0306aad93458> ; 
    dcterms:modified "2021-04-28T02:59:20"^^xsd:datetime ; 
. 

<http://linked.data.gov.au/def/tern-cv/919d93eb-d7f1-40b3-86ed-91426d925013> 
    a skos:Concept ; 
    skos:inScheme <http://linked.data.gov.au/def/tern-cv/5699eca7-9ef0-47a6-bcfb-9306e0e2b85e> ; 
    rdfs:isDefinedBy <http://linked.data.gov.au/def/tern-cv/5699eca7-9ef0-47a6-bcfb-9306e0e2b85e> ; 
    skos:prefLabel "tree condition"@en ; 
    skos:definition "The condition of the tree."@en ; 
    skos:broader <http://linked.data.gov.au/def/tern-cv/8fa1c4bd-73b3-432a-ab49-9ee89928e6d9> ; 
    dcterms:created "2021-05-07T00:29:09"^^xsd:datetime ; 
    dcterms:modified "2021-05-07T00:33:18"^^xsd:datetime ; 
. 

<http://linked.data.gov.au/def/tern-cv/6e0b10ba-b6f2-4d2f-8a86-6873c565e95d> 
    a skos:Concept ; 
    skos:inScheme <http://linked.data.gov.au/def/tern-cv/5699eca7-9ef0-47a6-bcfb-9306e0e2b85e> ; 
    rdfs:isDefinedBy <http://linked.data.gov.au/def/tern-cv/5699eca7-9ef0-47a6-bcfb-9306e0e2b85e> ; 
    skos:prefLabel "coarse woody debris stock mean"@en ; 
    skos:definition "Average mass of dead pieces of wood found on the ground including downed, dead tree and shrub boles, large limbs, and other woody pieces that are severed from their original source of growth with a diameter >7.6cm. Usually measured in mass/area."@en ; 
    skos:broader <http://linked.data.gov.au/def/tern-cv/45ae73d8-92bd-4261-a05f-7bfac228e1f7> ; 
    dcterms:created "2021-05-18T05:41:43"^^xsd:datetime ; 
    dcterms:modified "2021-05-18T06:07:04"^^xsd:datetime ; 
. 

<http://linked.data.gov.au/def/tern-cv/1e56b253-6497-49b8-9805-0eae69da1d9b> 
    a skos:Concept ; 
    skos:inScheme <http://linked.data.gov.au/def/tern-cv/5699eca7-9ef0-47a6-bcfb-9306e0e2b85e> ; 
    rdfs:isDefinedBy <http://linked.data.gov.au/def/tern-cv/5699eca7-9ef0-47a6-bcfb-9306e0e2b85e> ; 
    skos:prefLabel "coarse woody debris sd"@en ; 
    skos:definition "Standard deviation (sd) of the mass of dead pieces of wood found on the ground including downed, dead tree and shrub boles, large limbs, and other woody pieces that are severed from their original source of growth with a diameter >7.6cm. Measured in same units as coarse woody debris stock mean."@en ; 
    skos:broader <http://linked.data.gov.au/def/tern-cv/45ae73d8-92bd-4261-a05f-7bfac228e1f7> ; 
    dcterms:created "2021-05-18T05:48:05"^^xsd:datetime ; 
    dcterms:modified "2021-05-18T06:07:17"^^xsd:datetime ; 
. 

<http://linked.data.gov.au/def/tern-cv/3da7a464-609c-4294-9814-5f3aea0eb265> 
    a skos:Concept ; 
    skos:inScheme <http://linked.data.gov.au/def/tern-cv/5699eca7-9ef0-47a6-bcfb-9306e0e2b85e> ; 
    rdfs:isDefinedBy <http://linked.data.gov.au/def/tern-cv/5699eca7-9ef0-47a6-bcfb-9306e0e2b85e> ; 
    skos:prefLabel "fine woody debris production mean"@en ; 
    skos:definition "Average mass of dead branches, twigs, wood splinters 0.3 - 7.4 cm in diameter (0.1 to 2.9 inches ) that have fallen to the groun over a define area and timespan."@en ; 
    skos:broader <http://linked.data.gov.au/def/tern-cv/45ae73d8-92bd-4261-a05f-7bfac228e1f7> ; 
    dcterms:created "2021-05-18T05:53:10"^^xsd:datetime ; 
    dcterms:modified "2021-05-18T05:57:50"^^xsd:datetime ; 
. 

<http://linked.data.gov.au/def/tern-cv/3f11b33a-bdee-4c19-b9a0-47a1f894a0d3> 
    a skos:Concept ; 
    skos:inScheme <http://linked.data.gov.au/def/tern-cv/5699eca7-9ef0-47a6-bcfb-9306e0e2b85e> ; 
    rdfs:isDefinedBy <http://linked.data.gov.au/def/tern-cv/5699eca7-9ef0-47a6-bcfb-9306e0e2b85e> ; 
    skos:prefLabel "fine woody debris production sd"@en ; 
    skos:definition "Standard deviation of the  mass of dead branches, twigs, wood splinters 0.3 - 7.4 cm in diameter (0.1 to 2.9 inches ) that have fallen to the groun over a define area and timespan."@en ; 
    skos:broader <http://linked.data.gov.au/def/tern-cv/45ae73d8-92bd-4261-a05f-7bfac228e1f7> ; 
    dcterms:created "2021-05-18T05:58:19"^^xsd:datetime ; 
    dcterms:modified "2021-05-18T05:59:40"^^xsd:datetime ; 
. 

<http://linked.data.gov.au/def/tern-cv/035d3a8f-1d73-4990-850a-18fd80120f43> 
    a skos:Concept ; 
    skos:inScheme <http://linked.data.gov.au/def/tern-cv/5699eca7-9ef0-47a6-bcfb-9306e0e2b85e> ; 
    rdfs:isDefinedBy <http://linked.data.gov.au/def/tern-cv/5699eca7-9ef0-47a6-bcfb-9306e0e2b85e> ; 
    skos:prefLabel "leaf litter production mean"@en ; 
    skos:definition "Average mass of leaves and/or needles that has fallen to the ground. Usuallly measure over a specific area and timespan."@en ; 
    skos:broader <http://linked.data.gov.au/def/tern-cv/45ae73d8-92bd-4261-a05f-7bfac228e1f7> ; 
    dcterms:created "2021-05-18T06:01:08"^^xsd:datetime ; 
    dcterms:modified "2021-05-18T06:03:18"^^xsd:datetime ; 
. 

<http://linked.data.gov.au/def/tern-cv/564e7135-e4f5-4114-b522-13686007291f> 
    a skos:Concept ; 
    skos:inScheme <http://linked.data.gov.au/def/tern-cv/5699eca7-9ef0-47a6-bcfb-9306e0e2b85e> ; 
    rdfs:isDefinedBy <http://linked.data.gov.au/def/tern-cv/5699eca7-9ef0-47a6-bcfb-9306e0e2b85e> ; 
    skos:prefLabel "leaf litter production sd"@en ; 
    skos:definition "Standard deviation (sd) of values of mass of leaves and/or needles that has fallen to the ground. Measure in same units as leaf litter production mean"@en ; 
    skos:broader <http://linked.data.gov.au/def/tern-cv/45ae73d8-92bd-4261-a05f-7bfac228e1f7> ; 
    dcterms:created "2021-05-18T06:03:44"^^xsd:datetime ; 
    dcterms:modified "2021-05-18T06:05:28"^^xsd:datetime ; 
. 

<http://linked.data.gov.au/def/tern-cv/d0e0629e-7000-445a-a14f-40aca1cc6646> 
    a skos:Concept ; 
    skos:inScheme <http://linked.data.gov.au/def/tern-cv/5699eca7-9ef0-47a6-bcfb-9306e0e2b85e> ; 
    rdfs:isDefinedBy <http://linked.data.gov.au/def/tern-cv/5699eca7-9ef0-47a6-bcfb-9306e0e2b85e> ; 
    skos:prefLabel "leaf litter stock mean"@en ; 
    skos:definition "Average mass values of leaves and/or needles found on the ground."@en ; 
    skos:broader <http://linked.data.gov.au/def/tern-cv/45ae73d8-92bd-4261-a05f-7bfac228e1f7> ; 
    dcterms:created "2021-05-18T06:06:50"^^xsd:datetime ; 
    dcterms:modified "2021-05-18T06:14:26"^^xsd:datetime ; 
. 

<http://linked.data.gov.au/def/tern-cv/2e210a48-3c1c-4ef6-8449-9d836f8d8b31> 
    a skos:Concept ; 
    skos:inScheme <http://linked.data.gov.au/def/tern-cv/5699eca7-9ef0-47a6-bcfb-9306e0e2b85e> ; 
    rdfs:isDefinedBy <http://linked.data.gov.au/def/tern-cv/5699eca7-9ef0-47a6-bcfb-9306e0e2b85e> ; 
    skos:prefLabel "leaf litter stock sd"@en ; 
    skos:definition "Standard deviation (sd) of values of mass of leaves and/or needles found on the ground."@en ; 
    skos:broader <http://linked.data.gov.au/def/tern-cv/45ae73d8-92bd-4261-a05f-7bfac228e1f7> ; 
    dcterms:created "2021-05-18T06:07:54"^^xsd:datetime ; 
    dcterms:modified "2021-05-18T06:13:58"^^xsd:datetime ; 
. 

<http://linked.data.gov.au/def/tern-cv/0416e086-9568-48d5-9a12-bf90fd1889c4> 
    a skos:Concept ; 
    skos:inScheme <http://linked.data.gov.au/def/tern-cv/5699eca7-9ef0-47a6-bcfb-9306e0e2b85e> ; 
    rdfs:isDefinedBy <http://linked.data.gov.au/def/tern-cv/5699eca7-9ef0-47a6-bcfb-9306e0e2b85e> ; 
    skos:prefLabel "fine woody debris stock mean"@en ; 
    skos:definition "Average mass of dead branches, twigs, wood splinters 0.3 - 7.4 cm in diameter (0.1 to 2.9 inches ) found on the ground at the moment of sampling."@en ; 
    skos:broader <http://linked.data.gov.au/def/tern-cv/45ae73d8-92bd-4261-a05f-7bfac228e1f7> ; 
    dcterms:created "2021-05-18T06:15:09"^^xsd:datetime ; 
    dcterms:modified "2021-05-18T06:16:53"^^xsd:datetime ; 
. 

<http://linked.data.gov.au/def/tern-cv/968ce393-cc9c-49d0-b910-d64f54e5cdf8> 
    a skos:Concept ; 
    skos:inScheme <http://linked.data.gov.au/def/tern-cv/5699eca7-9ef0-47a6-bcfb-9306e0e2b85e> ; 
    rdfs:isDefinedBy <http://linked.data.gov.au/def/tern-cv/5699eca7-9ef0-47a6-bcfb-9306e0e2b85e> ; 
    skos:prefLabel "fine woody debris stock sd"@en ; 
    skos:definition "Standard deviation (sd) of the mass of dead branches, twigs, wood splinters 0.3 - 7.4 cm in diameter (0.1 to 2.9 inches ) found on the ground at the moment of sampling."@en ; 
    skos:broader <http://linked.data.gov.au/def/tern-cv/45ae73d8-92bd-4261-a05f-7bfac228e1f7> ; 
    dcterms:created "2021-05-18T06:15:41"^^xsd:datetime ; 
    dcterms:modified "2021-05-18T06:17:28"^^xsd:datetime ; 
. 

<http://linked.data.gov.au/def/tern-cv/91988f41-89de-4522-9f04-c8bf6bd68bfe> 
    a skos:Concept ; 
    skos:inScheme <http://linked.data.gov.au/def/tern-cv/5699eca7-9ef0-47a6-bcfb-9306e0e2b85e> ; 
    rdfs:isDefinedBy <http://linked.data.gov.au/def/tern-cv/5699eca7-9ef0-47a6-bcfb-9306e0e2b85e> ; 
    skos:prefLabel "fine woody debris turnover"@en ; 
    skos:definition "Loss rates of dead branches, twigs, wood splinters 0.3 - 7.4 cm in diameter (0.1 to 2.9 inches )."@en ; 
    skos:broader <http://linked.data.gov.au/def/tern-cv/45ae73d8-92bd-4261-a05f-7bfac228e1f7> ; 
    dcterms:created "2021-05-18T06:24:38"^^xsd:datetime ; 
    dcterms:modified "2021-05-18T06:37:39"^^xsd:datetime ; 
. 

<http://linked.data.gov.au/def/tern-cv/d2a16407-6155-4d3a-85e3-738006934b28> 
    a skos:Concept ; 
    skos:inScheme <http://linked.data.gov.au/def/tern-cv/5699eca7-9ef0-47a6-bcfb-9306e0e2b85e> ; 
    rdfs:isDefinedBy <http://linked.data.gov.au/def/tern-cv/5699eca7-9ef0-47a6-bcfb-9306e0e2b85e> ; 
    skos:prefLabel "leaf litter turnover"@en ; 
    skos:definition "Loss rates of leaves and/or needles."@en ; 
    skos:broader <http://linked.data.gov.au/def/tern-cv/45ae73d8-92bd-4261-a05f-7bfac228e1f7> ; 
    dcterms:created "2021-05-18T06:25:39"^^xsd:datetime ; 
    dcterms:modified "2021-05-18T06:38:22"^^xsd:datetime ; 
. 

<http://linked.data.gov.au/def/tern-cv/2fb464d4-feac-4e1b-b0ef-bb12e2d68480> 
    a skos:Concept ; 
    skos:inScheme <http://linked.data.gov.au/def/tern-cv/5699eca7-9ef0-47a6-bcfb-9306e0e2b85e> ; 
    rdfs:isDefinedBy <http://linked.data.gov.au/def/tern-cv/5699eca7-9ef0-47a6-bcfb-9306e0e2b85e> ; 
    skos:prefLabel "grass fuel load mean"@en ; 
    skos:definition "Average dry biomass of leaf litter present on the ground. Usually measure as mass per area."@en ; 
    skos:broader <http://linked.data.gov.au/def/tern-cv/45ae73d8-92bd-4261-a05f-7bfac228e1f7> ; 
    dcterms:created "2021-05-18T23:29:37"^^xsd:datetime ; 
    dcterms:modified "2021-05-18T23:45:40"^^xsd:datetime ; 
. 

<http://linked.data.gov.au/def/tern-cv/3f898b54-a260-4810-be35-f6b52c691345> 
    a skos:Concept ; 
    skos:inScheme <http://linked.data.gov.au/def/tern-cv/5699eca7-9ef0-47a6-bcfb-9306e0e2b85e> ; 
    rdfs:isDefinedBy <http://linked.data.gov.au/def/tern-cv/5699eca7-9ef0-47a6-bcfb-9306e0e2b85e> ; 
    skos:prefLabel "herbs fuel load mean"@en ; 
    skos:definition "Average dry biomass of herbs on the ground. Usually measure as mass per area"@en ; 
    skos:broader <http://linked.data.gov.au/def/tern-cv/45ae73d8-92bd-4261-a05f-7bfac228e1f7> ; 
    dcterms:created "2021-05-18T23:31:28"^^xsd:datetime ; 
    dcterms:modified "2021-05-18T23:37:52"^^xsd:datetime ; 
. 

<http://linked.data.gov.au/def/tern-cv/a609ef3e-0baf-4164-96b0-e5d100f56c2f> 
    a skos:Concept ; 
    skos:inScheme <http://linked.data.gov.au/def/tern-cv/5699eca7-9ef0-47a6-bcfb-9306e0e2b85e> ; 
    rdfs:isDefinedBy <http://linked.data.gov.au/def/tern-cv/5699eca7-9ef0-47a6-bcfb-9306e0e2b85e> ; 
    skos:prefLabel "grass fuel load sd"@en ; 
    skos:definition "Standard deviation of grass dry biomass measurements."@en ; 
    skos:broader <http://linked.data.gov.au/def/tern-cv/45ae73d8-92bd-4261-a05f-7bfac228e1f7> ; 
    dcterms:created "2021-05-18T23:38:37"^^xsd:datetime ; 
    dcterms:modified "2021-05-18T23:39:40"^^xsd:datetime ; 
. 

<http://linked.data.gov.au/def/tern-cv/0b093c5b-2c67-4d22-8a49-85fb3b89553d> 
    a skos:Concept ; 
    skos:inScheme <http://linked.data.gov.au/def/tern-cv/5699eca7-9ef0-47a6-bcfb-9306e0e2b85e> ; 
    rdfs:isDefinedBy <http://linked.data.gov.au/def/tern-cv/5699eca7-9ef0-47a6-bcfb-9306e0e2b85e> ; 
    skos:prefLabel "herbs fuel load sd"@en ; 
    skos:definition "Standard deviation of dry biomass of herbs measurements."@en ; 
    skos:broader <http://linked.data.gov.au/def/tern-cv/45ae73d8-92bd-4261-a05f-7bfac228e1f7> ; 
    dcterms:created "2021-05-18T23:40:06"^^xsd:datetime ; 
    dcterms:modified "2021-05-18T23:40:46"^^xsd:datetime ; 
. 

<http://linked.data.gov.au/def/tern-cv/49938851-6433-46bb-b070-56f1601a3033> 
    a skos:Concept ; 
    skos:inScheme <http://linked.data.gov.au/def/tern-cv/5699eca7-9ef0-47a6-bcfb-9306e0e2b85e> ; 
    rdfs:isDefinedBy <http://linked.data.gov.au/def/tern-cv/5699eca7-9ef0-47a6-bcfb-9306e0e2b85e> ; 
    skos:prefLabel "leaf litter fuel load mean"@en ; 
    skos:definition "Average leaf litter dry biomass on the ground. Usually measure as mass per area."@en ; 
    skos:broader <http://linked.data.gov.au/def/tern-cv/45ae73d8-92bd-4261-a05f-7bfac228e1f7> ; 
    dcterms:created "2021-05-18T23:42:24"^^xsd:datetime ; 
    dcterms:modified "2021-05-19T00:01:11"^^xsd:datetime ; 
. 

<http://linked.data.gov.au/def/tern-cv/35506cfc-c7f0-4cb4-be3d-54e41e4ac691> 
    a skos:Concept ; 
    skos:inScheme <http://linked.data.gov.au/def/tern-cv/5699eca7-9ef0-47a6-bcfb-9306e0e2b85e> ; 
    rdfs:isDefinedBy <http://linked.data.gov.au/def/tern-cv/5699eca7-9ef0-47a6-bcfb-9306e0e2b85e> ; 
    skos:prefLabel "leaf litter fuel load sd"@en ; 
    skos:definition "Standard deviation of dry biomass of leaf litter measurements."@en ; 
    skos:broader <http://linked.data.gov.au/def/tern-cv/45ae73d8-92bd-4261-a05f-7bfac228e1f7> ; 
    dcterms:created "2021-05-18T23:47:01"^^xsd:datetime ; 
    dcterms:modified "2021-05-18T23:53:24"^^xsd:datetime ; 
. 

<http://linked.data.gov.au/def/tern-cv/5653af0e-f853-4b98-b4c9-f8626456d314> 
    a skos:Concept ; 
    skos:inScheme <http://linked.data.gov.au/def/tern-cv/5699eca7-9ef0-47a6-bcfb-9306e0e2b85e> ; 
    rdfs:isDefinedBy <http://linked.data.gov.au/def/tern-cv/5699eca7-9ef0-47a6-bcfb-9306e0e2b85e> ; 
    skos:prefLabel "vines fuel load mean"@en ; 
    skos:definition "Average dry biomass of vines present on the ground. Usually measure as mass per area."@en ; 
    skos:broader <http://linked.data.gov.au/def/tern-cv/45ae73d8-92bd-4261-a05f-7bfac228e1f7> ; 
    dcterms:created "2021-05-19T00:00:26"^^xsd:datetime ; 
    dcterms:modified "2021-05-19T00:02:33"^^xsd:datetime ; 
. 

<http://linked.data.gov.au/def/tern-cv/1cb8ec7b-9aa5-4ac7-927a-7032684b600c> 
    a skos:Concept ; 
    skos:inScheme <http://linked.data.gov.au/def/tern-cv/5699eca7-9ef0-47a6-bcfb-9306e0e2b85e> ; 
    rdfs:isDefinedBy <http://linked.data.gov.au/def/tern-cv/5699eca7-9ef0-47a6-bcfb-9306e0e2b85e> ; 
    skos:prefLabel "vine fuel load sd"@en ; 
    skos:definition "Standard deviation of dry biomass of vines measurements."@en ; 
    skos:broader <http://linked.data.gov.au/def/tern-cv/45ae73d8-92bd-4261-a05f-7bfac228e1f7> ; 
    dcterms:created "2021-05-19T00:02:53"^^xsd:datetime ; 
    dcterms:modified "2021-05-19T00:03:28"^^xsd:datetime ; 
. 

<http://linked.data.gov.au/def/tern-cv/f9ae2722-732f-472a-8087-999240c6581a> 
    a skos:Concept ; 
    skos:inScheme <http://linked.data.gov.au/def/tern-cv/5699eca7-9ef0-47a6-bcfb-9306e0e2b85e> ; 
    rdfs:isDefinedBy <http://linked.data.gov.au/def/tern-cv/5699eca7-9ef0-47a6-bcfb-9306e0e2b85e> ; 
    skos:prefLabel "dead grass cover mean"@en ; 
    skos:definition "Average area cover by dead grass."@en ; 
    skos:broader <http://linked.data.gov.au/def/tern-cv/45ae73d8-92bd-4261-a05f-7bfac228e1f7> ; 
    dcterms:created "2021-05-19T00:05:25"^^xsd:datetime ; 
    dcterms:modified "2021-05-19T00:06:14"^^xsd:datetime ; 
. 

<http://linked.data.gov.au/def/tern-cv/fd9ffa6b-cffa-4e14-a536-06ab8e3505d7> 
    a skos:Concept ; 
    skos:inScheme <http://linked.data.gov.au/def/tern-cv/5699eca7-9ef0-47a6-bcfb-9306e0e2b85e> ; 
    rdfs:isDefinedBy <http://linked.data.gov.au/def/tern-cv/5699eca7-9ef0-47a6-bcfb-9306e0e2b85e> ; 
    skos:prefLabel "dead grass cover sd"@en ; 
    skos:definition "Standard deviation of dead grass cover measurements."@en ; 
    skos:broader <http://linked.data.gov.au/def/tern-cv/45ae73d8-92bd-4261-a05f-7bfac228e1f7> ; 
    dcterms:created "2021-05-19T00:06:34"^^xsd:datetime ; 
    dcterms:modified "2021-05-19T00:15:05"^^xsd:datetime ; 
. 

<http://linked.data.gov.au/def/tern-cv/869b3963-b276-48ac-a0b0-5d6e108eef50> 
    a skos:Concept ; 
    skos:inScheme <http://linked.data.gov.au/def/tern-cv/5699eca7-9ef0-47a6-bcfb-9306e0e2b85e> ; 
    rdfs:isDefinedBy <http://linked.data.gov.au/def/tern-cv/5699eca7-9ef0-47a6-bcfb-9306e0e2b85e> ; 
    skos:prefLabel "dead herbs cover mean"@en ; 
    skos:definition "Average cover of dead herbs on the ground."@en ; 
    skos:broader <http://linked.data.gov.au/def/tern-cv/45ae73d8-92bd-4261-a05f-7bfac228e1f7> ; 
    dcterms:created "2021-05-19T00:15:39"^^xsd:datetime ; 
    dcterms:modified "2021-05-19T00:17:03"^^xsd:datetime ; 
. 

<http://linked.data.gov.au/def/tern-cv/75208020-a087-4b31-89a3-c3028382b5eb> 
    a skos:Concept ; 
    skos:inScheme <http://linked.data.gov.au/def/tern-cv/5699eca7-9ef0-47a6-bcfb-9306e0e2b85e> ; 
    rdfs:isDefinedBy <http://linked.data.gov.au/def/tern-cv/5699eca7-9ef0-47a6-bcfb-9306e0e2b85e> ; 
    skos:prefLabel "dead herbs cover sd"@en ; 
    skos:definition "Standard deviation of dead herbs cover measurements."@en ; 
    skos:broader <http://linked.data.gov.au/def/tern-cv/45ae73d8-92bd-4261-a05f-7bfac228e1f7> ; 
    dcterms:created "2021-05-19T00:17:25"^^xsd:datetime ; 
    dcterms:modified "2021-05-19T00:18:01"^^xsd:datetime ; 
. 

<http://linked.data.gov.au/def/tern-cv/89ed531e-0ea0-49d6-8386-ef80c75f0f4f> 
    a skos:Concept ; 
    skos:inScheme <http://linked.data.gov.au/def/tern-cv/5699eca7-9ef0-47a6-bcfb-9306e0e2b85e> ; 
    rdfs:isDefinedBy <http://linked.data.gov.au/def/tern-cv/5699eca7-9ef0-47a6-bcfb-9306e0e2b85e> ; 
    skos:prefLabel "dead shrub cover mean"@en ; 
    skos:definition "Average area cover by dead shrubs."@en ; 
    skos:broader <http://linked.data.gov.au/def/tern-cv/45ae73d8-92bd-4261-a05f-7bfac228e1f7> ; 
    dcterms:created "2021-05-19T00:18:29"^^xsd:datetime ; 
    dcterms:modified "2021-05-19T00:19:01"^^xsd:datetime ; 
. 

<http://linked.data.gov.au/def/tern-cv/00c2b397-b61b-4dbe-8f07-7444c00a6af2> 
    a skos:Concept ; 
    skos:inScheme <http://linked.data.gov.au/def/tern-cv/5699eca7-9ef0-47a6-bcfb-9306e0e2b85e> ; 
    rdfs:isDefinedBy <http://linked.data.gov.au/def/tern-cv/5699eca7-9ef0-47a6-bcfb-9306e0e2b85e> ; 
    skos:prefLabel "dead shrub cover sd"@en ; 
    skos:definition "Standard deviation of dead shrub cover measurements."@en ; 
    skos:broader <http://linked.data.gov.au/def/tern-cv/45ae73d8-92bd-4261-a05f-7bfac228e1f7> ; 
    dcterms:created "2021-05-19T00:19:18"^^xsd:datetime ; 
    dcterms:modified "2021-05-19T00:19:46"^^xsd:datetime ; 
. 

<http://linked.data.gov.au/def/tern-cv/825b15c9-5f3f-4b24-9b71-baeb565d4201> 
    a skos:Concept ; 
    skos:inScheme <http://linked.data.gov.au/def/tern-cv/5699eca7-9ef0-47a6-bcfb-9306e0e2b85e> ; 
    rdfs:isDefinedBy <http://linked.data.gov.au/def/tern-cv/5699eca7-9ef0-47a6-bcfb-9306e0e2b85e> ; 
    skos:prefLabel "dead vine cover mean"@en ; 
    skos:definition "Average area cover by dead vines."@en ; 
    skos:broader <http://linked.data.gov.au/def/tern-cv/45ae73d8-92bd-4261-a05f-7bfac228e1f7> ; 
    dcterms:created "2021-05-19T00:20:14"^^xsd:datetime ; 
    dcterms:modified "2021-05-19T00:20:46"^^xsd:datetime ; 
. 

<http://linked.data.gov.au/def/tern-cv/8d763d15-1aa9-4369-a77b-a0ea4bd3d6ca> 
    a skos:Concept ; 
    skos:inScheme <http://linked.data.gov.au/def/tern-cv/5699eca7-9ef0-47a6-bcfb-9306e0e2b85e> ; 
    rdfs:isDefinedBy <http://linked.data.gov.au/def/tern-cv/5699eca7-9ef0-47a6-bcfb-9306e0e2b85e> ; 
    skos:prefLabel "dead vine cover sd"@en ; 
    skos:definition "Standard deviation of dead vine cover measurements."@en ; 
    skos:broader <http://linked.data.gov.au/def/tern-cv/45ae73d8-92bd-4261-a05f-7bfac228e1f7> ; 
    dcterms:created "2021-05-19T00:21:01"^^xsd:datetime ; 
    dcterms:modified "2021-05-19T00:21:26"^^xsd:datetime ; 
. 

<http://linked.data.gov.au/def/tern-cv/abce4dbb-e9e8-41ab-8f6d-fd4f63e2fb2a> 
    a skos:Concept ; 
    skos:inScheme <http://linked.data.gov.au/def/tern-cv/5699eca7-9ef0-47a6-bcfb-9306e0e2b85e> ; 
    rdfs:isDefinedBy <http://linked.data.gov.au/def/tern-cv/5699eca7-9ef0-47a6-bcfb-9306e0e2b85e> ; 
    skos:prefLabel "leaf litter cover mean"@en ; 
    skos:definition "Average area cover by leaf litter."@en ; 
    skos:broader <http://linked.data.gov.au/def/tern-cv/45ae73d8-92bd-4261-a05f-7bfac228e1f7> ; 
    dcterms:created "2021-05-19T00:21:57"^^xsd:datetime ; 
    dcterms:modified "2021-05-19T00:22:29"^^xsd:datetime ; 
. 

<http://linked.data.gov.au/def/tern-cv/6cd4c83a-6e69-4271-ae58-d9dd82ecd20b> 
    a skos:Concept ; 
    skos:inScheme <http://linked.data.gov.au/def/tern-cv/5699eca7-9ef0-47a6-bcfb-9306e0e2b85e> ; 
    rdfs:isDefinedBy <http://linked.data.gov.au/def/tern-cv/5699eca7-9ef0-47a6-bcfb-9306e0e2b85e> ; 
    skos:prefLabel "leaf litter cover sd"@en ; 
    skos:definition "Standard deviation of leaf litter cover measurements."@en ; 
    skos:broader <http://linked.data.gov.au/def/tern-cv/45ae73d8-92bd-4261-a05f-7bfac228e1f7> ; 
    dcterms:created "2021-05-19T00:22:51"^^xsd:datetime ; 
    dcterms:modified "2021-05-19T00:23:46"^^xsd:datetime ; 
. 

<http://linked.data.gov.au/def/tern-cv/e9947c8b-0d88-40d5-842a-4aa32fe6646a> 
    a skos:Concept ; 
    skos:inScheme <http://linked.data.gov.au/def/tern-cv/5699eca7-9ef0-47a6-bcfb-9306e0e2b85e> ; 
    rdfs:isDefinedBy <http://linked.data.gov.au/def/tern-cv/5699eca7-9ef0-47a6-bcfb-9306e0e2b85e> ; 
    skos:prefLabel "live grass cover mean"@en ; 
    skos:definition "Average cover of live grass."@en ; 
    skos:broader <http://linked.data.gov.au/def/tern-cv/45ae73d8-92bd-4261-a05f-7bfac228e1f7> ; 
    dcterms:created "2021-05-19T00:24:29"^^xsd:datetime ; 
    dcterms:modified "2021-05-19T01:40:37"^^xsd:datetime ; 
. 

<http://linked.data.gov.au/def/tern-cv/88b78054-2c46-43e4-9222-db33a79c1a3b> 
    a skos:Concept ; 
    skos:inScheme <http://linked.data.gov.au/def/tern-cv/5699eca7-9ef0-47a6-bcfb-9306e0e2b85e> ; 
    rdfs:isDefinedBy <http://linked.data.gov.au/def/tern-cv/5699eca7-9ef0-47a6-bcfb-9306e0e2b85e> ; 
    skos:prefLabel "live grass cover sd"@en ; 
    skos:definition "live grass cover sd"@en ; 
    skos:broader <http://linked.data.gov.au/def/tern-cv/45ae73d8-92bd-4261-a05f-7bfac228e1f7> ; 
    dcterms:created "2021-05-19T01:41:16"^^xsd:datetime ; 
. 

<http://linked.data.gov.au/def/tern-cv/2ed9a76c-195e-4c9c-aa7f-94339c0835b2> 
    a skos:Concept ; 
    skos:inScheme <http://linked.data.gov.au/def/tern-cv/5699eca7-9ef0-47a6-bcfb-9306e0e2b85e> ; 
    rdfs:isDefinedBy <http://linked.data.gov.au/def/tern-cv/5699eca7-9ef0-47a6-bcfb-9306e0e2b85e> ; 
    skos:prefLabel "live shubs cover mean"@en ; 
    skos:definition "Average area cover by live shrubs."@en ; 
    skos:broader <http://linked.data.gov.au/def/tern-cv/45ae73d8-92bd-4261-a05f-7bfac228e1f7> ; 
    dcterms:created "2021-05-19T01:42:07"^^xsd:datetime ; 
    dcterms:modified "2021-05-19T01:43:30"^^xsd:datetime ; 
. 

<http://linked.data.gov.au/def/tern-cv/eb29cf16-af57-4c8b-b5ec-8c35db9b9901> 
    a skos:Concept ; 
    skos:inScheme <http://linked.data.gov.au/def/tern-cv/5699eca7-9ef0-47a6-bcfb-9306e0e2b85e> ; 
    rdfs:isDefinedBy <http://linked.data.gov.au/def/tern-cv/5699eca7-9ef0-47a6-bcfb-9306e0e2b85e> ; 
    skos:prefLabel "live shrubs cover sd"@en ; 
    skos:definition "live shrubs cover sd"@en ; 
    skos:broader <http://linked.data.gov.au/def/tern-cv/45ae73d8-92bd-4261-a05f-7bfac228e1f7> ; 
    dcterms:created "2021-05-19T01:54:30"^^xsd:datetime ; 
. 

<http://linked.data.gov.au/def/tern-cv/39edcda9-ec99-47f7-9c73-5accc2e7aa72> 
    a skos:Concept ; 
    skos:inScheme <http://linked.data.gov.au/def/tern-cv/5699eca7-9ef0-47a6-bcfb-9306e0e2b85e> ; 
    rdfs:isDefinedBy <http://linked.data.gov.au/def/tern-cv/5699eca7-9ef0-47a6-bcfb-9306e0e2b85e> ; 
    skos:prefLabel "live vines cover mean"@en ; 
    skos:definition "Average area cover by live vines."@en ; 
    skos:broader <http://linked.data.gov.au/def/tern-cv/45ae73d8-92bd-4261-a05f-7bfac228e1f7> ; 
    dcterms:created "2021-05-19T02:10:47"^^xsd:datetime ; 
    dcterms:modified "2021-05-19T02:31:19"^^xsd:datetime ; 
. 

<http://linked.data.gov.au/def/tern-cv/df6d0f0e-81b0-4bf0-a567-382a4f4b8217> 
    a skos:Concept ; 
    skos:inScheme <http://linked.data.gov.au/def/tern-cv/5699eca7-9ef0-47a6-bcfb-9306e0e2b85e> ; 
    rdfs:isDefinedBy <http://linked.data.gov.au/def/tern-cv/5699eca7-9ef0-47a6-bcfb-9306e0e2b85e> ; 
    skos:prefLabel "live vines cover sd"@en ; 
    skos:definition "Standard deviation of live vines cover measurements."@en ; 
    skos:broader <http://linked.data.gov.au/def/tern-cv/45ae73d8-92bd-4261-a05f-7bfac228e1f7> ; 
    dcterms:created "2021-05-19T02:27:46"^^xsd:datetime ; 
    dcterms:modified "2021-05-19T02:31:43"^^xsd:datetime ; 
. 

<http://linked.data.gov.au/def/tern-cv/0bd7d3ce-9c2e-45ab-84b1-04003c0458d9> 
    a skos:Concept ; 
    skos:inScheme <http://linked.data.gov.au/def/tern-cv/5699eca7-9ef0-47a6-bcfb-9306e0e2b85e> ; 
    rdfs:isDefinedBy <http://linked.data.gov.au/def/tern-cv/5699eca7-9ef0-47a6-bcfb-9306e0e2b85e> ; 
    skos:prefLabel "duff depth mean"@en ; 
    skos:definition "Average depth of layer of decomposing organic materials lying below the litter layer and immediately above the mineral soil."@en ; 
    skos:broader <http://linked.data.gov.au/def/tern-cv/45ae73d8-92bd-4261-a05f-7bfac228e1f7> ; 
    dcterms:created "2021-05-19T02:32:15"^^xsd:datetime ; 
    dcterms:modified "2021-05-19T02:33:36"^^xsd:datetime ; 
. 

<http://linked.data.gov.au/def/tern-cv/2adc6b97-40f4-4331-8631-031008cb43d4> 
    a skos:Concept ; 
    skos:inScheme <http://linked.data.gov.au/def/tern-cv/5699eca7-9ef0-47a6-bcfb-9306e0e2b85e> ; 
    rdfs:isDefinedBy <http://linked.data.gov.au/def/tern-cv/5699eca7-9ef0-47a6-bcfb-9306e0e2b85e> ; 
    skos:prefLabel "duff depth sd"@en ; 
    skos:definition "Standarde deviation of duff depth measurements."@en ; 
    skos:broader <http://linked.data.gov.au/def/tern-cv/45ae73d8-92bd-4261-a05f-7bfac228e1f7> ; 
    dcterms:created "2021-05-19T02:33:53"^^xsd:datetime ; 
    dcterms:modified "2021-05-19T02:34:27"^^xsd:datetime ; 
. 

<http://linked.data.gov.au/def/tern-cv/4da6fe3c-5219-4ad6-97b1-df0225483de5> 
    a skos:Concept ; 
    skos:inScheme <http://linked.data.gov.au/def/tern-cv/5699eca7-9ef0-47a6-bcfb-9306e0e2b85e> ; 
    rdfs:isDefinedBy <http://linked.data.gov.au/def/tern-cv/5699eca7-9ef0-47a6-bcfb-9306e0e2b85e> ; 
    skos:prefLabel "live herbs cover mean"@en ; 
    skos:definition "Average area cover by live herbs."@en ; 
    skos:broader <http://linked.data.gov.au/def/tern-cv/45ae73d8-92bd-4261-a05f-7bfac228e1f7> ; 
    dcterms:created "2021-05-19T04:17:58"^^xsd:datetime ; 
    dcterms:modified "2021-05-19T04:18:55"^^xsd:datetime ; 
. 

<http://linked.data.gov.au/def/tern-cv/b216e89a-94a2-4e59-ba6b-b92edd028c47> 
    a skos:Concept ; 
    skos:inScheme <http://linked.data.gov.au/def/tern-cv/5699eca7-9ef0-47a6-bcfb-9306e0e2b85e> ; 
    rdfs:isDefinedBy <http://linked.data.gov.au/def/tern-cv/5699eca7-9ef0-47a6-bcfb-9306e0e2b85e> ; 
    skos:prefLabel "live herbs cover sd"@en ; 
    skos:definition "Standard deviation of live herbs cover measurements."@en ; 
    skos:broader <http://linked.data.gov.au/def/tern-cv/45ae73d8-92bd-4261-a05f-7bfac228e1f7> ; 
    dcterms:created "2021-05-19T04:18:16"^^xsd:datetime ; 
    dcterms:modified "2021-05-19T04:19:37"^^xsd:datetime ; 
. 

<http://linked.data.gov.au/def/tern-cv/5ddf2cec-0842-492f-b0fc-b507c421c4b3> 
    a skos:Concept ; 
    skos:inScheme <http://linked.data.gov.au/def/tern-cv/5699eca7-9ef0-47a6-bcfb-9306e0e2b85e> ; 
    rdfs:isDefinedBy <http://linked.data.gov.au/def/tern-cv/5699eca7-9ef0-47a6-bcfb-9306e0e2b85e> ; 
    skos:prefLabel "ecosystem respiration"@en ; 
    skos:definition "The chemical process that occurs in all living cells wherein organic compounds are broken down to release energy required for life processes. Nebel, Bernard J.and Richard T. Wright. Environmental Science-the Way the World Works. 1998. Prentice-Hall, Inc. Upper Saddle River, New Jersey."@en ; 
    skos:broader <http://linked.data.gov.au/def/tern-cv/45ae73d8-92bd-4261-a05f-7bfac228e1f7> ; 
    dcterms:created "2021-05-21T00:00:00"^^xsd:datetime ; 
    dcterms:modified "2021-05-24T01:22:02"^^xsd:datetime ; 
. 

<http://linked.data.gov.au/def/tern-cv/7402efec-a7ef-4f9c-a0ac-ccee0aeef26d> 
    a skos:Concept ; 
    skos:inScheme <http://linked.data.gov.au/def/tern-cv/5699eca7-9ef0-47a6-bcfb-9306e0e2b85e> ; 
    rdfs:isDefinedBy <http://linked.data.gov.au/def/tern-cv/5699eca7-9ef0-47a6-bcfb-9306e0e2b85e> ; 
    skos:prefLabel "net ecosystem exchange"@en ; 
    skos:definition "NEE of CO2 with the atmosphere is a fundamental measure of the balance between carbon uptake by the vegetation gross primary productivity (GPP) and carbon losses through autotrophic and heterotrophic respiration. National Snow and Ice Data Center, NSIDC, https://nsidc.org/"@en ; 
    skos:broader <http://linked.data.gov.au/def/tern-cv/45ae73d8-92bd-4261-a05f-7bfac228e1f7> ; 
    dcterms:created "2021-05-21T00:00:00"^^xsd:datetime ; 
    dcterms:modified "2021-05-24T00:44:12"^^xsd:datetime ; 
. 

<http://linked.data.gov.au/def/tern-cv/2f4c1e8a-7acd-4b79-b16b-04913233cc07> 
    a skos:Concept ; 
    skos:inScheme <http://linked.data.gov.au/def/tern-cv/5699eca7-9ef0-47a6-bcfb-9306e0e2b85e> ; 
    rdfs:isDefinedBy <http://linked.data.gov.au/def/tern-cv/5699eca7-9ef0-47a6-bcfb-9306e0e2b85e> ; 
    skos:prefLabel "net ecosystem productivity"@en ; 
    skos:definition "The difference between the amount of organic carbon fixed in an ecosystem by photosynthesis (gross primary productivity) and total ecosystem respiration. NEP represents the total amount of organic carbon available for storage or loss in the ecosystem. Whether NEP is greater or less than zero determines if an ecosystem is autrophic or heterotrophic."@en ; 
    skos:broader <http://linked.data.gov.au/def/tern-cv/45ae73d8-92bd-4261-a05f-7bfac228e1f7> ; 
    dcterms:created "2021-05-21T00:00:00"^^xsd:datetime ; 
    dcterms:modified "2021-05-24T01:23:54"^^xsd:datetime ; 
. 

<http://linked.data.gov.au/def/tern-cv/f63579ee-a834-4fc9-907a-82d6ae580efe> 
    a skos:Concept ; 
    skos:inScheme <http://linked.data.gov.au/def/tern-cv/5699eca7-9ef0-47a6-bcfb-9306e0e2b85e> ; 
    rdfs:isDefinedBy <http://linked.data.gov.au/def/tern-cv/5699eca7-9ef0-47a6-bcfb-9306e0e2b85e> ; 
    skos:prefLabel "available energy"@en ; 
    skos:definition "Available energy using net all-wave radiation (Fn) and ground heat flux (Fg)."@en ; 
    skos:broader <http://linked.data.gov.au/def/tern-cv/123f2efe-3891-4764-9047-609c8b30e925> ; 
    dcterms:created "2021-05-21T00:00:00"^^xsd:datetime ; 
    dcterms:modified "2021-05-24T01:33:51"^^xsd:datetime ; 
. 

<http://linked.data.gov.au/def/tern-cv/fb66fbb3-3cca-43cf-bf3c-df047ac68a63> 
    a skos:Concept ; 
    skos:inScheme <http://linked.data.gov.au/def/tern-cv/5699eca7-9ef0-47a6-bcfb-9306e0e2b85e> ; 
    rdfs:isDefinedBy <http://linked.data.gov.au/def/tern-cv/5699eca7-9ef0-47a6-bcfb-9306e0e2b85e> ; 
    skos:prefLabel "momentum flux"@en ; 
    skos:definition "The vertical flux of horizontal momentum, equal to the force per unit area, or stress."@en ; 
    skos:broader <http://linked.data.gov.au/def/tern-cv/123f2efe-3891-4764-9047-609c8b30e925> ; 
    dcterms:created "2021-05-21T00:00:00"^^xsd:datetime ; 
    dcterms:modified "2021-05-24T01:46:13"^^xsd:datetime ; 
. 

<http://linked.data.gov.au/def/tern-cv/993bad16-f465-4363-900e-b73637f7bdb8> 
    a skos:Concept ; 
    skos:inScheme <http://linked.data.gov.au/def/tern-cv/5699eca7-9ef0-47a6-bcfb-9306e0e2b85e> ; 
    rdfs:isDefinedBy <http://linked.data.gov.au/def/tern-cv/5699eca7-9ef0-47a6-bcfb-9306e0e2b85e> ; 
    skos:prefLabel "specific humidity deficit"@en ; 
    skos:definition "The amount by which the water vapor in the air must be increased to achieve saturation without changing the environmental temperature and pressure. The saturation deficit may be expressed in terms of a vapor pressure deficit, an absolute humidity deficit, or a relative humidity deficit."@en ; 
    skos:broader <http://linked.data.gov.au/def/tern-cv/123f2efe-3891-4764-9047-609c8b30e925> ; 
    dcterms:created "2021-05-21T00:00:00"^^xsd:datetime ; 
    dcterms:modified "2021-05-24T02:01:27"^^xsd:datetime ; 
. 

<http://linked.data.gov.au/def/tern-cv/376865de-c13b-41ae-a8ff-d564da40abb7> 
    a skos:Concept ; 
    skos:inScheme <http://linked.data.gov.au/def/tern-cv/5699eca7-9ef0-47a6-bcfb-9306e0e2b85e> ; 
    rdfs:isDefinedBy <http://linked.data.gov.au/def/tern-cv/5699eca7-9ef0-47a6-bcfb-9306e0e2b85e> ; 
    skos:prefLabel "friction velocity"@en ; 
    skos:definition "A reference wind velocity usually applied to motion near the ground where the shearing stress is often assumed to be independent of height and approximately proportional to the square of the mean velocity. The friction velocity is, therefore, exactly the velocity for which this square law would be valid. Sutton, O. G. 1953. Micrometeorology. p. 76."@en ; 
    skos:broader <http://linked.data.gov.au/def/tern-cv/123f2efe-3891-4764-9047-609c8b30e925> ; 
    dcterms:created "2021-05-21T00:00:00"^^xsd:datetime ; 
    dcterms:modified "2021-05-24T02:04:41"^^xsd:datetime ; 
. 

<http://linked.data.gov.au/def/tern-cv/c_fb538aea> 
    a skos:Concept ; 
    skos:inScheme <http://linked.data.gov.au/def/tern-cv/5699eca7-9ef0-47a6-bcfb-9306e0e2b85e> ; 
    rdfs:isDefinedBy <http://linked.data.gov.au/def/tern-cv/5699eca7-9ef0-47a6-bcfb-9306e0e2b85e> ; 
    skos:prefLabel "Monin-Obukhov length"@en ; 
    skos:definition "A parameter with dimension of length that, when used to scale the height above the ground z, yields a dimensionless stability parameter, z/L, that expresses the relative roles of shear and buoyancy in the production/consumption of turbulence kinetic energy."@en ; 
    skos:broader <http://linked.data.gov.au/def/tern-cv/123f2efe-3891-4764-9047-609c8b30e925> ; 
    dcterms:created "2021-05-24T01:04:02"^^xsd:datetime ; 
    dcterms:modified "2021-05-24T01:14:28"^^xsd:datetime ; 
. 

<http://linked.data.gov.au/def/tern-cv/c_fb538aea> 
    a skos:Concept ; 
    skos:inScheme <http://linked.data.gov.au/def/tern-cv/5699eca7-9ef0-47a6-bcfb-9306e0e2b85e> ; 
    rdfs:isDefinedBy <http://linked.data.gov.au/def/tern-cv/5699eca7-9ef0-47a6-bcfb-9306e0e2b85e> ; 
    skos:prefLabel "Monin-Obukhov length"@en ; 
    skos:definition "A parameter with dimension of length that, when used to scale the height above the ground z, yields a dimensionless stability parameter, z/L, that expresses the relative roles of shear and buoyancy in the production/consumption of turbulence kinetic energy."@en ; 
    skos:broader <http://linked.data.gov.au/def/tern-cv/45ae73d8-92bd-4261-a05f-7bfac228e1f7> ; 
    dcterms:created "2021-05-24T01:04:02"^^xsd:datetime ; 
    dcterms:modified "2021-05-24T01:14:28"^^xsd:datetime ;
.
