# a hierarchy of Concepts with one being broader than two others

@prefix dct: <http://purl.org/dc/terms/> .
@prefix dc: <http://purl.org/dc/elements/1.1/> .
@prefix owl: <http://www.w3.org/2002/07/owl#> .
@prefix rdfs: <http://www.w3.org/2000/01/rdf-schema#> .
@prefix skos: <http://www.w3.org/2004/02/skos/core#> .
@prefix xsd: <http://www.w3.org/2001/XMLSchema#> .

@prefix {SHORT_CODE}: <http://linked.data.gov.au/def/{URI_ID}/> .

<http://linked.data.gov.au/def/{URI_ID}> a owl:Ontology .

{SHORT_CODE}:{CONCEPT_1_ID} 
  a skos:Concept;
  skos:inScheme {SHORT_CODE}:conceptScheme;
  skos:prefLabel "{CONCEPT_1_LABEL}"@en ;
  skos:definition "{CONCEPT_1_DEFINITION}"@en ;
  dct:source {CONCEPT_1_SOURCE_WEB_ADDRESS_OR_TEXT} .

{SHORT_CODE}:{CONCEPT_2_ID} 
  a skos:Concept;
  skos:inScheme {SHORT_CODE}:conceptScheme;
  skos:prefLabel "{CONCEPT_2_LABEL}"@en ;
  skos:definition "{CONCEPT_2_DEFINITION}"@en ;
  dct:source {CONCEPT_2_SOURCE_WEB_ADDRESS_OR_TEXT} ;
  skos:broader {SHORT_CODE}:{CONCEPT_1_ID} .

{SHORT_CODE}:{CONCEPT_3_ID} 
  a skos:Concept;
  skos:inScheme {SHORT_CODE}:conceptScheme;
  skos:prefLabel "{CONCEPT_3_LABEL}"@en ;
  skos:definition "{CONCEPT_3_DEFINITION}"@en ;
  dct:source {CONCEPT_3_SOURCE_WEB_ADDRESS_OR_TEXT} ;
  skos:broader {SHORT_CODE}:{CONCEPT_1_ID} .


# Example vocab - Borehole Inclination - as per template above
# 
# @prefix bhinc: <http://linked.data.gov.au/def/borehole-inclination/> .
# 
# <http://linked.data.gov.au/def/borehole-inclination> a owl:Ontology .
# 
# bhinc:conceptScheme 
#   a skos:ConceptScheme;
#   skos:prefLabel "Borehole Inclination"@en ;
#   dct:description "The ways in which a borehole may be angled with respect to the vertical"@en ;
#   dct:source <https://www.opengeospatial.org/standards/geosciml> .
#
#   or, instead of dct:source with a web address
#
#   dct:source "This vocabulary's content is taken entirely from a code list table in the OGC's Geoscience Markup Language (GeoSciML) standard." .
# 
# bhinc:Inclined
#   a skos:Concept;
#   skos:topConceptOf bhinc:conceptScheme;
#   skos:prefLabel "Inclined"@en ;
#   skos:definition "A predomenently horizontal borehole's shaft is angled either up or down." .
#
# bhinc:InclinedUp 
#   a skos:Concept;
#   skos:inScheme bhinc:conceptScheme;
#   skos:prefLabel "Inclined Up"@en ;
#   skos:definition "A predomenently horizontal borehole's shaft is angled at a positive acute angle to the horizontal (up)." ;
#   skos:braoder bhinc:Inclined .
#
# bhinc:InclinedDown
#   a skos:Concept;
#   skos:inScheme bhinc:conceptScheme;
#   skos:prefLabel "Inclined Down"@en ;
#   skos:definition "A predomenently horizontal borehole's shaft is angled at a negative acute angle to the horizontal (down)." ;
#   skos:braoder bhinc:Inclined .
#

# Alternate implementation
#
# Here, the same hierarchy as above is expresse with one Concept having two narrower Concept
#
#
# bhinc:Inclined
#   a skos:Concept;
#   skos:topConceptOf bhinc:conceptScheme;
#   skos:prefLabel "Inclined"@en ;
#   skos:definition "A predomenently horizontal borehole's shaft is angled either up or down." ;
#   skos:narrower bhinc:InclinedUp , bhinc:InclinedDown .
#
# bhinc:InclinedUp 
#   a skos:Concept;
#   skos:inScheme bhinc:conceptScheme;
#   skos:prefLabel "Inclined Up"@en ;
#   skos:definition "A predomenently horizontal borehole's shaft is angled at a positive acute angle to the horizontal (up)." .
#
# bhinc:InclinedDown
#   a skos:Concept;
#   skos:inScheme bhinc:conceptScheme;
#   skos:prefLabel "Inclined Down"@en ;
#   skos:definition "A predomenently horizontal borehole's shaft is angled at a negative acute angle to the horizontal (down)." .
#
